# baseURI: https://spec.edmcouncil.org/fibo/ontology/master/2018Q1/BE/Partnerships/Partnerships/
# imports: https://spec.edmcouncil.org/fibo/ontology/master/2018Q1/BE/LegalEntities/CorporateBodies/
# imports: https://spec.edmcouncil.org/fibo/ontology/master/2018Q1/BE/LegalEntities/FormalBusinessOrganizations/
# imports: https://spec.edmcouncil.org/fibo/ontology/master/2018Q1/BE/LegalEntities/LegalPersons/
# imports: https://spec.edmcouncil.org/fibo/ontology/master/2018Q1/BE/OwnershipAndControl/ControlParties/
# imports: https://spec.edmcouncil.org/fibo/ontology/master/2018Q1/BE/OwnershipAndControl/OwnershipParties/
# imports: https://spec.edmcouncil.org/fibo/ontology/master/2018Q1/FND/Accounting/AccountingEquity/
# imports: https://spec.edmcouncil.org/fibo/ontology/master/2018Q1/FND/Agreements/Contracts/
# imports: https://spec.edmcouncil.org/fibo/ontology/master/2018Q1/FND/Law/LegalCapacity/
# imports: https://spec.edmcouncil.org/fibo/ontology/master/2018Q1/FND/OwnershipAndControl/Ownership/
# imports: https://spec.edmcouncil.org/fibo/ontology/master/2018Q1/FND/Parties/Parties/
# imports: https://spec.edmcouncil.org/fibo/ontology/master/2018Q1/FND/Parties/Roles/
# imports: https://spec.edmcouncil.org/fibo/ontology/master/2018Q1/FND/Relations/Relations/
# imports: https://spec.edmcouncil.org/fibo/ontology/master/2018Q1/FND/Utilities/AnnotationVocabulary/

@base <https://spec.edmcouncil.org/fibo/ontology/master/2018Q1/BE/Partnerships/Partnerships/> .
@prefix afn: <http://jena.apache.org/ARQ/function#> .
@prefix dc: <http://purl.org/dc/elements/1.1/> .
@prefix dct: <http://purl.org/dc/terms/> .
@prefix fibo-be-le-cb: <https://spec.edmcouncil.org/fibo/ontology/BE/LegalEntities/CorporateBodies/> .
@prefix fibo-be-le-fbo: <https://spec.edmcouncil.org/fibo/ontology/BE/LegalEntities/FormalBusinessOrganizations/> .
@prefix fibo-be-le-lp: <https://spec.edmcouncil.org/fibo/ontology/BE/LegalEntities/LegalPersons/> .
@prefix fibo-be-oac-cpty: <https://spec.edmcouncil.org/fibo/ontology/BE/OwnershipAndControl/ControlParties/> .
@prefix fibo-be-oac-opty: <https://spec.edmcouncil.org/fibo/ontology/BE/OwnershipAndControl/OwnershipParties/> .
@prefix fibo-be-ptr-ptr: <https://spec.edmcouncil.org/fibo/ontology/BE/Partnerships/Partnerships/> .
@prefix fibo-fnd-acc-aeq: <https://spec.edmcouncil.org/fibo/ontology/FND/Accounting/AccountingEquity/> .
@prefix fibo-fnd-agr-ctr: <https://spec.edmcouncil.org/fibo/ontology/FND/Agreements/Contracts/> .
@prefix fibo-fnd-law-lcap: <https://spec.edmcouncil.org/fibo/ontology/FND/Law/LegalCapacity/> .
@prefix fibo-fnd-oac-own: <https://spec.edmcouncil.org/fibo/ontology/FND/OwnershipAndControl/Ownership/> .
@prefix fibo-fnd-pty-pty: <https://spec.edmcouncil.org/fibo/ontology/FND/Parties/Parties/> .
@prefix fibo-fnd-pty-rl: <https://spec.edmcouncil.org/fibo/ontology/FND/Parties/Roles/> .
@prefix fibo-fnd-rel-rel: <https://spec.edmcouncil.org/fibo/ontology/FND/Relations/Relations/> .
@prefix fibo-fnd-utl-av: <https://spec.edmcouncil.org/fibo/ontology/FND/Utilities/AnnotationVocabulary/> .
@prefix grddl: <http://www.w3.org/2003/g/data-view#> .
@prefix owl: <http://www.w3.org/2002/07/owl#> .
@prefix rdf: <http://www.w3.org/1999/02/22-rdf-syntax-ns#> .
@prefix rdfs: <http://www.w3.org/2000/01/rdf-schema#> .
@prefix skos: <http://www.w3.org/2004/02/skos/core#> .
@prefix sm: <http://www.omg.org/techprocess/ab/SpecificationMetadata/> .
@prefix xsd: <http://www.w3.org/2001/XMLSchema#> .

<https://spec.edmcouncil.org/fibo/ontology/BE/Partnerships/Partnerships/>
	a owl:Ontology ;
	rdfs:label "Partnerships Ontology" ;
	dct:abstract "This ontology defines partnerships and related concepts. The concepts distinguish general from limited partners, as well as the types of equity that they hold. Included are abstract definitions of partnership types based on whether they have general, limited or both kinds of partners. Both legally incorporated and non incorporated forms of partnerships are covered." ;
	dct:license "http://opensource.org/licenses/MIT"^^xsd:anyURI ;
	sm:contentLanguage
		"http://www.omg.org/spec/ODM/"^^xsd:anyURI ,
		"http://www.w3.org/standards/techs/owl#w3c_all"^^xsd:anyURI
		;
	sm:copyright """Copyright (c) 2013-2016 EDM Council, Inc.
Copyright (c) 2013-2016 Object Management Group, Inc.""" ;
	sm:dependsOn
		"https://spec.edmcouncil.org/fibo/ontology/BE/LegalEntities/CorporateBodies/"^^xsd:anyURI ,
		"https://spec.edmcouncil.org/fibo/ontology/BE/LegalEntities/FormalBusinessOrganizations/"^^xsd:anyURI ,
		"https://spec.edmcouncil.org/fibo/ontology/BE/LegalEntities/LegalPersons/"^^xsd:anyURI ,
		"https://spec.edmcouncil.org/fibo/ontology/BE/OwnershipAndControl/ControlParties/"^^xsd:anyURI ,
		"https://spec.edmcouncil.org/fibo/ontology/BE/OwnershipAndControl/OwnershipParties/"^^xsd:anyURI ,
		"https://spec.edmcouncil.org/fibo/ontology/FND/"^^xsd:anyURI
		;
	sm:fileAbbreviation "fibo-be-ptr-ptr" ;
	sm:filename "Partnerships.rdf" ;
	rdfs:seeAlso
		"https://spec.edmcouncil.org/fibo/ontology/AboutTheEDMC-FIBOFamily/"^^xsd:anyURI ,
		"https://spec.edmcouncil.org/fibo/ontology/BE/AboutBE/"^^xsd:anyURI ,
		"https://spec.edmcouncil.org/fibo/ontology/BE/Partnerships/AboutPartnerships/"^^xsd:anyURI
		;
	owl:imports
		<https://spec.edmcouncil.org/fibo/ontology/master/2018Q1/BE/LegalEntities/CorporateBodies/> ,
		<https://spec.edmcouncil.org/fibo/ontology/master/2018Q1/BE/LegalEntities/FormalBusinessOrganizations/> ,
		<https://spec.edmcouncil.org/fibo/ontology/master/2018Q1/BE/LegalEntities/LegalPersons/> ,
		<https://spec.edmcouncil.org/fibo/ontology/master/2018Q1/BE/OwnershipAndControl/ControlParties/> ,
		<https://spec.edmcouncil.org/fibo/ontology/master/2018Q1/BE/OwnershipAndControl/OwnershipParties/> ,
		<https://spec.edmcouncil.org/fibo/ontology/master/2018Q1/FND/Accounting/AccountingEquity/> ,
		<https://spec.edmcouncil.org/fibo/ontology/master/2018Q1/FND/Agreements/Contracts/> ,
		<https://spec.edmcouncil.org/fibo/ontology/master/2018Q1/FND/Law/LegalCapacity/> ,
		<https://spec.edmcouncil.org/fibo/ontology/master/2018Q1/FND/OwnershipAndControl/Ownership/> ,
		<https://spec.edmcouncil.org/fibo/ontology/master/2018Q1/FND/Parties/Parties/> ,
		<https://spec.edmcouncil.org/fibo/ontology/master/2018Q1/FND/Parties/Roles/> ,
		<https://spec.edmcouncil.org/fibo/ontology/master/2018Q1/FND/Relations/Relations/> ,
		<https://spec.edmcouncil.org/fibo/ontology/master/2018Q1/FND/Utilities/AnnotationVocabulary/>
		;
	owl:versionIRI <https://spec.edmcouncil.org/fibo/ontology/master/2018Q1/BE/Partnerships/Partnerships/> ;
	skos:changeNote "The https://spec.edmcouncil.org/fibo/ontology/BE/Partnerships/Partnerships.rdf version of this ontology was modified per the issue resolutions identified in the FIBO BE 1.0 FTF report." ;
	fibo-fnd-utl-av:hasMaturityLevel fibo-fnd-utl-av:Release ;
	.

fibo-be-ptr-ptr:CorporateLimitedPartner
	a owl:Class ;
	rdfs:subClassOf
		fibo-be-ptr-ptr:LimitedPartner ,
		[
			a owl:Restriction ;
			owl:onProperty fibo-fnd-rel-rel:hasIdentity ;
			owl:onClass fibo-be-le-cb:Corporation ;
			owl:qualifiedCardinality "1"^^xsd:nonNegativeInteger ;
		]
		;
	rdfs:label "corporate limited partner" ;
	rdfs:isDefinedBy <https://spec.edmcouncil.org/fibo/ontology/BE/Partnerships/Partnerships/> ;
	skos:definition "A limited partner in a partnership, who is and may only be a Corporate Legal Person (i.e., not a natural person)" ;
	.

fibo-be-ptr-ptr:EquityApportionmentTermsSet
	a owl:Class ;
	rdfs:subClassOf fibo-fnd-agr-ctr:ContractTermsSet ;
	rdfs:label "equity apportionment terms set" ;
	rdfs:isDefinedBy <https://spec.edmcouncil.org/fibo/ontology/BE/Partnerships/Partnerships/> ;
	skos:definition "Terms setting out the apportionment of equity in some formal business organization." ;
	.

fibo-be-ptr-ptr:GeneralPartner
	a owl:Class ;
	rdfs:subClassOf
		fibo-be-oac-cpty:DeJureControllingInterestParty ,
		fibo-be-ptr-ptr:Partner ,
		[
			a owl:Restriction ;
			owl:onProperty fibo-fnd-rel-rel:hasIdentity ;
			owl:onClass fibo-be-le-lp:NaturalPerson ;
			owl:qualifiedCardinality "1"^^xsd:nonNegativeInteger ;
		] ,
		[
			a owl:Restriction ;
			owl:onProperty fibo-fnd-pty-rl:isPlayedBy ;
			owl:someValuesFrom [
				a owl:Restriction ;
				owl:onProperty fibo-be-ptr-ptr:holdsPartnershipEquityIn ;
				owl:allValuesFrom fibo-be-ptr-ptr:GeneralPartnerEquity ;
			] ;
		] ,
		[
			a owl:Restriction ;
			owl:onProperty fibo-fnd-pty-rl:isPlayedBy ;
			owl:someValuesFrom [
				a owl:Restriction ;
				owl:onProperty fibo-fnd-law-lcap:hasCapacity ;
				owl:allValuesFrom fibo-fnd-law-lcap:LiabilityCapacity ;
			] ;
		]
		;
	rdfs:label "general partner" ;
	rdfs:isDefinedBy <https://spec.edmcouncil.org/fibo/ontology/BE/Partnerships/Partnerships/> ;
	skos:definition "a partner in a partnership, who holds some part of the general partner equity and typically is jointly and severally liable with the other partners for the liabilities incurred by that partnership" ;
	.

fibo-be-ptr-ptr:GeneralPartnerEquity
	a owl:Class ;
	rdfs:subClassOf
		fibo-be-oac-opty:ControllingEquity ,
		fibo-be-ptr-ptr:PartnershipEquity ,
		[
			a owl:Restriction ;
			owl:onProperty fibo-fnd-rel-rel:confers ;
			owl:allValuesFrom fibo-be-oac-cpty:ConstitutionalDeJureControl ;
		]
		;
	rdfs:label "general partner equity" ;
	rdfs:isDefinedBy <https://spec.edmcouncil.org/fibo/ontology/BE/Partnerships/Partnerships/> ;
	skos:definition "Equity in a partnership held by general partners; this is typically accompanied by full liability capability on the part of the holders of the equity." ;
	skos:editorialNote "For a typical, non incorporated partnership, this is the only equity in the entity. Other typically incorporated partnerships may have additional limited equity in addition to or instead of this." ;
	.

fibo-be-ptr-ptr:LegallyIncorporatedPartnership
	a owl:Class ;
	rdfs:subClassOf
		fibo-be-le-cb:Corporation ,
		fibo-be-ptr-ptr:Partnership ,
		[
			a owl:Restriction ;
			owl:onProperty fibo-fnd-rel-rel:hasMember ;
			owl:onClass fibo-be-ptr-ptr:LegallyIncorporatedPartnershipMember ;
			owl:minQualifiedCardinality "2"^^xsd:nonNegativeInteger ;
		]
		;
	rdfs:label "legally incorporated partnership" ;
	rdfs:isDefinedBy <https://spec.edmcouncil.org/fibo/ontology/BE/Partnerships/Partnerships/> ;
	skos:definition "Any partnership which is defined as a legal person within a given jurisdiction, for example a limited liability partnership (if that is a legal person)." ;
	skos:editorialNote "The precise details and definition of these may vary from one jurisdiction to another. This type of entity is defined by being a legal person in its own right, as distinct from the usual type of partnership where the partners remain jointly and severally liable for debts." ;
	.

fibo-be-ptr-ptr:LegallyIncorporatedPartnershipMember
	a owl:Class ;
	rdfs:subClassOf fibo-be-ptr-ptr:Partner ;
	rdfs:label "legally incorporated partnership member" ;
	rdfs:isDefinedBy <https://spec.edmcouncil.org/fibo/ontology/BE/Partnerships/Partnerships/> ;
	skos:definition "a party that is a member or partner in a legally incorporated partnership such as an LLC or LLP" ;
	.

fibo-be-ptr-ptr:LiabilityApportionmentTermsSet
	a owl:Class ;
	rdfs:subClassOf fibo-fnd-agr-ctr:ContractTermsSet ;
	rdfs:label "liability apportionment terms set" ;
	rdfs:isDefinedBy <https://spec.edmcouncil.org/fibo/ontology/BE/Partnerships/Partnerships/> ;
	skos:definition "Terms setting out the apportionment of liabilities for debts or other liabilities accrued by some formal business organization." ;
	.

fibo-be-ptr-ptr:LimitedPartner
	a owl:Class ;
	rdfs:subClassOf
		fibo-be-ptr-ptr:Partner ,
		[
			a owl:Restriction ;
			owl:onProperty fibo-fnd-pty-rl:isPlayedBy ;
			owl:someValuesFrom [
				a owl:Restriction ;
				owl:onProperty fibo-be-ptr-ptr:holdsPartnershipEquityIn ;
				owl:allValuesFrom fibo-be-ptr-ptr:LimitedPartnerEquity ;
			] ;
		]
		;
	rdfs:label "limited partner" ;
	rdfs:isDefinedBy <https://spec.edmcouncil.org/fibo/ontology/BE/Partnerships/Partnerships/> ;
	skos:definition "A partner in a partnership whose liabilities are limited to the extent of their equity holding or guarantees" ;
	.

fibo-be-ptr-ptr:LimitedPartnerEquity
	a owl:Class ;
	rdfs:subClassOf
		fibo-be-ptr-ptr:PartnershipEquity ,
		fibo-fnd-acc-aeq:IssuedEquity
		;
	rdfs:label "limited partner equity" ;
	rdfs:isDefinedBy <https://spec.edmcouncil.org/fibo/ontology/BE/Partnerships/Partnerships/> ;
	skos:definition "equity in a partnership held by limited partners; this is not accompanied by any liability capability on the part of the holders of this equity." ;
	.

fibo-be-ptr-ptr:NaturalPersonLimitedPartner
	a owl:Class ;
	rdfs:subClassOf
		fibo-be-ptr-ptr:LimitedPartner ,
		[
			a owl:Restriction ;
			owl:onProperty fibo-fnd-rel-rel:hasIdentity ;
			owl:onClass fibo-be-le-lp:NaturalPerson ;
			owl:qualifiedCardinality "1"^^xsd:nonNegativeInteger ;
		]
		;
	rdfs:label "natural person limited partner" ;
	rdfs:isDefinedBy <https://spec.edmcouncil.org/fibo/ontology/BE/Partnerships/Partnerships/> ;
	skos:definition "A limited partner in a partnership, who is and may only be a Natural Person i.e. a human being." ;
	.

fibo-be-ptr-ptr:NonIncorporatedPartnership
	a owl:Class ;
	rdfs:subClassOf fibo-be-ptr-ptr:PartnershipWithGeneralPartners ;
	rdfs:label "non-incorporated partnership" ;
	rdfs:isDefinedBy <https://spec.edmcouncil.org/fibo/ontology/BE/Partnerships/Partnerships/> ;
	skos:definition "a partnership in which the partners are jointly and severally liable for liabilities incurred by the entity" ;
	.

fibo-be-ptr-ptr:Partner
	a owl:Class ;
	rdfs:subClassOf
		fibo-be-le-fbo:FormallyConstitutedOrganizationMember ,
		fibo-be-oac-opty:ConstitutionalOwner ,
		[
			a owl:Restriction ;
			owl:onProperty fibo-fnd-rel-rel:hasIdentity ;
			owl:onClass fibo-be-le-lp:LegalPerson ;
			owl:qualifiedCardinality "1"^^xsd:nonNegativeInteger ;
		] ,
		[
			a owl:Restriction ;
			owl:onProperty fibo-fnd-pty-rl:isPlayedBy ;
			owl:someValuesFrom [
				a owl:Restriction ;
				owl:onProperty fibo-fnd-rel-rel:isMemberOf ;
				owl:allValuesFrom fibo-be-ptr-ptr:Partnership ;
			] ;
		] ,
		[
			a owl:Restriction ;
			owl:onProperty fibo-fnd-pty-rl:isPlayedBy ;
			owl:someValuesFrom [
				a owl:Restriction ;
				owl:onProperty fibo-fnd-pty-pty:isAPartyTo ;
				owl:onClass fibo-be-ptr-ptr:PartnershipAgreement ;
				owl:qualifiedCardinality "1"^^xsd:nonNegativeInteger ;
			] ;
		]
		;
	rdfs:label "partner" ;
	rdfs:isDefinedBy <https://spec.edmcouncil.org/fibo/ontology/BE/Partnerships/Partnerships/> ;
	skos:definition "a member of a partnership" ;
	skos:scopeNote "This term is not referred to directly in specific kinds of partnership. Nearly all partnerships have General Partners, while forms of (mostly legally incorporated) partnerships have in addition Limited Partners. This term is the common ancestor of both." ;
	fibo-fnd-utl-av:definitionOrigin "http://www.investorwords.com/3608/partner.html"^^xsd:anyURI ;
	.

fibo-be-ptr-ptr:Partnership
	a owl:Class ;
	rdfs:subClassOf
		fibo-be-le-fbo:FormallyConstitutedOrganization ,
		fibo-be-le-lp:JuridicalPerson ,
		[
			a owl:Restriction ;
			owl:onProperty fibo-be-le-lp:hasObjective ;
			owl:onClass fibo-be-le-lp:ProfitObjective ;
			owl:minQualifiedCardinality "0"^^xsd:nonNegativeInteger ;
		] ,
		[
			a owl:Restriction ;
			owl:onProperty fibo-fnd-rel-rel:isGovernedBy ;
			owl:onClass fibo-be-ptr-ptr:PartnershipAgreement ;
			owl:minQualifiedCardinality "1"^^xsd:nonNegativeInteger ;
		] ,
		[
			a owl:Restriction ;
			owl:onProperty fibo-be-le-fbo:hasEquity ;
			owl:onClass fibo-be-ptr-ptr:PartnershipEquity ;
			owl:minQualifiedCardinality "1"^^xsd:nonNegativeInteger ;
		] ,
		[
			a owl:Restriction ;
			owl:onProperty fibo-fnd-rel-rel:hasMember ;
			owl:onClass fibo-be-ptr-ptr:Partner ;
			owl:minQualifiedCardinality "2"^^xsd:nonNegativeInteger ;
		] ,
		[
			a owl:Restriction ;
			owl:onProperty fibo-fnd-pty-pty:hasPartyInRole ;
			owl:someValuesFrom fibo-be-ptr-ptr:Partner ;
		]
		;
	rdfs:label "partnership" ;
	rdfs:isDefinedBy <https://spec.edmcouncil.org/fibo/ontology/BE/Partnerships/Partnerships/> ;
	skos:definition "venture in which two or more legal entities carry out some business activities under a common identity" ;
	skos:editorialNote "If the partnership doesn't limit the liability of the partners then the party to the contract is a natural person. If it does, then it's an artificial legal person (Body Corporate) - see Legally Incorporated Partnerships. Scope Note: This term of Partnership in the most general sense is ancestral to both of those." ;
	.

fibo-be-ptr-ptr:PartnershipAgreement
	a owl:Class ;
	rdfs:subClassOf
		fibo-be-le-fbo:OrganizationCoveringAgreement ,
		[
			a owl:Restriction ;
			owl:onProperty fibo-fnd-pty-pty:hasPartyInRole ;
			owl:someValuesFrom fibo-be-ptr-ptr:Partner ;
		]
		;
	rdfs:label "partnership agreement" ;
	rdfs:isDefinedBy <https://spec.edmcouncil.org/fibo/ontology/BE/Partnerships/Partnerships/> ;
	skos:definition "a document setting up a partnership, giving the details of the business and the amount each partner is contributing to it." ;
	fibo-fnd-utl-av:definitionOrigin "http://www.investorguide.com/definition/partnership-agreement.html"^^xsd:anyURI ;
	fibo-fnd-utl-av:synonym "articles of partnership" ;
	.

fibo-be-ptr-ptr:PartnershipEquity
	a owl:Class ;
	rdfs:subClassOf
		fibo-fnd-acc-aeq:StockholdersEquity ,
		[
			a owl:Restriction ;
			owl:onProperty fibo-fnd-acc-aeq:representsAnInterestIn ;
			owl:onClass fibo-be-ptr-ptr:Partnership ;
			owl:minQualifiedCardinality "1"^^xsd:nonNegativeInteger ;
		]
		;
	rdfs:label "partnership equity" ;
	rdfs:isDefinedBy <https://spec.edmcouncil.org/fibo/ontology/BE/Partnerships/Partnerships/> ;
	skos:definition "equity in some partnership" ;
	.

fibo-be-ptr-ptr:PartnershipIncorporatedByEquity
	a owl:Class ;
	rdfs:subClassOf
		fibo-be-le-cb:StockCorporation ,
		fibo-be-ptr-ptr:PartnershipWithLimitedPartners
		;
	rdfs:label "partnership incorporated by equity" ;
	rdfs:isDefinedBy <https://spec.edmcouncil.org/fibo/ontology/BE/Partnerships/Partnerships/> ;
	skos:definition "a partnership incorporated via the issuance of equity, with limited partners (i.e., partners whose liability is limited) that are necessarily not natural persons (i.e., cannot be individuals)" ;
	.

fibo-be-ptr-ptr:PartnershipIncorporatedThroughAgreement
	a owl:Class ;
	rdfs:subClassOf
		fibo-be-le-cb:BodyIncorporatedThroughAgreement ,
		fibo-be-ptr-ptr:Partnership
		;
	rdfs:label "partnership incorporated through agreement" ;
	rdfs:isDefinedBy <https://spec.edmcouncil.org/fibo/ontology/BE/Partnerships/Partnerships/> ;
	skos:definition "a partnership which has legal personhood, but for which there is not some issuance of limited partner equity" ;
	skos:editorialNote "An LLP (in the UK) is an example of this - in this case, the LLP document is the legal document which effectively constitutes the partnership" ;
	.

fibo-be-ptr-ptr:PartnershipWithCorporateLimitedPartners
	a owl:Class ;
	rdfs:subClassOf
		fibo-be-ptr-ptr:PartnershipWithLimitedPartners ,
		[
			a owl:Restriction ;
			owl:onProperty fibo-fnd-rel-rel:hasMember ;
			owl:onClass fibo-be-ptr-ptr:CorporateLimitedPartner ;
			owl:minQualifiedCardinality "1"^^xsd:nonNegativeInteger ;
		]
		;
	rdfs:label "partnership with corporate limited partners" ;
	rdfs:isDefinedBy <https://spec.edmcouncil.org/fibo/ontology/BE/Partnerships/Partnerships/> ;
	owl:disjointWith fibo-be-ptr-ptr:PartnershipWithNaturalPersonLimitedPartners ;
	skos:definition "A partnership with limited partners (partners whose liability is limited) and where those partners are necessarily non natural persons (i.e. cannot be individuals)." ;
	.

fibo-be-ptr-ptr:PartnershipWithGeneralAndLimitedPartners
	a owl:Class ;
	rdfs:subClassOf
		fibo-be-ptr-ptr:PartnershipWithGeneralPartners ,
		fibo-be-ptr-ptr:PartnershipWithLimitedPartners
		;
	rdfs:label "partnership with general and limited partners" ;
	rdfs:isDefinedBy <https://spec.edmcouncil.org/fibo/ontology/BE/Partnerships/Partnerships/> ;
	owl:disjointWith fibo-be-ptr-ptr:PartnershipWithOnlyLimitedPartners ;
	skos:definition "a partnership having both limited partners and general partners" ;
	.

fibo-be-ptr-ptr:PartnershipWithGeneralPartners
	a owl:Class ;
	rdfs:subClassOf
		fibo-be-ptr-ptr:Partnership ,
		[
			a owl:Restriction ;
			owl:onProperty fibo-fnd-rel-rel:hasMember ;
			owl:onClass fibo-be-ptr-ptr:GeneralPartner ;
			owl:minQualifiedCardinality "2"^^xsd:nonNegativeInteger ;
		]
		;
	rdfs:label "partnership with general partners" ;
	rdfs:isDefinedBy <https://spec.edmcouncil.org/fibo/ontology/BE/Partnerships/Partnerships/> ;
	skos:definition "a partnership that has two or more general partners" ;
	skos:editorialNote "The partnership may or may not also have limited partners. In a typical non-incorporated partnership, it does not. General partners of a partnership must be natural persons." ;
	.

fibo-be-ptr-ptr:PartnershipWithGeneralPartnersWithLimitedLiability
	a owl:Class ;
	rdfs:subClassOf fibo-be-ptr-ptr:PartnershipWithGeneralPartners ;
	rdfs:label "partnership with general partners with limited liability" ;
	rdfs:isDefinedBy <https://spec.edmcouncil.org/fibo/ontology/BE/Partnerships/Partnerships/> ;
	skos:definition "a partnership that has general partners, whose general partners have limited liability" ;
	skos:scopeNote "This is therefore necessarily a legal person (no-one else has liability); example in some US states is a limited liability limited partnership." ;
	.

fibo-be-ptr-ptr:PartnershipWithLimitedPartners
	a owl:Class ;
	rdfs:subClassOf
		fibo-be-ptr-ptr:Partnership ,
		[
			a owl:Restriction ;
			owl:onProperty fibo-fnd-rel-rel:hasMember ;
			owl:onClass fibo-be-ptr-ptr:LimitedPartner ;
			owl:minQualifiedCardinality "1"^^xsd:nonNegativeInteger ;
		]
		;
	rdfs:label "partnership with limited partners" ;
	rdfs:isDefinedBy <https://spec.edmcouncil.org/fibo/ontology/BE/Partnerships/Partnerships/> ;
	skos:definition "a partnership having limited partners, that is partners whose liabilities are limited to the extent of their equity or guarantees" ;
	skos:editorialNote "Possibly but not necessarily a Legal Person. If there are only Limited Partners then this is of necessity a Legal Person (no-one else has liability in this structure)." ;
	.

fibo-be-ptr-ptr:PartnershipWithNaturalPersonLimitedPartners
	a owl:Class ;
	rdfs:subClassOf
		fibo-be-ptr-ptr:PartnershipWithLimitedPartners ,
		[
			a owl:Restriction ;
			owl:onProperty fibo-fnd-rel-rel:hasMember ;
			owl:onClass fibo-be-ptr-ptr:NaturalPersonLimitedPartner ;
			owl:minQualifiedCardinality "1"^^xsd:nonNegativeInteger ;
		]
		;
	rdfs:label "partnership with natural person limited partners" ;
	rdfs:isDefinedBy <https://spec.edmcouncil.org/fibo/ontology/BE/Partnerships/Partnerships/> ;
	skos:definition "a partnership with limited partners (partners whose liability is limited) and where those partners are necessarily natural persons (i.e. cannot be corporates)" ;
	skos:scopeNote "Example in US, a Limited Liability Partnership" ;
	.

fibo-be-ptr-ptr:PartnershipWithOnlyLimitedPartners
	a owl:Class ;
	rdfs:subClassOf
		fibo-be-le-cb:Corporation ,
		fibo-be-ptr-ptr:PartnershipWithLimitedPartners
		;
	rdfs:label "partnership with only limited partners" ;
	rdfs:isDefinedBy <https://spec.edmcouncil.org/fibo/ontology/BE/Partnerships/Partnerships/> ;
	skos:definition "a partnership having limited partners but no general partners" ;
	.

fibo-be-ptr-ptr:dateTradingFrom
	a owl:DatatypeProperty ;
	rdfs:label "date trading from" ;
	rdfs:isDefinedBy <https://spec.edmcouncil.org/fibo/ontology/BE/Partnerships/Partnerships/> ;
	rdfs:range xsd:dateTime ;
	skos:definition "date on which the partnership started trading" ;
	.

fibo-be-ptr-ptr:holdsPartnershipEquityIn
	a owl:ObjectProperty ;
	rdfs:subPropertyOf fibo-fnd-oac-own:owns ;
	rdfs:label "holds partnership equity in" ;
	rdfs:isDefinedBy <https://spec.edmcouncil.org/fibo/ontology/BE/Partnerships/Partnerships/> ;
	rdfs:range fibo-be-ptr-ptr:PartnershipEquity ;
	skos:definition "relates a partner to the equity that partner holds in the partnership" ;
	.

fibo-be-ptr-ptr:setsOutEquityTermsIn
	a owl:ObjectProperty ;
	rdfs:subPropertyOf fibo-fnd-agr-ctr:hasTerms ;
	rdfs:label "sets out equity terms in" ;
	rdfs:domain fibo-be-le-fbo:OrganizationCoveringAgreement ;
	rdfs:isDefinedBy <https://spec.edmcouncil.org/fibo/ontology/BE/Partnerships/Partnerships/> ;
	rdfs:range fibo-be-ptr-ptr:EquityApportionmentTermsSet ;
	skos:definition "has terms setting out the apportionment of equity in some formal business organization" ;
	.

fibo-be-ptr-ptr:setsOutLiabilityTermsIn
	a owl:ObjectProperty ;
	rdfs:subPropertyOf fibo-fnd-agr-ctr:hasTerms ;
	rdfs:label "sets out liability terms in" ;
	rdfs:domain fibo-be-le-fbo:OrganizationCoveringAgreement ;
	rdfs:isDefinedBy <https://spec.edmcouncil.org/fibo/ontology/BE/Partnerships/Partnerships/> ;
	rdfs:range fibo-be-ptr-ptr:LiabilityApportionmentTermsSet ;
	skos:definition "has terms setting out the apportionment of liabilities for debts or other liabilities accrued by some formal business organization" ;
	.

