# baseURI: https://spec.edmcouncil.org/fibo/ontology/master/2018Q1/FND/Places/Facilities/
# imports: https://spec.edmcouncil.org/fibo/ontology/master/2018Q1/FND/Parties/Roles/
# imports: https://spec.edmcouncil.org/fibo/ontology/master/2018Q1/FND/Places/Addresses/
# imports: https://spec.edmcouncil.org/fibo/ontology/master/2018Q1/FND/Places/Locations/
# imports: https://spec.edmcouncil.org/fibo/ontology/master/2018Q1/FND/Relations/Relations/
# imports: https://spec.edmcouncil.org/fibo/ontology/master/2018Q1/FND/Utilities/AnnotationVocabulary/

@base <https://spec.edmcouncil.org/fibo/ontology/master/2018Q1/FND/Places/Facilities/> .
@prefix afn: <http://jena.apache.org/ARQ/function#> .
@prefix dc: <http://purl.org/dc/elements/1.1/> .
@prefix dct: <http://purl.org/dc/terms/> .
@prefix fibo-fnd-plc-adr: <https://spec.edmcouncil.org/fibo/ontology/FND/Places/Addresses/> .
@prefix fibo-fnd-plc-fac: <https://spec.edmcouncil.org/fibo/ontology/FND/Places/Facilities/> .
@prefix fibo-fnd-plc-loc: <https://spec.edmcouncil.org/fibo/ontology/FND/Places/Locations/> .
@prefix fibo-fnd-pty-rl: <https://spec.edmcouncil.org/fibo/ontology/FND/Parties/Roles/> .
@prefix fibo-fnd-rel-rel: <https://spec.edmcouncil.org/fibo/ontology/FND/Relations/Relations/> .
@prefix fibo-fnd-utl-av: <https://spec.edmcouncil.org/fibo/ontology/FND/Utilities/AnnotationVocabulary/> .
@prefix grddl: <http://www.w3.org/2003/g/data-view#> .
@prefix owl: <http://www.w3.org/2002/07/owl#> .
@prefix rdf: <http://www.w3.org/1999/02/22-rdf-syntax-ns#> .
@prefix rdfs: <http://www.w3.org/2000/01/rdf-schema#> .
@prefix skos: <http://www.w3.org/2004/02/skos/core#> .
@prefix sm: <http://www.omg.org/techprocess/ab/SpecificationMetadata/> .
@prefix xsd: <http://www.w3.org/2001/XMLSchema#> .

<https://spec.edmcouncil.org/fibo/ontology/FND/Places/Facilities/>
	a owl:Ontology ;
	rdfs:label "Facilities Ontology" ;
	dct:abstract "This ontology provides scaffolding for use in describing concepts related to facilities, both virtual and physical, including physical sites that provide various facilities." ;
	dct:license "http://opensource.org/licenses/MIT"^^xsd:anyURI ;
	sm:contentLanguage
		"http://www.omg.org/spec/ODM/"^^xsd:anyURI ,
		"http://www.w3.org/standards/techs/owl#w3c_all"^^xsd:anyURI
		;
	sm:copyright """Copyright (c) 2014 EDM Council, Inc.
Copyright (c) 2014 Object Management Group, Inc.""" ;
	sm:dependsOn
		"https://spec.edmcouncil.org/fibo/ontology/FND/Parties/Roles/"^^xsd:anyURI ,
		"https://spec.edmcouncil.org/fibo/ontology/FND/Places/Addresses/"^^xsd:anyURI ,
		"https://spec.edmcouncil.org/fibo/ontology/FND/Places/Locations/"^^xsd:anyURI ,
		"https://spec.edmcouncil.org/fibo/ontology/FND/Relations/Relations/"^^xsd:anyURI ,
		"https://spec.edmcouncil.org/fibo/ontology/FND/Utilities/AnnotationVocabulary/"^^xsd:anyURI
		;
	sm:fileAbbreviation "fibo-fnd-plc-fac" ;
	sm:filename "Facilities.rdf" ;
	rdfs:seeAlso
		"https://spec.edmcouncil.org/fibo/ontology/AboutTheEDMC-FIBOFamily/"^^xsd:anyURI ,
		"https://spec.edmcouncil.org/fibo/ontology/FND/AboutFND/"^^xsd:anyURI ,
		"https://spec.edmcouncil.org/fibo/ontology/FND/Places/AboutPlaces/"^^xsd:anyURI
		;
	owl:imports
		<https://spec.edmcouncil.org/fibo/ontology/master/2018Q1/FND/Parties/Roles/> ,
		<https://spec.edmcouncil.org/fibo/ontology/master/2018Q1/FND/Places/Addresses/> ,
		<https://spec.edmcouncil.org/fibo/ontology/master/2018Q1/FND/Places/Locations/> ,
		<https://spec.edmcouncil.org/fibo/ontology/master/2018Q1/FND/Relations/Relations/> ,
		<https://spec.edmcouncil.org/fibo/ontology/master/2018Q1/FND/Utilities/AnnotationVocabulary/>
		;
	owl:versionIRI <https://spec.edmcouncil.org/fibo/ontology/master/2018Q1/FND/Places/Facilities/> ;
	skos:changeNote "This ontology was added to Foundations in advance of the December 2014 Long Beach meeting in support of the SEC specification." ;
	fibo-fnd-utl-av:hasMaturityLevel fibo-fnd-utl-av:Release ;
	.

fibo-fnd-plc-fac:Capability
	a owl:Class ;
	rdfs:subClassOf [
		a owl:Restriction ;
		owl:onProperty fibo-fnd-rel-rel:involves ;
		owl:someValuesFrom fibo-fnd-plc-fac:Facility ;
	] ;
	rdfs:label "capability" ;
	rdfs:isDefinedBy <https://spec.edmcouncil.org/fibo/ontology/FND/Places/Facilities/> ;
	skos:definition "A capability represents the ability to perform a particular type of work and may involve people with particular skills and knowledge, intellectual property, defined practices, operating facilities, tools and equipment." ;
	fibo-fnd-utl-av:adaptedFrom "Value Delivery Modeling Language Specification, http://www.omg.org/spec/VDML/" ;
	.

fibo-fnd-plc-fac:Facility
	a owl:Class ;
	rdfs:subClassOf
		fibo-fnd-pty-rl:ThingInRole ,
		[
			a owl:Restriction ;
			owl:onProperty fibo-fnd-plc-fac:isSituatedAt ;
			owl:allValuesFrom fibo-fnd-plc-fac:Site ;
		] ,
		[
			a owl:Restriction ;
			owl:onProperty fibo-fnd-rel-rel:provides ;
			owl:someValuesFrom fibo-fnd-plc-fac:Capability ;
		]
		;
	rdfs:label "facility" ;
	rdfs:isDefinedBy <https://spec.edmcouncil.org/fibo/ontology/FND/Places/Facilities/> ;
	skos:definition "something that is built, contrived, established, or installed to serve a particular purpose, or make some course of action or operation easier, or provide some capability or service" ;
	fibo-fnd-utl-av:explanatoryNote "A facility may be concrete (as in a manufacturing facility) or abstract. Concrete facilities may be permanent, semi-permanent, or temporary structures, providing one or more capabilities at a given site.  A single site may include multiple facilities and a given facility may span multiple sites." ;
	.

fibo-fnd-plc-fac:PhysicalSite
	a owl:Class ;
	rdfs:subClassOf
		fibo-fnd-plc-fac:Site ,
		[
			a owl:Restriction ;
			owl:onProperty fibo-fnd-rel-rel:hasIdentity ;
			owl:onClass fibo-fnd-plc-adr:Address ;
			owl:qualifiedCardinality "1"^^xsd:nonNegativeInteger ;
		] ,
		[
			a owl:Restriction ;
			owl:onProperty fibo-fnd-plc-loc:isLocatedAt ;
			owl:onClass fibo-fnd-plc-loc:PhysicalLocation ;
			owl:qualifiedCardinality "1"^^xsd:nonNegativeInteger ;
		]
		;
	rdfs:label "physical site" ;
	rdfs:isDefinedBy <https://spec.edmcouncil.org/fibo/ontology/FND/Places/Facilities/> ;
	skos:definition "A physical site is a an actual location that situates something, typically a structure or building, archeological dig, landing location for an aircraft or spacecraft, etc.  From biology, this could also be the site of a wound, and active site, and so forth. A physical site has certain characteristics that contribute to the context it provides, including area, shape, accessibility, and in the case of a geographic site, landforms, soil and ground conditions, climate, and so forth." ;
	.

fibo-fnd-plc-fac:Site
	a owl:Class ;
	rdfs:subClassOf
		fibo-fnd-pty-rl:ThingInRole ,
		[
			a owl:Restriction ;
			owl:onProperty fibo-fnd-plc-loc:isLocatedAt ;
			owl:onClass fibo-fnd-plc-loc:Location ;
			owl:qualifiedCardinality "1"^^xsd:nonNegativeInteger ;
		] ,
		[
			a owl:Restriction ;
			owl:onProperty fibo-fnd-pty-rl:isPlayedBy ;
			owl:someValuesFrom [
				a owl:Restriction ;
				owl:onProperty fibo-fnd-plc-fac:situates ;
				owl:allValuesFrom owl:Thing ;
			] ;
		]
		;
	rdfs:label "site" ;
	rdfs:isDefinedBy <https://spec.edmcouncil.org/fibo/ontology/FND/Places/Facilities/> ;
	skos:definition "A site is a place, setting, or context in which something is situated." ;
	.

fibo-fnd-plc-fac:Venue
	a owl:Class ;
	rdfs:subClassOf
		fibo-fnd-plc-fac:Site ,
		[
			a owl:Restriction ;
			owl:onProperty fibo-fnd-rel-rel:hasContext ;
			owl:minCardinality "1"^^xsd:nonNegativeInteger ;
		]
		;
	rdfs:label "venue" ;
	rdfs:isDefinedBy <https://spec.edmcouncil.org/fibo/ontology/FND/Places/Facilities/> ;
	skos:definition "A place where something happens, described in the context of the event or activity that occurs there" ;
	.

fibo-fnd-plc-fac:hasLatitude
	a
		owl:DatatypeProperty ,
		owl:FunctionalProperty
		;
	rdfs:label "has latitude" ;
	sm:directSource "The National Atlas, nationalatlas.gov/articles/mapping/a_latlong.html" ;
	rdfs:isDefinedBy <https://spec.edmcouncil.org/fibo/ontology/FND/Places/Facilities/> ;
	rdfs:range xsd:string ;
	skos:definition "Latitude values indicate the angular distance between the Equator and points north or south of it on the surface of the Earth." ;
	.

fibo-fnd-plc-fac:hasLongitude
	a
		owl:DatatypeProperty ,
		owl:FunctionalProperty
		;
	rdfs:label "has longitude" ;
	sm:directSource "The National Atlas, nationalatlas.gov/articles/mapping/a_latlong.html" ;
	rdfs:isDefinedBy <https://spec.edmcouncil.org/fibo/ontology/FND/Places/Facilities/> ;
	rdfs:range xsd:string ;
	skos:definition "Lines of longitude, called meridians, run perpendicular to lines of latitude, and all pass through both poles. Longitude values indicate the angular distance between the Prime Meridian and points east or west of it on the surface of the Earth." ;
	.

fibo-fnd-plc-fac:isSituatedAt
	a owl:ObjectProperty ;
	rdfs:label "is situated at" ;
	rdfs:isDefinedBy <https://spec.edmcouncil.org/fibo/ontology/FND/Places/Facilities/> ;
	skos:definition "indicates that something has been positioned, located or placed at some site, or in some setting, situation, or context" ;
	.

fibo-fnd-plc-fac:situates
	a owl:ObjectProperty ;
	rdfs:label "situates" ;
	rdfs:isDefinedBy <https://spec.edmcouncil.org/fibo/ontology/FND/Places/Facilities/> ;
	owl:inverseOf fibo-fnd-plc-fac:isSituatedAt ;
	skos:definition "indicates the place, setting, or context in which something is situated" ;
	.

