# baseURI: https://spec.edmcouncil.org/fibo/ontology/master/2018Q1/BE/OwnershipAndControl/CorporateOwnership/
# imports: https://spec.edmcouncil.org/fibo/ontology/master/2018Q1/BE/Corporations/Corporations/
# imports: https://spec.edmcouncil.org/fibo/ontology/master/2018Q1/BE/LegalEntities/CorporateBodies/
# imports: https://spec.edmcouncil.org/fibo/ontology/master/2018Q1/BE/OwnershipAndControl/OwnershipParties/
# imports: https://spec.edmcouncil.org/fibo/ontology/master/2018Q1/FND/Accounting/AccountingEquity/
# imports: https://spec.edmcouncil.org/fibo/ontology/master/2018Q1/FND/AgentsAndPeople/Agents/
# imports: https://spec.edmcouncil.org/fibo/ontology/master/2018Q1/FND/Agreements/Contracts/
# imports: https://spec.edmcouncil.org/fibo/ontology/master/2018Q1/FND/Parties/Roles/
# imports: https://spec.edmcouncil.org/fibo/ontology/master/2018Q1/FND/Relations/Relations/
# imports: https://spec.edmcouncil.org/fibo/ontology/master/2018Q1/FND/Utilities/AnnotationVocabulary/

@base <https://spec.edmcouncil.org/fibo/ontology/master/2018Q1/BE/OwnershipAndControl/CorporateOwnership/> .
@prefix afn: <http://jena.apache.org/ARQ/function#> .
@prefix dc: <http://purl.org/dc/elements/1.1/> .
@prefix dct: <http://purl.org/dc/terms/> .
@prefix fibo-be-oac-cown: <https://spec.edmcouncil.org/fibo/ontology/BE/OwnershipAndControl/CorporateOwnership/> .
@prefix fibo-be-oac-opty: <https://spec.edmcouncil.org/fibo/ontology/BE/OwnershipAndControl/OwnershipParties/> .
@prefix fibo-fnd-acc-aeq: <https://spec.edmcouncil.org/fibo/ontology/FND/Accounting/AccountingEquity/> .
@prefix fibo-fnd-agr-ctr: <https://spec.edmcouncil.org/fibo/ontology/FND/Agreements/Contracts/> .
@prefix fibo-fnd-pty-rl: <https://spec.edmcouncil.org/fibo/ontology/FND/Parties/Roles/> .
@prefix fibo-fnd-utl-av: <https://spec.edmcouncil.org/fibo/ontology/FND/Utilities/AnnotationVocabulary/> .
@prefix grddl: <http://www.w3.org/2003/g/data-view#> .
@prefix owl: <http://www.w3.org/2002/07/owl#> .
@prefix rdf: <http://www.w3.org/1999/02/22-rdf-syntax-ns#> .
@prefix rdfs: <http://www.w3.org/2000/01/rdf-schema#> .
@prefix skos: <http://www.w3.org/2004/02/skos/core#> .
@prefix sm: <http://www.omg.org/techprocess/ab/SpecificationMetadata/> .
@prefix xsd: <http://www.w3.org/2001/XMLSchema#> .

<https://spec.edmcouncil.org/fibo/ontology/BE/OwnershipAndControl/CorporateOwnership/>
	a owl:Ontology ;
	rdfs:label "Corporate Ownership Ontology" ;
	dct:abstract "This ontology defines concepts relating to corporation-specific ownership. Roles are defined in terms of the ownership enjoyed by the party, and are the specific examples of these concepts as they apply to companies incorporated by the issuance of shares." ;
	dct:license "http://opensource.org/licenses/MIT"^^xsd:anyURI ;
	sm:contentLanguage
		"http://www.omg.org/spec/ODM/"^^xsd:anyURI ,
		"http://www.w3.org/standards/techs/owl#w3c_all"^^xsd:anyURI
		;
	sm:copyright """Copyright (c) 2013-2016 EDM Council, Inc.
Copyright (c) 2013-2016 Object Management Group, Inc.""" ;
	sm:dependsOn
		"https://spec.edmcouncil.org/fibo/ontology/BE/Corporations/Corporations/"^^xsd:anyURI ,
		"https://spec.edmcouncil.org/fibo/ontology/BE/OwnershipAndControl/OwnershipParties/"^^xsd:anyURI ,
		"https://spec.edmcouncil.org/fibo/ontology/FND/"^^xsd:anyURI
		;
	sm:fileAbbreviation "fibo-be-oac-cown" ;
	sm:filename "CorporateOwnership.rdf" ;
	rdfs:seeAlso
		"https://spec.edmcouncil.org/fibo/ontology/AboutTheEDMC-FIBOFamily/"^^xsd:anyURI ,
		"https://spec.edmcouncil.org/fibo/ontology/BE/AboutBE/"^^xsd:anyURI ,
		"https://spec.edmcouncil.org/fibo/ontology/BE/OwnershipAndControl/AboutBEOwnershipAndControl/"^^xsd:anyURI
		;
	owl:imports
		<https://spec.edmcouncil.org/fibo/ontology/master/2018Q1/BE/Corporations/Corporations/> ,
		<https://spec.edmcouncil.org/fibo/ontology/master/2018Q1/BE/LegalEntities/CorporateBodies/> ,
		<https://spec.edmcouncil.org/fibo/ontology/master/2018Q1/BE/OwnershipAndControl/OwnershipParties/> ,
		<https://spec.edmcouncil.org/fibo/ontology/master/2018Q1/FND/Accounting/AccountingEquity/> ,
		<https://spec.edmcouncil.org/fibo/ontology/master/2018Q1/FND/AgentsAndPeople/Agents/> ,
		<https://spec.edmcouncil.org/fibo/ontology/master/2018Q1/FND/Agreements/Contracts/> ,
		<https://spec.edmcouncil.org/fibo/ontology/master/2018Q1/FND/Parties/Roles/> ,
		<https://spec.edmcouncil.org/fibo/ontology/master/2018Q1/FND/Relations/Relations/> ,
		<https://spec.edmcouncil.org/fibo/ontology/master/2018Q1/FND/Utilities/AnnotationVocabulary/>
		;
	owl:versionIRI <https://spec.edmcouncil.org/fibo/ontology/master/2018Q1/BE/OwnershipAndControl/CorporateOwnership/> ;
	skos:changeNote "The https://spec.edmcouncil.org/fibo/ontology/BE/OwnershipAndControl/CorporateOwnership.rdf version of this ontology was modified per the issue resolutions identified in the FIBO BE 1.0 FTF report." ;
	fibo-fnd-utl-av:hasMaturityLevel fibo-fnd-utl-av:Release ;
	.

fibo-be-oac-cown:BeneficialOwner
	a owl:Class ;
	rdfs:subClassOf fibo-be-oac-cown:Shareholder ;
	rdfs:label "beneficial owner" ;
	rdfs:isDefinedBy <https://spec.edmcouncil.org/fibo/ontology/BE/OwnershipAndControl/CorporateOwnership/> ;
	skos:definition "Entity that enjoys the possession and/or benefits of ownership (such as receipt of income) of a property even though its ownership (title) is in the name of another entity (called a nominee or registered owner). Use of a nominee (who may be an agent, custodian, or a trustee) does not change the position regarding tax reporting and tax liability, and the beneficial-owner remains responsible." ;
	skos:editorialNote "This covers entities which have any kind of control. From World Bank Report: In identifying the beneficial owner, the focus should be on two factors: the control exercised and the benefit derived. Control of a corporate vehicle will always depend on context, as control can be exercised in many different ways, including through ownership, contractually or informally." ;
	fibo-fnd-utl-av:definitionOrigin "http://www.businessdictionary.com/definition/beneficial-owner.html"^^xsd:anyURI ;
	fibo-fnd-utl-av:synonym "actual owner" ;
	.

fibo-be-oac-cown:PublicShareholder
	a owl:Class ;
	rdfs:subClassOf fibo-be-oac-cown:Shareholder ;
	rdfs:label "public shareholder" ;
	rdfs:isDefinedBy <https://spec.edmcouncil.org/fibo/ontology/BE/OwnershipAndControl/CorporateOwnership/> ;
	skos:definition "a shareholder that holds publicly issued shares in a listed company" ;
	.

fibo-be-oac-cown:RegisteredShareholder
	a owl:Class ;
	rdfs:subClassOf fibo-be-oac-cown:Shareholder ;
	rdfs:label "registered shareholder" ;
	rdfs:isDefinedBy <https://spec.edmcouncil.org/fibo/ontology/BE/OwnershipAndControl/CorporateOwnership/> ;
	skos:definition "a shareholder that is registered on the shareholder registry for a company" ;
	.

fibo-be-oac-cown:Shareholder
	a owl:Class ;
	rdfs:subClassOf
		fibo-be-oac-opty:ConstitutionalOwner ,
		fibo-fnd-agr-ctr:TransferableContractHolder ,
		[
			a owl:Restriction ;
			owl:onProperty fibo-fnd-pty-rl:isPlayedBy ;
			owl:someValuesFrom [
				a owl:Restriction ;
				owl:onProperty fibo-be-oac-opty:holdsEquityIn ;
				owl:allValuesFrom fibo-fnd-acc-aeq:StockholdersEquity ;
			] ;
		]
		;
	rdfs:label "shareholder"@en ;
	rdfs:isDefinedBy <https://spec.edmcouncil.org/fibo/ontology/BE/OwnershipAndControl/CorporateOwnership/> ;
	skos:definition "An individual, group, or organization that owns one or more shares in a company, and in whose name the share certificate is issued.  It is legal for a company to have only one shareholder. Also called (in the US) stockholder." ;
	fibo-fnd-utl-av:definitionOrigin "http://www.businessdictionary.com/definition/shareholder.html"^^xsd:anyURI ;
	.

fibo-be-oac-cown:Shareholding
	a owl:Class ;
	rdfs:subClassOf
		fibo-fnd-acc-aeq:FinancialAsset ,
		[
			a owl:Restriction ;
			owl:onProperty fibo-be-oac-opty:isEquityHeldBy ;
			owl:allValuesFrom fibo-be-oac-cown:Shareholder ;
		]
		;
	rdfs:label "shareholding" ;
	rdfs:isDefinedBy <https://spec.edmcouncil.org/fibo/ontology/BE/OwnershipAndControl/CorporateOwnership/> ;
	skos:definition "Legal power of stockholders (shareholders) varies in proportion to their shareholdings. Typically, ten percent and below stockholding provides no protection. Fifteen percent stockholding may give the power to petition courts against changing the shares class rights. Up to 49.9 percent stockholding normally gives power to demand calling of an extraordinary general meeting. Fifty percent and over stockholding gives power to fire a director and force out minority stockholders by acquiring their shares as per the rules of the firm. Holder of 75 percent of the stock has the power to change the articles and memorandum of association and the firms name, reduce the share capital, allow the firm to buy its own shares from other stockholders, and to shut down the business. One hundred percent stockholding of course gives total power under the corporate legislation." ;
	fibo-fnd-utl-av:definitionOrigin "http://www.businessdictionary.com/definition/company-shareholdings.html"^^xsd:anyURI ;
	.

