# baseURI: https://spec.edmcouncil.org/fibo/ontology/master/2018Q1/BE/LegalEntities/LegalPersons/
# imports: https://spec.edmcouncil.org/fibo/ontology/master/2018Q1/FND/AgentsAndPeople/Agents/
# imports: https://spec.edmcouncil.org/fibo/ontology/master/2018Q1/FND/AgentsAndPeople/People/
# imports: https://spec.edmcouncil.org/fibo/ontology/master/2018Q1/FND/Agreements/Agreements/
# imports: https://spec.edmcouncil.org/fibo/ontology/master/2018Q1/FND/DatesAndTimes/BusinessDates/
# imports: https://spec.edmcouncil.org/fibo/ontology/master/2018Q1/FND/DatesAndTimes/FinancialDates/
# imports: https://spec.edmcouncil.org/fibo/ontology/master/2018Q1/FND/GoalsAndObjectives/Objectives/
# imports: https://spec.edmcouncil.org/fibo/ontology/master/2018Q1/FND/Law/Jurisdiction/
# imports: https://spec.edmcouncil.org/fibo/ontology/master/2018Q1/FND/Law/LegalCapacity/
# imports: https://spec.edmcouncil.org/fibo/ontology/master/2018Q1/FND/Organizations/FormalOrganizations/
# imports: https://spec.edmcouncil.org/fibo/ontology/master/2018Q1/FND/Parties/Parties/
# imports: https://spec.edmcouncil.org/fibo/ontology/master/2018Q1/FND/Parties/Roles/
# imports: https://spec.edmcouncil.org/fibo/ontology/master/2018Q1/FND/Relations/Relations/
# imports: https://spec.edmcouncil.org/fibo/ontology/master/2018Q1/FND/Utilities/AnnotationVocabulary/

@base <https://spec.edmcouncil.org/fibo/ontology/master/2018Q1/BE/LegalEntities/LegalPersons/> .
@prefix afn: <http://jena.apache.org/ARQ/function#> .
@prefix dc: <http://purl.org/dc/elements/1.1/> .
@prefix dct: <http://purl.org/dc/terms/> .
@prefix fibo-be-le-lp: <https://spec.edmcouncil.org/fibo/ontology/BE/LegalEntities/LegalPersons/> .
@prefix fibo-fnd-aap-agt: <https://spec.edmcouncil.org/fibo/ontology/FND/AgentsAndPeople/Agents/> .
@prefix fibo-fnd-aap-ppl: <https://spec.edmcouncil.org/fibo/ontology/FND/AgentsAndPeople/People/> .
@prefix fibo-fnd-agr-agr: <https://spec.edmcouncil.org/fibo/ontology/FND/Agreements/Agreements/> .
@prefix fibo-fnd-dt-bd: <https://spec.edmcouncil.org/fibo/ontology/FND/DatesAndTimes/BusinessDates/> .
@prefix fibo-fnd-dt-fd: <https://spec.edmcouncil.org/fibo/ontology/FND/DatesAndTimes/FinancialDates/> .
@prefix fibo-fnd-gao-obj: <https://spec.edmcouncil.org/fibo/ontology/FND/GoalsAndObjectives/Objectives/> .
@prefix fibo-fnd-law-jur: <https://spec.edmcouncil.org/fibo/ontology/FND/Law/Jurisdiction/> .
@prefix fibo-fnd-law-lcap: <https://spec.edmcouncil.org/fibo/ontology/FND/Law/LegalCapacity/> .
@prefix fibo-fnd-org-fm: <https://spec.edmcouncil.org/fibo/ontology/FND/Organizations/FormalOrganizations/> .
@prefix fibo-fnd-pty-pty: <https://spec.edmcouncil.org/fibo/ontology/FND/Parties/Parties/> .
@prefix fibo-fnd-pty-rl: <https://spec.edmcouncil.org/fibo/ontology/FND/Parties/Roles/> .
@prefix fibo-fnd-rel-rel: <https://spec.edmcouncil.org/fibo/ontology/FND/Relations/Relations/> .
@prefix fibo-fnd-utl-av: <https://spec.edmcouncil.org/fibo/ontology/FND/Utilities/AnnotationVocabulary/> .
@prefix grddl: <http://www.w3.org/2003/g/data-view#> .
@prefix owl: <http://www.w3.org/2002/07/owl#> .
@prefix rdf: <http://www.w3.org/1999/02/22-rdf-syntax-ns#> .
@prefix rdfs: <http://www.w3.org/2000/01/rdf-schema#> .
@prefix skos: <http://www.w3.org/2004/02/skos/core#> .
@prefix sm: <http://www.omg.org/techprocess/ab/SpecificationMetadata/> .
@prefix xsd: <http://www.w3.org/2001/XMLSchema#> .

<https://spec.edmcouncil.org/fibo/ontology/BE/LegalEntities/LegalPersons/>
	a owl:Ontology ;
	rdfs:label "Legal Persons Ontology" ;
	dct:abstract "This ontology defines legal personhood concepts. A legal person as defined here is any natural person or organization which is capable of accruing liability on its own part." ;
	dct:license "http://opensource.org/licenses/MIT"^^xsd:anyURI ;
	sm:contentLanguage
		"http://www.omg.org/spec/ODM/"^^xsd:anyURI ,
		"http://www.w3.org/standards/techs/owl#w3c_all"^^xsd:anyURI
		;
	sm:copyright """Copyright (c) 2013-2016 EDM Council, Inc.
Copyright (c) 2013-2016 Object Management Group, Inc.""" ;
	sm:dependsOn "https://spec.edmcouncil.org/fibo/ontology/FND/"^^xsd:anyURI ;
	sm:fileAbbreviation "fibo-be-le-lp" ;
	sm:filename "LegalPersons.rdf" ;
	rdfs:seeAlso
		"https://spec.edmcouncil.org/fibo/ontology/AboutTheEDMC-FIBOFamily/"^^xsd:anyURI ,
		"https://spec.edmcouncil.org/fibo/ontology/BE/AboutBE/"^^xsd:anyURI ,
		"https://spec.edmcouncil.org/fibo/ontology/BE/LegalEntities/AboutLegalEntities/"^^xsd:anyURI
		;
	owl:imports
		<https://spec.edmcouncil.org/fibo/ontology/master/2018Q1/FND/AgentsAndPeople/Agents/> ,
		<https://spec.edmcouncil.org/fibo/ontology/master/2018Q1/FND/AgentsAndPeople/People/> ,
		<https://spec.edmcouncil.org/fibo/ontology/master/2018Q1/FND/Agreements/Agreements/> ,
		<https://spec.edmcouncil.org/fibo/ontology/master/2018Q1/FND/DatesAndTimes/BusinessDates/> ,
		<https://spec.edmcouncil.org/fibo/ontology/master/2018Q1/FND/DatesAndTimes/FinancialDates/> ,
		<https://spec.edmcouncil.org/fibo/ontology/master/2018Q1/FND/GoalsAndObjectives/Objectives/> ,
		<https://spec.edmcouncil.org/fibo/ontology/master/2018Q1/FND/Law/Jurisdiction/> ,
		<https://spec.edmcouncil.org/fibo/ontology/master/2018Q1/FND/Law/LegalCapacity/> ,
		<https://spec.edmcouncil.org/fibo/ontology/master/2018Q1/FND/Organizations/FormalOrganizations/> ,
		<https://spec.edmcouncil.org/fibo/ontology/master/2018Q1/FND/Parties/Parties/> ,
		<https://spec.edmcouncil.org/fibo/ontology/master/2018Q1/FND/Parties/Roles/> ,
		<https://spec.edmcouncil.org/fibo/ontology/master/2018Q1/FND/Relations/Relations/> ,
		<https://spec.edmcouncil.org/fibo/ontology/master/2018Q1/FND/Utilities/AnnotationVocabulary/>
		;
	owl:versionIRI <https://spec.edmcouncil.org/fibo/ontology/master/2018Q1/BE/LegalEntities/LegalPersons/> ;
	skos:changeNote "The https://spec.edmcouncil.org/fibo/ontology/BE/LegalEntities/LegalPersons.rdf version of this ontology was modified per the issue resolutions identified in the FIBO BE 1.0 FTF report." ;
	fibo-fnd-utl-av:hasMaturityLevel fibo-fnd-utl-av:Release ;
	.

fibo-be-le-lp:BusinessEntity
	a owl:Class ;
	rdfs:subClassOf
		fibo-fnd-org-fm:FormalOrganization ,
		[
			a owl:Restriction ;
			owl:onProperty fibo-fnd-rel-rel:holds ;
			owl:onClass fibo-fnd-law-lcap:License ;
			owl:minQualifiedCardinality "0"^^xsd:nonNegativeInteger ;
		] ,
		[
			a owl:Restriction ;
			owl:onProperty fibo-be-le-lp:hasObjective ;
			owl:someValuesFrom fibo-be-le-lp:BusinessObjective ;
		]
		;
	rdfs:label "business entity" ;
	rdfs:isDefinedBy <https://spec.edmcouncil.org/fibo/ontology/BE/LegalEntities/LegalPersons/> ;
	skos:definition "an entity that is formed and administered as per commercial law in order to engage in business activities" ;
	fibo-fnd-utl-av:adaptedFrom
		"Barron's Dictionary of Business and Economics Terms, Fifth Edition, 2012" ,
		"http://en.wikipedia.org/wiki/Types_of_business_entity"^^xsd:anyURI
		;
	fibo-fnd-utl-av:explanatoryNote "There are many types of business entities defined in the legal systems of various countries. These include corporations, cooperatives, partnerships, sole proprietorships, sole traders, limited liability companies, certain trusts and trust companies, and so forth. The rules vary by country and by state or province. Some of the more widely recognized types in the US, UK, and EU are defined in FIBO, by region. However, the regulations governing particular types of entity, even those described as roughly equivalent, differ from jurisdiction to jurisdiction." ;
	.

fibo-be-le-lp:BusinessLicense
	a owl:Class ;
	rdfs:subClassOf
		fibo-fnd-law-lcap:License ,
		[
			a owl:Restriction ;
			owl:onProperty fibo-fnd-rel-rel:appliesTo ;
			owl:onClass fibo-be-le-lp:BusinessEntity ;
			owl:qualifiedCardinality "1"^^xsd:nonNegativeInteger ;
		] ,
		[
			a owl:Restriction ;
			owl:onProperty fibo-fnd-dt-bd:holdsDuring ;
			owl:onClass fibo-fnd-dt-fd:DatePeriod ;
			owl:qualifiedCardinality "1"^^xsd:nonNegativeInteger ;
		] ,
		[
			a owl:Restriction ;
			owl:onProperty fibo-be-le-lp:isRecognizedIn ;
			owl:someValuesFrom fibo-fnd-law-jur:Jurisdiction ;
		]
		;
	rdfs:label "business license" ;
	rdfs:isDefinedBy <https://spec.edmcouncil.org/fibo/ontology/BE/LegalEntities/LegalPersons/> ;
	skos:definition "a license that allows the holder to conduct business or carry out a specific profession within some jurisdiction for some period of time" ;
	fibo-fnd-utl-av:adaptedFrom "Barron's Dictionary of Business and Economics Terms, Fifth Edition, 2012" ;
	.

fibo-be-le-lp:BusinessObjective
	a owl:Class ;
	rdfs:subClassOf fibo-fnd-gao-obj:Objective ;
	rdfs:label "business objective" ;
	rdfs:isDefinedBy <https://spec.edmcouncil.org/fibo/ontology/BE/LegalEntities/LegalPersons/> ;
	skos:definition "an objective that reflects the strategic goals and direction of a business" ;
	fibo-fnd-utl-av:adaptedFrom "Barron's Dictionary of Business and Economics Terms, Fifth Edition, 2012" ;
	fibo-fnd-utl-av:explanatoryNote "Business objectives allow an organization to define its goals and direction. A company uses strategy and tactics at every level of its operation to achieve its objectives. These define the way a company allocates its resources and the strengths, weaknesses and opportunities it may have. Companies usually do not alter their objectives once they are implemented, unless changes in circumstances arise. Setting a clear course for the organization is key to its success." ;
	.

fibo-be-le-lp:CharteredLegalPerson
	a owl:Class ;
	rdfs:subClassOf fibo-be-le-lp:JuridicalPerson ;
	rdfs:label "chartered legal person" ;
	rdfs:isDefinedBy <https://spec.edmcouncil.org/fibo/ontology/BE/LegalEntities/LegalPersons/> ;
	skos:definition "a legal person created by a royal charter or decree" ;
	skos:editorialNote "In a monarchy or principality, the monarch typically vests the power to create such bodies, in an entity called (for example) the Privy Council." ;
	skos:example "Anything with 'Royal Institute' in the name. Also universities are generally set up by royal charter in a monarchy or principality, (often pre-dating any Privy Council i.e. directly be the monarch in the case of older universities). The Bank of England and the British Broadcasting Council (BBC) are also incorporated through Royal Charter." ;
	.

fibo-be-le-lp:JuridicalPerson
	a owl:Class ;
	rdfs:subClassOf
		fibo-be-le-lp:LegalEntity ,
		fibo-fnd-org-fm:FormalOrganization
		;
	rdfs:label "juridical person" ;
	rdfs:isDefinedBy <https://spec.edmcouncil.org/fibo/ontology/BE/LegalEntities/LegalPersons/> ;
	skos:definition "an entity, as a firm, that is not a single natural person, as a human being, authorized by law with duties and rights, recognized as a legal authority having a distinct identity, a legal personality" ;
	fibo-fnd-utl-av:definitionOrigin "Black's Law Dictionary Free Online, see http://thelawdictionary.org/juridical-person/" ;
	fibo-fnd-utl-av:synonym
		"artificial person" ,
		"juridical entity" ,
		"juristic person"
		;
	.

fibo-be-le-lp:LegalEntity
	a owl:Class ;
	rdfs:subClassOf
		fibo-be-le-lp:LegalPerson ,
		[
			a owl:Restriction ;
			owl:onProperty fibo-be-le-lp:isOrganizedIn ;
			owl:onClass fibo-fnd-law-jur:Jurisdiction ;
			owl:qualifiedCardinality "1"^^xsd:nonNegativeInteger ;
		]
		;
	rdfs:label "legal entity" ;
	rdfs:isDefinedBy <https://spec.edmcouncil.org/fibo/ontology/BE/LegalEntities/LegalPersons/> ;
	owl:disjointWith fibo-be-le-lp:NaturalPerson ;
	skos:definition "a partnership, corporation, or other organization having the capacity to negotiate contracts, assume financial obligations, and pay off debts, organized under the laws of some jurisdiction" ;
	skos:example """Examples of eligible legal entities include, without limitation:
-   all financial intermediaries;
-   banks and finance companies;
-   all entities that issue equity, debt or other securities for other capital structures;
-   all entities listed on an exchange;
-   all entities that trade stock or debt, investment vehicles, including mutual funds, pension funds and alternative investment vehicles constituted as corporate entities or collective investment agreements (including umbrella funds as well as funds under an umbrella structure, hedge funds, private equity funds, etc.);
-   all entities under the purview of a financial regulator and their affiliates, subsidiaries and holding companies;
-   counterparties to financial transactions.""" ;
	skos:scopeNote "The term 'legal entities' includes, but is not limited to, unique parties that are legally or financially responsible for the performance of financial transactions or have the legal right in their jurisdiction to enter independently into legal contracts, regardless of whether they are incorporated or constituted in some other way (e.g. trust, partnership, contractual). It excludes natural persons, but includes governmental organizations and supranationals." ;
	fibo-fnd-utl-av:adaptedFrom
		"Barron's Dictionary of Banking Terms, Sixth Edition, 2012, definition of legal entity" ,
		"ISO 17442, Financial services - Legal Entity Identifier (LEI), first edition, 2012-06-01, section 3.1"
		;
	.

fibo-be-le-lp:LegalPerson
	a owl:Class ;
	rdfs:subClassOf
		fibo-fnd-aap-agt:AutonomousAgent ,
		[
			a owl:Restriction ;
			owl:onProperty fibo-be-le-lp:isRecognizedIn ;
			owl:onClass fibo-fnd-law-jur:Jurisdiction ;
			owl:minQualifiedCardinality "1"^^xsd:nonNegativeInteger ;
		] ,
		[
			a owl:Restriction ;
			owl:onProperty fibo-fnd-law-lcap:hasCapacity ;
			owl:onClass fibo-fnd-law-lcap:LiabilityCapacity ;
			owl:minQualifiedCardinality "1"^^xsd:nonNegativeInteger ;
		]
		;
	rdfs:label "legal person"@en ;
	rdfs:isDefinedBy <https://spec.edmcouncil.org/fibo/ontology/BE/LegalEntities/LegalPersons/> ;
	skos:definition "any entity which can incur legal obligation and can be sued at law" ;
	fibo-fnd-utl-av:adaptedFrom "http://en.wikipedia.org/wiki/Legal_personality"^^xsd:anyURI ;
	fibo-fnd-utl-av:explanatoryNote "To have legal personality means to be capable of having legal rights and duties within a certain legal system, such as to enter into contracts, sue, and be sued. Legal personality is a prerequisite to legal capacity, the ability of any legal person to amend (enter into, transfer, etc.) rights and obligations." ;
	.

fibo-be-le-lp:NaturalPerson
	a owl:Class ;
	rdfs:subClassOf
		fibo-be-le-lp:LegalPerson ,
		fibo-fnd-aap-ppl:Adult
		;
	rdfs:label "natural person"@en ;
	rdfs:isDefinedBy <https://spec.edmcouncil.org/fibo/ontology/BE/LegalEntities/LegalPersons/> ;
	owl:disjointWith fibo-fnd-aap-ppl:IncapacitatedAdult ;
	skos:definition "A person of maturity who in the eyes of the law is able to assume obligations." ;
	.

fibo-be-le-lp:NotForProfitObjective
	a owl:Class ;
	rdfs:subClassOf fibo-fnd-gao-obj:Objective ;
	rdfs:label "not for profit objective" ;
	rdfs:isDefinedBy <https://spec.edmcouncil.org/fibo/ontology/BE/LegalEntities/LegalPersons/> ;
	owl:disjointWith fibo-be-le-lp:ProfitObjective ;
	skos:definition "an objective that reflects the charitable, educational, religious, humanitarian, public services, or other not for profit goals of an organization" ;
	fibo-fnd-utl-av:adaptedFrom
		"Barron's Dictionary of Business and Economics Terms, Fifth Edition, 2012" ,
		"http://www.investopedia.com/terms/n/not-for-profit.asp"^^xsd:anyURI
		;
	fibo-fnd-utl-av:explanatoryNote "The objective of all business activities is not to earn profits for its owners. All of the money earned by or donated to a not for profit organization is used in pursuing the organization's objectives." ;
	fibo-fnd-utl-av:synonym "nonprofit objective" ;
	.

fibo-be-le-lp:PowerOfAttorney
	a owl:Class ;
	rdfs:subClassOf
		fibo-fnd-law-lcap:LegalCapacity ,
		[
			a owl:Restriction ;
			owl:onProperty fibo-fnd-rel-rel:isConferredOn ;
			owl:onClass fibo-be-le-lp:NaturalPerson ;
			owl:minQualifiedCardinality "1"^^xsd:nonNegativeInteger ;
		]
		;
	rdfs:label "power of attorney" ;
	rdfs:isDefinedBy <https://spec.edmcouncil.org/fibo/ontology/BE/LegalEntities/LegalPersons/> ;
	skos:definition "Written legal authority given by one party (the principal) to another (the agent or attorney-in-fact) to act on the principals behalf. It may be a (1) General power Of attorney that authorizes the agent to act generally on behalf of the principal, or (2) Special power of attorney that is limited to a specific act or situation. Decisions made and actions taken by an attorney in fact (within the scope of his or her authority) are legally binding on the principal. A power of attorney can remain in force only so long as the principal is alive and does not become disabled or incapacitated. Although it is often conferred on the principals attorney, one does not need to be an attorney at law to be an attorney-in-fact." ;
	fibo-fnd-utl-av:definitionOrigin "http://www.businessdictionary.com/definition/power-of-attorney.html"^^xsd:anyURI ;
	.

fibo-be-le-lp:ProfitObjective
	a owl:Class ;
	rdfs:subClassOf fibo-be-le-lp:BusinessObjective ;
	rdfs:label "profit objective" ;
	rdfs:isDefinedBy <https://spec.edmcouncil.org/fibo/ontology/BE/LegalEntities/LegalPersons/> ;
	skos:definition "an objective that reflects pursuit of a financial benefit that may be realized when the amount of revenue gained from a business activity exceeds the expenses, costs and taxes needed to sustain that activity" ;
	fibo-fnd-utl-av:adaptedFrom
		"Barron's Dictionary of Business and Economics Terms, Fifth Edition, 2012" ,
		"http://www.investopedia.com/terms/p/profit.asp"^^xsd:anyURI
		;
	fibo-fnd-utl-av:explanatoryNote "Any profit that is gained goes to the business's owners, who may or may not decide to spend it on the business." ;
	fibo-fnd-utl-av:synonym
		"for profit objective" ,
		"profit motive"
		;
	.

fibo-be-le-lp:PublicPurpose
	a owl:Class ;
	rdfs:subClassOf fibo-fnd-gao-obj:Objective ;
	rdfs:label "public purpose" ;
	rdfs:isDefinedBy <https://spec.edmcouncil.org/fibo/ontology/BE/LegalEntities/LegalPersons/> ;
	skos:definition "an objective that reflects values generally thought to be shared by and that is intended to benefit the populace as a whole" ;
	fibo-fnd-utl-av:adaptedFrom
		"Barron's Dictionary of Business and Economics Terms, Fifth Edition, 2012" ,
		"http://www.yourdictionary.com/public-purpose"^^xsd:anyURI
		;
	fibo-fnd-utl-av:synonym "public interest" ;
	.

fibo-be-le-lp:ReligiousObjective
	a owl:Class ;
	rdfs:subClassOf fibo-be-le-lp:NotForProfitObjective ;
	rdfs:label "religious objective" ;
	rdfs:isDefinedBy <https://spec.edmcouncil.org/fibo/ontology/BE/LegalEntities/LegalPersons/> ;
	skos:definition "a not for profit objective that reflects the religious goals of an organization" ;
	.

fibo-be-le-lp:Signatory
	a owl:Class ;
	rdfs:subClassOf
		fibo-fnd-pty-pty:PartyInRole ,
		[
			a owl:Restriction ;
			owl:onProperty fibo-fnd-rel-rel:hasIdentity ;
			owl:onClass fibo-be-le-lp:NaturalPerson ;
			owl:qualifiedCardinality "1"^^xsd:nonNegativeInteger ;
		] ,
		[
			a owl:Restriction ;
			owl:onProperty fibo-fnd-pty-rl:isPlayedBy ;
			owl:someValuesFrom [
				a owl:Restriction ;
				owl:onProperty fibo-fnd-law-lcap:hasCapacity ;
				owl:onClass fibo-fnd-law-lcap:SignatoryCapacity ;
				owl:minQualifiedCardinality "1"^^xsd:nonNegativeInteger ;
			] ;
		]
		;
	rdfs:label "signatory" ;
	rdfs:isDefinedBy <https://spec.edmcouncil.org/fibo/ontology/BE/LegalEntities/LegalPersons/> ;
	skos:definition "Some agent who has the capacity to sign contracts on the part of some legal person" ;
	.

fibo-be-le-lp:StatutoryBody
	a owl:Class ;
	rdfs:subClassOf fibo-be-le-lp:JuridicalPerson ;
	rdfs:label "statutory body" ;
	rdfs:isDefinedBy <https://spec.edmcouncil.org/fibo/ontology/BE/LegalEntities/LegalPersons/> ;
	skos:definition "a body set up by a government to consider evidence and make judgements in some field of activity" ;
	fibo-fnd-utl-av:adaptedFrom "http://www.collinsdictionary.com/dictionary/english/statutory-body"^^xsd:anyURI ;
	.

fibo-be-le-lp:designatesSignatory
	a owl:ObjectProperty ;
	rdfs:subPropertyOf fibo-fnd-rel-rel:designates ;
	rdfs:label "designates signatory" ;
	rdfs:domain fibo-be-le-lp:LegalPerson ;
	rdfs:isDefinedBy <https://spec.edmcouncil.org/fibo/ontology/BE/LegalEntities/LegalPersons/> ;
	rdfs:range fibo-be-le-lp:Signatory ;
	skos:definition "designates a party able to sign contracts on the part of the legal person" ;
	.

fibo-be-le-lp:hasObjective
	a owl:ObjectProperty ;
	rdfs:subPropertyOf fibo-fnd-rel-rel:has ;
	rdfs:label "has objective" ;
	rdfs:domain fibo-fnd-aap-agt:AutonomousAgent ;
	rdfs:isDefinedBy <https://spec.edmcouncil.org/fibo/ontology/BE/LegalEntities/LegalPersons/> ;
	rdfs:range fibo-fnd-gao-obj:Objective ;
	skos:definition "relates an agent to a specific objective (result) that the agent aims to achieve within a time frame and with available resources" ;
	fibo-fnd-utl-av:adaptedFrom "http://www.businessdictionary.com/definition/objective.html"^^xsd:anyURI ;
	.

fibo-be-le-lp:isOrganizedIn
	a owl:ObjectProperty ;
	rdfs:subPropertyOf fibo-be-le-lp:isRecognizedIn ;
	rdfs:label "is organized in" ;
	rdfs:domain fibo-be-le-lp:LegalEntity ;
	rdfs:isDefinedBy <https://spec.edmcouncil.org/fibo/ontology/BE/LegalEntities/LegalPersons/> ;
	rdfs:range fibo-fnd-law-jur:Jurisdiction ;
	skos:definition "indicates the juridiction whose laws a legal entity is organized under" ;
	.

fibo-be-le-lp:isRecognizedIn
	a owl:ObjectProperty ;
	rdfs:label "is recognized in" ;
	rdfs:domain [
		a owl:Class ;
		owl:unionOf (
			fibo-be-le-lp:LegalPerson
			fibo-fnd-agr-agr:Agreement
		) ;
	] ;
	rdfs:isDefinedBy <https://spec.edmcouncil.org/fibo/ontology/BE/LegalEntities/LegalPersons/> ;
	rdfs:range fibo-fnd-law-jur:Jurisdiction ;
	skos:definition "indicates the jurisdiction in which a legal person is authorized to conduct business or an agreement may be acknowledged and possibly enforceable" ;
	.

