# baseURI: <http://data.archieven.nl/pnv/>

@prefix edm: <http://www.europeana.eu/schemas/edm/> .
@prefix owl: <http://www.w3.org/2002/07/owl#> .
@prefix rdf: <http://www.w3.org/1999/02/22-rdf-syntax-ns#> .
@prefix rdfs: <http://www.w3.org/2000/01/rdf-schema#> .
@prefix skos: <http://www.w3.org/2004/02/skos/core#> .
@prefix xsd: <http://www.w3.org/2001/XMLSchema#> .
@prefix dbo: <http://dbpedia.org/ontology/> .
@prefix dbp: <http://nl.dbpedia.org/resource/> .
@prefix foaf: <http://xmlns.com/foaf/0.1/> .
@prefix dc: <http://purl.org/dc/elements/1.1/> .
@prefix dct: <http://purl.org/dc/terms/> .
@prefix dcat: <http://www.w3.org/ns/dcat#> .
@prefix prov: <http://www.w3.org/ns/prov#> .
@prefix sh: <http://www.w3.org/ns/shacl#> .
@prefix nco: <http://www.semanticdesktop.org/ontologies/2007/03/22/nco#> .
@prefix org: <http://www.w3.org/ns/org#> .
@prefix vcard: <http://www.w3.org/2006/vcard/ns#> .
@prefix bf: <http://id.loc.gov/ontologies/bibframe/> .
@prefix eac-cpf: <http://www3.iath.virginia.edu/eac/cpf/> .
@prefix cidoc: <http://www.cidoc-crm.org/cidoc-crm/> .
@prefix bgn: <http://biographynet.nl/schema/> .
@prefix sem: <http://semanticweb.cs.vu.nl/2009/11/sem/> .
@prefix def: <http://almere.pilod.nl/NadereToegangen/ontology/> .
@prefix commBk: <http://almere.pilod.nl/NadereToegang/resource/Commissieboeken/> .

@prefix pnvDef: <http://data.archieven.nl/pnv/def/> .
@prefix pnv: <http://data.archieven.nl/pnv/> .
@prefix schema: <http://schema.org/> .


# === Defining a Person ====


pnvDef:Person a owl:Class  ;
    rdfs:label "Person"^^xsd:string ;
    owl:equivalentClass foaf:Person , bgn:Person , def:PersonEntity , schema:Person , cidoc:E21_person , foaf:Person , dbo:Person ;
    rdfs:comment "A Person is a human being whose individual existence can somehow be documented"^^xsd:string ;
.

# == Classes for Persons according to the BiographyNet model (partly still the same as BioDes) ==


pnvDef:PersonName rdf:type owl:Class ;
  rdfs:label "A Person's name"^^xsd:string ;
  owl:disjointWith pnvDef:Person ;
  owl:equivalentClass dbo:Name , bgn:Name ;
  rdfs:comment "A name is considered to be a resource type in its own right"^^xsd:string ;
.

# == Properties for naming and identifying persons ==

pnvDef:hasCountry rdf:type owl:ObjectProperty ;
  rdfs:domain pnvDef:Person ;
  rdfs:range dbo:Country ;
  rdfs:label "Has residence in country"^^xsd:string ;
  owl:equivalentProperty dbo:country ;
.
pnvDef:hasName rdf:type owl:ObjectProperty ;
  rdfs:domain pnvDef:Person ;
  rdfs:label "Has name"^^xsd:string ;
  rdfs:range pnvDef:PersonName ;
.

# === For sex/gender schema:gender is to be used ===
# === schema:gender is a property that may have as its range either a resource (http://schema.org/Male or http://schema.org/Female) or a text string ===

# == Properties for extension on BiographyNet == 

pnvDef:fullname rdf:type owl:DatatypeProperty ;
  rdfs:domain pnvDef:PersonName ;
  rdfs:label "Full name"^^xsd:string ;
  owl:equivalentProperty dbo:fullName ;
  rdfs:comment "Every person has to have a full name. If a name is not known at all, a text like 'Unknown' should be used"^^xsd:string ;
  rdfs:range xsd:string ;
.
pnvDef:maidenName rdf:type owl:DatatypeProperty ;
  rdfs:domain pnvDef:PersonName ;
  rdfs:label "Maiden name"^^xsd:string ;
  owl:equivalentProperty dbo:fullName ;
  rdfs:comment "A woman's family name preceding the name when after marriage she took the name of her husband, or combined both names"^^xsd:string ;
  rdfs:range xsd:string ;
.
pnvDef:prefix rdf:type owl:DatatypeProperty ;
  rdfs:domain pnvDef:PersonName ;
  rdfs:label "Prefix"^^xsd:string ;
  rdfs:comment "A Prefix designates a title of nobility or a civil grade"^^xsd:string ;
  rdfs:range xsd:string ;
.
pnvDef:familyName rdf:type owl:DatatypeProperty ;
  rdfs:domain pnvDef:PersonName ;
  rdfs:label "Family name"^^xsd:string ;
  rdfs:comment "A Family name is the name of the family a person is born into"^^xsd:string ;
  rdfs:range xsd:string ;
.
pnvDef:familyNamePrefix rdf:type owl:DatatypeProperty ;
  rdfs:domain pnvDef:PersonName ;
  rdfs:label "Family name prefix"^^xsd:string ;
  rdfs:comment "A Family name prefix refers to a preceding part of the family name"^^xsd:string ;
  rdfs:range xsd:string ;
.
pnvDef:firstName rdf:type owl:DatatypeProperty ;
  rdfs:domain pnvDef:PersonName ;
  rdfs:label "First name"^^xsd:string ;
  owl:equivalentProperty foaf:firstName , pnvDef:givenName ;
  rdfs:range xsd:string ;
  rdfs:comment "A First name is the same as a Given name"^^xsd:string ;
.
pnvDef:givenName rdf:type owl:DatatypeProperty ;
  rdfs:domain pnvDef:PersonName ;
  rdfs:label "Given name"^^xsd:string ;
  owl:equivalentProperty schema:givenName , pnvDef:firstName ;
  rdfs:range xsd:string ;
  rdfs:comment "A Given name designates the name(s) given to someone at birth"^^xsd:string ;
.
pnvDef:patronym rdf:type owl:DatatypeProperty ;
  rdfs:domain pnvDef:PersonName ;
  rdfs:label "Patronym"^^xsd:string ;
  rdfs:range xsd:string ;
  rdfs:comment "A Patronym refers to the father's name"^^xsd:string ;
.
pnvDef:trailingPatronym rdf:type owl:DatatypeProperty ;
  rdfs:subPropertyOf pnvDef:patronym ;
  rdfs:domain pnvDef:PersonName ;
  rdfs:label "Trailing patronym"^^xsd:string ;
  rdfs:range xsd:string ;
  rdfs:comment "A Trailing patronym refers to the father's name at the end of one's own name, mostly for disambiguation"^^xsd:string ;
.
pnvDef:infix rdf:type owl:DatatypeProperty ;
  rdfs:domain pnvDef:PersonName ;
  rdfs:label "Infix"^^xsd:string ;
  rdfs:comment "An Infix designates a name part in the middle of a name"^^xsd:string ;
  rdfs:range xsd:string ;
.
pnvDef:infixTitle rdf:type owl:DatatypeProperty ;
  rdfs:subPropertyOf pnvDef:infix ;
  rdfs:domain pnvDef:PersonName ;
  rdfs:label "Infix title"^^xsd:string ;
  rdfs:comment "An Infix title designates a title in the middle of a name"^^xsd:string ;
  rdfs:range xsd:string ;
.
pnvDef:suffix rdf:type owl:DatatypeProperty ;
  rdfs:domain pnvDef:PersonName ;
  rdfs:label "Suffix"^^xsd:string ;
  rdfs:comment "A Suffix is a name part that is appended to another name part"^^xsd:string ;
  rdfs:range xsd:string ;
.
pnvDef:honorificSuffix rdf:type owl:DatatypeProperty ;
  rdfs:subPropertyOf pnvDef:suffix ;
  rdfs:domain pnvDef:PersonName ;
  rdfs:label "Honorific suffix"^^xsd:string ;
  rdfs:comment "A Honorific suffix is a name part that is appended to distinguish someone"^^xsd:string ;
  rdfs:range xsd:string ;
.
pnvDef:disambiguatingDescription rdf:type owl:DatatypeProperty ;
  rdfs:subPropertyOf pnvDef:suffix ;
  rdfs:domain pnvDef:PersonName ;
  rdfs:label "Disambiguating description"^^xsd:string ;
  owl:equivalentProperty schema:disambiguatingDescription ;
  rdfs:comment "A Disambiguating description is a name part that is appended to make sure that the right person is designated"^^xsd:string ;
  rdfs:range xsd:string ;
.

# == Some definitions to keep the link to the Commissions ==

def:hasMember rdf:type owl:ObjectProperty ;
   rdfs:domain rdf:List ;
   rdfs:label "Deel in verzameling"^^xsd:string ;
   rdfs:comment "Extension meant to specify that the individual who is member of the List is the rdfs:domain, whereas for the range, an indvidual Resource is the part of the list"@en ;
   rdfs:range rdf:Resource ;
   owl:inverseOf def:memberOf ;
   skos:prefLabel "Deel in verzameling"@nl ;
   rdfs:subPropertyOf rdfs:member ;
.
def:memberOf rdf:type owl:ObjectProperty ;
   rdfs:domain rdf:Resource ;
   rdfs:label "Deel van verzameling"^^xsd:string ;
   rdfs:comment "Extension meant to specify that the Resource is the domain, whereas for the range, the List is the collection of which the Resource is part"@en ;
   rdfs:range rdf:List ;
   owl:inverseOf def:hasMember ;
   skos:prefLabel "Deel van verzameling"@nl ;
   rdfs:subPropertyOf rdfs:member ;
.

# == A List to keep the Persons who got into the Commission Books at hand, figuratively speaking ==


commBk:PersonenLijst a rdf:List , owl:NamedIndividual , prov:Entity ;
               rdfs:label "De lijst van unieke personen (resources met URI obv uniek gemaakte naam)"^^xsd:string ;
               prov:wasGeneratedBy [ a prov:Activity ; prov:startedAtTime "2017-02-13T01:01:01Z"^^xsd:dateTime ] ; 
.

