@prefix : <http://vocab.getty.edu/ontology/> .
@prefix cc: <http://creativecommons.org/ns#> .
@prefix dc: <http://purl.org/dc/elements/1.1/> .
@prefix rr: <http://www.w3.org/ns/r2rml#> .
@prefix sd: <http://www.w3.org/ns/sparql-service-description#> .
@prefix wv: <http://vocab.org/waiver/terms/> .
@prefix aat: <http://vocab.getty.edu/aat/> .
@prefix bio: <http://purl.org/vocab/bio/0.1/> .
@prefix dct: <http://purl.org/dc/terms/> .
@prefix fmt: <http://www.w3.org/ns/formats/> .
@prefix gvp: <http://vocab.getty.edu/ontology#> .
@prefix iso: <http://purl.org/iso25964/skos-thes#> .
@prefix luc: <http://www.ontotext.com/owlim/lucene#> .
@prefix owl: <http://www.w3.org/2002/07/owl#> .
@prefix rdf: <http://www.w3.org/1999/02/22-rdf-syntax-ns#> .
@prefix rrx: <http://purl.org/r2rml-ext/> .
@prefix tgn: <http://vocab.getty.edu/tgn/> .
@prefix wgs: <http://www.w3.org/2003/01/geo/wgs84_pos#> .
@prefix xml: <http://www.w3.org/XML/1998/namespace> .
@prefix xsd: <http://www.w3.org/2001/XMLSchema#> .
@prefix adms: <http://www.w3.org/ns/adms#> .
@prefix bibo: <http://purl.org/ontology/bibo/> .
@prefix dcat: <http://www.w3.org/ns/dcat#> .
@prefix foaf: <http://xmlns.com/foaf/0.1/> .
@prefix prov: <http://www.w3.org/ns/prov#> .
@prefix ptop: <http://www.ontotext.com/proton/protontop#> .
@prefix rdfs: <http://www.w3.org/2000/01/rdf-schema#> .
@prefix skos: <http://www.w3.org/2004/02/skos/core#> .
@prefix ulan: <http://vocab.getty.edu/ulan/> .
@prefix vaem: <http://www.linkedmodel.org/schema/vaem#> .
@prefix vann: <http://purl.org/vocab/vann/> .
@prefix vdpp: <http://data.lirmm.fr/ontologies/vdpp#> .
@prefix voaf: <http://purl.org/vocommons/voaf#> .
@prefix voag: <http://voag.linkedmodel.org/voag#> .
@prefix void: <http://rdfs.org/ns/void#> .
@prefix wdrs: <http://www.w3.org/2007/05/powder-s#> .
@prefix vcard: <http://www.w3.org/2006/vcard/ns#> .
@prefix dctype: <http://purl.org/dc/dcmitype/> .
@prefix schema: <http://schema.org/> .
@prefix sesame: <http://www.openrdf.org/schema/sesame#> .
@prefix skosxl: <http://www.w3.org/2008/05/skos-xl#> .
@prefix aat_rel: <http://vocab.getty.edu/aat/rel/> .
@prefix aat_rev: <http://vocab.getty.edu/aat/rev/> .
@prefix ontogeo: <http://www.ontotext.com/owlim/geo#> .
@prefix tgn_rel: <http://vocab.getty.edu/tgn/rel/> .
@prefix tgn_rev: <http://vocab.getty.edu/tgn/rev/> .
@prefix aat_term: <http://vocab.getty.edu/aat/term/> .
@prefix gvp_lang: <http://vocab.getty.edu/language/> .
@prefix tgn_term: <http://vocab.getty.edu/tgn/term/> .
@prefix ulan_bio: <http://vocab.getty.edu/ulan/bio/> .
@prefix ulan_rel: <http://vocab.getty.edu/ulan/rel/> .
@prefix ulan_rev: <http://vocab.getty.edu/ulan/rev/> .
@prefix ulan_term: <http://vocab.getty.edu/ulan/term/> .
@prefix aat_source: <http://vocab.getty.edu/aat/source/> .
@prefix tgn_source: <http://vocab.getty.edu/tgn/source/> .
@prefix ulan_event: <http://vocab.getty.edu/ulan/event/> .
@prefix aat_contrib: <http://vocab.getty.edu/aat/contrib/> .
@prefix tgn_contrib: <http://vocab.getty.edu/tgn/contrib/> .
@prefix ulan_source: <http://vocab.getty.edu/ulan/source/> .
@prefix ulan_contrib: <http://vocab.getty.edu/ulan/contrib/> .
@prefix aat_scopeNote: <http://vocab.getty.edu/aat/scopeNote/> .
@prefix tgn_scopeNote: <http://vocab.getty.edu/tgn/scopeNote/> .
@prefix aat_source_rev: <http://vocab.getty.edu/aat/source/rev/> .
@prefix tgn_source_rev: <http://vocab.getty.edu/tgn/source/rev/> .
@prefix ulan_scopeNote: <http://vocab.getty.edu/ulan/scopeNote/> .
@prefix ulan_source_rev: <http://vocab.getty.edu/ulan/source/rev/> .
@base <http://vocab.getty.edu/ontology> .

<http://vocab.getty.edu/ontology> rdf:type owl:Ontology ;
                                   owl:imports <http://www.w3.org/2008/05/skos-xl> ,
                                               <http://purl.org/iso25964/skos-thes> ,
                                               <http://www.w3.org/2004/02/skos/core> ;
                                   dct:creator <http://www.getty.edu/research/> ;
                                   rdfs:label "Getty Vocabulary Program ontology" ;
                                   rdfs:seeAlso <http://vocab.getty.edu/.well-known/void> ;
                                   dc:format "meta/rdf-schema" ;
                                   dct:modified "2016-04-25"^^xsd:date ;
                                   dct:issued "2014-02-20"^^xsd:date ;
                                   owl:versionInfo "3.3" ;
                                   skos:changeNote <http://vocab.getty.edu/doc#Version_2.0> ;
                                   rdfs:seeAlso <http://vocab.getty.edu/doc/queries> ;
                                   skos:changeNote <http://vocab.getty.edu/doc#Version_3.0> ;
                                   rdfs:seeAlso <http://vocab.getty.edu/doc> ;
                                   vann:preferredNamespacePrefix "gvp" ;
                                   rdfs:comment """The GVP Ontology defines classes, properties and values (skos:Concepts) used in GVP LOD.
As of version 3.0, it is complete regarding AAT, TGN and ULAN, and will be extended in time with more elements needed for other GVP vocabularies (CONA).
It uses the SKOS, SKOS-XL, ISO 25964; DC, DCT, BIBO, FOAF, BIO, Schema, PROV, WGS84 ontologies, but we import only the first 3""" ;
                                   dct:created "2014-02-15"^^xsd:date ;
                                   dct:creator <http://www.ontotext.com> ;
                                   rdfs:seeAlso <http://lov.okfn.org/dataset/lov/details/vocabulary_gvp.html> ;
                                   skos:changeNote <http://vocab.getty.edu/doc#Version_3.3> ;
                                   vann:preferredNamespaceUri "http://vocab.getty.edu/ontology#" ;
                                   skos:changeNote """2.0 changes: replaced gvp:broaderTransitive with gvp:broaderExtended.
3.0 changes: replaced schema:startDate, endDate with gvp:estStart, estEnd; added ULAN). See details in referenced links.
3.1 & 3.2: no changes.
3.3: added 6 associative relations: gvp:aat2886_used-function_as - gvp:aat2887_exemplified_by, gvp:tgn3103_located_on - gvp:tgn3104_is_location_of, and gvp:ulan2583_chairman_of - gvp:ulan2584_chaired_by""" ;
                                   rdfs:seeAlso <http://www.getty.edu/research/tools/vocabularies/lod/> .

#################################################################
#    Annotation properties
#################################################################

###  http://purl.org/dc/elements/1.1/identifier
dc:identifier rdf:type owl:AnnotationProperty .


###  http://purl.org/dc/elements/1.1/title
dc:title rdf:type owl:AnnotationProperty .


###  http://purl.org/dc/terms/contributor
dct:contributor rdf:type owl:AnnotationProperty .


###  http://purl.org/dc/terms/created
dct:created rdf:type owl:AnnotationProperty .


###  http://purl.org/dc/terms/creator
dct:creator rdf:type owl:AnnotationProperty .


###  http://purl.org/dc/terms/description
dct:description rdf:type owl:AnnotationProperty .


###  http://purl.org/vocab/vann/preferredNamespacePrefix
vann:preferredNamespacePrefix rdf:type owl:AnnotationProperty .


###  http://purl.org/vocab/vann/preferredNamespaceUri
vann:preferredNamespaceUri rdf:type owl:AnnotationProperty .


###  http://vocab.getty.edu/ontology#contributorAlternatePreferred
gvp:contributorAlternatePreferred rdf:type owl:AnnotationProperty ;
                                  rdfs:subPropertyOf dct:contributor .


###  http://vocab.getty.edu/ontology#contributorNonPreferred
gvp:contributorNonPreferred rdf:type owl:AnnotationProperty ;
                            rdfs:subPropertyOf dct:contributor .


###  http://vocab.getty.edu/ontology#contributorPreferred
gvp:contributorPreferred rdf:type owl:AnnotationProperty ;
                         rdfs:subPropertyOf dct:contributor .


###  http://www.ontotext.com/proton/protontop#conclusion
ptop:conclusion rdf:type owl:AnnotationProperty .


###  http://www.ontotext.com/proton/protontop#premise
ptop:premise rdf:type owl:AnnotationProperty .


###  http://www.ontotext.com/proton/protontop#premise1
ptop:premise1 rdf:type owl:AnnotationProperty .


###  http://www.ontotext.com/proton/protontop#premise2
ptop:premise2 rdf:type owl:AnnotationProperty .


###  http://www.ontotext.com/proton/protontop#restriction
ptop:restriction rdf:type owl:AnnotationProperty .


###  http://www.ontotext.com/proton/protontop#type1
ptop:type1 rdf:type owl:AnnotationProperty .


###  http://www.ontotext.com/proton/protontop#type2
ptop:type2 rdf:type owl:AnnotationProperty .


###  http://xmlns.com/foaf/0.1/homepage
foaf:homepage rdf:type owl:AnnotationProperty .


###  http://xmlns.com/foaf/0.1/name
foaf:name rdf:type owl:AnnotationProperty .


#################################################################
#    Object Properties
#################################################################

###  http://purl.org/dc/terms/isReplacedBy
dct:isReplacedBy rdf:type owl:ObjectProperty ;
                 owl:inverseOf dct:replaces .


###  http://purl.org/dc/terms/replaces
dct:replaces rdf:type owl:ObjectProperty .


###  http://purl.org/dc/terms/source
dct:source rdf:type owl:ObjectProperty .


###  http://purl.org/vocab/bio/0.1/event
bio:event rdf:type owl:ObjectProperty .


###  http://schema.org/dissolutionLocation
schema:dissolutionLocation rdf:type owl:ObjectProperty ;
                           rdfs:domain schema:Organization ;
                           rdfs:range schema:Place ;
                           dct:description """The place where the Organization was dissolved.
Schema has properties foundationLocation and dissolutionDate but no dissolutionLocation. 
In contrast, for a person all 4 properties are present: birth/death place/date.
We posted issue https://github.com/schemaorg/schemaorg/issues/302, which looks like it will have a positive outcome in the far future.
And we define the property here""" ;
                           rdfs:comment "The place where the Organization was dissolved" ;
                           rdfs:isDefinedBy <http://vocab.getty.edu/ontology> ;
                           rdfs:label "dissolutionLocation" ;
                           rdfs:seeAlso <https://github.com/schemaorg/schemaorg/issues/302> .


###  http://schema.org/nationality
schema:nationality rdf:type owl:ObjectProperty .


###  http://vocab.getty.edu/ontology#aat2000_related_to
gvp:aat2000_related_to rdf:type owl:ObjectProperty ;
                       rdfs:subPropertyOf skos:related ;
                       rdf:type owl:SymmetricProperty ;
                       rdfs:domain skos:Concept ;
                       rdfs:range skos:Concept ;
                       dc:identifier "2000" ;
                       dc:title "related to - any" ;
                       dct:description """any - related to - any; generic relationship, not explained.
Example: gulf red is related to light red (pigment)""" ;
                       rdfs:isDefinedBy <http://vocab.getty.edu/ontology> ,
                                        aat: ;
                       skos:example "gulf red is related to light red (pigment)" ;
                       skos:prefLabel "aat2000_related_to" ;
                       skos:scopeNote "generic relationship, not explained" .


###  http://vocab.getty.edu/ontology#aat2001_formerly_referred_to
gvp:aat2001_formerly_referred_to rdf:type owl:ObjectProperty ;
                                 rdfs:subPropertyOf skos:related ;
                                 rdf:type owl:SymmetricProperty ;
                                 rdfs:domain skos:Concept ;
                                 rdfs:range skos:Concept ;
                                 dc:identifier "2001" ;
                                 dc:title "formerly referred to - any" ;
                                 dct:description """any - formerly referred - any.
Example: gigues formerly referred to fiddles""" ;
                                 rdfs:isDefinedBy <http://vocab.getty.edu/ontology> ,
                                                  aat: ;
                                 skos:example "gigues formerly referred to fiddles" ;
                                 skos:prefLabel "aat2001_formerly_referred_to" .


###  http://vocab.getty.edu/ontology#aat2100_distinguished_from
gvp:aat2100_distinguished_from rdf:type owl:ObjectProperty ;
                               rdfs:subPropertyOf skos:related ;
                               rdf:type owl:SymmetricProperty ;
                               rdfs:domain skos:Concept ;
                               rdfs:range skos:Concept ;
                               dc:identifier "2100" ;
                               dc:title "distinguished from - any" ;
                               dct:description """any - distinguished from - any.
Example: historic farms are distinguished from abandoned farms; naive art is distinguished from outsider art""" ;
                               rdfs:isDefinedBy <http://vocab.getty.edu/ontology> ,
                                                aat: ;
                               skos:example "historic farms are distinguished from abandoned farms" ,
                                            "naive art is distinguished from outsider art" ;
                               skos:prefLabel "aat2100_distinguished_from" .


###  http://vocab.getty.edu/ontology#aat2110_meaning-usage_overlaps_with
gvp:aat2110_meaning-usage_overlaps_with rdf:type owl:ObjectProperty ;
                                        rdfs:subPropertyOf skos:related ;
                                        rdf:type owl:SymmetricProperty ;
                                        rdfs:domain skos:Concept ;
                                        rdfs:range skos:Concept ;
                                        dc:identifier "2110" ;
                                        dc:title "meaning/usage overlaps with - any" ;
                                        dct:description """any - meaning/usage overlaps with - any.
Example: chimney hoods has meaning/usage that overlaps with chimney caps; scribes has meaning/usage that overlaps with copyists""" ;
                                        rdfs:isDefinedBy <http://vocab.getty.edu/ontology> ,
                                                         aat: ;
                                        skos:example "chimney hoods has meaning/usage that overlaps with chimney caps" ,
                                                     "scribes has meaning/usage that overlaps with copyists" ;
                                        skos:prefLabel "aat2110_meaning-usage_overlaps_with" .


###  http://vocab.getty.edu/ontology#aat2203_associated_with
gvp:aat2203_associated_with rdf:type owl:ObjectProperty ;
                            rdfs:subPropertyOf skos:related ;
                            rdf:type owl:SymmetricProperty ;
                            rdfs:domain skos:Concept ;
                            rdfs:range skos:Concept ;
                            dc:identifier "2203" ;
                            dc:title "associated with - activity/event" ;
                            dct:description """activity/event/[process/function] - [is] associated with - activity/event/[process/function].
Example: Easter is associated with Lent; cavalry exercises are associated with dressage""" ;
                            rdfs:isDefinedBy <http://vocab.getty.edu/ontology> ,
                                             aat: ;
                            skos:example "Easter is associated with Lent" ,
                                         "cavalry exercises are associated with dressage" ;
                            skos:prefLabel "aat2203_associated_with" .


###  http://vocab.getty.edu/ontology#aat2205_causes-is_required
gvp:aat2205_causes-is_required rdf:type owl:ObjectProperty ;
                               rdfs:subPropertyOf skos:related ;
                               owl:inverseOf gvp:aat2206_caused_by-requires ;
                               rdfs:domain skos:Concept ;
                               rdfs:range skos:Concept ;
                               dc:identifier "2205" ;
                               dc:title "causes/is required - activity/event" ;
                               dct:description """activity/event/[process/function] - causes/is required for - activity/event/[process/function].
Example: on-demand printing causes/is required for on-demand publishing;  preserving causes/is required for preservation""" ;
                               rdfs:isDefinedBy <http://vocab.getty.edu/ontology> ,
                                                aat: ;
                               skos:example "on-demand printing causes/is required for on-demand publishing" ,
                                            "preserving causes/is required for preservation" ;
                               skos:prefLabel "aat2205_causes-is_required" .


###  http://vocab.getty.edu/ontology#aat2206_caused_by-requires
gvp:aat2206_caused_by-requires rdf:type owl:ObjectProperty ;
                               rdfs:subPropertyOf skos:related ;
                               rdfs:domain skos:Concept ;
                               rdfs:range skos:Concept ;
                               dc:identifier "2206" ;
                               dc:title "caused by/requires - activity/event" ;
                               dct:description """activity/event/[process/function] - [is] caused by/dependent upon - activity/event/[process/function].
Example: on-demand publishing is caused by/requires on-demand printing; preservation is caused by/requires preserving""" ;
                               rdfs:isDefinedBy <http://vocab.getty.edu/ontology> ,
                                                aat: ;
                               skos:example "on-demand publishing is caused by/requires on-demand printing" ,
                                            "preservation is caused by/requires preserving" ;
                               skos:prefLabel "aat2206_caused_by-requires" .


###  http://vocab.getty.edu/ontology#aat2208_locus-setting_for
gvp:aat2208_locus-setting_for rdf:type owl:ObjectProperty ;
                              rdfs:subPropertyOf skos:related ;
                              owl:inverseOf gvp:aat2209_used-located_in ;
                              rdfs:domain skos:Concept ;
                              rdfs:range skos:Concept ;
                              dc:identifier "2208" ;
                              dc:title "locus/setting for - things" ;
                              dct:description """locus/setting - [is] locus/setting for - things.
Example: glassworks (buildings) are the locus/setting for glassware; caves are the locus/setting for cave paintings""" ;
                              rdfs:isDefinedBy <http://vocab.getty.edu/ontology> ,
                                               aat: ;
                              skos:example "caves are the locus/setting for cave paintings" ,
                                           "glassworks (buildings) are the locus/setting for glassware" ;
                              skos:prefLabel "aat2208_locus-setting_for" .


###  http://vocab.getty.edu/ontology#aat2209_used-located_in
gvp:aat2209_used-located_in rdf:type owl:ObjectProperty ;
                            rdfs:subPropertyOf skos:related ;
                            rdfs:domain skos:Concept ;
                            rdfs:range skos:Concept ;
                            dc:identifier "2209" ;
                            dc:title "used/located in - locus/setting" ;
                            dct:description """things -used/located in -  locus/setting.
Example: glassware is used/located in glassworks (buildings); cave paintings are located in caves""" ;
                            rdfs:isDefinedBy <http://vocab.getty.edu/ontology> ,
                                             aat: ;
                            skos:example "cave paintings are located in caves" ,
                                         "glassware is used/located in glassworks (buildings)" ;
                            skos:prefLabel "aat2209_used-located_in" .


###  http://vocab.getty.edu/ontology#aat2211_produce
gvp:aat2211_produce rdf:type owl:ObjectProperty ;
                    rdfs:subPropertyOf skos:related ;
                    owl:inverseOf gvp:aat2212_produced_by ;
                    rdfs:domain skos:Concept ;
                    rdfs:range skos:Concept ;
                    dc:identifier "2211" ;
                    dc:title "produce - things" ;
                    dct:description """things/[equipment] - produce - things.
Example: stereoscopic cameras produce stereoscopic photographs; punches (marking tools) produce punchwork""" ;
                    rdfs:isDefinedBy <http://vocab.getty.edu/ontology> ,
                                     aat: ;
                    skos:example "punches (marking tools) produce punchwork" ,
                                 "stereoscopic cameras produce stereoscopic photographs" ;
                    skos:prefLabel "aat2211_produce" .


###  http://vocab.getty.edu/ontology#aat2212_produced_by
gvp:aat2212_produced_by rdf:type owl:ObjectProperty ;
                        rdfs:subPropertyOf skos:related ;
                        rdfs:domain skos:Concept ;
                        rdfs:range skos:Concept ;
                        dc:identifier "2212" ;
                        dc:title "produced by - things" ;
                        dct:description """things - [are] produced by - things/[equipment].
Example: stereoscopic photographs are produced by stereoscopic cameras; punchwork is produced by punches (marking tools)""" ;
                        rdfs:isDefinedBy <http://vocab.getty.edu/ontology> ,
                                         aat: ;
                        skos:example "punchwork is produced by punches (marking tools)" ,
                                     "stereoscopic photographs are produced by stereoscopic cameras" ;
                        skos:prefLabel "aat2212_produced_by" .


###  http://vocab.getty.edu/ontology#aat2215_required_for
gvp:aat2215_required_for rdf:type owl:ObjectProperty ;
                         rdfs:subPropertyOf skos:related ;
                         owl:inverseOf gvp:aat2216_require ;
                         rdfs:domain skos:Concept ;
                         rdfs:range skos:Concept ;
                         dc:identifier "2215" ;
                         dc:title "required for - things" ;
                         dct:description """things - [are] required for -  things.
Example: eyelets are required for broderie anglaise; compact discs are required for compact disc players""" ;
                         rdfs:isDefinedBy <http://vocab.getty.edu/ontology> ,
                                          aat: ;
                         skos:example "compact discs are required for compact disc players" ,
                                      "eyelets are required for broderie anglaise" ;
                         skos:prefLabel "aat2215_required_for" .


###  http://vocab.getty.edu/ontology#aat2216_require
gvp:aat2216_require rdf:type owl:ObjectProperty ;
                    rdfs:subPropertyOf skos:related ;
                    rdfs:domain skos:Concept ;
                    rdfs:range skos:Concept ;
                    dc:identifier "2216" ;
                    dc:title "require - things" ;
                    dct:description """things - require - things [in order to exist or work].
Example: broderie anglaise requires eyelets; compact disc players require compact discs""" ;
                    rdfs:isDefinedBy <http://vocab.getty.edu/ontology> ,
                                     aat: ;
                    skos:example "broderie anglaise requires eyelets" ,
                                 "compact disc players require compact discs" ;
                    skos:prefLabel "aat2216_require" .


###  http://vocab.getty.edu/ontology#aat2218_used-function_as
gvp:aat2218_used-function_as rdf:type owl:ObjectProperty ;
                             rdfs:subPropertyOf skos:related ;
                             owl:inverseOf gvp:aat2219_have_form ;
                             rdfs:domain skos:Concept ;
                             rdfs:range skos:Concept ;
                             dc:identifier "2218" ;
                             dc:title "used/function as - things" ;
                             dct:description """things - [are] used/function as - things.
Example: arc lamps are used/function as lighthouse lamps;  toile peinte is used/function as cartoons (working drawings)""" ;
                             rdfs:isDefinedBy <http://vocab.getty.edu/ontology> ,
                                              aat: ;
                             skos:example "arc lamps are used/function as lighthouse lamps" ,
                                          "toile peinte is used/function as cartoons (working drawings)" ;
                             skos:prefLabel "aat2218_used-function_as" .


###  http://vocab.getty.edu/ontology#aat2219_have_form
gvp:aat2219_have_form rdf:type owl:ObjectProperty ;
                      rdfs:subPropertyOf skos:related ;
                      rdfs:domain skos:Concept ;
                      rdfs:range skos:Concept ;
                      dc:identifier "2219" ;
                      dc:title "have form - things" ;
                      dct:description """things - have form [of] - things.
Example: lighthouse lamps have the form of arc lamps; cartoons (working drawings) have the form of toile peinte""" ;
                      rdfs:isDefinedBy <http://vocab.getty.edu/ontology> ,
                                       aat: ;
                      skos:example "cartoons (working drawings) have the form of toile peinte" ,
                                   "lighthouse lamps have the form of arc lamps" ;
                      skos:prefLabel "aat2219_have_form" .


###  http://vocab.getty.edu/ontology#aat2221_act_upon
gvp:aat2221_act_upon rdf:type owl:ObjectProperty ;
                     rdfs:subPropertyOf skos:related ;
                     owl:inverseOf gvp:aat2222_are_acted_upon ;
                     rdfs:domain skos:Concept ;
                     rdfs:range skos:Concept ;
                     dc:identifier "2221" ;
                     dc:title "act upon - genus/species" ;
                     dct:description """[actors having] role - act upon - genus/species.
Example: jockeys act upon Equus caballus(species); tappers act upon Acer saccharum(species)""" ;
                     rdfs:isDefinedBy <http://vocab.getty.edu/ontology> ,
                                      aat: ;
                     skos:example "jockeys act upon Equus caballus(species)" ,
                                  "tappers act upon Acer saccharum(species)" ;
                     skos:prefLabel "aat2221_act_upon" .


###  http://vocab.getty.edu/ontology#aat2222_are_acted_upon
gvp:aat2222_are_acted_upon rdf:type owl:ObjectProperty ;
                           rdfs:subPropertyOf skos:related ;
                           rdfs:domain skos:Concept ;
                           rdfs:range skos:Concept ;
                           dc:identifier "2222" ;
                           dc:title "are acted upon - role" ;
                           dct:description """genus/species - is acted upon [by] - [actors having] role.
Example: Equus caballus(species) is acted upon by jockeys; Acer saccharum(species) is acted upon by tappers""" ;
                           rdfs:isDefinedBy <http://vocab.getty.edu/ontology> ,
                                            aat: ;
                           skos:example "Acer saccharum(species) is acted upon by tappers" ,
                                        "Equus caballus(species) is acted upon by jockeys" ;
                           skos:prefLabel "aat2222_are_acted_upon" .


###  http://vocab.getty.edu/ontology#aat2281_have_counterpart
gvp:aat2281_have_counterpart rdf:type owl:ObjectProperty ;
                             rdfs:subPropertyOf skos:related ;
                             rdf:type owl:SymmetricProperty ;
                             rdfs:domain skos:Concept ;
                             rdfs:range skos:Concept ;
                             dc:identifier "2281" ;
                             dc:title "have counterpart - role" ;
                             dct:description """role -[is] counterpart to - role.
Example: duchesses have counterpart dukes; godesses have counterpart gods""" ;
                             rdfs:isDefinedBy <http://vocab.getty.edu/ontology> ,
                                              aat: ;
                             skos:example "duchesses have counterpart dukes" ,
                                          "godesses have counterpart gods" ;
                             skos:prefLabel "aat2281_have_counterpart" .


###  http://vocab.getty.edu/ontology#aat2285_practiced-studied_by
gvp:aat2285_practiced-studied_by rdf:type owl:ObjectProperty ;
                                 rdfs:subPropertyOf skos:related ;
                                 owl:inverseOf gvp:aat2286_practice-study ;
                                 rdfs:domain skos:Concept ;
                                 rdfs:range skos:Concept ;
                                 dc:identifier "2285" ;
                                 dc:title "practiced/studied by - role" ;
                                 dct:description """field [of study, genre]/discipline - [is] practiced/studied by - a role.
Example: Egyptology is practiced/studied by Egyptologists; architectural history is practiced/studied by architectural historians""" ;
                                 rdfs:isDefinedBy <http://vocab.getty.edu/ontology> ,
                                                  aat: ;
                                 skos:example "Egyptology is practiced/studied by Egyptologists" ,
                                              "architectural history is practiced/studied by architectural historians" ;
                                 skos:prefLabel "aat2285_practiced-studied_by" .


###  http://vocab.getty.edu/ontology#aat2286_practice-study
gvp:aat2286_practice-study rdf:type owl:ObjectProperty ;
                           rdfs:subPropertyOf skos:related ;
                           rdfs:domain skos:Concept ;
                           rdfs:range skos:Concept ;
                           dc:identifier "2286" ;
                           dc:title "practice/study - field/discipline" ;
                           dct:description """[actor having] role - practice/study - field [of study, genre]/discipline.
Example: Egyptologists practice/study Egyptology; architectural historians practice/study architectural history""" ;
                           rdfs:isDefinedBy <http://vocab.getty.edu/ontology> ,
                                            aat: ;
                           skos:example "Egyptologists practice/study Egyptology" ,
                                        "architectural historians practice/study architectural history" ;
                           skos:prefLabel "aat2286_practice-study" .


###  http://vocab.getty.edu/ontology#aat2291_locus-setting_for
gvp:aat2291_locus-setting_for rdf:type owl:ObjectProperty ;
                              rdfs:subPropertyOf skos:related ;
                              owl:inverseOf gvp:aat2292_work-live_in ;
                              rdfs:domain skos:Concept ;
                              rdfs:range skos:Concept ;
                              dc:identifier "2291" ;
                              dc:title "locus/setting for - role" ;
                              dct:description """locus/setting - [is] locus setting for - [actor or institution having] role.
Example: roperies are the locus/setting of rope-makers; convents (built complexes) are the locus/setting of nuns; libraries (buildings) are the locus/setting of libraries (institutions)""" ;
                              rdfs:isDefinedBy <http://vocab.getty.edu/ontology> ,
                                               aat: ;
                              skos:example "convents (built complexes) are the locus/setting of nuns" ,
                                           "libraries (buildings) are the locus/setting of libraries (institutions)" ,
                                           "roperies are the locus/setting of rope-makers" ;
                              skos:prefLabel "aat2291_locus-setting_for" .


###  http://vocab.getty.edu/ontology#aat2292_work-live_in
gvp:aat2292_work-live_in rdf:type owl:ObjectProperty ;
                         rdfs:subPropertyOf skos:related ;
                         rdfs:domain skos:Concept ;
                         rdfs:range skos:Concept ;
                         dc:identifier "2292" ;
                         dc:title "work/live in - locus/setting" ;
                         dct:description """[actor or institution having] role - work/live/[exist] in - locus/setting.
Example: rope-makers live/work in roperies; nuns live/work in convents (nunneries); libraries (institutions) live/work in libraries (buildings)""" ;
                         rdfs:isDefinedBy <http://vocab.getty.edu/ontology> ,
                                          aat: ;
                         skos:example "libraries (institutions) live/work in libraries (buildings)" ,
                                      "nuns live/work in convents (nunneries)" ,
                                      "rope-makers live/work in roperies" ;
                         skos:prefLabel "aat2292_work-live_in" .


###  http://vocab.getty.edu/ontology#aat2294_locus-setting_for
gvp:aat2294_locus-setting_for rdf:type owl:ObjectProperty ;
                              rdfs:subPropertyOf skos:related ;
                              owl:inverseOf gvp:aat2295_located_in ;
                              rdfs:domain skos:Concept ;
                              rdfs:range skos:Concept ;
                              dc:identifier "2294" ;
                              dc:title "locus/setting for - locus/setting" ;
                              dct:description """locus/setting - [is] locus setting for - locus/setting.
Example: nations are the locus/setting for national capitals; mountain ranges are the locus/setting for mountains""" ;
                              rdfs:isDefinedBy <http://vocab.getty.edu/ontology> ,
                                               aat: ;
                              skos:example "mountain ranges are the locus/setting for mountains" ,
                                           "nations are the locus/setting for national capitals" ;
                              skos:prefLabel "aat2294_locus-setting_for" .


###  http://vocab.getty.edu/ontology#aat2295_located_in
gvp:aat2295_located_in rdf:type owl:ObjectProperty ;
                       rdfs:subPropertyOf skos:related ;
                       rdfs:domain skos:Concept ;
                       rdfs:range skos:Concept ;
                       dc:identifier "2295" ;
                       dc:title "located in - locus/setting" ;
                       dct:description """locus/setting - [is] located in - locus/setting.
Example: national capitals are located in nations; mountains are located in mountain ranges""" ;
                       rdfs:isDefinedBy <http://vocab.getty.edu/ontology> ,
                                        aat: ;
                       skos:example "mountains are located in mountain ranges" ,
                                    "national capitals are located in nations" ;
                       skos:prefLabel "aat2295_located_in" .


###  http://vocab.getty.edu/ontology#aat2311_performed_by
gvp:aat2311_performed_by rdf:type owl:ObjectProperty ;
                         rdfs:subPropertyOf skos:related ;
                         owl:inverseOf gvp:aat2312_perform ;
                         rdfs:domain skos:Concept ;
                         rdfs:range skos:Concept ;
                         dc:identifier "2311" ;
                         dc:title "performed by - role" ;
                         dct:description """activity/event/[process/function] - [is] performed by - [actors having] a role.
Example: clockmaking is performed by clockmakers; curating is performed by curators""" ;
                         rdfs:isDefinedBy <http://vocab.getty.edu/ontology> ,
                                          aat: ;
                         skos:example "clockmaking is performed by clockmakers" ,
                                      "curating is performed by curators" ;
                         skos:prefLabel "aat2311_performed_by" .


###  http://vocab.getty.edu/ontology#aat2312_perform
gvp:aat2312_perform rdf:type owl:ObjectProperty ;
                    rdfs:subPropertyOf skos:related ;
                    rdfs:domain skos:Concept ;
                    rdfs:range skos:Concept ;
                    dc:identifier "2312" ;
                    dc:title "perform - activity/event" ;
                    dct:description """[actors having] a role - perform - activity/event/process.
Example: clockmakers perform clockmaking; curators perform curating""" ;
                    rdfs:isDefinedBy <http://vocab.getty.edu/ontology> ,
                                     aat: ;
                    skos:example "clockmakers perform clockmaking" ,
                                 "curators perform curating" ;
                    skos:prefLabel "aat2312_perform" .


###  http://vocab.getty.edu/ontology#aat2315_used_by
gvp:aat2315_used_by rdf:type owl:ObjectProperty ;
                    rdfs:subPropertyOf skos:related ;
                    owl:inverseOf gvp:aat2316_use ;
                    rdfs:domain skos:Concept ;
                    rdfs:range skos:Concept ;
                    dc:identifier "2315" ;
                    dc:title "used by - role" ;
                    dct:description """material - [is] used by - [actor having] role.
Example: precious stone is used by lapidiaries; brass (alloy) is used by braziers (metalworkers)""" ;
                    rdfs:isDefinedBy <http://vocab.getty.edu/ontology> ,
                                     aat: ;
                    skos:example "brass (alloy) is used by braziers (metalworkers)" ,
                                 "precious stone is used by lapidiaries" ;
                    skos:prefLabel "aat2315_used_by" .


###  http://vocab.getty.edu/ontology#aat2316_use
gvp:aat2316_use rdf:type owl:ObjectProperty ;
                rdfs:subPropertyOf skos:related ;
                rdfs:domain skos:Concept ;
                rdfs:range skos:Concept ;
                dc:identifier "2316" ;
                dc:title "use - material" ;
                dct:description """[actors having] role - use - material.
Example: lapidaries use precious stone; braziers (metalworkers) use brass (alloy)""" ;
                rdfs:isDefinedBy <http://vocab.getty.edu/ontology> ,
                                 aat: ;
                skos:example "braziers (metalworkers) use brass (alloy)" ,
                             "lapidaries use precious stone" ;
                skos:prefLabel "aat2316_use" .


###  http://vocab.getty.edu/ontology#aat2318_involved_in
gvp:aat2318_involved_in rdf:type owl:ObjectProperty ;
                        rdfs:subPropertyOf skos:related ;
                        owl:inverseOf gvp:aat2319_involves ;
                        rdfs:domain skos:Concept ;
                        rdfs:range skos:Concept ;
                        dc:identifier "2318" ;
                        dc:title "involved in - activity/event" ;
                        dct:description """[actors having] role -[are] involved - activity/event.
Example: bridegrooms are involved in weddings; martyrs are involved in martyrdoms""" ;
                        rdfs:isDefinedBy <http://vocab.getty.edu/ontology> ,
                                         aat: ;
                        skos:example "bridegrooms are involved in weddings" ,
                                     "martyrs are involved in martyrdoms" ;
                        skos:prefLabel "aat2318_involved_in" .


###  http://vocab.getty.edu/ontology#aat2319_involves
gvp:aat2319_involves rdf:type owl:ObjectProperty ;
                     rdfs:subPropertyOf skos:related ;
                     rdfs:domain skos:Concept ;
                     rdfs:range skos:Concept ;
                     dc:identifier "2319" ;
                     dc:title "involves - role" ;
                     dct:description """activity/event - involves - [actors having] role.
Example: weddings involve bridegrooms; martyrdoms involve martyrs""" ;
                     rdfs:isDefinedBy <http://vocab.getty.edu/ontology> ,
                                      aat: ;
                     skos:example "martyrdoms involve martyrs" ,
                                  "weddings involve bridegrooms" ;
                     skos:prefLabel "aat2319_involves" .


###  http://vocab.getty.edu/ontology#aat2321_used_by
gvp:aat2321_used_by rdf:type owl:ObjectProperty ;
                    rdfs:subPropertyOf skos:related ;
                    owl:inverseOf gvp:aat2322_use ;
                    rdfs:domain skos:Concept ;
                    rdfs:range skos:Concept ;
                    dc:identifier "2321" ;
                    dc:title "used by - role" ;
                    dct:description """things/equipment - [are] used by - [actors having] role.
Example: violoncellos are used by violoncellists; surveying instruments are used by surveyors""" ;
                    rdfs:isDefinedBy <http://vocab.getty.edu/ontology> ,
                                     aat: ;
                    skos:example "surveying instruments are used by surveyors" ,
                                 "violoncellos are used by violoncellists" ;
                    skos:prefLabel "aat2321_used_by" .


###  http://vocab.getty.edu/ontology#aat2322_use
gvp:aat2322_use rdf:type owl:ObjectProperty ;
                rdfs:subPropertyOf skos:related ;
                rdfs:domain skos:Concept ;
                rdfs:range skos:Concept ;
                dc:identifier "2322" ;
                dc:title "use - things" ;
                dct:description """[actors having] role - use - things/equipment.
Example: violoncellists use violoncellos; surveyors use surveying instruments""" ;
                rdfs:isDefinedBy <http://vocab.getty.edu/ontology> ,
                                 aat: ;
                skos:example "surveyors use surveying instruments" ,
                             "violoncellists use violoncellos" ;
                skos:prefLabel "aat2322_use" .


###  http://vocab.getty.edu/ontology#aat2325_created_by
gvp:aat2325_created_by rdf:type owl:ObjectProperty ;
                       rdfs:subPropertyOf skos:related ;
                       owl:inverseOf gvp:aat2326_create ;
                       rdfs:domain skos:Concept ;
                       rdfs:range skos:Concept ;
                       dc:identifier "2325" ;
                       dc:title "created by - role" ;
                       dct:description """things - [are] created by - [actors having] role.
Example: drawings are created by draftsmen; poems are created by poets""" ;
                       rdfs:isDefinedBy <http://vocab.getty.edu/ontology> ,
                                        aat: ;
                       skos:example "drawings are created by draftsmen" ,
                                    "poems are created by poets" ;
                       skos:prefLabel "aat2325_created_by" .


###  http://vocab.getty.edu/ontology#aat2326_create
gvp:aat2326_create rdf:type owl:ObjectProperty ;
                   rdfs:subPropertyOf skos:related ;
                   rdfs:domain skos:Concept ;
                   rdfs:range skos:Concept ;
                   dc:identifier "2326" ;
                   dc:title "create - things" ;
                   dct:description """[actors having] role - create - things.
Example: draftsmen create drawings; poets create poems""" ;
                   rdfs:isDefinedBy <http://vocab.getty.edu/ontology> ,
                                    aat: ;
                   skos:example "draftsmen create drawings" ,
                                "poets create poems" ;
                   skos:prefLabel "aat2326_create" .


###  http://vocab.getty.edu/ontology#aat2328_involved_with
gvp:aat2328_involved_with rdf:type owl:ObjectProperty ;
                          rdfs:subPropertyOf skos:related ;
                          owl:inverseOf gvp:aat2329_involves ;
                          rdfs:domain skos:Concept ;
                          rdfs:range skos:Concept ;
                          dc:identifier "2328" ;
                          dc:title "involved with - things" ;
                          dct:description """[actors having] role - [are] involved in- things.
Example: sitters are involved with portraits; actors (performing artists) are involved with motion pictures (visual works)""" ;
                          rdfs:isDefinedBy <http://vocab.getty.edu/ontology> ,
                                           aat: ;
                          skos:example "actors (performing artists) are involved with motion pictures (visual works)" ,
                                       "sitters are involved with portraits" ;
                          skos:prefLabel "aat2328_involved_with" .


###  http://vocab.getty.edu/ontology#aat2329_involves
gvp:aat2329_involves rdf:type owl:ObjectProperty ;
                     rdfs:subPropertyOf skos:related ;
                     rdfs:domain skos:Concept ;
                     rdfs:range skos:Concept ;
                     dc:identifier "2329" ;
                     dc:title "involves - role" ;
                     dct:description """things - involve - [actors having] role.
Example: portraits involve sitters; motion pictures (visual works) involve actors (performing artists)""" ;
                     rdfs:isDefinedBy <http://vocab.getty.edu/ontology> ,
                                      aat: ;
                     skos:example "motion pictures (visual works) involve actors (performing artists)" ,
                                  "portraits involve sitters" ;
                     skos:prefLabel "aat2329_involves" .


###  http://vocab.getty.edu/ontology#aat2332_affiliated_with
gvp:aat2332_affiliated_with rdf:type owl:ObjectProperty ;
                            rdfs:subPropertyOf skos:related ;
                            owl:inverseOf gvp:aat2333_have_affiliates ;
                            rdfs:domain skos:Concept ;
                            rdfs:range skos:Concept ;
                            dc:identifier "2332" ;
                            dc:title "affiliated with - role" ;
                            dct:description """[actors having] role - [are] affiliated with - role [organization].
Example: students are affiliated with schools (organizations); dukes are affiliated with duchies""" ;
                            rdfs:isDefinedBy <http://vocab.getty.edu/ontology> ,
                                             aat: ;
                            skos:example "dukes are affiliated with duchies" ,
                                         "students are affiliated with schools (organizations)" ;
                            skos:prefLabel "aat2332_affiliated_with" .


###  http://vocab.getty.edu/ontology#aat2333_have_affiliates
gvp:aat2333_have_affiliates rdf:type owl:ObjectProperty ;
                            rdfs:subPropertyOf skos:related ;
                            rdfs:domain skos:Concept ;
                            rdfs:range skos:Concept ;
                            dc:identifier "2333" ;
                            dc:title "have affiliates - role" ;
                            dct:description """role [organizations] - have affiliates - [actors having] role.
Example: schools (organizations) have as affiliates students; duchies have as affiliates dukes""" ;
                            rdfs:isDefinedBy <http://vocab.getty.edu/ontology> ,
                                             aat: ;
                            skos:example "duchies have as affiliates dukes" ,
                                         "schools (organizations) have as affiliates students" ;
                            skos:prefLabel "aat2333_have_affiliates" .


###  http://vocab.getty.edu/ontology#aat2335_associated_with
gvp:aat2335_associated_with rdf:type owl:ObjectProperty ;
                            rdfs:subPropertyOf skos:related ;
                            owl:inverseOf gvp:aat2336_has_associates ;
                            rdfs:domain skos:Concept ;
                            rdfs:range skos:Concept ;
                            dc:identifier "2335" ;
                            dc:title "associated with - style/period/culture" ;
                            dct:description """[actors having] role - [are] associated with - style/period/culture/[religion/ideology].
Example: abstract artists are associated with Abstract (fine arts style); popes are associated with Roman Catholicism""" ;
                            rdfs:isDefinedBy <http://vocab.getty.edu/ontology> ,
                                             aat: ;
                            skos:example "abstract artists are associated with Abstract (fine arts style)" ,
                                         "popes are associated with Roman Catholicism" ;
                            skos:prefLabel "aat2335_associated_with" .


###  http://vocab.getty.edu/ontology#aat2336_has_associates
gvp:aat2336_has_associates rdf:type owl:ObjectProperty ;
                           rdfs:subPropertyOf skos:related ;
                           rdfs:domain skos:Concept ;
                           rdfs:range skos:Concept ;
                           dc:identifier "2336" ;
                           dc:title "has associates - role" ;
                           dct:description """style/period/culture/[relgion] - has associates - [actors having] role.
Example: Abstract (fine arts style) has associates abstract artists; Roman Catholicism has associates popes""" ;
                           rdfs:isDefinedBy <http://vocab.getty.edu/ontology> ,
                                            aat: ;
                           skos:example "Abstract (fine arts style) has associates abstract artists" ,
                                        "Roman Catholicism has associates popes" ;
                           skos:prefLabel "aat2336_has_associates" .


###  http://vocab.getty.edu/ontology#aat2397_focus_of
gvp:aat2397_focus_of rdf:type owl:ObjectProperty ;
                     rdfs:subPropertyOf skos:related ;
                     owl:inverseOf gvp:aat2398_focuses_on ;
                     rdfs:domain skos:Concept ;
                     rdfs:range skos:Concept ;
                     dc:identifier "2397" ;
                     dc:title "focus of - field/discipline" ;
                     dct:description """any - [is] focus of - field [of study]/discipline.
Example: manuscripts are the focus of codicology; music is the focus of musicology; Plantae (kingdom) is the focus of botany""" ;
                     rdfs:isDefinedBy <http://vocab.getty.edu/ontology> ,
                                      aat: ;
                     skos:example "Plantae (kingdom) is the focus of botany" ,
                                  "manuscripts are the focus of codicology" ,
                                  "music is the focus of musicology" ;
                     skos:prefLabel "aat2397_focus_of" .


###  http://vocab.getty.edu/ontology#aat2398_focuses_on
gvp:aat2398_focuses_on rdf:type owl:ObjectProperty ;
                       rdfs:subPropertyOf skos:related ;
                       rdfs:domain skos:Concept ;
                       rdfs:range skos:Concept ;
                       dc:identifier "2398" ;
                       dc:title "focuses on - any" ;
                       dct:description """field [of study]/discipline - focuses on - any.
Example: codicology focuses on manuscripts; musicology focuses on music; bontany focuses on Plantae (kingdom)""" ;
                       rdfs:isDefinedBy <http://vocab.getty.edu/ontology> ,
                                        aat: ;
                       skos:example "bontany focuses on Plantae (kingdom)" ,
                                    "codicology focuses on manuscripts" ,
                                    "musicology focuses on music" ;
                       skos:prefLabel "aat2398_focuses_on" .


###  http://vocab.getty.edu/ontology#aat2408_locus-setting_for
gvp:aat2408_locus-setting_for rdf:type owl:ObjectProperty ;
                              rdfs:subPropertyOf skos:related ;
                              owl:inverseOf gvp:aat2409_takes_place_in ;
                              rdfs:domain skos:Concept ;
                              rdfs:range skos:Concept ;
                              dc:identifier "2408" ;
                              dc:title "locus/setting for - field/discipline" ;
                              dct:description """locus/setting - [is] locus/setting for - field of study/discipline.
Example: schools (buildings) are the locus/setting for education; hospitals (buildings) are the locus/setting for medicine (discipline)""" ;
                              rdfs:isDefinedBy <http://vocab.getty.edu/ontology> ,
                                               aat: ;
                              skos:example "hospitals (buildings) are the locus/setting for medicine (discipline)" ,
                                           "schools (buildings) are the locus/setting for education" ;
                              skos:prefLabel "aat2408_locus-setting_for" .


###  http://vocab.getty.edu/ontology#aat2409_takes_place_in
gvp:aat2409_takes_place_in rdf:type owl:ObjectProperty ;
                           rdfs:subPropertyOf skos:related ;
                           rdfs:domain skos:Concept ;
                           rdfs:range skos:Concept ;
                           dc:identifier "2409" ;
                           dc:title "takes place in - locus/setting" ;
                           dct:description """field of study/discipline - takes place in - locus/setting.
Example: education takes place in schools (buildings); medicine (discipline) takes place in hospitals (buildings)""" ;
                           rdfs:isDefinedBy <http://vocab.getty.edu/ontology> ,
                                            aat: ;
                           skos:example "education takes place in schools (buildings)" ,
                                        "medicine (discipline) takes place in hospitals (buildings)" ;
                           skos:prefLabel "aat2409_takes_place_in" .


###  http://vocab.getty.edu/ontology#aat2411_involved_in
gvp:aat2411_involved_in rdf:type owl:ObjectProperty ;
                        rdfs:subPropertyOf skos:related ;
                        owl:inverseOf gvp:aat2412_involves ;
                        rdfs:domain skos:Concept ;
                        rdfs:range skos:Concept ;
                        dc:identifier "2411" ;
                        dc:title "involved in - field/discipline" ;
                        dct:description """activity/event/[process/function] - [is] involved in - field/discipline.
Example: journalistic photography is involved in photojournalism (discipline); gardening is involved in horticulture""" ;
                        rdfs:isDefinedBy <http://vocab.getty.edu/ontology> ,
                                         aat: ;
                        skos:example "gardening is involved in horticulture" ,
                                     "journalistic photography is involved in photojournalism (discipline)" ;
                        skos:prefLabel "aat2411_involved_in" .


###  http://vocab.getty.edu/ontology#aat2412_involves
gvp:aat2412_involves rdf:type owl:ObjectProperty ;
                     rdfs:subPropertyOf skos:related ;
                     rdfs:domain skos:Concept ;
                     rdfs:range skos:Concept ;
                     dc:identifier "2412" ;
                     dc:title "involves - activity/event" ;
                     dct:description """field/discipline - involves - activity/event/[process/function].
Example: photojournalism (discipline) involves journalistic photography; horticulture involves gardening""" ;
                     rdfs:isDefinedBy <http://vocab.getty.edu/ontology> ,
                                      aat: ;
                     skos:example "horticulture involves gardening" ,
                                  "photojournalism (discipline) involves journalistic photography" ;
                     skos:prefLabel "aat2412_involves" .


###  http://vocab.getty.edu/ontology#aat2415_required_for
gvp:aat2415_required_for rdf:type owl:ObjectProperty ;
                         rdfs:subPropertyOf skos:related ;
                         owl:inverseOf gvp:aat2416_requires ;
                         rdfs:domain skos:Concept ;
                         rdfs:range skos:Concept ;
                         dc:identifier "2415" ;
                         dc:title "required for - activity/event" ;
                         dct:description """material - [is] required for - activity/event/[process/function].
Example: dye is required for dying; pewter is required for pewtersmithing""" ;
                         rdfs:isDefinedBy <http://vocab.getty.edu/ontology> ,
                                          aat: ;
                         skos:example "dye is required for dying" ,
                                      "pewter is required for pewtersmithing" ;
                         skos:prefLabel "aat2415_required_for" .


###  http://vocab.getty.edu/ontology#aat2416_requires
gvp:aat2416_requires rdf:type owl:ObjectProperty ;
                     rdfs:subPropertyOf skos:related ;
                     rdfs:domain skos:Concept ;
                     rdfs:range skos:Concept ;
                     dc:identifier "2416" ;
                     dc:title "requires - material" ;
                     dct:description """activity/event/[process/function] - requires - material.
Example: dying requires dye; pewtersmithing requires pewter""" ;
                     rdfs:isDefinedBy <http://vocab.getty.edu/ontology> ,
                                      aat: ;
                     skos:example "dying requires dye" ,
                                  "pewtersmithing requires pewter" ;
                     skos:prefLabel "aat2416_requires" .


###  http://vocab.getty.edu/ontology#aat2418_uses
gvp:aat2418_uses rdf:type owl:ObjectProperty ;
                 rdfs:subPropertyOf skos:related ;
                 owl:inverseOf gvp:aat2419_used_for ;
                 rdfs:domain skos:Concept ;
                 rdfs:range skos:Concept ;
                 dc:identifier "2418" ;
                 dc:title "uses - things" ;
                 dct:description """field [of study]/discipline - uses - things/[equipment].
Example: astronomy uses astronomical instruments; divination [discipline] uses divination objects""" ;
                 rdfs:isDefinedBy <http://vocab.getty.edu/ontology> ,
                                  aat: ;
                 skos:example "astronomy uses astronomical instruments" ,
                              "divination [discipline] uses divination objects" ;
                 skos:prefLabel "aat2418_uses" .


###  http://vocab.getty.edu/ontology#aat2419_used_for
gvp:aat2419_used_for rdf:type owl:ObjectProperty ;
                     rdfs:subPropertyOf skos:related ;
                     rdfs:domain skos:Concept ;
                     rdfs:range skos:Concept ;
                     dc:identifier "2419" ;
                     dc:title "used for - field/discipline" ;
                     dct:description """things/[equipment] - [are] used for - field [of study]/discipline.
Example: astronomical instruments are used for astronomy; divination objects are used for divination [discipline]""" ;
                     rdfs:isDefinedBy <http://vocab.getty.edu/ontology> ,
                                      aat: ;
                     skos:example "astronomical instruments are used for astronomy" ,
                                  "divination objects are used for divination [discipline]" ;
                     skos:prefLabel "aat2419_used_for" .


###  http://vocab.getty.edu/ontology#aat2421_locus-setting_for
gvp:aat2421_locus-setting_for rdf:type owl:ObjectProperty ;
                              rdfs:subPropertyOf skos:related ;
                              owl:inverseOf gvp:aat2422_takes_place_in ;
                              rdfs:domain skos:Concept ;
                              rdfs:range skos:Concept ;
                              dc:identifier "2421" ;
                              dc:title "locus/setting for - activity/event" ;
                              dct:description """locus/setting - [is] locus/setting for - activity/event/[process/function].
Example: smelters (metalworking plants) are the locus/setting for smelting; pilgrimage centers are the locus/setting for pilgrimages""" ;
                              rdfs:isDefinedBy <http://vocab.getty.edu/ontology> ,
                                               aat: ;
                              skos:example "pilgrimage centers are the locus/setting for pilgrimages" ,
                                           "smelters (metalworking plants) are the locus/setting for smelting" ;
                              skos:prefLabel "aat2421_locus-setting_for" .


###  http://vocab.getty.edu/ontology#aat2422_takes_place_in
gvp:aat2422_takes_place_in rdf:type owl:ObjectProperty ;
                           rdfs:subPropertyOf skos:related ;
                           rdfs:domain skos:Concept ;
                           rdfs:range skos:Concept ;
                           dc:identifier "2422" ;
                           dc:title "takes place in - locus/setting" ;
                           dct:description """activity/event/[process/function] - takes place in - locus/setting.
Example: smelting takes place in smelters (metalworking plants); pilgrimages take place in pilgrimage centers""" ;
                           rdfs:isDefinedBy <http://vocab.getty.edu/ontology> ,
                                            aat: ;
                           skos:example "pilgrimages take place in pilgrimage centers" ,
                                        "smelting takes place in smelters (metalworking plants)" ;
                           skos:prefLabel "aat2422_takes_place_in" .


###  http://vocab.getty.edu/ontology#aat2424_produced_by
gvp:aat2424_produced_by rdf:type owl:ObjectProperty ;
                        rdfs:subPropertyOf skos:related ;
                        owl:inverseOf gvp:aat2425_produces ;
                        rdfs:domain skos:Concept ;
                        rdfs:range skos:Concept ;
                        dc:identifier "2424" ;
                        dc:title "produced by - activity/event/process" ;
                        dct:description """material - [is] produced by - activity/event/process.
Example: wire is produced by wiredrawing; paper is produced by papermaking""" ;
                        rdfs:isDefinedBy <http://vocab.getty.edu/ontology> ,
                                         aat: ;
                        skos:example "paper is produced by papermaking" ,
                                     "wire is produced by wiredrawing" ;
                        skos:prefLabel "aat2424_produced_by" .


###  http://vocab.getty.edu/ontology#aat2425_produces
gvp:aat2425_produces rdf:type owl:ObjectProperty ;
                     rdfs:subPropertyOf skos:related ;
                     rdfs:domain skos:Concept ;
                     rdfs:range skos:Concept ;
                     dc:identifier "2425" ;
                     dc:title "produces - material" ;
                     dct:description """activity/event/process - produces - material.
Example: wiredrawing produces wire; papermaking produces paper""" ;
                     rdfs:isDefinedBy <http://vocab.getty.edu/ontology> ,
                                      aat: ;
                     skos:example "papermaking produces paper" ,
                                  "wiredrawing produces wire" ;
                     skos:prefLabel "aat2425_produces" .


###  http://vocab.getty.edu/ontology#aat2427_produced_by
gvp:aat2427_produced_by rdf:type owl:ObjectProperty ;
                        rdfs:subPropertyOf skos:related ;
                        owl:inverseOf gvp:aat2428_produces ;
                        rdfs:domain skos:Concept ;
                        rdfs:range skos:Concept ;
                        dc:identifier "2427" ;
                        dc:title "produced by - activity/event/process" ;
                        dct:description """things - [are] produced by - activity/event/process.
Example: vase paintings (visual works) are produced by vase painting (image making); forgeries are produced by forging (copying)""" ;
                        rdfs:isDefinedBy <http://vocab.getty.edu/ontology> ,
                                         aat: ;
                        skos:example "forgeries are produced by forging (copying)" ,
                                     "vase paintings (visual works) are produced by vase painting (image making)" ;
                        skos:prefLabel "aat2427_produced_by" .


###  http://vocab.getty.edu/ontology#aat2428_produces
gvp:aat2428_produces rdf:type owl:ObjectProperty ;
                     rdfs:subPropertyOf skos:related ;
                     rdfs:domain skos:Concept ;
                     rdfs:range skos:Concept ;
                     dc:identifier "2428" ;
                     dc:title "produces - things" ;
                     dct:description """activity/event/process - produces - things.
Example: vase painting (image making) produces vase paintings (visual works); forging (copying) produces forgeries""" ;
                     rdfs:isDefinedBy <http://vocab.getty.edu/ontology> ,
                                      aat: ;
                     skos:example "forging (copying) produces forgeries" ,
                                  "vase painting (image making) produces vase paintings (visual works)" ;
                     skos:prefLabel "aat2428_produces" .


###  http://vocab.getty.edu/ontology#aat2431_required_for
gvp:aat2431_required_for rdf:type owl:ObjectProperty ;
                         rdfs:subPropertyOf skos:related ;
                         owl:inverseOf gvp:aat2432_requires ;
                         rdfs:domain skos:Concept ;
                         rdfs:range skos:Concept ;
                         dc:identifier "2431" ;
                         dc:title "required for - activity/event/process" ;
                         dct:description """things/equipment - [are] required for - activity/event/process.
Example: painting equipment is required for painting (image making); dowels are required for doweling""" ;
                         rdfs:isDefinedBy <http://vocab.getty.edu/ontology> ,
                                          aat: ;
                         skos:example "dowels are required for doweling" ,
                                      "painting equipment is required for painting (image making)" ;
                         skos:prefLabel "aat2431_required_for" .


###  http://vocab.getty.edu/ontology#aat2432_requires
gvp:aat2432_requires rdf:type owl:ObjectProperty ;
                     rdfs:subPropertyOf skos:related ;
                     rdfs:domain skos:Concept ;
                     rdfs:range skos:Concept ;
                     dc:identifier "2432" ;
                     dc:title "requires - things" ;
                     dct:description """activity/event/process - requires - things/equipment.
Example: painting (image making) requires painting equipment; doweling requires dowels""" ;
                     rdfs:isDefinedBy <http://vocab.getty.edu/ontology> ,
                                      aat: ;
                     skos:example "doweling requires dowels" ,
                                  "painting (image making) requires painting equipment" ;
                     skos:prefLabel "aat2432_requires" .


###  http://vocab.getty.edu/ontology#aat2434_contextualized_in
gvp:aat2434_contextualized_in rdf:type owl:ObjectProperty ;
                              rdfs:subPropertyOf skos:related ;
                              owl:inverseOf gvp:aat2435_context_for ;
                              rdfs:domain skos:Concept ;
                              rdfs:range skos:Concept ;
                              dc:identifier "2434" ;
                              dc:title "contextualized in - activity/event/process" ;
                              dct:description """things - [are] context for - activity/event/process.
Example: funeral books are contextualized in funerals; Christmas trees are contextualized in Christmas""" ;
                              rdfs:isDefinedBy <http://vocab.getty.edu/ontology> ,
                                               aat: ;
                              skos:example "Christmas trees are contextualized in Christmas" ,
                                           "funeral books are contextualized in funerals" ;
                              skos:prefLabel "aat2434_contextualized_in" .


###  http://vocab.getty.edu/ontology#aat2435_context_for
gvp:aat2435_context_for rdf:type owl:ObjectProperty ;
                        rdfs:subPropertyOf skos:related ;
                        rdfs:domain skos:Concept ;
                        rdfs:range skos:Concept ;
                        dc:identifier "2435" ;
                        dc:title "context for - things" ;
                        dct:description """activity/event/process - [is] contextualized in - thing.
Example: funerals are the context for funeral books; Christmas is the context for Christmas trees""" ;
                        rdfs:isDefinedBy <http://vocab.getty.edu/ontology> ,
                                         aat: ;
                        skos:example "Christmas is the context for Christmas trees" ,
                                     "funerals are the context for funeral books" ;
                        skos:prefLabel "aat2435_context_for" .


###  http://vocab.getty.edu/ontology#aat2501_made_of-require
gvp:aat2501_made_of-require rdf:type owl:ObjectProperty ;
                            rdfs:subPropertyOf skos:related ;
                            owl:inverseOf gvp:aat2502_material_for ;
                            rdfs:domain skos:Concept ;
                            rdfs:range skos:Concept ;
                            dc:identifier "2501" ;
                            dc:title "made of/require - material" ;
                            dct:description """things - [are] made of/require - material.
Example: obsidian mirrors are made of/require obsidian; ivories (sculptures) are made of/require ivory""" ;
                            rdfs:isDefinedBy <http://vocab.getty.edu/ontology> ,
                                             aat: ;
                            skos:example "ivories (sculptures) are made of/require ivory" ,
                                         "obsidian mirrors are made of/require obsidian" ;
                            skos:prefLabel "aat2501_made_of-require" .


###  http://vocab.getty.edu/ontology#aat2502_material_for
gvp:aat2502_material_for rdf:type owl:ObjectProperty ;
                         rdfs:subPropertyOf skos:related ;
                         rdfs:domain skos:Concept ;
                         rdfs:range skos:Concept ;
                         dc:identifier "2502" ;
                         dc:title "material for - things" ;
                         dct:description """material - [is] material for - things.
Example: obsidian is material for obsidian mirrors; ivory is material for ivories (sculptures)""" ;
                         rdfs:isDefinedBy <http://vocab.getty.edu/ontology> ,
                                          aat: ;
                         skos:example "ivory is material for ivories (sculptures)" ,
                                      "obsidian is material for obsidian mirrors" ;
                         skos:prefLabel "aat2502_material_for" .


###  http://vocab.getty.edu/ontology#aat2504_used-located_in
gvp:aat2504_used-located_in rdf:type owl:ObjectProperty ;
                            rdfs:subPropertyOf skos:related ;
                            owl:inverseOf gvp:aat2505_locus-setting_for ;
                            rdfs:domain skos:Concept ;
                            rdfs:range skos:Concept ;
                            dc:identifier "2504" ;
                            dc:title "used/located in - locus/setting" ;
                            dct:description """material - [is] used/located in - locus/setting.
Example: tephra is used/located in [at] volcanoes; brick (clay product) is used/located in brickworks (factories)""" ;
                            rdfs:isDefinedBy <http://vocab.getty.edu/ontology> ,
                                             aat: ;
                            skos:example "brick (clay product) is used/located in brickworks (factories)" ,
                                         "tephra is used/located in [at] volcanoes" ;
                            skos:prefLabel "aat2504_used-located_in" .


###  http://vocab.getty.edu/ontology#aat2505_locus-setting_for
gvp:aat2505_locus-setting_for rdf:type owl:ObjectProperty ;
                              rdfs:subPropertyOf skos:related ;
                              rdfs:domain skos:Concept ;
                              rdfs:range skos:Concept ;
                              dc:identifier "2505" ;
                              dc:title "locus/setting for - material" ;
                              dct:description """locus/setting - [is] locus/setting for - material.
Example: volcanoes are locus/setting for  tephra; brickworks (factories) are locus/setting for brick (clay product)""" ;
                              rdfs:isDefinedBy <http://vocab.getty.edu/ontology> ,
                                               aat: ;
                              skos:example "brickworks (factories) are locus/setting for brick (clay product)" ,
                                           "volcanoes are locus/setting for  tephra" ;
                              skos:prefLabel "aat2505_locus-setting_for" .


###  http://vocab.getty.edu/ontology#aat2507_produce-process
gvp:aat2507_produce-process rdf:type owl:ObjectProperty ;
                            rdfs:subPropertyOf skos:related ;
                            owl:inverseOf gvp:aat2508_produced-processed_by ;
                            rdfs:domain skos:Concept ;
                            rdfs:range skos:Concept ;
                            dc:identifier "2507" ;
                            dc:title "produce/process - material" ;
                            dct:description """things/[equipment] - produce/process - material.
Example: cotton (fiber) is produced/processed by cotton gins; groundwater is produced/processed by water wells""" ;
                            rdfs:isDefinedBy <http://vocab.getty.edu/ontology> ,
                                             aat: ;
                            skos:example "cotton (fiber) is produced/processed by cotton gins" ,
                                         "groundwater is produced/processed by water wells" ;
                            skos:prefLabel "aat2507_produce-process" .


###  http://vocab.getty.edu/ontology#aat2508_produced-processed_by
gvp:aat2508_produced-processed_by rdf:type owl:ObjectProperty ;
                                  rdfs:subPropertyOf skos:related ;
                                  rdfs:domain skos:Concept ;
                                  rdfs:range skos:Concept ;
                                  dc:identifier "2508" ;
                                  dc:title "produced/processed by - things" ;
                                  dct:description """material - [is] produced/processed by - things/[equipment].
Example: cotton gins produce/process cotton (fiber); waterwells produce/process groundwater""" ;
                                  rdfs:isDefinedBy <http://vocab.getty.edu/ontology> ,
                                                   aat: ;
                                  skos:example "cotton gins produce/process cotton (fiber)" ,
                                               "waterwells produce/process groundwater" ;
                                  skos:prefLabel "aat2508_produced-processed_by" .


###  http://vocab.getty.edu/ontology#aat2551_reflect-produced_by
gvp:aat2551_reflect-produced_by rdf:type owl:ObjectProperty ;
                                rdfs:subPropertyOf skos:related ;
                                owl:inverseOf gvp:aat2552_reflected_in-produces ;
                                rdfs:domain skos:Concept ;
                                rdfs:range skos:Concept ;
                                dc:identifier "2551" ;
                                dc:title "reflect/produced by - style/period/culture" ;
                                dct:description """things - reflect/[are] produced by - style/period/culture/[religion/ideology].
Example: Nasca lines reflect/are produced by Nasca [culture]; Judaica reflects/is produced by Judaism""" ;
                                rdfs:isDefinedBy <http://vocab.getty.edu/ontology> ,
                                                 aat: ;
                                skos:example "Judaica reflects/is produced by Judaism" ,
                                             "Nasca lines reflect/are produced by Nasca [culture]" ;
                                skos:prefLabel "aat2551_reflect-produced_by" .


###  http://vocab.getty.edu/ontology#aat2552_reflected_in-produces
gvp:aat2552_reflected_in-produces rdf:type owl:ObjectProperty ;
                                  rdfs:subPropertyOf skos:related ;
                                  rdfs:domain skos:Concept ;
                                  rdfs:range skos:Concept ;
                                  dc:identifier "2552" ;
                                  dc:title "reflected in/produces - things" ;
                                  dct:description """style/period/culture/[religion/ideology] - [is] reflected in/produces - things.
Example: Nasca [culture] produces/is reflected in Nasca lines; Judaism produces/is reflected in Judaica""" ;
                                  rdfs:isDefinedBy <http://vocab.getty.edu/ontology> ,
                                                   aat: ;
                                  skos:example "Judaism produces/is reflected in Judaica" ,
                                               "Nasca [culture] produces/is reflected in Nasca lines" ;
                                  skos:prefLabel "aat2552_reflected_in-produces" .


###  http://vocab.getty.edu/ontology#aat2554_reflects
gvp:aat2554_reflects rdf:type owl:ObjectProperty ;
                     rdfs:subPropertyOf skos:related ;
                     owl:inverseOf gvp:aat2555_reflected_in ;
                     rdfs:domain skos:Concept ;
                     rdfs:range skos:Concept ;
                     dc:identifier "2554" ;
                     dc:title "reflects - style/period/culture" ;
                     dct:description """activity/event - reflects - style/period/culture /[religion/ideology].
Example: dhokra (casting technique) reflects Dhokra (culture); red-figure vase painting reflects Red-figure [style]""" ;
                     rdfs:isDefinedBy <http://vocab.getty.edu/ontology> ,
                                      aat: ;
                     skos:example "dhokra (casting technique) reflects Dhokra (culture)" ,
                                  "red-figure vase painting reflects Red-figure [style]" ;
                     skos:prefLabel "aat2554_reflects" .


###  http://vocab.getty.edu/ontology#aat2555_reflected_in
gvp:aat2555_reflected_in rdf:type owl:ObjectProperty ;
                         rdfs:subPropertyOf skos:related ;
                         rdfs:domain skos:Concept ;
                         rdfs:range skos:Concept ;
                         dc:identifier "2555" ;
                         dc:title "reflected in - activity/event" ;
                         dct:description """style/period/culture /[religion/ideology] - [is] reflected in activity/event.
Example: Dhokra (culture) is reflected in dhokra (casting technique); Red-figure [style] is reflected in red-figure vase painting""" ;
                         rdfs:isDefinedBy <http://vocab.getty.edu/ontology> ,
                                          aat: ;
                         skos:example "Dhokra (culture) is reflected in dhokra (casting technique)" ,
                                      "Red-figure [style] is reflected in red-figure vase painting" ;
                         skos:prefLabel "aat2555_reflected_in" .


###  http://vocab.getty.edu/ontology#aat2557_reflects
gvp:aat2557_reflects rdf:type owl:ObjectProperty ;
                     rdfs:subPropertyOf skos:related ;
                     owl:inverseOf gvp:aat2558_reflected_in ;
                     rdfs:domain skos:Concept ;
                     rdfs:range skos:Concept ;
                     dc:identifier "2557" ;
                     dc:title "reflects - style/period/culture" ;
                     dct:description """field/discipline - reflects - style/period/culture /[religion/ideology].
Example: bugatu [dance discipline] reflects Buddhism; church history reflects Christianity; classics (discipline) reflects Ancient Greek [culture]""" ;
                     rdfs:isDefinedBy <http://vocab.getty.edu/ontology> ,
                                      aat: ;
                     skos:example "bugatu [dance discipline] reflects Buddhism" ,
                                  "church history reflects Christianity" ,
                                  "classics (discipline) reflects Ancient Greek [culture]" ;
                     skos:prefLabel "aat2557_reflects" .


###  http://vocab.getty.edu/ontology#aat2558_reflected_in
gvp:aat2558_reflected_in rdf:type owl:ObjectProperty ;
                         rdfs:subPropertyOf skos:related ;
                         rdfs:domain skos:Concept ;
                         rdfs:range skos:Concept ;
                         dc:identifier "2558" ;
                         dc:title "reflected in - field/discipline" ;
                         dct:description """style/period/culture /[religion/ideology] - [is] reflected in field/discipline.
Example: Buddhism is reflected in bugatu [dance discipline]; Christianity is reflected in church history; Ancient Greek [culture] is reflected in classics (discipline)""" ;
                         rdfs:isDefinedBy <http://vocab.getty.edu/ontology> ,
                                          aat: ;
                         skos:example "Ancient Greek [culture] is reflected in classics (discipline)" ,
                                      "Buddhism is reflected in bugatu [dance discipline]" ,
                                      "Christianity is reflected in church history" ;
                         skos:prefLabel "aat2558_reflected_in" .


###  http://vocab.getty.edu/ontology#aat2562_locus-setting_for
gvp:aat2562_locus-setting_for rdf:type owl:ObjectProperty ;
                              rdfs:subPropertyOf skos:related ;
                              owl:inverseOf gvp:aat2563_located_in ;
                              rdfs:domain skos:Concept ;
                              rdfs:range skos:Concept ;
                              dc:identifier "2562" ;
                              dc:title "locus/setting for - style/period/culture" ;
                              dct:description """locus/setting - [is] locus/setting for - style/period/culture/[religion/ideology].
Example: First Nations reserves are the locus/setting for First Nations (culture); agraharas are the locus/setting for Brahmanism""" ;
                              rdfs:isDefinedBy <http://vocab.getty.edu/ontology> ,
                                               aat: ;
                              skos:example "First Nations reserves are the locus/setting for First Nations (culture)" ,
                                           "agraharas are the locus/setting for Brahmanism" ;
                              skos:prefLabel "aat2562_locus-setting_for" .


###  http://vocab.getty.edu/ontology#aat2563_located_in
gvp:aat2563_located_in rdf:type owl:ObjectProperty ;
                       rdfs:subPropertyOf skos:related ;
                       rdfs:domain skos:Concept ;
                       rdfs:range skos:Concept ;
                       dc:identifier "2563" ;
                       dc:title "located in - locus/setting" ;
                       dct:description """style/period/culture/[religion/ideology] - is located/[reflected] in - locus/setting.
Example: First Nations (culture) is located/reflected in First Nations reserves; Brahmanism is located/reflected in agraharas""" ;
                       rdfs:isDefinedBy <http://vocab.getty.edu/ontology> ,
                                        aat: ;
                       skos:example "Brahmanism is located/reflected in agraharas" ,
                                    "First Nations (culture) is located/reflected in First Nations reserves" ;
                       skos:prefLabel "aat2563_located_in" .


###  http://vocab.getty.edu/ontology#aat2601_possessed_by-existing_in
gvp:aat2601_possessed_by-existing_in rdf:type owl:ObjectProperty ;
                                     rdfs:subPropertyOf skos:related ;
                                     owl:inverseOf gvp:aat2602_possess-exist_in ;
                                     rdfs:domain skos:Concept ;
                                     rdfs:range skos:Concept ;
                                     dc:identifier "2601" ;
                                     dc:title "possessed by/existing in - role" ;
                                     dct:description """attributes /associated concepts - [is] possessed by/existing in - role [of actors].
Example: adulthood is possessed by/existing in adults; nomadism is possessed by/existing in nomads""" ;
                                     rdfs:isDefinedBy <http://vocab.getty.edu/ontology> ,
                                                      aat: ;
                                     skos:example "adulthood is possessed by/existing in adults" ,
                                                  "nomadism is possessed by/existing in nomads" ;
                                     skos:prefLabel "aat2601_possessed_by-existing_in" .


###  http://vocab.getty.edu/ontology#aat2602_possess-exist_in
gvp:aat2602_possess-exist_in rdf:type owl:ObjectProperty ;
                             rdfs:subPropertyOf skos:related ;
                             rdfs:domain skos:Concept ;
                             rdfs:range skos:Concept ;
                             dc:identifier "2602" ;
                             dc:title "possess/exist in - attributes /associated concepts" ;
                             dct:description """role [of actors] - possess/exist in - attributes /associated concepts.
Example: adults possess/exist in adulthood; nomads possess/exist in [state of] nomadism""" ;
                             rdfs:isDefinedBy <http://vocab.getty.edu/ontology> ,
                                              aat: ;
                             skos:example "adults possess/exist in adulthood" ,
                                          "nomads possess/exist in [state of] nomadism" ;
                             skos:prefLabel "aat2602_possess-exist_in" .


###  http://vocab.getty.edu/ontology#aat2604_possessed_by-existing_in
gvp:aat2604_possessed_by-existing_in rdf:type owl:ObjectProperty ;
                                     rdfs:subPropertyOf skos:related ;
                                     owl:inverseOf gvp:aat2605_possess-exist_in ;
                                     rdfs:domain skos:Concept ;
                                     rdfs:range skos:Concept ;
                                     dc:identifier "2604" ;
                                     dc:title "possessed by/existing in - things" ;
                                     dct:description """attributes /associated concepts - [is] possessed by/existing in - things.
Example: boudoir (photograph size) is possessed by/existing in boudoir photographs; ruined [condition] is possessed by/existing in ruins""" ;
                                     rdfs:isDefinedBy <http://vocab.getty.edu/ontology> ,
                                                      aat: ;
                                     skos:example "boudoir (photograph size) is possessed by/existing in boudoir photographs" ,
                                                  "ruined [condition] is possessed by/existing in ruins" ;
                                     skos:prefLabel "aat2604_possessed_by-existing_in" .


###  http://vocab.getty.edu/ontology#aat2605_possess-exist_in
gvp:aat2605_possess-exist_in rdf:type owl:ObjectProperty ;
                             rdfs:subPropertyOf skos:related ;
                             rdfs:domain skos:Concept ;
                             rdfs:range skos:Concept ;
                             dc:identifier "2605" ;
                             dc:title "possess/exist in - attributes /associated concepts" ;
                             dct:description """things - possess/exist in - attributes /associated concepts.
Example: boudoir photographs possess/exist in boudoir (photograph size); ruins possess/exist in ruined [contition]""" ;
                             rdfs:isDefinedBy <http://vocab.getty.edu/ontology> ,
                                              aat: ;
                             skos:example "boudoir photographs possess/exist in boudoir (photograph size)" ,
                                          "ruins possess/exist in ruined [contition]" ;
                             skos:prefLabel "aat2605_possess-exist_in" .


###  http://vocab.getty.edu/ontology#aat2607_caused_by-requires
gvp:aat2607_caused_by-requires rdf:type owl:ObjectProperty ;
                               rdfs:subPropertyOf skos:related ;
                               owl:inverseOf gvp:aat2608_causes-required_for ;
                               rdfs:domain skos:Concept ;
                               rdfs:range skos:Concept ;
                               dc:identifier "2607" ;
                               dc:title "caused by/requires - activity/event" ;
                               dct:description """attributes /associated concepts - [is] caused by/requires - an activity/event/[process/function].
Example: watertightness is caused by/requires waterproofing; creases (condition) is caused by/requires creasing (process)""" ;
                               rdfs:isDefinedBy <http://vocab.getty.edu/ontology> ,
                                                aat: ;
                               skos:example "creases (condition) is caused by/requires creasing (process)" ,
                                            "watertightness is caused by/requires waterproofing" ;
                               skos:prefLabel "aat2607_caused_by-requires" .


###  http://vocab.getty.edu/ontology#aat2608_causes-required_for
gvp:aat2608_causes-required_for rdf:type owl:ObjectProperty ;
                                rdfs:subPropertyOf skos:related ;
                                rdfs:domain skos:Concept ;
                                rdfs:range skos:Concept ;
                                dc:identifier "2608" ;
                                dc:title "causes/required for - attributes /associated concepts" ;
                                dct:description """activity/event/[process/function] - causes/[is] required for - [a] state/condition/attributes.
Example: waterproofing causes/is required for watertighness; creasing (process) causes/is required for creases (condition)""" ;
                                rdfs:isDefinedBy <http://vocab.getty.edu/ontology> ,
                                                 aat: ;
                                skos:example "creasing (process) causes/is required for creases (condition)" ,
                                             "waterproofing causes/is required for watertighness" ;
                                skos:prefLabel "aat2608_causes-required_for" .


###  http://vocab.getty.edu/ontology#aat2612_possessed_by-existing_in
gvp:aat2612_possessed_by-existing_in rdf:type owl:ObjectProperty ;
                                     rdfs:subPropertyOf skos:related ;
                                     owl:inverseOf gvp:aat2613_possess-exist_in ;
                                     rdfs:domain skos:Concept ;
                                     rdfs:range skos:Concept ;
                                     dc:identifier "2612" ;
                                     dc:title "possessed by/existing in - material" ;
                                     dct:description """attributes /associated concepts - is possessed by/existing in - material.
Example: dry rot is possessed by/existing in wood(plant material); dielectric properties are possessed by/existing in dielectric (material)""" ;
                                     rdfs:isDefinedBy <http://vocab.getty.edu/ontology> ,
                                                      aat: ;
                                     skos:example "dielectric properties are possessed by/existing in dielectric (material)" ,
                                                  "dry rot is possessed by/existing in wood(plant material)" ;
                                     skos:prefLabel "aat2612_possessed_by-existing_in" .


###  http://vocab.getty.edu/ontology#aat2613_possess-exist_in
gvp:aat2613_possess-exist_in rdf:type owl:ObjectProperty ;
                             rdfs:subPropertyOf skos:related ;
                             rdfs:domain skos:Concept ;
                             rdfs:range skos:Concept ;
                             dc:identifier "2613" ;
                             dc:title "possess/exist in - attributes /associated concepts" ;
                             dct:description """material - possesses/exists in - condition/state/[property].
Example: wood(plant material) possesses/exists in [condition of] dry rot; dielectric (material) possesses/exists in dielectric properties""" ;
                             rdfs:isDefinedBy <http://vocab.getty.edu/ontology> ,
                                              aat: ;
                             skos:example "dielectric (material) possesses/exists in dielectric properties" ,
                                          "wood(plant material) possesses/exists in [condition of] dry rot" ;
                             skos:prefLabel "aat2613_possess-exist_in" .


###  http://vocab.getty.edu/ontology#aat2801_conjuncted_with
gvp:aat2801_conjuncted_with rdf:type owl:ObjectProperty ;
                            rdfs:subPropertyOf skos:related ;
                            rdf:type owl:SymmetricProperty ;
                            rdfs:domain skos:Concept ;
                            rdfs:range skos:Concept ;
                            dc:identifier "2801" ;
                            dc:title "conjuncted with - things" ;
                            dct:description """things - [are] conjuncted with - things.
Example: cups are conjuncted with saucers; dining tables are conjuncted with dining chairs""" ;
                            rdfs:isDefinedBy <http://vocab.getty.edu/ontology> ,
                                             aat: ;
                            skos:example "cups are conjuncted with saucers" ,
                                         "dining tables are conjuncted with dining chairs" ;
                            skos:prefLabel "aat2801_conjuncted_with" .


###  http://vocab.getty.edu/ontology#aat2802_exemplified_by
gvp:aat2802_exemplified_by rdf:type owl:ObjectProperty ;
                           rdfs:subPropertyOf skos:related ;
                           owl:inverseOf gvp:aat2803_example_of ;
                           rdfs:domain skos:Concept ;
                           rdfs:range skos:Concept ;
                           dc:identifier "2802" ;
                           dc:title "exemplified by - brand name" ;
                           dct:description """material - [is] exemplified by - brand name.
Example: petrolium jelly is exemplified by Vaseline (TM); polytetrafluoroethyelene is exemplified by Teflon (TM)""" ;
                           rdfs:isDefinedBy <http://vocab.getty.edu/ontology> ,
                                            aat: ;
                           skos:example "petrolium jelly is exemplified by Vaseline (TM)" ,
                                        "polytetrafluoroethyelene is exemplified by Teflon (TM)" ;
                           skos:prefLabel "aat2802_exemplified_by" .


###  http://vocab.getty.edu/ontology#aat2803_example_of
gvp:aat2803_example_of rdf:type owl:ObjectProperty ;
                       rdfs:subPropertyOf skos:related ;
                       rdfs:domain skos:Concept ;
                       rdfs:range skos:Concept ;
                       dc:identifier "2803" ;
                       dc:title "example of - material" ;
                       dct:description """brand name - [is] example of - material.
Example: Vaseline (TM) is an example of petrolium jelly; Teflon (TM) is an example of polytetrafluoroethyelene""" ;
                       rdfs:isDefinedBy <http://vocab.getty.edu/ontology> ,
                                        aat: ;
                       skos:example "Teflon (TM) is an example of polytetrafluoroethyelene" ,
                                    "Vaseline (TM) is an example of petrolium jelly" ;
                       skos:prefLabel "aat2803_example_of" .


###  http://vocab.getty.edu/ontology#aat2805_contextualized_in
gvp:aat2805_contextualized_in rdf:type owl:ObjectProperty ;
                              rdfs:subPropertyOf skos:related ;
                              owl:inverseOf gvp:aat2806_provide_context ;
                              rdfs:domain skos:Concept ;
                              rdfs:range skos:Concept ;
                              dc:identifier "2805" ;
                              dc:title "contextualized in - things" ;
                              dct:description """[smaller] things - [are] contextualized in - [larger] things.
Example: predellas are contextualized in altarpieces; chapters are contextualized in books""" ;
                              rdfs:isDefinedBy <http://vocab.getty.edu/ontology> ,
                                               aat: ;
                              skos:example "chapters are contextualized in books" ,
                                           "predellas are contextualized in altarpieces" ;
                              skos:prefLabel "aat2805_contextualized_in" .


###  http://vocab.getty.edu/ontology#aat2806_provide_context
gvp:aat2806_provide_context rdf:type owl:ObjectProperty ;
                            rdfs:subPropertyOf skos:related ;
                            rdfs:domain skos:Concept ;
                            rdfs:range skos:Concept ;
                            dc:identifier "2806" ;
                            dc:title "provide context - things" ;
                            dct:description """[larger] things - provide context [for] - [smaller] things.
Example: altarpieces provide context for predellas; books provide context for chapters""" ;
                            rdfs:isDefinedBy <http://vocab.getty.edu/ontology> ,
                                             aat: ;
                            skos:example "altarpieces provide context for predellas" ,
                                         "books provide context for chapters" ;
                            skos:prefLabel "aat2806_provide_context" .


###  http://vocab.getty.edu/ontology#aat2807_derived_from_common_source
gvp:aat2807_derived_from_common_source rdf:type owl:ObjectProperty ;
                                       rdfs:subPropertyOf skos:related ;
                                       rdf:type owl:SymmetricProperty ;
                                       rdfs:domain skos:Concept ;
                                       rdfs:range skos:Concept ;
                                       dc:identifier "2807" ;
                                       dc:title "derived from common source - material" ;
                                       dct:description """material - [is] derived from common source [as] - material.
Example: malachite (mineral) is derived from common source with azurite (mineral); mustard(material) is derived from common source with mustard oil""" ;
                                       rdfs:isDefinedBy <http://vocab.getty.edu/ontology> ,
                                                        aat: ;
                                       skos:example "malachite (mineral) is derived from common source with azurite (mineral)" ,
                                                    "mustard(material) is derived from common source with mustard oil" ;
                                       skos:prefLabel "aat2807_derived_from_common_source" .


###  http://vocab.getty.edu/ontology#aat2809_coexisted_with
gvp:aat2809_coexisted_with rdf:type owl:ObjectProperty ;
                           rdfs:subPropertyOf skos:related ;
                           rdf:type owl:SymmetricProperty ;
                           rdfs:domain skos:Concept ;
                           rdfs:range skos:Concept ;
                           dc:identifier "2809" ;
                           dc:title "coexisted with - style/period/culture" ;
                           dct:description """style/period/culture/[religion/ideology] - coexisted with -  style/period/culture/[religion/ideology].
Example: Sangoan coexisted with Fauresmith; Early Minoan coexisted with Prepalatial""" ;
                           rdfs:isDefinedBy <http://vocab.getty.edu/ontology> ,
                                            aat: ;
                           skos:example "Early Minoan coexisted with Prepalatial" ,
                                        "Sangoan coexisted with Fauresmith" ;
                           skos:prefLabel "aat2809_coexisted_with" .


###  http://vocab.getty.edu/ontology#aat2811_preceded
gvp:aat2811_preceded rdf:type owl:ObjectProperty ;
                     rdfs:subPropertyOf skos:related ;
                     owl:inverseOf gvp:aat2812_followed ;
                     rdfs:domain skos:Concept ;
                     rdfs:range skos:Concept ;
                     dc:identifier "2811" ;
                     dc:title "preceded - style/period/culture" ;
                     dct:description """style/period/culture/[religion/ideology] - preceded  - style/period/culture/[religion/ideology].
Example: Impressionist preceded Abstract Impressionist; Acheulian preceded Micoquian""" ;
                     rdfs:isDefinedBy <http://vocab.getty.edu/ontology> ,
                                      aat: ;
                     skos:example "Acheulian preceded Micoquian" ,
                                  "Impressionist preceded Abstract Impressionist" ;
                     skos:prefLabel "aat2811_preceded" .


###  http://vocab.getty.edu/ontology#aat2812_followed
gvp:aat2812_followed rdf:type owl:ObjectProperty ;
                     rdfs:subPropertyOf skos:related ;
                     rdfs:domain skos:Concept ;
                     rdfs:range skos:Concept ;
                     dc:identifier "2812" ;
                     dc:title "followed - style/period/culture" ;
                     dct:description """style/period/culture/[religion/ideology] - followed  - style/period/culture/[religion/ideology].
Example: Abstract Impressionism followed Impressionist; Micoquian followed Acheulian""" ;
                     rdfs:isDefinedBy <http://vocab.getty.edu/ontology> ,
                                      aat: ;
                     skos:example "Abstract Impressionism followed Impressionist" ,
                                  "Micoquian followed Acheulian" ;
                     skos:prefLabel "aat2812_followed" .


###  http://vocab.getty.edu/ontology#aat2814_constituent_of
gvp:aat2814_constituent_of rdf:type owl:ObjectProperty ;
                           rdfs:subPropertyOf skos:related ;
                           owl:inverseOf gvp:aat2815_composed_of ;
                           rdfs:domain skos:Concept ;
                           rdfs:range skos:Concept ;
                           dc:identifier "2814" ;
                           dc:title "constituent of - material" ;
                           dct:description """material - [is] constituent of - material.
Example: titanium white is a constituent of composite white; iron oxide is a constituent of desert varnish""" ;
                           rdfs:isDefinedBy <http://vocab.getty.edu/ontology> ,
                                            aat: ;
                           skos:example "iron oxide is a constituent of desert varnish" ,
                                        "titanium white is a constituent of composite white" ;
                           skos:prefLabel "aat2814_constituent_of" .


###  http://vocab.getty.edu/ontology#aat2815_composed_of
gvp:aat2815_composed_of rdf:type owl:ObjectProperty ;
                        rdfs:subPropertyOf skos:related ;
                        rdfs:domain skos:Concept ;
                        rdfs:range skos:Concept ;
                        dc:identifier "2815" ;
                        dc:title "composed of - material" ;
                        dct:description """material - [is] composed of - material.
Example: composite white is composed of titanium white; desert varnish is composed of iron oxide""" ;
                        rdfs:isDefinedBy <http://vocab.getty.edu/ontology> ,
                                         aat: ;
                        skos:example "composite white is composed of titanium white" ,
                                     "desert varnish is composed of iron oxide" ;
                        skos:prefLabel "aat2815_composed_of" .


###  http://vocab.getty.edu/ontology#aat2817_derived-made_from
gvp:aat2817_derived-made_from rdf:type owl:ObjectProperty ;
                              rdfs:subPropertyOf skos:related ;
                              owl:inverseOf gvp:aat2818_source_for ;
                              rdfs:domain skos:Concept ;
                              rdfs:range skos:Concept ;
                              dc:identifier "2817" ;
                              dc:title "derived/made from - material" ;
                              dct:description """material - [is] derived/made from - material.
Example: gypsum is derived/made from from anhydrite; wood board is derived/made from timber (lumber)""" ;
                              rdfs:isDefinedBy <http://vocab.getty.edu/ontology> ,
                                               aat: ;
                              skos:example "gypsum is derived/made from from anhydrite" ,
                                           "wood board is derived/made from timber (lumber)" ;
                              skos:prefLabel "aat2817_derived-made_from" .


###  http://vocab.getty.edu/ontology#aat2818_source_for
gvp:aat2818_source_for rdf:type owl:ObjectProperty ;
                       rdfs:subPropertyOf skos:related ;
                       rdfs:domain skos:Concept ;
                       rdfs:range skos:Concept ;
                       dc:identifier "2818" ;
                       dc:title "source for - material" ;
                       dct:description """material - [is] source for - material.
Example: anhydrite is the source for gypsum; timber (lumber) is the source for wood board""" ;
                       rdfs:isDefinedBy <http://vocab.getty.edu/ontology> ,
                                        aat: ;
                       skos:example "anhydrite is the source for gypsum" ,
                                    "timber (lumber) is the source for wood board" ;
                       skos:prefLabel "aat2818_source_for" .


###  http://vocab.getty.edu/ontology#aat2821_based_on
gvp:aat2821_based_on rdf:type owl:ObjectProperty ;
                     rdfs:subPropertyOf skos:related ;
                     owl:inverseOf gvp:aat2822_basis_of ;
                     rdfs:domain skos:Concept ;
                     rdfs:range skos:Concept ;
                     dc:identifier "2821" ;
                     dc:title "based on - any" ;
                     dct:description """any - [is] based on - any.
Example: Neo-Gothic is based on Gothic (Medieval); curved [form attribute] is based on curves (geometric figures); pencils are based on plummets""" ;
                     rdfs:isDefinedBy <http://vocab.getty.edu/ontology> ,
                                      aat: ;
                     skos:example "Neo-Gothic is based on Gothic (Medieval)" ,
                                  "curved [form attribute] is based on curves (geometric figures)" ,
                                  "pencils are based on plummets" ;
                     skos:prefLabel "aat2821_based_on" .


###  http://vocab.getty.edu/ontology#aat2822_basis_of
gvp:aat2822_basis_of rdf:type owl:ObjectProperty ;
                     rdfs:subPropertyOf skos:related ;
                     rdfs:domain skos:Concept ;
                     rdfs:range skos:Concept ;
                     dc:identifier "2822" ;
                     dc:title "basis of - any" ;
                     dct:description """any - [is] basis of - any.
Example: Gothic (Medieval) is the basis of Neo-Gothic; curves (geometric figures) are the basis of curved [form attribute]; plummets are the basis of pencils""" ;
                     rdfs:isDefinedBy <http://vocab.getty.edu/ontology> ,
                                      aat: ;
                     skos:example "Gothic (Medieval) is the basis of Neo-Gothic" ,
                                  "curves (geometric figures) are the basis of curved [form attribute]" ,
                                  "plummets are the basis of pencils" ;
                     skos:prefLabel "aat2822_basis_of" .


###  http://vocab.getty.edu/ontology#aat2824_has_parallels_with
gvp:aat2824_has_parallels_with rdf:type owl:ObjectProperty ;
                               rdfs:subPropertyOf skos:related ;
                               rdf:type owl:SymmetricProperty ;
                               rdfs:domain skos:Concept ;
                               rdfs:range skos:Concept ;
                               dc:identifier "2824" ;
                               dc:title "has parallels with - style/period/culture" ;
                               dct:description """style/period/culture/[religion/ideology] - has parallels with - style/period/culture/[religion/ideology].
Example: Lagozza [culture] has parallels with Chasseen [culture];  Gnathian (pottery style) has parallels with West Slope (pottery style)""" ;
                               rdfs:isDefinedBy <http://vocab.getty.edu/ontology> ,
                                                aat: ;
                               skos:example "Gnathian (pottery style) has parallels with West Slope (pottery style)" ,
                                            "Lagozza [culture] has parallels with Chasseen [culture]" ;
                               skos:prefLabel "aat2824_has_parallels_with" .


###  http://vocab.getty.edu/ontology#aat2826_used_with
gvp:aat2826_used_with rdf:type owl:ObjectProperty ;
                      rdfs:subPropertyOf skos:related ;
                      rdf:type owl:SymmetricProperty ;
                      rdfs:domain skos:Concept ;
                      rdfs:range skos:Concept ;
                      dc:identifier "2826" ;
                      dc:title "used with - material" ;
                      dct:description """material - [is] used with - material.
Example: watercolor paper is used with watercolor (paint); arriccio is used with intonaco""" ;
                      rdfs:isDefinedBy <http://vocab.getty.edu/ontology> ,
                                       aat: ;
                      skos:example "arriccio is used with intonaco" ,
                                   "watercolor paper is used with watercolor (paint)" ;
                      skos:prefLabel "aat2826_used_with" .


###  http://vocab.getty.edu/ontology#aat2828_use-require
gvp:aat2828_use-require rdf:type owl:ObjectProperty ;
                        rdfs:subPropertyOf skos:related ;
                        owl:inverseOf gvp:aat2829_used-required_for ;
                        rdfs:domain skos:Concept ;
                        rdfs:range skos:Concept ;
                        dc:identifier "2828" ;
                        dc:title "use/require - material" ;
                        dct:description """things - use/require - material.
Example: oil paintings use/require varnish; wine glasses use/require wine""" ;
                        rdfs:isDefinedBy <http://vocab.getty.edu/ontology> ,
                                         aat: ;
                        skos:example "oil paintings use/require varnish" ,
                                     "wine glasses use/require wine" ;
                        skos:prefLabel "aat2828_use-require" .


###  http://vocab.getty.edu/ontology#aat2829_used-required_for
gvp:aat2829_used-required_for rdf:type owl:ObjectProperty ;
                              rdfs:subPropertyOf skos:related ;
                              rdfs:domain skos:Concept ;
                              rdfs:range skos:Concept ;
                              dc:identifier "2829" ;
                              dc:title "used/required for - things" ;
                              dct:description """material - [is] required/used for - things.
Example: varnish is used/required for oil paintings; wine is required/used for wine glasses""" ;
                              rdfs:isDefinedBy <http://vocab.getty.edu/ontology> ,
                                               aat: ;
                              skos:example "varnish is used/required for oil paintings" ,
                                           "wine is required/used for wine glasses" ;
                              skos:prefLabel "aat2829_used-required_for" .


###  http://vocab.getty.edu/ontology#aat2831_associated_with
gvp:aat2831_associated_with rdf:type owl:ObjectProperty ;
                            rdfs:subPropertyOf skos:related ;
                            rdf:type owl:SymmetricProperty ;
                            rdfs:domain skos:Concept ;
                            rdfs:range skos:Concept ;
                            dc:identifier "2831" ;
                            dc:title "associated with - genus/species" ;
                            dct:description """genus/species/[other living organism term] - [is] associated with - genus/species.
Example: Anthonomus grandis (species) [boll weevil] is associated with Gossypium (genus) [cotton]; Amphiprioninae (subfamily) [clown fish] is associated with Actiniaria (order) [sea anemone]""" ;
                            rdfs:isDefinedBy <http://vocab.getty.edu/ontology> ,
                                             aat: ;
                            skos:example "Amphiprioninae (subfamily) [clown fish] is associated with Actiniaria (order) [sea anemone]" ,
                                         "Anthonomus grandis (species) [boll weevil] is associated with Gossypium (genus) [cotton]" ;
                            skos:prefLabel "aat2831_associated_with" .


###  http://vocab.getty.edu/ontology#aat2833_ancestor_of
gvp:aat2833_ancestor_of rdf:type owl:ObjectProperty ;
                        rdfs:subPropertyOf skos:related ;
                        owl:inverseOf gvp:aat2834_decendant_of ;
                        rdfs:domain skos:Concept ;
                        rdfs:range skos:Concept ;
                        dc:identifier "2833" ;
                        dc:title "ancestor of - genus/species" ;
                        dct:description """genus/species - is ancestor of -  another genus/species.
Example: Canis lupus is the ancestor of Canis familiaris; Equus asinus is the ancestor of donkeys""" ;
                        rdfs:isDefinedBy <http://vocab.getty.edu/ontology> ,
                                         aat: ;
                        skos:example "Canis lupus is the ancestor of Canis familiaris" ,
                                     "Equus asinus is the ancestor of donkeys" ;
                        skos:prefLabel "aat2833_ancestor_of" .


###  http://vocab.getty.edu/ontology#aat2834_decendant_of
gvp:aat2834_decendant_of rdf:type owl:ObjectProperty ;
                         rdfs:subPropertyOf skos:related ;
                         rdfs:domain skos:Concept ;
                         rdfs:range skos:Concept ;
                         dc:identifier "2834" ;
                         dc:title "decendant of - genus/species" ;
                         dct:description """genus/species - is decendant of -  genus/species.
Example: Canis familiaris is the descendant of Canis lupus; donkeys are the descendents of Equus asinus""" ;
                         rdfs:isDefinedBy <http://vocab.getty.edu/ontology> ,
                                          aat: ;
                         skos:example "Canis familiaris is the descendant of Canis lupus" ,
                                      "donkeys are the descendents of Equus asinus" ;
                         skos:prefLabel "aat2834_decendant_of" .


###  http://vocab.getty.edu/ontology#aat2836_derived-made_from
gvp:aat2836_derived-made_from rdf:type owl:ObjectProperty ;
                              rdfs:subPropertyOf skos:related ;
                              owl:inverseOf gvp:aat2837_source_for ;
                              rdfs:domain skos:Concept ;
                              rdfs:range skos:Concept ;
                              dc:identifier "2836" ;
                              dc:title "derived/made from - genus/species" ;
                              dct:description """things - [are] derived/made from - genus/species [or its parts].
Example: k?kaku are derived/made from Phormium tenax (species); ostrich-egg cups are derived/made from Struthio camelus (species)""" ;
                              rdfs:isDefinedBy <http://vocab.getty.edu/ontology> ,
                                               aat: ;
                              skos:example "k?kaku are derived/made from Phormium tenax (species)" ,
                                           "ostrich-egg cups are derived/made from Struthio camelus (species)" ;
                              skos:prefLabel "aat2836_derived-made_from" .


###  http://vocab.getty.edu/ontology#aat2837_source_for
gvp:aat2837_source_for rdf:type owl:ObjectProperty ;
                       rdfs:subPropertyOf skos:related ;
                       rdfs:domain skos:Concept ;
                       rdfs:range skos:Concept ;
                       dc:identifier "2837" ;
                       dc:title "source for - things" ;
                       dct:description """genus/species [or its parts] - [is] source for - things.
Example: Phormium tenax (species) is the source for k?kaku; Struthio camelus(species) is the source for ostrich-egg cups""" ;
                       rdfs:isDefinedBy <http://vocab.getty.edu/ontology> ,
                                        aat: ;
                       skos:example "Phormium tenax (species) is the source for k?kaku" ,
                                    "Struthio camelus(species) is the source for ostrich-egg cups" ;
                       skos:prefLabel "aat2837_source_for" .


###  http://vocab.getty.edu/ontology#aat2841_derived-made_from
gvp:aat2841_derived-made_from rdf:type owl:ObjectProperty ;
                              rdfs:subPropertyOf skos:related ;
                              owl:inverseOf gvp:aat2842_source_for ;
                              rdfs:domain skos:Concept ;
                              rdfs:range skos:Concept ;
                              dc:identifier "2841" ;
                              dc:title "derived/made from - genus/species" ;
                              dct:description """material - [is] derived/made from - genus/species.
Example: alpaca (wool) is derived from Vicugna pacos (species); maple (wood) is derived from Acer (genus)""" ;
                              rdfs:isDefinedBy <http://vocab.getty.edu/ontology> ,
                                               aat: ;
                              skos:example "alpaca (wool) is derived from Vicugna pacos (species)" ,
                                           "maple (wood) is derived from Acer (genus)" ;
                              skos:prefLabel "aat2841_derived-made_from" .


###  http://vocab.getty.edu/ontology#aat2842_source_for
gvp:aat2842_source_for rdf:type owl:ObjectProperty ;
                       rdfs:subPropertyOf skos:related ;
                       rdfs:domain skos:Concept ;
                       rdfs:range skos:Concept ;
                       dc:identifier "2842" ;
                       dc:title "source for - material" ;
                       dct:description """genus/species - [is] source for - material.
Example: Vicugna pacos (species) is the source for alpaca (wool); Acer (genus) is the source for maple (wood)""" ;
                       rdfs:isDefinedBy <http://vocab.getty.edu/ontology> ,
                                        aat: ;
                       skos:example "Acer (genus) is the source for maple (wood)" ,
                                    "Vicugna pacos (species) is the source for alpaca (wool)" ;
                       skos:prefLabel "aat2842_source_for" .


###  http://vocab.getty.edu/ontology#aat2845_used-located_in
gvp:aat2845_used-located_in rdf:type owl:ObjectProperty ;
                            rdfs:subPropertyOf skos:related ;
                            owl:inverseOf gvp:aat2846_locus-setting_for ;
                            rdfs:domain skos:Concept ;
                            rdfs:range skos:Concept ;
                            dc:identifier "2845" ;
                            dc:title "used/located in - locus/setting" ;
                            dct:description """genus/species - [is] used/located in -  locus/setting.
Example: Elephantidae(family) are used/located in elephant houses; Vitaceae (family) is used/located in vineyards""" ;
                            rdfs:isDefinedBy <http://vocab.getty.edu/ontology> ,
                                             aat: ;
                            skos:example "Elephantidae(family) are used/located in elephant houses" ,
                                         "Vitaceae (family) is used/located in vineyards" ;
                            skos:prefLabel "aat2845_used-located_in" .


###  http://vocab.getty.edu/ontology#aat2846_locus-setting_for
gvp:aat2846_locus-setting_for rdf:type owl:ObjectProperty ;
                              rdfs:subPropertyOf skos:related ;
                              rdfs:domain skos:Concept ;
                              rdfs:range skos:Concept ;
                              dc:identifier "2846" ;
                              dc:title "locus/setting for - genus/species" ;
                              dct:description """locus/setting - [is] locus/setting for - genus/species.
Example: elephant houses are the locus/setting for Elephantidae(family); vineyards are the locus/setting of Vitaceae (family)""" ;
                              rdfs:isDefinedBy <http://vocab.getty.edu/ontology> ,
                                               aat: ;
                              skos:example "elephant houses are the locus/setting for Elephantidae(family)" ,
                                           "vineyards are the locus/setting of Vitaceae (family)" ;
                              skos:prefLabel "aat2846_locus-setting_for" .


###  http://vocab.getty.edu/ontology#aat2848_involved_in
gvp:aat2848_involved_in rdf:type owl:ObjectProperty ;
                        rdfs:subPropertyOf skos:related ;
                        owl:inverseOf gvp:aat2849_involves ;
                        rdfs:domain skos:Concept ;
                        rdfs:range skos:Concept ;
                        dc:identifier "2848" ;
                        dc:title "involved in - activity/event" ;
                        dct:description """genus/species - is involved in - activity/event.
Example: bulls (animals) are involved in bullfighting; Equus caballus (species) is involved in polo(field sport)""" ;
                        rdfs:isDefinedBy <http://vocab.getty.edu/ontology> ,
                                         aat: ;
                        skos:example "Equus caballus (species) is involved in polo(field sport)" ,
                                     "bulls (animals) are involved in bullfighting" ;
                        skos:prefLabel "aat2848_involved_in" .


###  http://vocab.getty.edu/ontology#aat2849_involves
gvp:aat2849_involves rdf:type owl:ObjectProperty ;
                     rdfs:subPropertyOf skos:related ;
                     rdfs:domain skos:Concept ;
                     rdfs:range skos:Concept ;
                     dc:identifier "2849" ;
                     dc:title "involves - genus/species" ;
                     dct:description """activity/event - involves - genus/species.
Example: bullfighting involves bulls (animals); polo (field sport) involves Equus caballus (species)""" ;
                     rdfs:isDefinedBy <http://vocab.getty.edu/ontology> ,
                                      aat: ;
                     skos:example "bullfighting involves bulls (animals)" ,
                                  "polo (field sport) involves Equus caballus (species)" ;
                     skos:prefLabel "aat2849_involves" .


###  http://vocab.getty.edu/ontology#aat2852_involved_with
gvp:aat2852_involved_with rdf:type owl:ObjectProperty ;
                          rdfs:subPropertyOf skos:related ;
                          owl:inverseOf gvp:aat2853_involve ;
                          rdfs:domain skos:Concept ;
                          rdfs:range skos:Concept ;
                          dc:identifier "2852" ;
                          dc:title "involved with - things" ;
                          dct:description """genus/species - [is] involved with - things/[equipment].
Example: Rosa (genus) is involved with rose bowls; Camelus (genus) is involved with camel saddles""" ;
                          rdfs:isDefinedBy <http://vocab.getty.edu/ontology> ,
                                           aat: ;
                          skos:example "Camelus (genus) is involved with camel saddles" ,
                                       "Rosa (genus) is involved with rose bowls" ;
                          skos:prefLabel "aat2852_involved_with" .


###  http://vocab.getty.edu/ontology#aat2853_involve
gvp:aat2853_involve rdf:type owl:ObjectProperty ;
                    rdfs:subPropertyOf skos:related ;
                    rdfs:domain skos:Concept ;
                    rdfs:range skos:Concept ;
                    dc:identifier "2853" ;
                    dc:title "involve - genus/species" ;
                    dct:description """things/[equipment] - involve - genus/species.
Example: rose bowls involve Rosa (genus); camel saddles involve Camelus (genus)""" ;
                    rdfs:isDefinedBy <http://vocab.getty.edu/ontology> ,
                                     aat: ;
                    skos:example "camel saddles involve Camelus (genus)" ,
                                 "rose bowls involve Rosa (genus)" ;
                    skos:prefLabel "aat2853_involve" .


###  http://vocab.getty.edu/ontology#aat2875_characteristic_of
gvp:aat2875_characteristic_of rdf:type owl:ObjectProperty ;
                              rdfs:subPropertyOf skos:related ;
                              owl:inverseOf gvp:aat2876_characterized_by ;
                              rdfs:domain skos:Concept ;
                              rdfs:range skos:Concept ;
                              dc:identifier "2875" ;
                              dc:title "characteristic of - style/period/culture" ;
                              dct:description """language - [is] characteristic of - style/period/culture.
Example: Afar (language) is characteristic of Afar (culture); Celtic (language) was characteristic of Celtic (culture)""" ;
                              rdfs:isDefinedBy <http://vocab.getty.edu/ontology> ,
                                               aat: ;
                              skos:example "Afar (language) is characteristic of Afar (culture)" ,
                                           "Celtic (language) was characteristic of Celtic (culture)" ;
                              skos:prefLabel "aat2875_characteristic_of" .


###  http://vocab.getty.edu/ontology#aat2876_characterized_by
gvp:aat2876_characterized_by rdf:type owl:ObjectProperty ;
                             rdfs:subPropertyOf skos:related ;
                             rdfs:domain skos:Concept ;
                             rdfs:range skos:Concept ;
                             dc:identifier "2876" ;
                             dc:title "characterized by - language" ;
                             dct:description """style/period/culture - [is] characterized by - language.
Example: Afar (culture) is characterized by Afar (language); Celtic (culture) is characterized by Celtic (language)""" ;
                             rdfs:isDefinedBy <http://vocab.getty.edu/ontology> ,
                                              aat: ;
                             skos:example "Afar (culture) is characterized by Afar (language)" ,
                                          "Celtic (culture) is characterized by Celtic (language)" ;
                             skos:prefLabel "aat2876_characterized_by" .


###  http://vocab.getty.edu/ontology#aat2878_preceded-source_for
gvp:aat2878_preceded-source_for rdf:type owl:ObjectProperty ;
                                rdfs:subPropertyOf skos:related ;
                                owl:inverseOf gvp:aat2879_followed-developed_from ;
                                rdfs:domain skos:Concept ;
                                rdfs:range skos:Concept ;
                                dc:identifier "2878" ;
                                dc:title "preceded/source for - language" ;
                                dct:description """language - preceded/[is] source for - language.
Example: Ancient Greek (language) preceded/is source for Greek (modern language); Ancient Egyptian (language) preceded/is source for Egyptian, Coptic (language)""" ;
                                rdfs:isDefinedBy <http://vocab.getty.edu/ontology> ,
                                                 aat: ;
                                skos:example "Ancient Egyptian (language) preceded/is source for Egyptian, Coptic (language)" ,
                                             "Ancient Greek (language) preceded/is source for Greek (modern language)" ;
                                skos:prefLabel "aat2878_preceded-source_for" .


###  http://vocab.getty.edu/ontology#aat2879_followed-developed_from
gvp:aat2879_followed-developed_from rdf:type owl:ObjectProperty ;
                                    rdfs:subPropertyOf skos:related ;
                                    rdfs:domain skos:Concept ;
                                    rdfs:range skos:Concept ;
                                    dc:identifier "2879" ;
                                    dc:title "followed/developed from - language" ;
                                    dct:description """language - followed/developed from - language.
Example: Greek (modern language) followed/developed from Ancient Greek (language); Egyptian, Coptic (language) followed/developed from Ancient Egyptian (language)""" ;
                                    rdfs:isDefinedBy <http://vocab.getty.edu/ontology> ,
                                                     aat: ;
                                    skos:example "Egyptian, Coptic (language) followed/developed from Ancient Egyptian (language)" ,
                                                 "Greek (modern language) followed/developed from Ancient Greek (language)" ;
                                    skos:prefLabel "aat2879_followed-developed_from" .


###  http://vocab.getty.edu/ontology#aat2881_reflected_in
gvp:aat2881_reflected_in rdf:type owl:ObjectProperty ;
                         rdfs:subPropertyOf skos:related ;
                         owl:inverseOf gvp:aat2882_reflect ;
                         rdfs:domain skos:Concept ;
                         rdfs:range skos:Concept ;
                         dc:identifier "2881" ;
                         dc:title "reflected in - things" ;
                         dct:description """language - [is] reflected in - things.
Example: Greek (language) is reflected in Greek alphabet; Sanskrit is reflected in Vedas""" ;
                         rdfs:isDefinedBy <http://vocab.getty.edu/ontology> ,
                                          aat: ;
                         skos:example "Greek (language) is reflected in Greek alphabet" ,
                                      "Sanskrit is reflected in Vedas" ;
                         skos:prefLabel "aat2881_reflected_in" .


###  http://vocab.getty.edu/ontology#aat2882_reflect
gvp:aat2882_reflect rdf:type owl:ObjectProperty ;
                    rdfs:subPropertyOf skos:related ;
                    rdfs:domain skos:Concept ;
                    rdfs:range skos:Concept ;
                    dc:identifier "2882" ;
                    dc:title "reflect - language" ;
                    dct:description """things - reflect - language.
Example: Greek alphabet reflects Greek (language); Vedas reflect Sanskrit""" ;
                    rdfs:isDefinedBy <http://vocab.getty.edu/ontology> ,
                                     aat: ;
                    skos:example "Greek alphabet reflects Greek (language)" ,
                                 "Vedas reflect Sanskrit" ;
                    skos:prefLabel "aat2882_reflect" .


###  http://vocab.getty.edu/ontology#aat2884_involved_with
gvp:aat2884_involved_with rdf:type owl:ObjectProperty ;
                          rdfs:subPropertyOf skos:related ;
                          owl:inverseOf gvp:aat2885_involves ;
                          rdfs:domain skos:Concept ;
                          rdfs:range skos:Concept ;
                          dc:identifier "2884" ;
                          dc:title "involved with - any" ;
                          dct:description """attributes /associated concepts - [are] involved with - any.
Example: climate is involved with climate change; insect damage is involved with infestation; Celtic crosses (design motif) are involved with Celtic culture""" ;
                          rdfs:isDefinedBy <http://vocab.getty.edu/ontology> ,
                                           aat: ;
                          skos:example "Celtic crosses (design motif) are involved with Celtic culture" ,
                                       "climate is involved with climate change" ,
                                       "insect damage is involved with infestation" ;
                          skos:prefLabel "aat2884_involved_with" .


###  http://vocab.getty.edu/ontology#aat2885_involves
gvp:aat2885_involves rdf:type owl:ObjectProperty ;
                     rdfs:subPropertyOf skos:related ;
                     rdfs:domain skos:Concept ;
                     rdfs:range skos:Concept ;
                     dc:identifier "2885" ;
                     dc:title "involves - attributes /associated concepts" ;
                     dct:description """any - involves - attributes /associated concepts.
Example: climate change involves climate;  infestation involves insect damage; Celtic culture involves Celtic crosses (design motif)""" ;
                     rdfs:isDefinedBy <http://vocab.getty.edu/ontology> ,
                                      aat: ;
                     skos:example "Celtic culture involves Celtic crosses (design motif)" ,
                                  "climate change involves climate" ,
                                  "infestation involves insect damage" ;
                     skos:prefLabel "aat2885_involves" .


###  http://vocab.getty.edu/ontology#aat2886_used-function_as
gvp:aat2886_used-function_as rdf:type owl:ObjectProperty ;
                             rdfs:subPropertyOf skos:related ;
                             owl:inverseOf gvp:aat2887_exemplified_by ;
                             rdfs:domain skos:Concept ;
                             rdfs:range skos:Concept ;
                             dc:identifier "2886" ;
                             dc:title "used/function as - material" ;
                             dct:description """material - used/function as - material.
Example: carbon disulfide - is used/functions as - solvent""" ;
                             rdfs:isDefinedBy <http://vocab.getty.edu/ontology> ,
                                              aat: ;
                             skos:example "carbon disulfide - is used/functions as - solvent" ;
                             skos:prefLabel "aat2886_used-function_as" .


###  http://vocab.getty.edu/ontology#aat2887_exemplified_by
gvp:aat2887_exemplified_by rdf:type owl:ObjectProperty ;
                           rdfs:subPropertyOf skos:related ;
                           rdfs:domain skos:Concept ;
                           rdfs:range skos:Concept ;
                           dc:identifier "2887" ;
                           dc:title "exemplified by - material" ;
                           dct:description """material - exemplified by - material.
Example: solvent - exemplified by - carbon disulfide""" ;
                           rdfs:isDefinedBy <http://vocab.getty.edu/ontology> ,
                                            aat: ;
                           skos:example "solvent - exemplified by - carbon disulfide" ;
                           skos:prefLabel "aat2887_exemplified_by" .


###  http://vocab.getty.edu/ontology#aat2891_exemplified_by
gvp:aat2891_exemplified_by rdf:type owl:ObjectProperty ;
                           rdfs:subPropertyOf skos:related ;
                           owl:inverseOf gvp:aat2892_example_of ;
                           rdfs:domain skos:Concept ;
                           rdfs:range skos:Concept ;
                           dc:identifier "2891" ;
                           dc:title "exemplified by - brand name" ;
                           dct:description """things - [are] exemplied by - brand name.
Example: photothermographic transfer prints are exemplified by Pictrography (TM) prints""" ;
                           rdfs:isDefinedBy <http://vocab.getty.edu/ontology> ,
                                            aat: ;
                           skos:example "photothermographic transfer prints are exemplified by Pictrography (TM) prints" ;
                           skos:prefLabel "aat2891_exemplified_by" .


###  http://vocab.getty.edu/ontology#aat2892_example_of
gvp:aat2892_example_of rdf:type owl:ObjectProperty ;
                       rdfs:subPropertyOf skos:related ;
                       rdfs:domain skos:Concept ;
                       rdfs:range skos:Concept ;
                       dc:identifier "2892" ;
                       dc:title "example of - things" ;
                       dct:description """brand name - [is] example of - things.
Example: Pictrography (TM) prints are examples of photothermographic transfer prints""" ;
                       rdfs:isDefinedBy <http://vocab.getty.edu/ontology> ,
                                        aat: ;
                       skos:example "Pictrography (TM) prints are examples of photothermographic transfer prints" ;
                       skos:prefLabel "aat2892_example_of" .


###  http://vocab.getty.edu/ontology#aat2894_exemplified_by
gvp:aat2894_exemplified_by rdf:type owl:ObjectProperty ;
                           rdfs:subPropertyOf skos:related ;
                           owl:inverseOf gvp:aat2895_example_of ;
                           rdfs:domain skos:Concept ;
                           rdfs:range skos:Concept ;
                           dc:identifier "2894" ;
                           dc:title "exemplified by - brand name" ;
                           dct:description """activity/event/[process/function] - [is] exemplified by - brand name.
Example: deacidification [process/function] is exemplified by Papersave Process (TM)""" ;
                           rdfs:isDefinedBy <http://vocab.getty.edu/ontology> ,
                                            aat: ;
                           skos:example "deacidification [process/function] is exemplified by Papersave Process (TM)" ;
                           skos:prefLabel "aat2894_exemplified_by" .


###  http://vocab.getty.edu/ontology#aat2895_example_of
gvp:aat2895_example_of rdf:type owl:ObjectProperty ;
                       rdfs:subPropertyOf skos:related ;
                       rdfs:domain skos:Concept ;
                       rdfs:range skos:Concept ;
                       dc:identifier "2895" ;
                       dc:title "example of - activity/event" ;
                       dct:description """brand name - [is] example of - activity/event/[process/function].
Example: Papersave Process (TM) is example of deacidification [process/function]""" ;
                       rdfs:isDefinedBy <http://vocab.getty.edu/ontology> ,
                                        aat: ;
                       skos:example "Papersave Process (TM) is example of deacidification [process/function]" ;
                       skos:prefLabel "aat2895_example_of" .


###  http://vocab.getty.edu/ontology#aat2900_miscellaneous_relationship
gvp:aat2900_miscellaneous_relationship rdf:type owl:ObjectProperty ;
                                       rdfs:subPropertyOf skos:related ;
                                       rdf:type owl:SymmetricProperty ;
                                       rdfs:domain skos:Concept ;
                                       rdfs:range skos:Concept ;
                                       dc:identifier "2900" ;
                                       dc:title "miscellaneous relationship - any" ;
                                       dct:description """any - [has] miscellaneous relationship [to] - any.
Example: Conditions and Effects has miscellaneous relationship with Processes and Techniques""" ;
                                       rdfs:isDefinedBy <http://vocab.getty.edu/ontology> ,
                                                        aat: ;
                                       skos:example "Conditions and Effects has miscellaneous relationship with Processes and Techniques" ;
                                       skos:prefLabel "aat2900_miscellaneous_relationship" .


###  http://vocab.getty.edu/ontology#agentType
gvp:agentType rdf:type owl:ObjectProperty ;
              rdfs:domain gvp:Subject ;
              rdfs:range gvp:Subject ;
              dct:description "Type of a ULAN PersonConcept or GroupConcept. Domain is ULAN concept, range is AAT concept" ;
              rdfs:comment "Type of a ULAN PersonConcept or GroupConcept. Domain is ULAN concept, range is AAT concept" ;
              rdfs:isDefinedBy <http://vocab.getty.edu/ontology> ;
              rdfs:label "agentType" .


###  http://vocab.getty.edu/ontology#agentTypeNonPreferred
gvp:agentTypeNonPreferred rdf:type owl:ObjectProperty ;
                          rdfs:subPropertyOf gvp:agentType ;
                          rdfs:domain gvp:Subject ;
                          rdfs:range gvp:Subject ;
                          dct:description """A secondary type of a ULAN Person or Corporate body. Domain is ULAN concept, range is AAT concept.
Example: Non-preferred types of \"Albrecht Duerer Workshop\" (ULAN) include \"printmakers\" and painters\" (AAT)""" ;
                          rdfs:comment "A secondary type of a ULAN Person or Corporate body. Domain is ULAN concept, range is AAT concept" ;
                          rdfs:isDefinedBy <http://vocab.getty.edu/ontology> ;
                          rdfs:label "agentTypeNonPreferred" ;
                          skos:example "Non-preferred types of \"Albrecht Duerer Workshop\" (ULAN) include \"printmakers\" and painters\" (AAT)" .


###  http://vocab.getty.edu/ontology#agentTypePreferred
gvp:agentTypePreferred rdf:type owl:ObjectProperty ;
                       rdfs:subPropertyOf gvp:agentType ;
                       rdfs:domain gvp:Subject ;
                       rdfs:range gvp:Subject ;
                       dct:description """The primary type of a ULAN Person or Corporate body. Domain is ULAN concept, range is AAT concept.
Example: The preferred type of \"Albrecht Duerer Workshop\" (ULAN) is \"workshop\" (AAT)""" ;
                       rdfs:comment "The primary type of a ULAN Person or Corporate body. Domain is ULAN concept, range is AAT concept" ;
                       rdfs:isDefinedBy <http://vocab.getty.edu/ontology> ;
                       rdfs:label "agentTypePreferred" ;
                       skos:example "The preferred type of \"Albrecht Duerer Workshop\" (ULAN) is \"workshop\" (AAT)" .


###  http://vocab.getty.edu/ontology#biography
gvp:biography rdf:type owl:ObjectProperty ;
              rdfs:subPropertyOf gvp:biography ;
              rdfs:range gvp:Biography ;
              dct:description "Biography of an ULAN agent. Domain is schema:Person/Organization, range is gvp:Biography. The preferred biography fields are also directly available in the Person/Organization" ;
              rdfs:comment "Biography of an ULAN agent. Domain is schema:Person/Organization, range is gvp:Biography. The preferred biography fields are also directly available in the Person/Organization" ;
              rdfs:isDefinedBy <http://vocab.getty.edu/ontology> ;
              rdfs:label "biography" .


###  http://vocab.getty.edu/ontology#biographyNonPreferred
gvp:biographyNonPreferred rdf:type owl:ObjectProperty ;
                          rdfs:subPropertyOf gvp:biography ;
                          rdfs:range gvp:Biography ;
                          dct:description "Non-preferred biography of an ULAN agent. Domain is schema:Person/Organization, range is gvp:Biography" ;
                          rdfs:comment "Non-preferred biography of an ULAN agent. Domain is schema:Person/Organization, range is gvp:Biography" ;
                          rdfs:isDefinedBy <http://vocab.getty.edu/ontology> ;
                          rdfs:label "biographyNonPreferred" .


###  http://vocab.getty.edu/ontology#biographyPreferred
gvp:biographyPreferred rdf:type owl:ObjectProperty ;
                       rdfs:subPropertyOf gvp:biography ;
                       rdfs:range gvp:Biography ;
                       dct:description "Preferred biography of an ULAN agent. Domain is schema:Person/Organization, range is gvp:Biography. The biography fields are also directly available in the Person/Organization" ;
                       rdfs:comment "Preferred biography of an ULAN agent. Domain is schema:Person/Organization, range is gvp:Biography. The biography fields are also directly available in the Person/Organization" ;
                       rdfs:isDefinedBy <http://vocab.getty.edu/ontology> ;
                       rdfs:label "biographyPreferred" .


###  http://vocab.getty.edu/ontology#broader
gvp:broader rdf:type owl:ObjectProperty ;
            rdfs:domain gvp:Subject ;
            rdfs:range gvp:Subject ;
            dct:description "Parents of a subject. Each broader is also Preferred|NonPreferred and Partitive|Instantial|Generic" ;
            rdfs:comment "Parents of a subject. Each broader is also Preferred|NonPreferred and Partitive|Instantial|Generic" ;
            rdfs:isDefinedBy <http://vocab.getty.edu/ontology> ;
            rdfs:label "broader" .


###  http://vocab.getty.edu/ontology#broaderExtended
gvp:broaderExtended rdf:type owl:ObjectProperty ;
                    rdfs:domain gvp:Subject ;
                    rdfs:range gvp:Subject ;
                    dct:description """Appropriate ancestors. Meaningful closure of gvp:broader for query expansion. Use this, not skos:broaderTransitive.
Example: Mt Athos has ancestor places (BTPE) World, Europe, Greece, Macedonia, Pangaíon Óros regional division;
and place types (BTIE) inhabited place; and orthodox religious center, Christian religious center, religious center""" ;
                    rdfs:comment "Appropriate ancestors. Meaningful closure of gvp:broader for query expansion. Use this, not skos:broaderTransitive" ;
                    rdfs:isDefinedBy <http://vocab.getty.edu/ontology> ;
                    rdfs:label "broaderExtended" ;
                    skos:example """Mt Athos has ancestor places (BTPE) World, Europe, Greece, Macedonia, Pangaíon Óros regional division;
and place types (BTIE) inhabited place; and orthodox religious center, Christian religious center, religious center""" .


###  http://vocab.getty.edu/ontology#broaderGeneric
gvp:broaderGeneric rdf:type owl:ObjectProperty ;
                   rdfs:subPropertyOf gvp:broader ,
                                      gvp:broaderGenericExtended ;
                   rdfs:domain gvp:Subject ;
                   rdfs:range gvp:Subject ;
                   dct:description """BTG (Genus/Species, \"is a\") relation. We also infer iso-thes:broaderGeneric, which goes only between Concepts.
Example: calcite (AAT) BTG mineral (AAT)""" ;
                   rdfs:comment "BTG (Genus/Species, \"is a\") relation. We also infer iso-thes:broaderGeneric, which goes only between Concepts" ;
                   rdfs:isDefinedBy <http://vocab.getty.edu/ontology> ;
                   rdfs:label "broaderGeneric" ;
                   skos:example "calcite (AAT) BTG mineral (AAT)" .


###  http://vocab.getty.edu/ontology#broaderGenericExtended
gvp:broaderGenericExtended rdf:type owl:ObjectProperty ;
                           rdfs:subPropertyOf gvp:broaderExtended ;
                           rdfs:domain gvp:Subject ;
                           rdfs:range gvp:Subject ;
                           owl:propertyChainAxiom ( gvp:broaderGenericExtended
                                                    gvp:broaderGeneric
                                                  ) ;
                           dct:description """Ancestors (Generic). Meaningful closure of gvp:broaderGeneric. Infers iso:broaderGeneric for pairs of directly related skos:Concepts.
Example: <anvils and anvil accessories> BTG <forging and metal-shaping tools> BTG <forging and metal-shaping equipment>,
so <anvils and anvil accessories> BTGE <forging and metal-shaping equipment>""" ;
                           rdfs:comment "Ancestors (Generic). Meaningful closure of gvp:broaderGeneric. Infers iso:broaderGeneric for pairs of directly related skos:Concepts" ;
                           rdfs:isDefinedBy <http://vocab.getty.edu/ontology> ;
                           rdfs:label "broaderGenericExtended" ;
                           skos:example """<anvils and anvil accessories> BTG <forging and metal-shaping tools> BTG <forging and metal-shaping equipment>,
so <anvils and anvil accessories> BTGE <forging and metal-shaping equipment>""" .


###  http://vocab.getty.edu/ontology#broaderInstantial
gvp:broaderInstantial rdf:type owl:ObjectProperty ;
                      rdfs:subPropertyOf gvp:broader ,
                                         gvp:broaderInstantialExtended ;
                      rdfs:domain gvp:Subject ;
                      rdfs:range gvp:Subject ;
                      dct:description """BTI (Kind/Instance, \"example of\") relation. We also infer iso-thes:broaderInstantial, which goes only between Concepts.
Example: Rembrandt van Rijn BTI Persons/Artists (ULAN)""" ;
                      rdfs:comment "BTI (Kind/Instance, \"example of\") relation. We also infer iso-thes:broaderInstantial, which goes only between Concepts" ;
                      rdfs:isDefinedBy <http://vocab.getty.edu/ontology> ;
                      rdfs:label "broaderInstantial" ;
                      skos:example "Rembrandt van Rijn BTI Persons/Artists (ULAN)" .


###  http://vocab.getty.edu/ontology#broaderInstantialExtended
gvp:broaderInstantialExtended rdf:type owl:ObjectProperty ;
                              rdfs:subPropertyOf gvp:broaderExtended ;
                              rdfs:domain gvp:Subject ;
                              rdfs:range gvp:Subject ;
                              owl:propertyChainAxiom ( gvp:broaderInstantialExtended
                                                       gvp:broaderGeneric
                                                     ) ;
                              dct:description "Ancestors (Instantial). Meaningful closure of gvp:broaderInstantial. Infers iso:broaderInstantial for pairs of directly related skos:Concepts." ;
                              rdfs:isDefinedBy <http://vocab.getty.edu/ontology> ;
                              rdfs:label "broaderInstantialExtended" ;
                              skos:example """Mt Athos (TGN) BTI orthodox religious center (AAT) BTG Christian religious center (AAT),
so Mt Athos (TGN) BTIE Christian religious center (AAT)""" .


###  http://vocab.getty.edu/ontology#broaderNonConcept
gvp:broaderNonConcept rdf:type owl:ObjectProperty ;
                      rdfs:domain skos:Concept ;
                      rdfs:range gvp:GuideTerm ;
                      dct:description "Chain of gvp:broader from Concept to GuideTerms, without intervening Concept" ;
                      rdfs:comment "Chain of gvp:broader from Concept to GuideTerms, without intervening Concept" ;
                      rdfs:isDefinedBy <http://vocab.getty.edu/ontology> ;
                      rdfs:label "broaderNonConcept" .


###  http://vocab.getty.edu/ontology#broaderNonPreferred
gvp:broaderNonPreferred rdf:type owl:ObjectProperty ;
                        rdfs:subPropertyOf gvp:broader ;
                        rdfs:domain gvp:Subject ;
                        rdfs:range gvp:Subject ;
                        dct:description """Auxiliary parents of a subject. Very often there are several non-preferred parents (poly-hierarchy). Can use to mark such parents with [N] in displays .
Example: Non-preferred: \"baking dishes\" BTG \"dishes (vessels)\" (AAT)""" ;
                        rdfs:comment "Auxiliary parents of a subject. Very often there are several non-preferred parents (poly-hierarchy). Can use to mark such parents with [N] in displays " ;
                        rdfs:isDefinedBy <http://vocab.getty.edu/ontology> ;
                        rdfs:label "broaderNonPreferred" ;
                        skos:example "Non-preferred: \"baking dishes\" BTG \"dishes (vessels)\" (AAT)" .


###  http://vocab.getty.edu/ontology#broaderPartitive
gvp:broaderPartitive rdf:type owl:ObjectProperty ;
                     rdfs:subPropertyOf gvp:broader ,
                                        gvp:broaderPartitiveExtended ;
                     rdfs:domain gvp:Subject ;
                     rdfs:range gvp:Subject ;
                     dct:description """BTP (Part/Whole, \"part of\") relation. We also infer iso-thes:broaderPartitive, which goes only between Concepts.
Example: Tuscany (TGN) BTP Italy (TGN)""" ;
                     rdfs:comment "BTP (Part/Whole, \"part of\") relation. We also infer iso-thes:broaderPartitive, which goes only between Concepts" ;
                     rdfs:isDefinedBy <http://vocab.getty.edu/ontology> ;
                     rdfs:label "broaderPartitive" ;
                     skos:example "Tuscany (TGN) BTP Italy (TGN)" .


###  http://vocab.getty.edu/ontology#broaderPartitiveExtended
gvp:broaderPartitiveExtended rdf:type owl:ObjectProperty ;
                             rdfs:subPropertyOf gvp:broaderExtended ;
                             rdfs:domain gvp:Subject ;
                             rdfs:range gvp:Subject ;
                             owl:propertyChainAxiom ( gvp:broaderGeneric
                                                      gvp:broaderPartitiveExtended
                                                    ) ,
                                                    ( gvp:broaderPartitiveExtended
                                                      gvp:broaderGeneric
                                                    ) ,
                                                    ( gvp:broaderPartitiveExtended
                                                      gvp:broaderPartitive
                                                    ) ;
                             dct:description """Ancestors (Partitive). Meaningful closure of gvp:broaderPartitive. Infers iso:broaderPartitive for pairs of directly related skos:Concepts.
Example: anvil components BTP <anvils and anvil accessories> BTG <forging and metal-shaping tools>,
so anvil components BTPE <forging and metal-shaping tools>""" ;
                             rdfs:comment "Ancestors (Partitive). Meaningful closure of gvp:broaderPartitive. Infers iso:broaderPartitive for pairs of directly related skos:Concepts" ;
                             rdfs:isDefinedBy <http://vocab.getty.edu/ontology> ;
                             rdfs:label "broaderPartitiveExtended" ;
                             skos:example """anvil components BTP <anvils and anvil accessories> BTG <forging and metal-shaping tools>,
so anvil components BTPE <forging and metal-shaping tools>""" .


###  http://vocab.getty.edu/ontology#broaderPreferred
gvp:broaderPreferred rdf:type owl:ObjectProperty ;
                     rdfs:subPropertyOf gvp:broader ,
                                        gvp:broaderPreferredExtended ;
                     rdfs:domain gvp:Subject ;
                     rdfs:range gvp:Subject ;
                     dct:description """Main parent of a subject. Needed to display the hierarchy.
Example: Preferred: \"baking dishes\" (AAT) BTG \"bakeware\" (AAT); Sofia (TGN) BTP Bulgaria (TGN)""" ;
                     rdfs:comment "Main parent of a subject. Needed to display the hierarchy" ;
                     rdfs:isDefinedBy <http://vocab.getty.edu/ontology> ;
                     rdfs:label "broaderPreferred" ;
                     skos:example "Preferred: \"baking dishes\" (AAT) BTG \"bakeware\" (AAT); Sofia (TGN) BTP Bulgaria (TGN)" .


###  http://vocab.getty.edu/ontology#broaderPreferredExtended
gvp:broaderPreferredExtended rdf:type owl:ObjectProperty ;
                             rdfs:domain gvp:Subject ;
                             rdfs:range gvp:Subject ;
                             dct:description """Preferred Ancestors. Meaningful closure of gvp:broaderPreferred. Needed to display the hierarchy.
Example: Mt Athos has preferred ancestor places (BTPE) World, Europe, Greece, Macedonia, Pangaíon Óros regional division;
and prefererd place type (BTIE) inhabited place""" ;
                             rdfs:comment "Preferred Ancestors. Meaningful closure of gvp:broaderPreferred. Needed to display the hierarchy" ;
                             rdfs:isDefinedBy <http://vocab.getty.edu/ontology> ;
                             rdfs:label "broaderPreferredExtended" ;
                             skos:example """Mt Athos has preferred ancestor places (BTPE) World, Europe, Greece, Macedonia, Pangaíon Óros regional division;
and prefererd place type (BTIE) inhabited place""" .


###  http://vocab.getty.edu/ontology#contributorAlternatePreferred
gvp:contributorAlternatePreferred rdf:type owl:ObjectProperty ;
                                  rdfs:domain skosxl:Label ;
                                  rdfs:range foaf:Agent .


###  http://vocab.getty.edu/ontology#contributorNonPreferred
gvp:contributorNonPreferred rdf:type owl:ObjectProperty ;
                            rdfs:domain skosxl:Label ;
                            rdfs:range foaf:Agent .


###  http://vocab.getty.edu/ontology#contributorPreferred
gvp:contributorPreferred rdf:type owl:ObjectProperty ;
                         rdfs:domain skosxl:Label ;
                         rdfs:range foaf:Agent .


###  http://vocab.getty.edu/ontology#eventNonPreferred
gvp:eventNonPreferred rdf:type owl:ObjectProperty ;
                      rdfs:subPropertyOf bio:event ;
                      rdfs:range bio:Event ;
                      dct:description "Non-preferred life event of an ULAN agent. Domain is schema:Person/Organization, range is bio:Event" ;
                      rdfs:comment "Non-preferred life event of an ULAN agent. Domain is schema:Person/Organization, range is bio:Event" ;
                      rdfs:isDefinedBy <http://vocab.getty.edu/ontology> ;
                      rdfs:label "eventNonPreferred" .


###  http://vocab.getty.edu/ontology#eventPreferred
gvp:eventPreferred rdf:type owl:ObjectProperty ;
                   rdfs:subPropertyOf bio:event ;
                   rdfs:range bio:Event ;
                   dct:description "Preferred life event of an ULAN agent. Domain is schema:Person/Organization, range is bio:Event" ;
                   rdfs:comment "Preferred life event of an ULAN agent. Domain is schema:Person/Organization, range is bio:Event" ;
                   rdfs:isDefinedBy <http://vocab.getty.edu/ontology> ;
                   rdfs:label "eventPreferred" .


###  http://vocab.getty.edu/ontology#historicFlag
gvp:historicFlag rdf:type owl:ObjectProperty ;
                 rdfs:range skos:Concept ;
                 dct:description "Historic Flag" ;
                 rdfs:isDefinedBy <http://vocab.getty.edu/ontology> ;
                 rdfs:label "historicFlag" .


###  http://vocab.getty.edu/ontology#nationalityNonPreferred
gvp:nationalityNonPreferred rdf:type owl:ObjectProperty ;
                            rdfs:subPropertyOf schema:nationality ;
                            rdfs:range gvp:Subject ;
                            dct:description "Non-preferred nationality/culture/race/ethnicity/religion/sexual orientation of an ULAN agent. Domain is schema:Person/Organization, range is AAT concept" ;
                            rdfs:comment "Non-preferred nationality/culture/race/ethnicity/religion/sexual orientation of an ULAN agent. Domain is schema:Person/Organization, range is AAT concept" ;
                            rdfs:isDefinedBy <http://vocab.getty.edu/ontology> ;
                            rdfs:label "nationalityNonPreferred" .


###  http://vocab.getty.edu/ontology#nationalityPreferred
gvp:nationalityPreferred rdf:type owl:ObjectProperty ;
                         rdfs:subPropertyOf schema:nationality ;
                         rdfs:range gvp:Subject ;
                         dct:description "Preferred nationality/culture/race/ethnicity/religion/sexual orientation of an ULAN agent. Domain is schema:Person/Organization, range is AAT concept" ;
                         rdfs:comment "Preferred nationality/culture/race/ethnicity/religion/sexual orientation of an ULAN agent. Domain is schema:Person/Organization, range is AAT concept" ;
                         rdfs:isDefinedBy <http://vocab.getty.edu/ontology> ;
                         rdfs:label "nationalityPreferred" .


###  http://vocab.getty.edu/ontology#parentString
gvp:parentString rdf:type owl:ObjectProperty ;
                 rdfs:domain gvp:Subject ;
                 rdfs:range rdf:Literal .


###  http://vocab.getty.edu/ontology#parentStringAbbrev
gvp:parentStringAbbrev rdf:type owl:ObjectProperty ;
                       rdfs:domain gvp:Subject ;
                       rdfs:range rdf:Literal .


###  http://vocab.getty.edu/ontology#placeType
gvp:placeType rdf:type owl:ObjectProperty ;
              rdfs:domain gvp:Subject ;
              rdfs:range gvp:Subject ;
              dct:description """Type for a TGN place. Domain is TGN concept (AdminPlaceConcept or PhysPlaceConcept), range is AAT Concept.
Example: Machupicchu, Peru has preferred type \"deserted settlement\" (current) and non-preferred type \"Inca center\" (historic)""" ;
              rdfs:comment "Type for a TGN place. Domain is TGN concept (AdminPlaceConcept or PhysPlaceConcept), range is AAT Concept" ;
              rdfs:isDefinedBy <http://vocab.getty.edu/ontology> ;
              rdfs:label "placeType" ;
              skos:example "Machupicchu, Peru has preferred type \"deserted settlement\" (current) and non-preferred type \"Inca center\" (historic)" .


###  http://vocab.getty.edu/ontology#placeTypeNonPreferred
gvp:placeTypeNonPreferred rdf:type owl:ObjectProperty ;
                          rdfs:subPropertyOf gvp:placeType ;
                          rdfs:domain gvp:Subject ;
                          rdfs:range gvp:Subject ;
                          dct:description """A secondary type for a TGN Place. Domain is TGN concept, range is AAT concept.
Example: A non-preferred type of Machupicchu, Peru is \"Inca center\" (historical)""" ;
                          rdfs:comment "A secondary type for a TGN Place. Domain is TGN concept, range is AAT concept" ;
                          rdfs:isDefinedBy <http://vocab.getty.edu/ontology> ;
                          rdfs:label "placeTypeNonPreferred" ;
                          skos:example "A non-preferred type of Machupicchu, Peru is \"Inca center\" (historical)" .


###  http://vocab.getty.edu/ontology#placeTypePreferred
gvp:placeTypePreferred rdf:type owl:ObjectProperty ;
                       rdfs:subPropertyOf gvp:placeType ;
                       rdfs:domain gvp:Subject ;
                       rdfs:range gvp:Subject ;
                       dct:description """The primary type of a TGN Place. Domain is TGN concept, range is AAT concept.
Example: The preferred place type of Machupicchu, Peru is \"deserted settlement\" (current)""" ;
                       rdfs:comment "The primary type of a TGN Place. Domain is TGN concept, range is AAT concept" ;
                       rdfs:isDefinedBy <http://vocab.getty.edu/ontology> ;
                       rdfs:label "placeTypePreferred" ;
                       skos:example "The preferred place type of Machupicchu, Peru is \"deserted settlement\" (current)" .


###  http://vocab.getty.edu/ontology#prefLabelGVP
gvp:prefLabelGVP rdf:type owl:ObjectProperty ;
                 rdfs:domain gvp:Subject ;
                 rdfs:range skosxl:Label ;
                 dct:description "Term preferred by the Getty Vocabulary Program. The language is usually English. Applicable to AAT, ULAN, TGN. Used with skosxl:prefLabel" ;
                 rdfs:comment "Term preferred by the Getty Vocabulary Program. The language is usually English. Applicable to AAT, ULAN, TGN. Used with skosxl:prefLabel" ;
                 rdfs:isDefinedBy <http://vocab.getty.edu/ontology> ;
                 rdfs:label "prefLabelGVP" .


###  http://vocab.getty.edu/ontology#prefLabelLoC
gvp:prefLabelLoC rdf:type owl:ObjectProperty ;
                 rdfs:domain gvp:Subject ;
                 rdfs:range skosxl:Label ;
                 dct:description "Term preferred by Library of Congress, thus used for cataloging according to AACR2. Applicable to AAT and ULAN. Used with skosxl:prefLabel" ;
                 rdfs:comment "Term preferred by Library of Congress, thus used for cataloging according to AACR2. Applicable to AAT and ULAN. Used with skosxl:prefLabel" ;
                 rdfs:isDefinedBy <http://vocab.getty.edu/ontology> ;
                 rdfs:label "prefLabelLoC" .


###  http://vocab.getty.edu/ontology#qualifier
gvp:qualifier rdf:type owl:ObjectProperty ;
              rdfs:domain skosxl:Label ;
              rdfs:range rdf:Literal .


###  http://vocab.getty.edu/ontology#sourceAlternatePreferred
gvp:sourceAlternatePreferred rdf:type owl:ObjectProperty ;
                             rdfs:subPropertyOf dct:source ;
                             rdfs:domain skosxl:Label ;
                             rdfs:range bibo:Document ;
                             dct:description """Source for which the term is Alternate Preferred. Range is bibo:Document or bibo:DocumentPart.
Example: \"Kayseri\" is alternate preferred in Webster's New Geographical Dictionary (1988)""" ;
                             rdfs:comment "Source for which the term is Alternate Preferred. Range is bibo:Document or bibo:DocumentPart" ;
                             rdfs:isDefinedBy <http://vocab.getty.edu/ontology> ;
                             rdfs:label "sourceAlternatePreferred" ;
                             skos:example "\"Kayseri\" is alternate preferred in Webster's New Geographical Dictionary (1988)" .


###  http://vocab.getty.edu/ontology#sourceNonPreferred
gvp:sourceNonPreferred rdf:type owl:ObjectProperty ;
                       rdfs:subPropertyOf dct:source ;
                       rdfs:domain skosxl:Label ;
                       rdfs:range bibo:Document ;
                       dct:description """Source for which the term is Non-preferred. Range is bibo:Document or bibo:DocumentPart.
Example: \"Panderma\" is non-preferred in Webster's New Geographical Dictionary (1988)""" ;
                       rdfs:comment "Source for which the term is Non-preferred. Range is bibo:Document or bibo:DocumentPart" ;
                       rdfs:isDefinedBy <http://vocab.getty.edu/ontology> ;
                       rdfs:label "sourceNonPreferred" ;
                       skos:example "\"Panderma\" is non-preferred in Webster's New Geographical Dictionary (1988)" .


###  http://vocab.getty.edu/ontology#sourcePreferred
gvp:sourcePreferred rdf:type owl:ObjectProperty ;
                    rdfs:subPropertyOf dct:source ;
                    rdfs:domain skosxl:Label ;
                    rdfs:range bibo:Document ;
                    dct:description """Source for which the term is Preferred. Range is bibo:Document or bibo:DocumentPart.
Example: \"Isfahan\" is preferred in Webster's New Geographical Dictionary (1988)""" ;
                    rdfs:comment "Source for which the term is Preferred. Range is bibo:Document or bibo:DocumentPart" ;
                    rdfs:isDefinedBy <http://vocab.getty.edu/ontology> ;
                    rdfs:label "sourcePreferred" ;
                    skos:example "\"Isfahan\" is preferred in Webster's New Geographical Dictionary (1988)" .


###  http://vocab.getty.edu/ontology#term
gvp:term rdf:type owl:ObjectProperty ;
         rdfs:domain skosxl:Label ;
         rdfs:range rdf:Literal .


###  http://vocab.getty.edu/ontology#termDisplay
gvp:termDisplay rdf:type owl:ObjectProperty ;
                rdfs:domain skosxl:Label ;
                rdfs:range skos:Concept ;
                dct:description "Term Display" ;
                rdfs:isDefinedBy <http://vocab.getty.edu/ontology> ;
                rdfs:label "termDisplay" .


###  http://vocab.getty.edu/ontology#termFlag
gvp:termFlag rdf:type owl:ObjectProperty ;
             rdfs:domain skosxl:Label ;
             rdfs:range skos:Concept ;
             dct:description "Term Flag" ;
             rdfs:isDefinedBy <http://vocab.getty.edu/ontology> ;
             rdfs:label "termFlag" .


###  http://vocab.getty.edu/ontology#termKind
gvp:termKind rdf:type owl:ObjectProperty ;
             rdfs:domain skosxl:Label ;
             rdfs:range skos:Concept ;
             dct:description "Term Kind" ;
             rdfs:isDefinedBy <http://vocab.getty.edu/ontology> ;
             rdfs:label "termKind" .


###  http://vocab.getty.edu/ontology#termPOS
gvp:termPOS rdf:type owl:ObjectProperty ;
            rdfs:domain skosxl:Label ;
            rdfs:range skos:Concept ;
            dct:description "Part of Speech" ;
            rdfs:isDefinedBy <http://vocab.getty.edu/ontology> ;
            rdfs:label "termPOS" .


###  http://vocab.getty.edu/ontology#termType
gvp:termType rdf:type owl:ObjectProperty ;
             rdfs:domain skosxl:Label ;
             rdfs:range skos:Concept ;
             dct:description "Term Type" ;
             rdfs:isDefinedBy <http://vocab.getty.edu/ontology> ;
             rdfs:label "termType" .


###  http://vocab.getty.edu/ontology#tgn3000_related_to
gvp:tgn3000_related_to rdf:type owl:ObjectProperty ;
                       rdfs:subPropertyOf skos:related ;
                       rdf:type owl:SymmetricProperty ;
                       rdfs:domain skos:Concept ;
                       rdfs:range skos:Concept ;
                       dc:identifier "3000" ;
                       dc:title "related to - any" ;
                       dct:description """any - related to - any.
Example: Fountains Abbey is related to Studley Royal; Austria-Hungary is related to Magyarorszag""" ;
                       rdfs:isDefinedBy <http://vocab.getty.edu/ontology> ,
                                        tgn: ;
                       skos:example "Austria-Hungary is related to Magyarorszag" ,
                                    "Fountains Abbey is related to Studley Royal" ;
                       skos:prefLabel "tgn3000_related_to" .


###  http://vocab.getty.edu/ontology#tgn3001_distinguished_from
gvp:tgn3001_distinguished_from rdf:type owl:ObjectProperty ;
                               rdfs:subPropertyOf skos:related ;
                               rdf:type owl:SymmetricProperty ;
                               rdfs:domain skos:Concept ;
                               rdfs:range skos:Concept ;
                               dc:identifier "3001" ;
                               dc:title "distinguished from - any" ;
                               dct:description """any - distinguished from - any.
Example: The Ancient Mesopotamian Kingdom 'Assyria' is distinguished from the Roman Province of the same name""" ;
                               rdfs:isDefinedBy <http://vocab.getty.edu/ontology> ,
                                                tgn: ;
                               skos:example "The Ancient Mesopotamian Kingdom 'Assyria' is distinguished from the Roman Province of the same name" ;
                               skos:prefLabel "tgn3001_distinguished_from" .


###  http://vocab.getty.edu/ontology#tgn3005_possibly_identified_as
gvp:tgn3005_possibly_identified_as rdf:type owl:ObjectProperty ;
                                   rdfs:subPropertyOf skos:related ;
                                   rdf:type owl:SymmetricProperty ;
                                   rdfs:domain skos:Concept ;
                                   rdfs:range skos:Concept ;
                                   dc:identifier "3005" ;
                                   dc:title "possibly identified as - place" ;
                                   dct:description """place - possibly identified as - place.
Example: The lost settlement of Sharuhen is possibly identified as Tel el-Far'ah (As Suwayda', Syria) (deserted settlement)""" ;
                                   rdfs:isDefinedBy <http://vocab.getty.edu/ontology> ,
                                                    tgn: ;
                                   skos:example "The lost settlement of Sharuhen is possibly identified as Tel el-Far'ah (As Suwayda', Syria) (deserted settlement)" ;
                                   skos:prefLabel "tgn3005_possibly_identified_as" .


###  http://vocab.getty.edu/ontology#tgn3006_formerly_identified_as
gvp:tgn3006_formerly_identified_as rdf:type owl:ObjectProperty ;
                                   rdfs:subPropertyOf skos:related ;
                                   rdf:type owl:SymmetricProperty ;
                                   rdfs:domain skos:Concept ;
                                   rdfs:range skos:Concept ;
                                   dc:identifier "3006" ;
                                   dc:title "formerly identified as - place" ;
                                   dct:description """place - formerly identified as - place; New.
Example: The deserted settlement of Machupicchu was formerly identified as Tampu Tocco""" ;
                                   rdfs:isDefinedBy <http://vocab.getty.edu/ontology> ,
                                                    tgn: ;
                                   skos:example "The deserted settlement of Machupicchu was formerly identified as Tampu Tocco" ;
                                   skos:prefLabel "tgn3006_formerly_identified_as" ;
                                   skos:scopeNote "New" .


###  http://vocab.getty.edu/ontology#tgn3101_near-adjacent_to
gvp:tgn3101_near-adjacent_to rdf:type owl:ObjectProperty ;
                             rdfs:subPropertyOf skos:related ;
                             rdf:type owl:SymmetricProperty ;
                             rdfs:domain skos:Concept ;
                             rdfs:range skos:Concept ;
                             dc:identifier "3101" ;
                             dc:title "near/adjacent to - any" ;
                             dct:description """any - near/adjacent to - any.
Example: Saint Paul (Minnesota, USA), is linked to its 'Twin City' Minneapolis (Hennepin county, Minnesota, USA)""" ;
                             rdfs:isDefinedBy <http://vocab.getty.edu/ontology> ,
                                              tgn: ;
                             skos:example "Saint Paul (Minnesota, USA), is linked to its 'Twin City' Minneapolis (Hennepin county, Minnesota, USA)" ;
                             skos:prefLabel "tgn3101_near-adjacent_to" .


###  http://vocab.getty.edu/ontology#tgn3102_coextensive_with
gvp:tgn3102_coextensive_with rdf:type owl:ObjectProperty ;
                             rdfs:subPropertyOf skos:related ;
                             rdf:type owl:SymmetricProperty ;
                             rdfs:domain skos:Concept ;
                             rdfs:range skos:Concept ;
                             dc:identifier "3102" ;
                             dc:title "coextensive with - place" ;
                             dct:description """place - coextensive with - place.
Example: Kings county (New York, USA) is coextensive with Brooklyn (New York, USA)""" ;
                             rdfs:isDefinedBy <http://vocab.getty.edu/ontology> ,
                                              tgn: ;
                             skos:example "Kings county (New York, USA) is coextensive with Brooklyn (New York, USA)" ;
                             skos:prefLabel "tgn3102_coextensive_with" .


###  http://vocab.getty.edu/ontology#tgn3103_located_on
gvp:tgn3103_located_on rdf:type owl:ObjectProperty ;
                       rdfs:subPropertyOf skos:related ;
                       owl:inverseOf gvp:tgn3104_is_location_of ;
                       rdfs:domain skos:Concept ;
                       rdfs:range skos:Concept ;
                       dc:identifier "3103" ;
                       dc:title "located on - place" ;
                       dct:description """place - located on - place.
Example: tgn:7018835 Palmyra is located on tgn:7031416 Silk Road""" ;
                       rdfs:isDefinedBy <http://vocab.getty.edu/ontology> ,
                                        tgn: ;
                       skos:example "tgn:7018835 Palmyra is located on tgn:7031416 Silk Road" ;
                       skos:prefLabel "tgn3103_located_on" .


###  http://vocab.getty.edu/ontology#tgn3104_is_location_of
gvp:tgn3104_is_location_of rdf:type owl:ObjectProperty ;
                           rdfs:subPropertyOf skos:related ;
                           rdfs:domain skos:Concept ;
                           rdfs:range skos:Concept ;
                           dc:identifier "3104" ;
                           dc:title "is location of - place" ;
                           dct:description """place - is location of - place.
Example: tgn:7031416 Silk Road is location of tgn:7018835 Palmyra""" ;
                           rdfs:isDefinedBy <http://vocab.getty.edu/ontology> ,
                                            tgn: ;
                           skos:example "tgn:7031416 Silk Road is location of tgn:7018835 Palmyra" ;
                           skos:prefLabel "tgn3104_is_location_of" .


###  http://vocab.getty.edu/ontology#tgn3110_meaning-usage_overlaps_with
gvp:tgn3110_meaning-usage_overlaps_with rdf:type owl:ObjectProperty ;
                                        rdfs:subPropertyOf skos:related ;
                                        rdf:type owl:SymmetricProperty ;
                                        rdfs:domain skos:Concept ;
                                        rdfs:range skos:Concept ;
                                        dc:identifier "3110" ;
                                        dc:title "meaning/usage overlaps with - any" ;
                                        dct:description """any - meaning/usage overlaps with - any.
Example: Judaea (Israel) (historical region) meaning/usage overlaps with Holy Land (Asia) (historical region)""" ;
                                        rdfs:isDefinedBy <http://vocab.getty.edu/ontology> ,
                                                         tgn: ;
                                        skos:example "Judaea (Israel) (historical region) meaning/usage overlaps with Holy Land (Asia) (historical region)" ;
                                        skos:prefLabel "tgn3110_meaning-usage_overlaps_with" .


###  http://vocab.getty.edu/ontology#tgn3201_capital_of
gvp:tgn3201_capital_of rdf:type owl:ObjectProperty ;
                       rdfs:subPropertyOf skos:related ;
                       owl:inverseOf gvp:tgn3202_capital_is ;
                       rdfs:domain skos:Concept ;
                       rdfs:range skos:Concept ;
                       dc:identifier "3201" ;
                       dc:title "capital of - nation" ;
                       dct:description """city - capital of - nation.
Example: Thecapital of Maxima Caesariensis from 296 to 800 CE was London""" ;
                       rdfs:isDefinedBy <http://vocab.getty.edu/ontology> ,
                                        tgn: ;
                       skos:example "Thecapital of Maxima Caesariensis from 296 to 800 CE was London" ;
                       skos:prefLabel "tgn3201_capital_of" .


###  http://vocab.getty.edu/ontology#tgn3202_capital_is
gvp:tgn3202_capital_is rdf:type owl:ObjectProperty ;
                       rdfs:subPropertyOf skos:related ;
                       rdfs:domain skos:Concept ;
                       rdfs:range skos:Concept ;
                       dc:identifier "3202" ;
                       dc:title "capital is - city" ;
                       dct:description """nation - capital is - city.
Example: London was the capital of Maxima Caesariensis from 296 to 800 CE""" ;
                       rdfs:isDefinedBy <http://vocab.getty.edu/ontology> ,
                                        tgn: ;
                       skos:example "London was the capital of Maxima Caesariensis from 296 to 800 CE" ;
                       skos:prefLabel "tgn3202_capital_is" .


###  http://vocab.getty.edu/ontology#tgn3301_ally_of
gvp:tgn3301_ally_of rdf:type owl:ObjectProperty ;
                    rdfs:subPropertyOf skos:related ;
                    rdf:type owl:SymmetricProperty ;
                    rdfs:domain skos:Concept ;
                    rdfs:range skos:Concept ;
                    dc:identifier "3301" ;
                    dc:title "ally of - nation" ;
                    dct:description """nation - ally of - nation.
Example: Siena, Arezzo, Pisa, and Pistoia were Ghibeline allies during the 13th and 14th centuries.""" ;
                    rdfs:isDefinedBy <http://vocab.getty.edu/ontology> ,
                                     tgn: ;
                    skos:example "Siena, Arezzo, Pisa, and Pistoia were Ghibeline allies during the 13th and 14th centuries." ;
                    skos:prefLabel "tgn3301_ally_of" .


###  http://vocab.getty.edu/ontology#tgn3317_member_of
gvp:tgn3317_member_of rdf:type owl:ObjectProperty ;
                      rdfs:subPropertyOf skos:related ;
                      owl:inverseOf gvp:tgn3318_member_is ;
                      rdfs:domain skos:Concept ;
                      rdfs:range skos:Concept ;
                      dc:identifier "3317" ;
                      dc:title "member of - union" ;
                      dct:description """nation - member of - union.
Example: Austria is a member of the European Union since 1915; Belgium is a member of the European Union since 1958""" ;
                      rdfs:isDefinedBy <http://vocab.getty.edu/ontology> ,
                                       tgn: ;
                      skos:example "Austria is a member of the European Union since 1915" ,
                                   "Belgium is a member of the European Union since 1958" ;
                      skos:prefLabel "tgn3317_member_of" .


###  http://vocab.getty.edu/ontology#tgn3318_member_is
gvp:tgn3318_member_is rdf:type owl:ObjectProperty ;
                      rdfs:subPropertyOf skos:related ;
                      rdfs:domain skos:Concept ;
                      rdfs:range skos:Concept ;
                      dc:identifier "3318" ;
                      dc:title "member is - nation" ;
                      dct:description """union - member is - nation.
Example: Austria is a member of the European Union since 1915; Belgium is a member of the European Union since 1958""" ;
                      rdfs:isDefinedBy <http://vocab.getty.edu/ontology> ,
                                       tgn: ;
                      skos:example "Austria is a member of the European Union since 1915" ,
                                   "Belgium is a member of the European Union since 1958" ;
                      skos:prefLabel "tgn3318_member_is" .


###  http://vocab.getty.edu/ontology#tgn3401_moved_from
gvp:tgn3401_moved_from rdf:type owl:ObjectProperty ;
                       rdfs:subPropertyOf skos:related ;
                       owl:inverseOf gvp:tgn3402_moved_to ;
                       rdfs:domain skos:Concept ;
                       rdfs:range skos:Concept ;
                       dc:identifier "3401" ;
                       dc:title "moved from - place" ;
                       dct:description """place - moved from - place; Note: places that were physically moved from one location to another, often due to the threat or occurrence of natural disaster..
Example: Troupville, Georgia, USA was moved to Valdosta (Lowndes county, Georgia, USA)""" ;
                       rdfs:isDefinedBy <http://vocab.getty.edu/ontology> ,
                                        tgn: ;
                       skos:example "Troupville, Georgia, USA was moved to Valdosta (Lowndes county, Georgia, USA)" ;
                       skos:prefLabel "tgn3401_moved_from" ;
                       skos:scopeNote "Note: places that were physically moved from one location to another, often due to the threat or occurrence of natural disaster." .


###  http://vocab.getty.edu/ontology#tgn3402_moved_to
gvp:tgn3402_moved_to rdf:type owl:ObjectProperty ;
                     rdfs:subPropertyOf skos:related ;
                     rdfs:domain skos:Concept ;
                     rdfs:range skos:Concept ;
                     dc:identifier "3402" ;
                     dc:title "moved to - place" ;
                     dct:description """place - moved to - place.
Example: Valdosta (Lowndes county, Georgia, USA) moved from Troupville (Georgia, USA)""" ;
                     rdfs:isDefinedBy <http://vocab.getty.edu/ontology> ,
                                      tgn: ;
                     skos:example "Valdosta (Lowndes county, Georgia, USA) moved from Troupville (Georgia, USA)" ;
                     skos:prefLabel "tgn3402_moved_to" .


###  http://vocab.getty.edu/ontology#tgn3411_successor_of
gvp:tgn3411_successor_of rdf:type owl:ObjectProperty ;
                         rdfs:subPropertyOf skos:related ;
                         owl:inverseOf gvp:tgn3412_predecessor_of ;
                         rdfs:domain skos:Concept ;
                         rdfs:range skos:Concept ;
                         dc:identifier "3411" ;
                         dc:title "successor of - nation" ;
                         dct:description """nation - successor of - nation.
Example: Iran (nation) is the successor of Persia""" ;
                         rdfs:isDefinedBy <http://vocab.getty.edu/ontology> ,
                                          tgn: ;
                         skos:example "Iran (nation) is the successor of Persia" ;
                         skos:prefLabel "tgn3411_successor_of" .


###  http://vocab.getty.edu/ontology#tgn3412_predecessor_of
gvp:tgn3412_predecessor_of rdf:type owl:ObjectProperty ;
                           rdfs:subPropertyOf skos:related ;
                           rdfs:domain skos:Concept ;
                           rdfs:range skos:Concept ;
                           dc:identifier "3412" ;
                           dc:title "predecessor of - nation" ;
                           dct:description """nation - predecessor of - nation.
Example: Persia is the predecessor of Iran (nation)""" ;
                           rdfs:isDefinedBy <http://vocab.getty.edu/ontology> ,
                                            tgn: ;
                           skos:example "Persia is the predecessor of Iran (nation)" ;
                           skos:prefLabel "tgn3412_predecessor_of" .


###  http://vocab.getty.edu/ontology#tgn3510_historical_connection
gvp:tgn3510_historical_connection rdf:type owl:ObjectProperty ;
                                  rdfs:subPropertyOf skos:related ;
                                  rdf:type owl:SymmetricProperty ;
                                  rdfs:domain skos:Concept ;
                                  rdfs:range skos:Concept ;
                                  dc:identifier "3510" ;
                                  dc:title "historical connection - any" ;
                                  dct:description """any - historical connection - any.
Example: Guyenne, France (historical region) has a historical connection to Gascogne (France) (historical region)""" ;
                                  rdfs:isDefinedBy <http://vocab.getty.edu/ontology> ,
                                                   tgn: ;
                                  skos:example "Guyenne, France (historical region) has a historical connection to Gascogne (France) (historical region)" ;
                                  skos:prefLabel "tgn3510_historical_connection" .


###  http://vocab.getty.edu/ontology#tgn3611_administrative_dependent_of
gvp:tgn3611_administrative_dependent_of rdf:type owl:ObjectProperty ;
                                        rdfs:subPropertyOf skos:related ;
                                        owl:inverseOf gvp:tgn3612_administrative_entity_for ;
                                        rdfs:domain skos:Concept ;
                                        rdfs:range skos:Concept ;
                                        dc:identifier "3611" ;
                                        dc:title "administrative dependent of - place" ;
                                        dct:description """place - administrative dependent of - place; New.
Example: Luni (La Spezia province, Liguria, Italy) is the admisistrative dependent of Ortonovo (Massa-Carrara province, Tuscany, Italy)""" ;
                                        rdfs:isDefinedBy <http://vocab.getty.edu/ontology> ,
                                                         tgn: ;
                                        skos:example "Luni (La Spezia province, Liguria, Italy) is the admisistrative dependent of Ortonovo (Massa-Carrara province, Tuscany, Italy)" ;
                                        skos:prefLabel "tgn3611_administrative_dependent_of" ;
                                        skos:scopeNote "New" .


###  http://vocab.getty.edu/ontology#tgn3612_administrative_entity_for
gvp:tgn3612_administrative_entity_for rdf:type owl:ObjectProperty ;
                                      rdfs:subPropertyOf skos:related ;
                                      rdfs:domain skos:Concept ;
                                      rdfs:range skos:Concept ;
                                      dc:identifier "3612" ;
                                      dc:title "administrative entity for - place" ;
                                      dct:description """place - administrative entity for - place.
Example: Ortonovo (Massa-Carra province, Tuscany, Italy) is the administrative entity for Luni (La Spezia province, Liguria, Italy)""" ;
                                      rdfs:isDefinedBy <http://vocab.getty.edu/ontology> ,
                                                       tgn: ;
                                      skos:example "Ortonovo (Massa-Carra province, Tuscany, Italy) is the administrative entity for Luni (La Spezia province, Liguria, Italy)" ;
                                      skos:prefLabel "tgn3612_administrative_entity_for" .


###  http://vocab.getty.edu/ontology#ulan1000_related_to
gvp:ulan1000_related_to rdf:type owl:ObjectProperty ;
                        rdfs:subPropertyOf skos:related ;
                        rdf:type owl:SymmetricProperty ;
                        rdfs:domain skos:Concept ;
                        rdfs:range skos:Concept ;
                        dc:identifier "1000" ;
                        dc:title "related to - any" ;
                        dct:description """any - related to - any.
Example: Frank Lloyd Wright is related to Francis Conroy Sullivan; Herman Miller, Inc. is related to Irving Harper; National Endowment for the Humanities is related to Connecticut Humanities Council""" ;
                        rdfs:isDefinedBy <http://vocab.getty.edu/ontology> ,
                                         ulan: ;
                        skos:example "Frank Lloyd Wright is related to Francis Conroy Sullivan" ,
                                     "Herman Miller, Inc. is related to Irving Harper" ,
                                     "National Endowment for the Humanities is related to Connecticut Humanities Council" ;
                        skos:prefLabel "ulan1000_related_to" .


###  http://vocab.getty.edu/ontology#ulan1003_associated_with
gvp:ulan1003_associated_with rdf:type owl:ObjectProperty ;
                             rdfs:subPropertyOf skos:related ;
                             rdf:type owl:SymmetricProperty ;
                             rdfs:domain skos:Concept ;
                             rdfs:range skos:Concept ;
                             dc:identifier "1003" ;
                             dc:title "associated with - any" ;
                             dct:description """any - associated with - any.
Example: Richard Meier is associated with Renny B.Saltzman; United Nations is associated with World Bank""" ;
                             rdfs:isDefinedBy <http://vocab.getty.edu/ontology> ,
                                              ulan: ;
                             skos:example "Richard Meier is associated with Renny B.Saltzman" ,
                                          "United Nations is associated with World Bank" ;
                             skos:prefLabel "ulan1003_associated_with" .


###  http://vocab.getty.edu/ontology#ulan1005_possibly_identified_with
gvp:ulan1005_possibly_identified_with rdf:type owl:ObjectProperty ;
                                      rdfs:subPropertyOf skos:related ;
                                      rdf:type owl:SymmetricProperty ;
                                      rdfs:domain skos:Concept ;
                                      rdfs:range skos:Concept ;
                                      dc:identifier "1005" ;
                                      dc:title "possibly identified with - any" ;
                                      dct:description """any - possibly identified with - any.
Example: Master of the Saint John Altarpiece is possibly identified with Hughe Jacobsz; Bauart is possibly identified with Gruppe BAUart""" ;
                                      rdfs:isDefinedBy <http://vocab.getty.edu/ontology> ,
                                                       ulan: ;
                                      skos:example "Bauart is possibly identified with Gruppe BAUart" ,
                                                   "Master of the Saint John Altarpiece is possibly identified with Hughe Jacobsz" ;
                                      skos:prefLabel "ulan1005_possibly_identified_with" .


###  http://vocab.getty.edu/ontology#ulan1006_formerly_identified_with
gvp:ulan1006_formerly_identified_with rdf:type owl:ObjectProperty ;
                                      rdfs:subPropertyOf skos:related ;
                                      rdf:type owl:SymmetricProperty ;
                                      rdfs:domain skos:Concept ;
                                      rdfs:range skos:Concept ;
                                      dc:identifier "1006" ;
                                      dc:title "formerly identified with - any" ;
                                      dct:description """any - formerly identified with - any.
Example: Tommaso is formerly identified with Tommaso di Stefano Lunetti; GreenWorks is formerly identified with Mike Faha & Associates""" ;
                                      rdfs:isDefinedBy <http://vocab.getty.edu/ontology> ,
                                                       ulan: ;
                                      skos:example "GreenWorks is formerly identified with Mike Faha & Associates" ,
                                                   "Tommaso is formerly identified with Tommaso di Stefano Lunetti" ;
                                      skos:prefLabel "ulan1006_formerly_identified_with" .


###  http://vocab.getty.edu/ontology#ulan1007_distinguished_from
gvp:ulan1007_distinguished_from rdf:type owl:ObjectProperty ;
                                rdfs:subPropertyOf skos:related ;
                                rdf:type owl:SymmetricProperty ;
                                rdfs:domain skos:Concept ;
                                rdfs:range skos:Concept ;
                                dc:identifier "1007" ;
                                dc:title "distinguished from - any" ;
                                dct:description """any - distinguished from - any.
Example: Laura Theresa Alma-Tadema is distinguished from Lawrence Alma-Tadema; The Noguchi Museum is distinguished form Isamu Noguchi Garden Museum Japan""" ;
                                rdfs:isDefinedBy <http://vocab.getty.edu/ontology> ,
                                                 ulan: ;
                                skos:example "Laura Theresa Alma-Tadema is distinguished from Lawrence Alma-Tadema" ,
                                             "The Noguchi Museum is distinguished form Isamu Noguchi Garden Museum Japan" ;
                                skos:prefLabel "ulan1007_distinguished_from" .


###  http://vocab.getty.edu/ontology#ulan1008_meaning_-usage_overlaps_with
gvp:ulan1008_meaning_-usage_overlaps_with rdf:type owl:ObjectProperty ;
                                          rdfs:subPropertyOf skos:related ;
                                          rdf:type owl:SymmetricProperty ;
                                          rdfs:domain skos:Concept ;
                                          rdfs:range skos:Concept ;
                                          dc:identifier "1008" ;
                                          dc:title "meaning /usage overlaps with - any" ;
                                          dct:description """any - meaning /usage overlaps with - any.
Example: The meaning or usage of unknown Zimbabwean overlaps with unknown Rodesian""" ;
                                          rdfs:isDefinedBy <http://vocab.getty.edu/ontology> ,
                                                           ulan: ;
                                          skos:example "The meaning or usage of unknown Zimbabwean overlaps with unknown Rodesian" ;
                                          skos:prefLabel "ulan1008_meaning_-usage_overlaps_with" .


###  http://vocab.getty.edu/ontology#ulan1101_teacher_of
gvp:ulan1101_teacher_of rdf:type owl:ObjectProperty ;
                        rdfs:subPropertyOf skos:related ;
                        owl:inverseOf gvp:ulan1102_student_of ;
                        rdfs:domain skos:Concept ;
                        rdfs:range skos:Concept ;
                        dc:identifier "1101" ;
                        dc:title "teacher of - person" ;
                        dct:description """person - teacher of - person.
Example: Rivalz, Antoine was the teacher of Pierre Subleyras""" ;
                        rdfs:isDefinedBy <http://vocab.getty.edu/ontology> ,
                                         ulan: ;
                        skos:example "Rivalz, Antoine was the teacher of Pierre Subleyras" ;
                        skos:prefLabel "ulan1101_teacher_of" .


###  http://vocab.getty.edu/ontology#ulan1102_student_of
gvp:ulan1102_student_of rdf:type owl:ObjectProperty ;
                        rdfs:subPropertyOf skos:related ;
                        rdfs:domain skos:Concept ;
                        rdfs:range skos:Concept ;
                        dc:identifier "1102" ;
                        dc:title "student of - person" ;
                        dct:description """person - student of - person.
Example: Pierre Subleyras was the student of Rivalz, Antoine""" ;
                        rdfs:isDefinedBy <http://vocab.getty.edu/ontology> ,
                                         ulan: ;
                        skos:example "Pierre Subleyras was the student of Rivalz, Antoine" ;
                        skos:prefLabel "ulan1102_student_of" .


###  http://vocab.getty.edu/ontology#ulan1105_apprentice_of
gvp:ulan1105_apprentice_of rdf:type owl:ObjectProperty ;
                           rdfs:subPropertyOf skos:related ;
                           owl:inverseOf gvp:ulan1106_apprentice_was ;
                           rdfs:domain skos:Concept ;
                           rdfs:range skos:Concept ;
                           dc:identifier "1105" ;
                           dc:title "apprentice of - person" ;
                           dct:description """person - apprentice of - person.
Example: Nicolas Hawksmoor was the apprentice of Christopher Wren""" ;
                           rdfs:isDefinedBy <http://vocab.getty.edu/ontology> ,
                                            ulan: ;
                           skos:example "Nicolas Hawksmoor was the apprentice of Christopher Wren" ;
                           skos:prefLabel "ulan1105_apprentice_of" .


###  http://vocab.getty.edu/ontology#ulan1106_apprentice_was
gvp:ulan1106_apprentice_was rdf:type owl:ObjectProperty ;
                            rdfs:subPropertyOf skos:related ;
                            rdfs:domain skos:Concept ;
                            rdfs:range skos:Concept ;
                            dc:identifier "1106" ;
                            dc:title "apprentice was - person" ;
                            dct:description """person - apprentice was - person.
Example: Nicolas Hawksmoor was the apprentice of Christopher Wren""" ;
                            rdfs:isDefinedBy <http://vocab.getty.edu/ontology> ,
                                             ulan: ;
                            skos:example "Nicolas Hawksmoor was the apprentice of Christopher Wren" ;
                            skos:prefLabel "ulan1106_apprentice_was" .


###  http://vocab.getty.edu/ontology#ulan1107_influenced
gvp:ulan1107_influenced rdf:type owl:ObjectProperty ;
                        rdfs:subPropertyOf skos:related ;
                        owl:inverseOf gvp:ulan1108_influenced_by ;
                        rdfs:domain skos:Concept ;
                        rdfs:range skos:Concept ;
                        dc:identifier "1107" ;
                        dc:title "influenced - person" ;
                        dct:description """person - influenced - person.
Example: Rembrandt van Rijn influenced Salomon Koninck""" ;
                        rdfs:isDefinedBy <http://vocab.getty.edu/ontology> ,
                                         ulan: ;
                        skos:example "Rembrandt van Rijn influenced Salomon Koninck" ;
                        skos:prefLabel "ulan1107_influenced" .


###  http://vocab.getty.edu/ontology#ulan1108_influenced_by
gvp:ulan1108_influenced_by rdf:type owl:ObjectProperty ;
                           rdfs:subPropertyOf skos:related ;
                           rdfs:domain skos:Concept ;
                           rdfs:range skos:Concept ;
                           dc:identifier "1108" ;
                           dc:title "influenced by - person" ;
                           dct:description """person - influenced by - person.
Example: Salomon Koninck was influenced by Rembrandt van Rijn""" ;
                           rdfs:isDefinedBy <http://vocab.getty.edu/ontology> ,
                                            ulan: ;
                           skos:example "Salomon Koninck was influenced by Rembrandt van Rijn" ;
                           skos:prefLabel "ulan1108_influenced_by" .


###  http://vocab.getty.edu/ontology#ulan1111_master_of
gvp:ulan1111_master_of rdf:type owl:ObjectProperty ;
                       rdfs:subPropertyOf skos:related ;
                       owl:inverseOf gvp:ulan1112_master_was ;
                       rdfs:domain skos:Concept ;
                       rdfs:range skos:Concept ;
                       dc:identifier "1111" ;
                       dc:title "master of - person" ;
                       dct:description """person - master of - person.
Example: Peter Paul Rubens - master of Jan Thomas""" ;
                       rdfs:isDefinedBy <http://vocab.getty.edu/ontology> ,
                                        ulan: ;
                       skos:example "Peter Paul Rubens - master of Jan Thomas" ;
                       skos:prefLabel "ulan1111_master_of" .


###  http://vocab.getty.edu/ontology#ulan1112_master_was
gvp:ulan1112_master_was rdf:type owl:ObjectProperty ;
                        rdfs:subPropertyOf skos:related ;
                        rdfs:domain skos:Concept ;
                        rdfs:range skos:Concept ;
                        dc:identifier "1112" ;
                        dc:title "master was - person" ;
                        dct:description """person - master was - person.
Example: Peter Paul Rubens - master of Jan Thomas""" ;
                        rdfs:isDefinedBy <http://vocab.getty.edu/ontology> ,
                                         ulan: ;
                        skos:example "Peter Paul Rubens - master of Jan Thomas" ;
                        skos:prefLabel "ulan1112_master_was" .


###  http://vocab.getty.edu/ontology#ulan1113_fellow_student_of
gvp:ulan1113_fellow_student_of rdf:type owl:ObjectProperty ;
                               rdfs:subPropertyOf skos:related ;
                               rdf:type owl:SymmetricProperty ;
                               rdfs:domain skos:Concept ;
                               rdfs:range skos:Concept ;
                               dc:identifier "1113" ;
                               dc:title "fellow student of - person" ;
                               dct:description """person - fellow student of - person.
Example: Alexander Calder was a fellow student of John Sloan; John Sloan was a fellow student of Thomas Hart Benton""" ;
                               rdfs:isDefinedBy <http://vocab.getty.edu/ontology> ,
                                                ulan: ;
                               skos:example "Alexander Calder was a fellow student of John Sloan" ,
                                            "John Sloan was a fellow student of Thomas Hart Benton" ;
                               skos:prefLabel "ulan1113_fellow_student_of" .


###  http://vocab.getty.edu/ontology#ulan1201_patron_of
gvp:ulan1201_patron_of rdf:type owl:ObjectProperty ;
                       rdfs:subPropertyOf skos:related ;
                       owl:inverseOf gvp:ulan1202_patron_was ;
                       rdfs:domain skos:Concept ;
                       rdfs:range skos:Concept ;
                       dc:identifier "1201" ;
                       dc:title "patron of - person/firm/family" ;
                       dct:description """person - patron of - person/firm/family.
Example: Cosimo I, Grand-Duke of Tuscany was the patron of Donatello""" ;
                       rdfs:isDefinedBy <http://vocab.getty.edu/ontology> ,
                                        ulan: ;
                       skos:example "Cosimo I, Grand-Duke of Tuscany was the patron of Donatello" ;
                       skos:prefLabel "ulan1201_patron_of" .


###  http://vocab.getty.edu/ontology#ulan1202_patron_was
gvp:ulan1202_patron_was rdf:type owl:ObjectProperty ;
                        rdfs:subPropertyOf skos:related ;
                        rdfs:domain skos:Concept ;
                        rdfs:range skos:Concept ;
                        dc:identifier "1202" ;
                        dc:title "patron was - person" ;
                        dct:description """person/firm/family - patron was - person.
Example: The patron of Donatello was Cosimo I, Grand-Duke of Tuscany""" ;
                        rdfs:isDefinedBy <http://vocab.getty.edu/ontology> ,
                                         ulan: ;
                        skos:example "The patron of Donatello was Cosimo I, Grand-Duke of Tuscany" ;
                        skos:prefLabel "ulan1202_patron_was" .


###  http://vocab.getty.edu/ontology#ulan1203_donor_of
gvp:ulan1203_donor_of rdf:type owl:ObjectProperty ;
                      rdfs:subPropertyOf skos:related ;
                      owl:inverseOf gvp:ulan1204_donor_was ;
                      rdfs:domain skos:Concept ;
                      rdfs:range skos:Concept ;
                      dc:identifier "1203" ;
                      dc:title "donor of - person/firm/family" ;
                      dct:description """person/firm/family - donor of - person/firm/family.
Example: Andrew W. Mellon was a donor of National Gallery of Art""" ;
                      rdfs:isDefinedBy <http://vocab.getty.edu/ontology> ,
                                       ulan: ;
                      skos:example "Andrew W. Mellon was a donor of National Gallery of Art" ;
                      skos:prefLabel "ulan1203_donor_of" .


###  http://vocab.getty.edu/ontology#ulan1204_donor_was
gvp:ulan1204_donor_was rdf:type owl:ObjectProperty ;
                       rdfs:subPropertyOf skos:related ;
                       rdfs:domain skos:Concept ;
                       rdfs:range skos:Concept ;
                       dc:identifier "1204" ;
                       dc:title "donor was - person/firm/family" ;
                       dct:description """person/firm/family - donor was - person/firm/family.
Example: Donor to the National Gallery of Art was Andrew W. Mellon""" ;
                       rdfs:isDefinedBy <http://vocab.getty.edu/ontology> ,
                                        ulan: ;
                       skos:example "Donor to the National Gallery of Art was Andrew W. Mellon" ;
                       skos:prefLabel "ulan1204_donor_was" .


###  http://vocab.getty.edu/ontology#ulan1205_client_of
gvp:ulan1205_client_of rdf:type owl:ObjectProperty ;
                       rdfs:subPropertyOf skos:related ;
                       owl:inverseOf gvp:ulan1206_client_was ;
                       rdfs:domain skos:Concept ;
                       rdfs:range skos:Concept ;
                       dc:identifier "1205" ;
                       dc:title "client of - person/firm/family" ;
                       dct:description """person/firm/family - client of - person/firm/family.
Example: The Chicago Herald was the client of Burnham and Root""" ;
                       rdfs:isDefinedBy <http://vocab.getty.edu/ontology> ,
                                        ulan: ;
                       skos:example "The Chicago Herald was the client of Burnham and Root" ;
                       skos:prefLabel "ulan1205_client_of" .


###  http://vocab.getty.edu/ontology#ulan1206_client_was
gvp:ulan1206_client_was rdf:type owl:ObjectProperty ;
                        rdfs:subPropertyOf skos:related ;
                        rdfs:domain skos:Concept ;
                        rdfs:range skos:Concept ;
                        dc:identifier "1206" ;
                        dc:title "client was - person/firm/family" ;
                        dct:description """person/firm/family - client was - person/firm/family.
Example: Burnham and Root's client was the Chicago Herald""" ;
                        rdfs:isDefinedBy <http://vocab.getty.edu/ontology> ,
                                         ulan: ;
                        skos:example "Burnham and Root's client was the Chicago Herald" ;
                        skos:prefLabel "ulan1206_client_was" .


###  http://vocab.getty.edu/ontology#ulan1211_artist_to
gvp:ulan1211_artist_to rdf:type owl:ObjectProperty ;
                       rdfs:subPropertyOf skos:related ;
                       owl:inverseOf gvp:ulan1212_artist_was ;
                       rdfs:domain skos:Concept ;
                       rdfs:range skos:Concept ;
                       dc:identifier "1211" ;
                       dc:title "artist to - person" ;
                       dct:description """person - artist to - person.
Example: Artist to Louis XIV, King of France was Charles-Pierre Coustou""" ;
                       rdfs:isDefinedBy <http://vocab.getty.edu/ontology> ,
                                        ulan: ;
                       skos:example "Artist to Louis XIV, King of France was Charles-Pierre Coustou" ;
                       skos:prefLabel "ulan1211_artist_to" .


###  http://vocab.getty.edu/ontology#ulan1212_artist_was
gvp:ulan1212_artist_was rdf:type owl:ObjectProperty ;
                        rdfs:subPropertyOf skos:related ;
                        rdfs:domain skos:Concept ;
                        rdfs:range skos:Concept ;
                        dc:identifier "1212" ;
                        dc:title "artist was - person" ;
                        dct:description """person - artist was - person.
Example: Charles-Pierre Coustou was artist to Louis XIV, King of France""" ;
                        rdfs:isDefinedBy <http://vocab.getty.edu/ontology> ,
                                         ulan: ;
                        skos:example "Charles-Pierre Coustou was artist to Louis XIV, King of France" ;
                        skos:prefLabel "ulan1212_artist_was" .


###  http://vocab.getty.edu/ontology#ulan1213_court_artist_to
gvp:ulan1213_court_artist_to rdf:type owl:ObjectProperty ;
                             rdfs:subPropertyOf skos:related ;
                             owl:inverseOf gvp:ulan1214_court_artist_was ;
                             rdfs:domain skos:Concept ;
                             rdfs:range skos:Concept ;
                             dc:identifier "1213" ;
                             dc:title "court artist to - person" ;
                             dct:description """person - court artist to - person.
Example: Court artist to Gonzaga Vincenzo I, Duke of Mantua was Peter Paul Rubens; court artist to Charles IV, King of Spain was Francisco de Goya""" ;
                             rdfs:isDefinedBy <http://vocab.getty.edu/ontology> ,
                                              ulan: ;
                             skos:example "Court artist to Gonzaga Vincenzo I, Duke of Mantua was Peter Paul Rubens" ,
                                          "court artist to Charles IV, King of Spain was Francisco de Goya" ;
                             skos:prefLabel "ulan1213_court_artist_to" .


###  http://vocab.getty.edu/ontology#ulan1214_court_artist_was
gvp:ulan1214_court_artist_was rdf:type owl:ObjectProperty ;
                              rdfs:subPropertyOf skos:related ;
                              rdfs:domain skos:Concept ;
                              rdfs:range skos:Concept ;
                              dc:identifier "1214" ;
                              dc:title "court artist was - person" ;
                              dct:description """person - court artist was - person.
Example: Peter Paul Rubens was court artist to Gonzaga Vincenzo I, Duke of Mantua; Francisco de Goya was court artist to Charles IV, King of Spain""" ;
                              rdfs:isDefinedBy <http://vocab.getty.edu/ontology> ,
                                               ulan: ;
                              skos:example "Francisco de Goya was court artist to Charles IV, King of Spain" ,
                                           "Peter Paul Rubens was court artist to Gonzaga Vincenzo I, Duke of Mantua" ;
                              skos:prefLabel "ulan1214_court_artist_was" .


###  http://vocab.getty.edu/ontology#ulan1217_employee_of
gvp:ulan1217_employee_of rdf:type owl:ObjectProperty ;
                         rdfs:subPropertyOf skos:related ;
                         owl:inverseOf gvp:ulan1218_employee_was ;
                         rdfs:domain skos:Concept ;
                         rdfs:range skos:Concept ;
                         dc:identifier "1217" ;
                         dc:title "employee of - person" ;
                         dct:description """person/firm - employee of - person.
Example: Employee of Christopher Wren was Jean Tijou""" ;
                         rdfs:isDefinedBy <http://vocab.getty.edu/ontology> ,
                                          ulan: ;
                         skos:example "Employee of Christopher Wren was Jean Tijou" ;
                         skos:prefLabel "ulan1217_employee_of" .


###  http://vocab.getty.edu/ontology#ulan1218_employee_was
gvp:ulan1218_employee_was rdf:type owl:ObjectProperty ;
                          rdfs:subPropertyOf skos:related ;
                          rdfs:domain skos:Concept ;
                          rdfs:range skos:Concept ;
                          dc:identifier "1218" ;
                          dc:title "employee was - person/firm" ;
                          dct:description """person - employee was - person/firm.
Example: Jean Tijou was an employee of Christopher Wren""" ;
                          rdfs:isDefinedBy <http://vocab.getty.edu/ontology> ,
                                           ulan: ;
                          skos:example "Jean Tijou was an employee of Christopher Wren" ;
                          skos:prefLabel "ulan1218_employee_was" .


###  http://vocab.getty.edu/ontology#ulan1221_appointed_by
gvp:ulan1221_appointed_by rdf:type owl:ObjectProperty ;
                          rdfs:subPropertyOf skos:related ;
                          owl:inverseOf gvp:ulan1222_appointee_of ;
                          rdfs:domain skos:Concept ;
                          rdfs:range skos:Concept ;
                          dc:identifier "1221" ;
                          dc:title "appointed by - person" ;
                          dct:description """person - appointed by - person.
Example: Pope Urban VIII appointed Virginio Cesarini""" ;
                          rdfs:isDefinedBy <http://vocab.getty.edu/ontology> ,
                                           ulan: ;
                          skos:example "Pope Urban VIII appointed Virginio Cesarini" ;
                          skos:prefLabel "ulan1221_appointed_by" .


###  http://vocab.getty.edu/ontology#ulan1222_appointee_of
gvp:ulan1222_appointee_of rdf:type owl:ObjectProperty ;
                          rdfs:subPropertyOf skos:related ;
                          rdfs:domain skos:Concept ;
                          rdfs:range skos:Concept ;
                          dc:identifier "1222" ;
                          dc:title "appointee of - person" ;
                          dct:description """person - appointee of - person.
Example: Virginio Cesarini was appointee by Pope Urban VIII""" ;
                          rdfs:isDefinedBy <http://vocab.getty.edu/ontology> ,
                                           ulan: ;
                          skos:example "Virginio Cesarini was appointee by Pope Urban VIII" ;
                          skos:prefLabel "ulan1222_appointee_of" .


###  http://vocab.getty.edu/ontology#ulan1223_crowned_by
gvp:ulan1223_crowned_by rdf:type owl:ObjectProperty ;
                        rdfs:subPropertyOf skos:related ;
                        owl:inverseOf gvp:ulan1224_crowned ;
                        rdfs:domain skos:Concept ;
                        rdfs:range skos:Concept ;
                        dc:identifier "1223" ;
                        dc:title "crowned by - person" ;
                        dct:description """person - crowned by - person.
Example: Pope Leo III crowned Emperor Charlemagne""" ;
                        rdfs:isDefinedBy <http://vocab.getty.edu/ontology> ,
                                         ulan: ;
                        skos:example "Pope Leo III crowned Emperor Charlemagne" ;
                        skos:prefLabel "ulan1223_crowned_by" .


###  http://vocab.getty.edu/ontology#ulan1224_crowned
gvp:ulan1224_crowned rdf:type owl:ObjectProperty ;
                     rdfs:subPropertyOf skos:related ;
                     rdfs:domain skos:Concept ;
                     rdfs:range skos:Concept ;
                     dc:identifier "1224" ;
                     dc:title "crowned - person" ;
                     dct:description """person - crowned - person.
Example: Emperor Charlemagne was crowned by Pope Leo III""" ;
                     rdfs:isDefinedBy <http://vocab.getty.edu/ontology> ,
                                      ulan: ;
                     skos:example "Emperor Charlemagne was crowned by Pope Leo III" ;
                     skos:prefLabel "ulan1224_crowned" .


###  http://vocab.getty.edu/ontology#ulan1301_colleague_of
gvp:ulan1301_colleague_of rdf:type owl:ObjectProperty ;
                          rdfs:subPropertyOf skos:related ;
                          rdf:type owl:SymmetricProperty ;
                          rdfs:domain skos:Concept ;
                          rdfs:range skos:Concept ;
                          dc:identifier "1301" ;
                          dc:title "colleague of - person" ;
                          dct:description """person - colleague of - person.
Example: Titian was a colleague of Maria Giovanni Verdizotti""" ;
                          rdfs:isDefinedBy <http://vocab.getty.edu/ontology> ,
                                           ulan: ;
                          skos:example "Titian was a colleague of Maria Giovanni Verdizotti" ;
                          skos:prefLabel "ulan1301_colleague_of" .


###  http://vocab.getty.edu/ontology#ulan1302_associate_of
gvp:ulan1302_associate_of rdf:type owl:ObjectProperty ;
                          rdfs:subPropertyOf skos:related ;
                          rdf:type owl:SymmetricProperty ;
                          rdfs:domain skos:Concept ;
                          rdfs:range skos:Concept ;
                          dc:identifier "1302" ;
                          dc:title "associate of - person" ;
                          dct:description """person - associate of - person.
Example: Frank Lloyd Wright was an associate of Giannini and Hilgart""" ;
                          rdfs:isDefinedBy <http://vocab.getty.edu/ontology> ,
                                           ulan: ;
                          skos:example "Frank Lloyd Wright was an associate of Giannini and Hilgart" ;
                          skos:prefLabel "ulan1302_associate_of" .


###  http://vocab.getty.edu/ontology#ulan1303_collaborated_with
gvp:ulan1303_collaborated_with rdf:type owl:ObjectProperty ;
                               rdfs:subPropertyOf skos:related ;
                               rdf:type owl:SymmetricProperty ;
                               rdfs:domain skos:Concept ;
                               rdfs:range skos:Concept ;
                               dc:identifier "1303" ;
                               dc:title "collaborated with - person" ;
                               dct:description """person - collaborated with - person.
Example: Pablo Picasso collaborated with Georges Braque""" ;
                               rdfs:isDefinedBy <http://vocab.getty.edu/ontology> ,
                                                ulan: ;
                               skos:example "Pablo Picasso collaborated with Georges Braque" ;
                               skos:prefLabel "ulan1303_collaborated_with" .


###  http://vocab.getty.edu/ontology#ulan1305_worked_with
gvp:ulan1305_worked_with rdf:type owl:ObjectProperty ;
                         rdfs:subPropertyOf skos:related ;
                         rdf:type owl:SymmetricProperty ;
                         rdfs:domain skos:Concept ;
                         rdfs:range skos:Concept ;
                         dc:identifier "1305" ;
                         dc:title "worked with - person" ;
                         dct:description """person - worked with - person.
Example: William Cleare worked with Christopher Wren; Frank Lloyd Wright work with Aaron G. Green""" ;
                         rdfs:isDefinedBy <http://vocab.getty.edu/ontology> ,
                                          ulan: ;
                         skos:example "Frank Lloyd Wright work with Aaron G. Green" ,
                                      "William Cleare worked with Christopher Wren" ;
                         skos:prefLabel "ulan1305_worked_with" .


###  http://vocab.getty.edu/ontology#ulan1306_performs_with
gvp:ulan1306_performs_with rdf:type owl:ObjectProperty ;
                           rdfs:subPropertyOf skos:related ;
                           rdf:type owl:SymmetricProperty ;
                           rdfs:domain skos:Concept ;
                           rdfs:range skos:Concept ;
                           dc:identifier "1306" ;
                           dc:title "performs with - person" ;
                           dct:description """person - performs with - person.
Example: Harry Kipper performs with Harry Kipper (as part of 'The Kipper Kids')""" ;
                           rdfs:isDefinedBy <http://vocab.getty.edu/ontology> ,
                                            ulan: ;
                           skos:example "Harry Kipper performs with Harry Kipper (as part of 'The Kipper Kids')" ;
                           skos:prefLabel "ulan1306_performs_with" .


###  http://vocab.getty.edu/ontology#ulan1307_assistant_of
gvp:ulan1307_assistant_of rdf:type owl:ObjectProperty ;
                          rdfs:subPropertyOf skos:related ;
                          owl:inverseOf gvp:ulan1308_assisted_by ;
                          rdfs:domain skos:Concept ;
                          rdfs:range skos:Concept ;
                          dc:identifier "1307" ;
                          dc:title "assistant of - person" ;
                          dct:description """person - assistant of - person.
Example: Bernard Castelli was assistant of Pablo Picasso""" ;
                          rdfs:isDefinedBy <http://vocab.getty.edu/ontology> ,
                                           ulan: ;
                          skos:example "Bernard Castelli was assistant of Pablo Picasso" ;
                          skos:prefLabel "ulan1307_assistant_of" .


###  http://vocab.getty.edu/ontology#ulan1308_assisted_by
gvp:ulan1308_assisted_by rdf:type owl:ObjectProperty ;
                         rdfs:subPropertyOf skos:related ;
                         rdfs:domain skos:Concept ;
                         rdfs:range skos:Concept ;
                         dc:identifier "1308" ;
                         dc:title "assisted by - person" ;
                         dct:description """person - assisted by - person.
Example: Pablo Picasso was assisted by Bernard Castelli""" ;
                         rdfs:isDefinedBy <http://vocab.getty.edu/ontology> ,
                                          ulan: ;
                         skos:example "Pablo Picasso was assisted by Bernard Castelli" ;
                         skos:prefLabel "ulan1308_assisted_by" .


###  http://vocab.getty.edu/ontology#ulan1309_advisor_of
gvp:ulan1309_advisor_of rdf:type owl:ObjectProperty ;
                        rdfs:subPropertyOf skos:related ;
                        owl:inverseOf gvp:ulan1310_advised_by ;
                        rdfs:domain skos:Concept ;
                        rdfs:range skos:Concept ;
                        dc:identifier "1309" ;
                        dc:title "advisor of - person" ;
                        dct:description """person - advisor of - person.
Example: Thomas Cromwell, Earl of Essex was the advisor of Henry VIII, King of England""" ;
                        rdfs:isDefinedBy <http://vocab.getty.edu/ontology> ,
                                         ulan: ;
                        skos:example "Thomas Cromwell, Earl of Essex was the advisor of Henry VIII, King of England" ;
                        skos:prefLabel "ulan1309_advisor_of" .


###  http://vocab.getty.edu/ontology#ulan1310_advised_by
gvp:ulan1310_advised_by rdf:type owl:ObjectProperty ;
                        rdfs:subPropertyOf skos:related ;
                        rdfs:domain skos:Concept ;
                        rdfs:range skos:Concept ;
                        dc:identifier "1310" ;
                        dc:title "advised by - person" ;
                        dct:description """person - advised by - person.
Example: Henry VIII, King of England was advised by Thomas Cromwell, Earl of Essex""" ;
                        rdfs:isDefinedBy <http://vocab.getty.edu/ontology> ,
                                         ulan: ;
                        skos:example "Henry VIII, King of England was advised by Thomas Cromwell, Earl of Essex" ;
                        skos:prefLabel "ulan1310_advised_by" .


###  http://vocab.getty.edu/ontology#ulan1311_partner_of
gvp:ulan1311_partner_of rdf:type owl:ObjectProperty ;
                        rdfs:subPropertyOf skos:related ;
                        rdf:type owl:SymmetricProperty ;
                        rdfs:domain skos:Concept ;
                        rdfs:range skos:Concept ;
                        dc:identifier "1311" ;
                        dc:title "partner of - person" ;
                        dct:description """person - partner of - person.
Example: Frank Gehry and James Glymph are partners""" ;
                        rdfs:isDefinedBy <http://vocab.getty.edu/ontology> ,
                                         ulan: ;
                        skos:example "Frank Gehry and James Glymph are partners" ;
                        skos:prefLabel "ulan1311_partner_of" .


###  http://vocab.getty.edu/ontology#ulan1313_partner_in
gvp:ulan1313_partner_in rdf:type owl:ObjectProperty ;
                        rdfs:subPropertyOf skos:related ;
                        owl:inverseOf gvp:ulan1314_partner_was ;
                        rdfs:domain skos:Concept ;
                        rdfs:range skos:Concept ;
                        dc:identifier "1313" ;
                        dc:title "partner in - firm" ;
                        dct:description """person - partner in - firm.
Example: Parners of Adler and Sullivan included Louis H. Sullivan and Dankmar Adler""" ;
                        rdfs:isDefinedBy <http://vocab.getty.edu/ontology> ,
                                         ulan: ;
                        skos:example "Parners of Adler and Sullivan included Louis H. Sullivan and Dankmar Adler" ;
                        skos:prefLabel "ulan1313_partner_in" .


###  http://vocab.getty.edu/ontology#ulan1314_partner_was
gvp:ulan1314_partner_was rdf:type owl:ObjectProperty ;
                         rdfs:subPropertyOf skos:related ;
                         rdfs:domain skos:Concept ;
                         rdfs:range skos:Concept ;
                         dc:identifier "1314" ;
                         dc:title "partner was - person" ;
                         dct:description """firm - partner was - person.
Example: Louis H. Sullivan and Dankmar Adler were partners in Adler and Sullivan""" ;
                         rdfs:isDefinedBy <http://vocab.getty.edu/ontology> ,
                                          ulan: ;
                         skos:example "Louis H. Sullivan and Dankmar Adler were partners in Adler and Sullivan" ;
                         skos:prefLabel "ulan1314_partner_was" .


###  http://vocab.getty.edu/ontology#ulan1315_principal_in
gvp:ulan1315_principal_in rdf:type owl:ObjectProperty ;
                          rdfs:subPropertyOf skos:related ;
                          owl:inverseOf gvp:ulan1316_principal_was ;
                          rdfs:domain skos:Concept ;
                          rdfs:range skos:Concept ;
                          dc:identifier "1315" ;
                          dc:title "principal in - firm" ;
                          dct:description """person - principal in - firm.
Example: Principal in Fontana Workshop was Orazio Fontana""" ;
                          rdfs:isDefinedBy <http://vocab.getty.edu/ontology> ,
                                           ulan: ;
                          skos:example "Principal in Fontana Workshop was Orazio Fontana" ;
                          skos:prefLabel "ulan1315_principal_in" .


###  http://vocab.getty.edu/ontology#ulan1316_principal_was
gvp:ulan1316_principal_was rdf:type owl:ObjectProperty ;
                           rdfs:subPropertyOf skos:related ;
                           rdfs:domain skos:Concept ;
                           rdfs:range skos:Concept ;
                           dc:identifier "1316" ;
                           dc:title "principal was - person" ;
                           dct:description """firm - principal was - person.
Example: Orazio Fontana was principal in Fontana Workshop""" ;
                           rdfs:isDefinedBy <http://vocab.getty.edu/ontology> ,
                                            ulan: ;
                           skos:example "Orazio Fontana was principal in Fontana Workshop" ;
                           skos:prefLabel "ulan1316_principal_was" .


###  http://vocab.getty.edu/ontology#ulan1317_member_of
gvp:ulan1317_member_of rdf:type owl:ObjectProperty ;
                       rdfs:subPropertyOf skos:related ;
                       owl:inverseOf gvp:ulan1318_member_was ;
                       rdfs:domain skos:Concept ;
                       rdfs:range skos:Concept ;
                       dc:identifier "1317" ;
                       dc:title "member of - person/firm/group" ;
                       dct:description """firm/group - member of - person/firm/group.
Example: A member of the Foundation of Documents of Architecture is the National Gallery of Art""" ;
                       rdfs:isDefinedBy <http://vocab.getty.edu/ontology> ,
                                        ulan: ;
                       skos:example "A member of the Foundation of Documents of Architecture is the National Gallery of Art" ;
                       skos:prefLabel "ulan1317_member_of" .


###  http://vocab.getty.edu/ontology#ulan1318_member_was
gvp:ulan1318_member_was rdf:type owl:ObjectProperty ;
                        rdfs:subPropertyOf skos:related ;
                        rdfs:domain skos:Concept ;
                        rdfs:range skos:Concept ;
                        dc:identifier "1318" ;
                        dc:title "member was - firm/group" ;
                        dct:description """person/firm/group - member was - firm/group.
Example: The National Gallery of Art was/is a member of the Foundation of Documentation of Architecture""" ;
                        rdfs:isDefinedBy <http://vocab.getty.edu/ontology> ,
                                         ulan: ;
                        skos:example "The National Gallery of Art was/is a member of the Foundation of Documentation of Architecture" ;
                        skos:prefLabel "ulan1318_member_was" .


###  http://vocab.getty.edu/ontology#ulan1321_school_of
gvp:ulan1321_school_of rdf:type owl:ObjectProperty ;
                       rdfs:subPropertyOf skos:related ;
                       owl:inverseOf gvp:ulan1322_school_was ;
                       rdfs:domain skos:Concept ;
                       rdfs:range skos:Concept ;
                       dc:identifier "1321" ;
                       dc:title "school of - firm/group" ;
                       dct:description """person - school of - firm/group.
Example: The school of Pierre Saalburg was the Architectural Association. School of Architecture""" ;
                       rdfs:isDefinedBy <http://vocab.getty.edu/ontology> ,
                                        ulan: ;
                       skos:example "The school of Pierre Saalburg was the Architectural Association. School of Architecture" ;
                       skos:prefLabel "ulan1321_school_of" .


###  http://vocab.getty.edu/ontology#ulan1322_school_was
gvp:ulan1322_school_was rdf:type owl:ObjectProperty ;
                        rdfs:subPropertyOf skos:related ;
                        rdfs:domain skos:Concept ;
                        rdfs:range skos:Concept ;
                        dc:identifier "1322" ;
                        dc:title "school was - person" ;
                        dct:description """firm/group - school was - person.
Example: Pierre Saalburg attended Architectural Association. School of Architecture""" ;
                        rdfs:isDefinedBy <http://vocab.getty.edu/ontology> ,
                                         ulan: ;
                        skos:example "Pierre Saalburg attended Architectural Association. School of Architecture" ;
                        skos:prefLabel "ulan1322_school_was" .


###  http://vocab.getty.edu/ontology#ulan1331_worked_with
gvp:ulan1331_worked_with rdf:type owl:ObjectProperty ;
                         rdfs:subPropertyOf skos:related ;
                         owl:inverseOf gvp:ulan1332_worker_was ;
                         rdfs:domain skos:Concept ;
                         rdfs:range skos:Concept ;
                         dc:identifier "1331" ;
                         dc:title "worked with - person" ;
                         dct:description """any - worked with - person.
Example: Scarsellino and Domenichino worked with the Carracci family""" ;
                         rdfs:isDefinedBy <http://vocab.getty.edu/ontology> ,
                                          ulan: ;
                         skos:example "Scarsellino and Domenichino worked with the Carracci family" ;
                         skos:prefLabel "ulan1331_worked_with" .


###  http://vocab.getty.edu/ontology#ulan1332_worker_was
gvp:ulan1332_worker_was rdf:type owl:ObjectProperty ;
                        rdfs:subPropertyOf skos:related ;
                        rdfs:domain skos:Concept ;
                        rdfs:range skos:Concept ;
                        dc:identifier "1332" ;
                        dc:title "worker was - any" ;
                        dct:description """person - worker was - any.
Example: Workers for the Carracci family included Scarsellino and Domenichino""" ;
                        rdfs:isDefinedBy <http://vocab.getty.edu/ontology> ,
                                         ulan: ;
                        skos:example "Workers for the Carracci family included Scarsellino and Domenichino" ;
                        skos:prefLabel "ulan1332_worker_was" .


###  http://vocab.getty.edu/ontology#ulan1411_successor_of
gvp:ulan1411_successor_of rdf:type owl:ObjectProperty ;
                          rdfs:subPropertyOf skos:related ;
                          owl:inverseOf gvp:ulan1412_predecessor_of ;
                          rdfs:domain skos:Concept ;
                          rdfs:range skos:Concept ;
                          dc:identifier "1411" ;
                          dc:title "successor of - firm/group" ;
                          dct:description """firm/group - successor of - firm/group.
Example: Richard Meier & Partners Architects LLP is the successor of Richard Meier & Associates""" ;
                          rdfs:isDefinedBy <http://vocab.getty.edu/ontology> ,
                                           ulan: ;
                          skos:example "Richard Meier & Partners Architects LLP is the successor of Richard Meier & Associates" ;
                          skos:prefLabel "ulan1411_successor_of" .


###  http://vocab.getty.edu/ontology#ulan1412_predecessor_of
gvp:ulan1412_predecessor_of rdf:type owl:ObjectProperty ;
                            rdfs:subPropertyOf skos:related ;
                            rdfs:domain skos:Concept ;
                            rdfs:range skos:Concept ;
                            dc:identifier "1412" ;
                            dc:title "predecessor of - firm/group" ;
                            dct:description """firm/group - predecessor of - firm/group.
Example: Richard Meier & Associates is the predecessor of Richard Meier & Partners Architects LLP""" ;
                            rdfs:isDefinedBy <http://vocab.getty.edu/ontology> ,
                                             ulan: ;
                            skos:example "Richard Meier & Associates is the predecessor of Richard Meier & Partners Architects LLP" ;
                            skos:prefLabel "ulan1412_predecessor_of" .


###  http://vocab.getty.edu/ontology#ulan1413_administration_overlaps_with
gvp:ulan1413_administration_overlaps_with rdf:type owl:ObjectProperty ;
                                          rdfs:subPropertyOf skos:related ;
                                          rdf:type owl:SymmetricProperty ;
                                          rdfs:domain skos:Concept ;
                                          rdfs:range skos:Concept ;
                                          dc:identifier "1413" ;
                                          dc:title "administration overlaps with - firm/group" ;
                                          dct:description """firm/group - administration overlaps with - firm/group.
Example: The administration of the Numismatic Collection overlaps with Bode Museum""" ;
                                          rdfs:isDefinedBy <http://vocab.getty.edu/ontology> ,
                                                           ulan: ;
                                          skos:example "The administration of the Numismatic Collection overlaps with Bode Museum" ;
                                          skos:prefLabel "ulan1413_administration_overlaps_with" .


###  http://vocab.getty.edu/ontology#ulan1414_joint_venture_with
gvp:ulan1414_joint_venture_with rdf:type owl:ObjectProperty ;
                                rdfs:subPropertyOf skos:related ;
                                rdf:type owl:SymmetricProperty ;
                                rdfs:domain skos:Concept ;
                                rdfs:range skos:Concept ;
                                dc:identifier "1414" ;
                                dc:title "joint venture with - firm/group" ;
                                dct:description """firm/group - joint venture with - firm/group.
Example: Schwetye Luchini Architects is in a joint venture with ACME Architects""" ;
                                rdfs:isDefinedBy <http://vocab.getty.edu/ontology> ,
                                                 ulan: ;
                                skos:example "Schwetye Luchini Architects is in a joint venture with ACME Architects" ;
                                skos:prefLabel "ulan1414_joint_venture_with" .


###  http://vocab.getty.edu/ontology#ulan1421_founded_by
gvp:ulan1421_founded_by rdf:type owl:ObjectProperty ;
                        rdfs:subPropertyOf skos:related ;
                        owl:inverseOf gvp:ulan1422_founded ;
                        rdfs:domain skos:Concept ;
                        rdfs:range skos:Concept ;
                        dc:identifier "1421" ;
                        dc:title "founded by - firm/group" ;
                        dct:description """firm/group - founded by - firm/group.
Example: National Gallery of Art was founded by United States Congress""" ;
                        rdfs:isDefinedBy <http://vocab.getty.edu/ontology> ,
                                         ulan: ;
                        skos:example "National Gallery of Art was founded by United States Congress" ;
                        skos:prefLabel "ulan1421_founded_by" .


###  http://vocab.getty.edu/ontology#ulan1422_founded
gvp:ulan1422_founded rdf:type owl:ObjectProperty ;
                     rdfs:subPropertyOf skos:related ;
                     rdfs:domain skos:Concept ;
                     rdfs:range skos:Concept ;
                     dc:identifier "1422" ;
                     dc:title "founded - firm/group" ;
                     dct:description """firm/group - founded - firm/group.
Example: The United States Congress founded the National Gallery of Art""" ;
                     rdfs:isDefinedBy <http://vocab.getty.edu/ontology> ,
                                      ulan: ;
                     skos:example "The United States Congress founded the National Gallery of Art" ;
                     skos:prefLabel "ulan1422_founded" .


###  http://vocab.getty.edu/ontology#ulan1500_related_to
gvp:ulan1500_related_to rdf:type owl:ObjectProperty ;
                        rdfs:subPropertyOf skos:related ;
                        rdf:type owl:SymmetricProperty ;
                        rdfs:domain skos:Concept ;
                        rdfs:range skos:Concept ;
                        dc:identifier "1500" ;
                        dc:title "related to - person" ;
                        dct:description """person - related to (familial relationship) - person.
Example: Titian and Tizianello have a familial relationship with each other""" ;
                        rdfs:isDefinedBy <http://vocab.getty.edu/ontology> ,
                                         ulan: ;
                        skos:example "Titian and Tizianello have a familial relationship with each other" ;
                        skos:prefLabel "ulan1500_related_to" .


###  http://vocab.getty.edu/ontology#ulan1501_sibling_of
gvp:ulan1501_sibling_of rdf:type owl:ObjectProperty ;
                        rdfs:subPropertyOf skos:related ;
                        rdf:type owl:SymmetricProperty ;
                        rdfs:domain skos:Concept ;
                        rdfs:range skos:Concept ;
                        dc:identifier "1501" ;
                        dc:title "sibling of - person" ;
                        dct:description """person - sibling of - person.
Example: Philippe Rubens is the sibling of Peter Paul Rubens""" ;
                        rdfs:isDefinedBy <http://vocab.getty.edu/ontology> ,
                                         ulan: ;
                        skos:example "Philippe Rubens is the sibling of Peter Paul Rubens" ;
                        skos:prefLabel "ulan1501_sibling_of" .


###  http://vocab.getty.edu/ontology#ulan1511_child_of
gvp:ulan1511_child_of rdf:type owl:ObjectProperty ;
                      rdfs:subPropertyOf skos:related ;
                      owl:inverseOf gvp:ulan1512_parent_of ;
                      rdfs:domain skos:Concept ;
                      rdfs:range skos:Concept ;
                      dc:identifier "1511" ;
                      dc:title "child of - person" ;
                      dct:description """person - child of - person.
Example: Rembrandt van Rijn is the child of Neeltgen Willemsdr van Zuydtbroeck""" ;
                      rdfs:isDefinedBy <http://vocab.getty.edu/ontology> ,
                                       ulan: ;
                      skos:example "Rembrandt van Rijn is the child of Neeltgen Willemsdr van Zuydtbroeck" ;
                      skos:prefLabel "ulan1511_child_of" .


###  http://vocab.getty.edu/ontology#ulan1512_parent_of
gvp:ulan1512_parent_of rdf:type owl:ObjectProperty ;
                       rdfs:subPropertyOf skos:related ;
                       rdfs:domain skos:Concept ;
                       rdfs:range skos:Concept ;
                       dc:identifier "1512" ;
                       dc:title "parent of - person" ;
                       dct:description """person - parent of - person.
Example: Rembrandt van Rijn is the parent of Rumbertus van Rijn""" ;
                       rdfs:isDefinedBy <http://vocab.getty.edu/ontology> ,
                                        ulan: ;
                       skos:example "Rembrandt van Rijn is the parent of Rumbertus van Rijn" ;
                       skos:prefLabel "ulan1512_parent_of" .


###  http://vocab.getty.edu/ontology#ulan1513_grandchild_of
gvp:ulan1513_grandchild_of rdf:type owl:ObjectProperty ;
                           rdfs:subPropertyOf skos:related ;
                           owl:inverseOf gvp:ulan1514_gandparent_of ;
                           rdfs:domain skos:Concept ;
                           rdfs:range skos:Concept ;
                           dc:identifier "1513" ;
                           dc:title "grandchild of - person" ;
                           dct:description """person - grandchild of - person.
Example: Eric Lloyd Wright is the grandchild of Frank Lloyd Wright""" ;
                           rdfs:isDefinedBy <http://vocab.getty.edu/ontology> ,
                                            ulan: ;
                           skos:example "Eric Lloyd Wright is the grandchild of Frank Lloyd Wright" ;
                           skos:prefLabel "ulan1513_grandchild_of" .


###  http://vocab.getty.edu/ontology#ulan1514_gandparent_of
gvp:ulan1514_gandparent_of rdf:type owl:ObjectProperty ;
                           rdfs:subPropertyOf skos:related ;
                           rdfs:domain skos:Concept ;
                           rdfs:range skos:Concept ;
                           dc:identifier "1514" ;
                           dc:title "gandparent of - person" ;
                           dct:description """person - gandparent of - person.
Example: Frank Lloyd Wright is the grandparent of Eric Lloyd Wright""" ;
                           rdfs:isDefinedBy <http://vocab.getty.edu/ontology> ,
                                            ulan: ;
                           skos:example "Frank Lloyd Wright is the grandparent of Eric Lloyd Wright" ;
                           skos:prefLabel "ulan1514_gandparent_of" .


###  http://vocab.getty.edu/ontology#ulan1515_great-grandparent_of
gvp:ulan1515_great-grandparent_of rdf:type owl:ObjectProperty ;
                                  rdfs:subPropertyOf skos:related ;
                                  owl:inverseOf gvp:ulan1516_great-grandchild_of ;
                                  rdfs:domain skos:Concept ;
                                  rdfs:range skos:Concept ;
                                  dc:identifier "1515" ;
                                  dc:title "great-grandparent of - person" ;
                                  dct:description """person - great-grandparent of - person.
Example: Albrecht Adam is the great-grandparent of Richard Benno Adam""" ;
                                  rdfs:isDefinedBy <http://vocab.getty.edu/ontology> ,
                                                   ulan: ;
                                  skos:example "Albrecht Adam is the great-grandparent of Richard Benno Adam" ;
                                  skos:prefLabel "ulan1515_great-grandparent_of" .


###  http://vocab.getty.edu/ontology#ulan1516_great-grandchild_of
gvp:ulan1516_great-grandchild_of rdf:type owl:ObjectProperty ;
                                 rdfs:subPropertyOf skos:related ;
                                 rdfs:domain skos:Concept ;
                                 rdfs:range skos:Concept ;
                                 dc:identifier "1516" ;
                                 dc:title "great-grandchild of - person" ;
                                 dct:description """person - great-grandchild of - person.
Example: Richard Benno Adam is the great-grandchild of Albrecht Adam""" ;
                                 rdfs:isDefinedBy <http://vocab.getty.edu/ontology> ,
                                                  ulan: ;
                                 skos:example "Richard Benno Adam is the great-grandchild of Albrecht Adam" ;
                                 skos:prefLabel "ulan1516_great-grandchild_of" .


###  http://vocab.getty.edu/ontology#ulan1521_cousin_of
gvp:ulan1521_cousin_of rdf:type owl:ObjectProperty ;
                       rdfs:subPropertyOf skos:related ;
                       rdf:type owl:SymmetricProperty ;
                       rdfs:domain skos:Concept ;
                       rdfs:range skos:Concept ;
                       dc:identifier "1521" ;
                       dc:title "cousin of - person" ;
                       dct:description """person - cousin of - person.
Example: Richard Meier and Frank Gehry are cousins""" ;
                       rdfs:isDefinedBy <http://vocab.getty.edu/ontology> ,
                                        ulan: ;
                       skos:example "Richard Meier and Frank Gehry are cousins" ;
                       skos:prefLabel "ulan1521_cousin_of" .


###  http://vocab.getty.edu/ontology#ulan1531_nephew-niece_of
gvp:ulan1531_nephew-niece_of rdf:type owl:ObjectProperty ;
                             rdfs:subPropertyOf skos:related ;
                             owl:inverseOf gvp:ulan1532_uncle-aunt_of ;
                             rdfs:domain skos:Concept ;
                             rdfs:range skos:Concept ;
                             dc:identifier "1531" ;
                             dc:title "nephew/niece of - person" ;
                             dct:description """person - nephew/niece of - person.
Example: Jan Brueghel, the elder is the nephew/neice of  Pieter Coecke van Aeist, the younger""" ;
                             rdfs:isDefinedBy <http://vocab.getty.edu/ontology> ,
                                              ulan: ;
                             skos:example "Jan Brueghel, the elder is the nephew/neice of  Pieter Coecke van Aeist, the younger" ;
                             skos:prefLabel "ulan1531_nephew-niece_of" .


###  http://vocab.getty.edu/ontology#ulan1532_uncle-aunt_of
gvp:ulan1532_uncle-aunt_of rdf:type owl:ObjectProperty ;
                           rdfs:subPropertyOf skos:related ;
                           rdfs:domain skos:Concept ;
                           rdfs:range skos:Concept ;
                           dc:identifier "1532" ;
                           dc:title "uncle/aunt of - person" ;
                           dct:description """person - uncle/aunt of - person.
Example: Edouard Manet is the uncle/aunt of Julie Manet""" ;
                           rdfs:isDefinedBy <http://vocab.getty.edu/ontology> ,
                                            ulan: ;
                           skos:example "Edouard Manet is the uncle/aunt of Julie Manet" ;
                           skos:prefLabel "ulan1532_uncle-aunt_of" .


###  http://vocab.getty.edu/ontology#ulan1541_spouse_of
gvp:ulan1541_spouse_of rdf:type owl:ObjectProperty ;
                       rdfs:subPropertyOf skos:related ;
                       rdf:type owl:SymmetricProperty ;
                       rdfs:domain skos:Concept ;
                       rdfs:range skos:Concept ;
                       dc:identifier "1541" ;
                       dc:title "spouse of - person" ;
                       dct:description """person - spouse of - person.
Example: Alfred Stieglitz and Georgia O'Keeffe were married to each other""" ;
                       rdfs:isDefinedBy <http://vocab.getty.edu/ontology> ,
                                        ulan: ;
                       skos:example "Alfred Stieglitz and Georgia O'Keeffe were married to each other" ;
                       skos:prefLabel "ulan1541_spouse_of" .


###  http://vocab.getty.edu/ontology#ulan1542_consort_of
gvp:ulan1542_consort_of rdf:type owl:ObjectProperty ;
                        rdfs:subPropertyOf skos:related ;
                        owl:inverseOf gvp:ulan1543_consort_was ;
                        rdfs:domain skos:Concept ;
                        rdfs:range skos:Concept ;
                        dc:identifier "1542" ;
                        dc:title "consort of - person" ;
                        dct:description """person - consort of - person.
Example: Empress Livia was the consort of Augustus, Emperor of Rome""" ;
                        rdfs:isDefinedBy <http://vocab.getty.edu/ontology> ,
                                         ulan: ;
                        skos:example "Empress Livia was the consort of Augustus, Emperor of Rome" ;
                        skos:prefLabel "ulan1542_consort_of" .


###  http://vocab.getty.edu/ontology#ulan1543_consort_was
gvp:ulan1543_consort_was rdf:type owl:ObjectProperty ;
                         rdfs:subPropertyOf skos:related ;
                         rdfs:domain skos:Concept ;
                         rdfs:range skos:Concept ;
                         dc:identifier "1543" ;
                         dc:title "consort was - person" ;
                         dct:description """person - consort was - person.
Example: Augustus, Emperor of Rome's consort was Empress Livia""" ;
                         rdfs:isDefinedBy <http://vocab.getty.edu/ontology> ,
                                          ulan: ;
                         skos:example "Augustus, Emperor of Rome's consort was Empress Livia" ;
                         skos:prefLabel "ulan1543_consort_was" .


###  http://vocab.getty.edu/ontology#ulan1544_significant_other_of
gvp:ulan1544_significant_other_of rdf:type owl:ObjectProperty ;
                                  rdfs:subPropertyOf skos:related ;
                                  rdf:type owl:SymmetricProperty ;
                                  rdfs:domain skos:Concept ;
                                  rdfs:range skos:Concept ;
                                  dc:identifier "1544" ;
                                  dc:title "significant other of - person" ;
                                  dct:description """person - significant other of - person.
Example: Jeanne Hebuterne was the significant other of Amedeo Modigliani""" ;
                                  rdfs:isDefinedBy <http://vocab.getty.edu/ontology> ,
                                                   ulan: ;
                                  skos:example "Jeanne Hebuterne was the significant other of Amedeo Modigliani" ;
                                  skos:prefLabel "ulan1544_significant_other_of" .


###  http://vocab.getty.edu/ontology#ulan1547_romantic_partner_of
gvp:ulan1547_romantic_partner_of rdf:type owl:ObjectProperty ;
                                 rdfs:subPropertyOf skos:related ;
                                 rdf:type owl:SymmetricProperty ;
                                 rdfs:domain skos:Concept ;
                                 rdfs:range skos:Concept ;
                                 dc:identifier "1547" ;
                                 dc:title "romantic partner of - person" ;
                                 dct:description """person - romantic partner of - person.
Example: Pablo Picasso and Gaby Lespinasse were romantic partners; Vincent van Gogh and Clasina Hoornik were romantic partners""" ;
                                 rdfs:isDefinedBy <http://vocab.getty.edu/ontology> ,
                                                  ulan: ;
                                 skos:example "Pablo Picasso and Gaby Lespinasse were romantic partners" ,
                                              "Vincent van Gogh and Clasina Hoornik were romantic partners" ;
                                 skos:prefLabel "ulan1547_romantic_partner_of" .


###  http://vocab.getty.edu/ontology#ulan1548_domestic_partner_of
gvp:ulan1548_domestic_partner_of rdf:type owl:ObjectProperty ;
                                 rdfs:subPropertyOf skos:related ;
                                 rdf:type owl:SymmetricProperty ;
                                 rdfs:domain skos:Concept ;
                                 rdfs:range skos:Concept ;
                                 dc:identifier "1548" ;
                                 dc:title "domestic partner of - person" ;
                                 dct:description "person - domestic partner of - person" ;
                                 rdfs:isDefinedBy <http://vocab.getty.edu/ontology> ,
                                                  ulan: ;
                                 skos:prefLabel "ulan1548_domestic_partner_of" .


###  http://vocab.getty.edu/ontology#ulan1550_relative_by_marriage
gvp:ulan1550_relative_by_marriage rdf:type owl:ObjectProperty ;
                                  rdfs:subPropertyOf skos:related ;
                                  rdf:type owl:SymmetricProperty ;
                                  rdfs:domain skos:Concept ;
                                  rdfs:range skos:Concept ;
                                  dc:identifier "1550" ;
                                  dc:title "relative by marriage - person" ;
                                  dct:description """person - relative by marriage (in-law) - person.
Example: Juana Galarza d Goicoechea and Francisco de Goya are related by marriage""" ;
                                  rdfs:isDefinedBy <http://vocab.getty.edu/ontology> ,
                                                   ulan: ;
                                  skos:example "Juana Galarza d Goicoechea and Francisco de Goya are related by marriage" ;
                                  skos:prefLabel "ulan1550_relative_by_marriage" .


###  http://vocab.getty.edu/ontology#ulan1551_sibling_by_marriage_of
gvp:ulan1551_sibling_by_marriage_of rdf:type owl:ObjectProperty ;
                                    rdfs:subPropertyOf skos:related ;
                                    rdf:type owl:SymmetricProperty ;
                                    rdfs:domain skos:Concept ;
                                    rdfs:range skos:Concept ;
                                    dc:identifier "1551" ;
                                    dc:title "sibling by marriage of - person" ;
                                    dct:description """person - sibling by marriage (step sibling) - person.
Example: Peter Paul Rubens and Susanne Fourment are siblings by marriage""" ;
                                    rdfs:isDefinedBy <http://vocab.getty.edu/ontology> ,
                                                     ulan: ;
                                    skos:example "Peter Paul Rubens and Susanne Fourment are siblings by marriage" ;
                                    skos:prefLabel "ulan1551_sibling_by_marriage_of" .


###  http://vocab.getty.edu/ontology#ulan1552_parent_by_marriage_of
gvp:ulan1552_parent_by_marriage_of rdf:type owl:ObjectProperty ;
                                   rdfs:subPropertyOf skos:related ;
                                   owl:inverseOf gvp:ulan1553_child_by_marriage_of ;
                                   rdfs:domain skos:Concept ;
                                   rdfs:range skos:Concept ;
                                   dc:identifier "1552" ;
                                   dc:title "parent by marriage of - person" ;
                                   dct:description """person - parent by marriage (step parent) - person.
Example: Frans Hals is a parent by marriage of Pieter Gerritsz van Roestraten""" ;
                                   rdfs:isDefinedBy <http://vocab.getty.edu/ontology> ,
                                                    ulan: ;
                                   skos:example "Frans Hals is a parent by marriage of Pieter Gerritsz van Roestraten" ;
                                   skos:prefLabel "ulan1552_parent_by_marriage_of" .


###  http://vocab.getty.edu/ontology#ulan1553_child_by_marriage_of
gvp:ulan1553_child_by_marriage_of rdf:type owl:ObjectProperty ;
                                  rdfs:subPropertyOf skos:related ;
                                  rdfs:domain skos:Concept ;
                                  rdfs:range skos:Concept ;
                                  dc:identifier "1553" ;
                                  dc:title "child by marriage of - person" ;
                                  dct:description """person - child by marriage (step child) - person.
Example: Pieter Gerritsz van Roestraten is the child by marriage of Frans Hals""" ;
                                  rdfs:isDefinedBy <http://vocab.getty.edu/ontology> ,
                                                   ulan: ;
                                  skos:example "Pieter Gerritsz van Roestraten is the child by marriage of Frans Hals" ;
                                  skos:prefLabel "ulan1553_child_by_marriage_of" .


###  http://vocab.getty.edu/ontology#ulan1554_adoptive_parent_of
gvp:ulan1554_adoptive_parent_of rdf:type owl:ObjectProperty ;
                                rdfs:subPropertyOf skos:related ;
                                owl:inverseOf gvp:ulan1555_adopted_child_of ;
                                rdfs:domain skos:Concept ;
                                rdfs:range skos:Concept ;
                                dc:identifier "1554" ;
                                dc:title "adoptive parent of - person" ;
                                dct:description """person - adoptive parent of - person.
Example: Julius Caesar is the adoptive parent of Augustus, Emperor of Rome""" ;
                                rdfs:isDefinedBy <http://vocab.getty.edu/ontology> ,
                                                 ulan: ;
                                skos:example "Julius Caesar is the adoptive parent of Augustus, Emperor of Rome" ;
                                skos:prefLabel "ulan1554_adoptive_parent_of" .


###  http://vocab.getty.edu/ontology#ulan1555_adopted_child_of
gvp:ulan1555_adopted_child_of rdf:type owl:ObjectProperty ;
                              rdfs:subPropertyOf skos:related ;
                              rdfs:domain skos:Concept ;
                              rdfs:range skos:Concept ;
                              dc:identifier "1555" ;
                              dc:title "adopted child of - person" ;
                              dct:description """person - adopted child of - person.
Example: Augusts, Emperor of Rome is the adopted child of Julius Caesar""" ;
                              rdfs:isDefinedBy <http://vocab.getty.edu/ontology> ,
                                               ulan: ;
                              skos:example "Augusts, Emperor of Rome is the adopted child of Julius Caesar" ;
                              skos:prefLabel "ulan1555_adopted_child_of" .


###  http://vocab.getty.edu/ontology#ulan1556_half-sibling_of
gvp:ulan1556_half-sibling_of rdf:type owl:ObjectProperty ;
                             rdfs:subPropertyOf skos:related ;
                             rdf:type owl:SymmetricProperty ;
                             rdfs:domain skos:Concept ;
                             rdfs:range skos:Concept ;
                             dc:identifier "1556" ;
                             dc:title "half-sibling of - person" ;
                             dct:description """person - half-sibling of - person.
Example: Juan Bautista Monegro and Luis de Carbajal are half siblings""" ;
                             rdfs:isDefinedBy <http://vocab.getty.edu/ontology> ,
                                              ulan: ;
                             skos:example "Juan Bautista Monegro and Luis de Carbajal are half siblings" ;
                             skos:prefLabel "ulan1556_half-sibling_of" .


###  http://vocab.getty.edu/ontology#ulan1557_step-sibling_of
gvp:ulan1557_step-sibling_of rdf:type owl:ObjectProperty ;
                             rdfs:subPropertyOf skos:related ;
                             rdf:type owl:SymmetricProperty ;
                             rdfs:domain skos:Concept ;
                             rdfs:range skos:Concept ;
                             dc:identifier "1557" ;
                             dc:title "step-sibling of - person" ;
                             dct:description """person - step-sibling of - person.
Example: W. L. Wyllie and Lionel Percy Smythe are step-siblings""" ;
                             rdfs:isDefinedBy <http://vocab.getty.edu/ontology> ,
                                              ulan: ;
                             skos:example "W. L. Wyllie and Lionel Percy Smythe are step-siblings" ;
                             skos:prefLabel "ulan1557_step-sibling_of" .


###  http://vocab.getty.edu/ontology#ulan1561_step-child_of
gvp:ulan1561_step-child_of rdf:type owl:ObjectProperty ;
                           rdfs:subPropertyOf skos:related ;
                           owl:inverseOf gvp:ulan1562_step-parent_of ;
                           rdfs:domain skos:Concept ;
                           rdfs:range skos:Concept ;
                           dc:identifier "1561" ;
                           dc:title "step-child of - person" ;
                           dct:description """person - step-child of - person.
Example: Hortense, Quene consort of Louis Bonaparte is the step-child of Napoleon I, Emperor of the French""" ;
                           rdfs:isDefinedBy <http://vocab.getty.edu/ontology> ,
                                            ulan: ;
                           skos:example "Hortense, Quene consort of Louis Bonaparte is the step-child of Napoleon I, Emperor of the French" ;
                           skos:prefLabel "ulan1561_step-child_of" .


###  http://vocab.getty.edu/ontology#ulan1562_step-parent_of
gvp:ulan1562_step-parent_of rdf:type owl:ObjectProperty ;
                            rdfs:subPropertyOf skos:related ;
                            rdfs:domain skos:Concept ;
                            rdfs:range skos:Concept ;
                            dc:identifier "1562" ;
                            dc:title "step-parent of - person" ;
                            dct:description """person - step-parent of - person.
Example: Napoleon I, Emperor of the French is the step-parent of Hortense, Quene consort of Louis Bonaparte""" ;
                            rdfs:isDefinedBy <http://vocab.getty.edu/ontology> ,
                                             ulan: ;
                            skos:example "Napoleon I, Emperor of the French is the step-parent of Hortense, Quene consort of Louis Bonaparte" ;
                            skos:prefLabel "ulan1562_step-parent_of" .


###  http://vocab.getty.edu/ontology#ulan1571_guardian_of
gvp:ulan1571_guardian_of rdf:type owl:ObjectProperty ;
                         rdfs:subPropertyOf skos:related ;
                         owl:inverseOf gvp:ulan1573_ward_of ;
                         rdfs:domain skos:Concept ;
                         rdfs:range skos:Concept ;
                         dc:identifier "1571" ;
                         dc:title "guardian of - person" ;
                         dct:description """person - guardian of - person.
Example: John Hoskins, the elder was the guardian of Samuel Cooper""" ;
                         rdfs:isDefinedBy <http://vocab.getty.edu/ontology> ,
                                          ulan: ;
                         skos:example "John Hoskins, the elder was the guardian of Samuel Cooper" ;
                         skos:prefLabel "ulan1571_guardian_of" .


###  http://vocab.getty.edu/ontology#ulan1573_ward_of
gvp:ulan1573_ward_of rdf:type owl:ObjectProperty ;
                     rdfs:subPropertyOf skos:related ;
                     rdfs:domain skos:Concept ;
                     rdfs:range skos:Concept ;
                     dc:identifier "1573" ;
                     dc:title "ward of - person" ;
                     dct:description """person - ward of - person.
Example: Samuel Cooper was a ward of John Hoskins, the elder""" ;
                     rdfs:isDefinedBy <http://vocab.getty.edu/ontology> ,
                                      ulan: ;
                     skos:example "Samuel Cooper was a ward of John Hoskins, the elder" ;
                     skos:prefLabel "ulan1573_ward_of" .


###  http://vocab.getty.edu/ontology#ulan1574_godparent_of
gvp:ulan1574_godparent_of rdf:type owl:ObjectProperty ;
                          rdfs:subPropertyOf skos:related ;
                          owl:inverseOf gvp:ulan1575_godchild_of ;
                          rdfs:domain skos:Concept ;
                          rdfs:range skos:Concept ;
                          dc:identifier "1574" ;
                          dc:title "godparent of - person" ;
                          dct:description """person - godparent of - person.
Example: Jean-Baptiste Goy is godparent of Jean I Nocret""" ;
                          rdfs:isDefinedBy <http://vocab.getty.edu/ontology> ,
                                           ulan: ;
                          skos:example "Jean-Baptiste Goy is godparent of Jean I Nocret" ;
                          skos:prefLabel "ulan1574_godparent_of" .


###  http://vocab.getty.edu/ontology#ulan1575_godchild_of
gvp:ulan1575_godchild_of rdf:type owl:ObjectProperty ;
                         rdfs:subPropertyOf skos:related ;
                         rdfs:domain skos:Concept ;
                         rdfs:range skos:Concept ;
                         dc:identifier "1575" ;
                         dc:title "godchild of - person" ;
                         dct:description """person - godchild of - person.
Example: Jean I Nocret is the godchild of Jean-Baptiste Goy""" ;
                         rdfs:isDefinedBy <http://vocab.getty.edu/ontology> ,
                                          ulan: ;
                         skos:example "Jean I Nocret is the godchild of Jean-Baptiste Goy" ;
                         skos:prefLabel "ulan1575_godchild_of" .


###  http://vocab.getty.edu/ontology#ulan1581_descendant_of
gvp:ulan1581_descendant_of rdf:type owl:ObjectProperty ;
                           rdfs:subPropertyOf skos:related ;
                           owl:inverseOf gvp:ulan1582_ancestor_of ;
                           rdfs:domain skos:Concept ;
                           rdfs:range skos:Concept ;
                           dc:identifier "1581" ;
                           dc:title "descendant of - person" ;
                           dct:description """person - descendant of - person.
Example: Paolo Caliari is the descendant of Paolo Veronese""" ;
                           rdfs:isDefinedBy <http://vocab.getty.edu/ontology> ,
                                            ulan: ;
                           skos:example "Paolo Caliari is the descendant of Paolo Veronese" ;
                           skos:prefLabel "ulan1581_descendant_of" .


###  http://vocab.getty.edu/ontology#ulan1582_ancestor_of
gvp:ulan1582_ancestor_of rdf:type owl:ObjectProperty ;
                         rdfs:subPropertyOf skos:related ;
                         rdfs:domain skos:Concept ;
                         rdfs:range skos:Concept ;
                         dc:identifier "1582" ;
                         dc:title "ancestor of - person" ;
                         dct:description """person - ancestor of - person.
Example: Paolo Veronese is the ancestor of Paolo Caliari""" ;
                         rdfs:isDefinedBy <http://vocab.getty.edu/ontology> ,
                                          ulan: ;
                         skos:example "Paolo Veronese is the ancestor of Paolo Caliari" ;
                         skos:prefLabel "ulan1582_ancestor_of" .


###  http://vocab.getty.edu/ontology#ulan1590_possibly_related_to
gvp:ulan1590_possibly_related_to rdf:type owl:ObjectProperty ;
                                 rdfs:subPropertyOf skos:related ;
                                 rdf:type owl:SymmetricProperty ;
                                 rdfs:domain skos:Concept ;
                                 rdfs:range skos:Concept ;
                                 dc:identifier "1590" ;
                                 dc:title "possibly related to - person" ;
                                 dct:description """person - possibly related to (familial relationship) - person.
Example: A familial relationship between Ramon Destorrents, the younger and Ramon Destorrents, the elder is possible""" ;
                                 rdfs:isDefinedBy <http://vocab.getty.edu/ontology> ,
                                                  ulan: ;
                                 skos:example "A familial relationship between Ramon Destorrents, the younger and Ramon Destorrents, the elder is possible" ;
                                 skos:prefLabel "ulan1590_possibly_related_to" .


###  http://vocab.getty.edu/ontology#ulan2550_friend_of
gvp:ulan2550_friend_of rdf:type owl:ObjectProperty ;
                       rdfs:subPropertyOf skos:related ;
                       rdf:type owl:SymmetricProperty ;
                       rdfs:domain skos:Concept ;
                       rdfs:range skos:Concept ;
                       dc:identifier "2550" ;
                       dc:title "friend of - person" ;
                       dct:description """person - friend of (personal relationship) - person.
Example: Alfred Stieglitz and Frank Simon Herrmann were friends""" ;
                       rdfs:isDefinedBy <http://vocab.getty.edu/ontology> ,
                                        ulan: ;
                       skos:example "Alfred Stieglitz and Frank Simon Herrmann were friends" ;
                       skos:prefLabel "ulan2550_friend_of" .


###  http://vocab.getty.edu/ontology#ulan2572_founder_of
gvp:ulan2572_founder_of rdf:type owl:ObjectProperty ;
                        rdfs:subPropertyOf skos:related ;
                        owl:inverseOf gvp:ulan2573_founded_by ;
                        rdfs:domain skos:Concept ;
                        rdfs:range skos:Concept ;
                        dc:identifier "2572" ;
                        dc:title "founder of - institution" ;
                        dct:description """person - founder of - institution.
Example: Louis Comfort Tiffany was the founder of Tiffany Glass & Decorating Company""" ;
                        rdfs:isDefinedBy <http://vocab.getty.edu/ontology> ,
                                         ulan: ;
                        skos:example "Louis Comfort Tiffany was the founder of Tiffany Glass & Decorating Company" ;
                        skos:prefLabel "ulan2572_founder_of" .


###  http://vocab.getty.edu/ontology#ulan2573_founded_by
gvp:ulan2573_founded_by rdf:type owl:ObjectProperty ;
                        rdfs:subPropertyOf skos:related ;
                        rdfs:domain skos:Concept ;
                        rdfs:range skos:Concept ;
                        dc:identifier "2573" ;
                        dc:title "founded by - person" ;
                        dct:description """institution - founded by - person.
Example: Tiffany Glass & Decorating Company was founded by Louis Comfort Tiffany""" ;
                        rdfs:isDefinedBy <http://vocab.getty.edu/ontology> ,
                                         ulan: ;
                        skos:example "Tiffany Glass & Decorating Company was founded by Louis Comfort Tiffany" ;
                        skos:prefLabel "ulan2573_founded_by" .


###  http://vocab.getty.edu/ontology#ulan2574_director_of
gvp:ulan2574_director_of rdf:type owl:ObjectProperty ;
                         rdfs:subPropertyOf skos:related ;
                         owl:inverseOf gvp:ulan2575_directed_by ;
                         rdfs:domain skos:Concept ;
                         rdfs:range skos:Concept ;
                         dc:identifier "2574" ;
                         dc:title "director of - institution" ;
                         dct:description """person - director of - institution.
Example: Jean Jans I directed Gobelins Tapestry Manufactory""" ;
                         rdfs:isDefinedBy <http://vocab.getty.edu/ontology> ,
                                          ulan: ;
                         skos:example "Jean Jans I directed Gobelins Tapestry Manufactory" ;
                         skos:prefLabel "ulan2574_director_of" .


###  http://vocab.getty.edu/ontology#ulan2575_directed_by
gvp:ulan2575_directed_by rdf:type owl:ObjectProperty ;
                         rdfs:subPropertyOf skos:related ;
                         rdfs:domain skos:Concept ;
                         rdfs:range skos:Concept ;
                         dc:identifier "2575" ;
                         dc:title "directed by - person" ;
                         dct:description """institution - directed by - person.
Example: Gobelins Tapestry Manufactory was directed by Jean Jans I""" ;
                         rdfs:isDefinedBy <http://vocab.getty.edu/ontology> ,
                                          ulan: ;
                         skos:example "Gobelins Tapestry Manufactory was directed by Jean Jans I" ;
                         skos:prefLabel "ulan2575_directed_by" .


###  http://vocab.getty.edu/ontology#ulan2576_patron_of
gvp:ulan2576_patron_of rdf:type owl:ObjectProperty ;
                       rdfs:subPropertyOf skos:related ;
                       owl:inverseOf gvp:ulan2577_patron_was ;
                       rdfs:domain skos:Concept ;
                       rdfs:range skos:Concept ;
                       dc:identifier "2576" ;
                       dc:title "patron of - person" ;
                       dct:description """person - patron of - person.
Example: The patron of William Chambers was James Caulfiel, Earl of Charlemont""" ;
                       rdfs:isDefinedBy <http://vocab.getty.edu/ontology> ,
                                        ulan: ;
                       skos:example "The patron of William Chambers was James Caulfiel, Earl of Charlemont" ;
                       skos:prefLabel "ulan2576_patron_of" .


###  http://vocab.getty.edu/ontology#ulan2577_patron_was
gvp:ulan2577_patron_was rdf:type owl:ObjectProperty ;
                        rdfs:subPropertyOf skos:related ;
                        rdfs:domain skos:Concept ;
                        rdfs:range skos:Concept ;
                        dc:identifier "2577" ;
                        dc:title "patron was - person" ;
                        dct:description """person - patron was - person.
Example: James Caulfiel, Earl of Charlemont was the patron of William Chambers""" ;
                        rdfs:isDefinedBy <http://vocab.getty.edu/ontology> ,
                                         ulan: ;
                        skos:example "James Caulfiel, Earl of Charlemont was the patron of William Chambers" ;
                        skos:prefLabel "ulan2577_patron_was" .


###  http://vocab.getty.edu/ontology#ulan2578_trustee_of
gvp:ulan2578_trustee_of rdf:type owl:ObjectProperty ;
                        rdfs:subPropertyOf skos:related ;
                        owl:inverseOf gvp:ulan2579_trustee_was ;
                        rdfs:domain skos:Concept ;
                        rdfs:range skos:Concept ;
                        dc:identifier "2578" ;
                        dc:title "trustee of - institution" ;
                        dct:description """person - trustee of - institution.
Example: George Douglas Haig was a trustee of the National Galleries of Scotland""" ;
                        rdfs:isDefinedBy <http://vocab.getty.edu/ontology> ,
                                         ulan: ;
                        skos:example "George Douglas Haig was a trustee of the National Galleries of Scotland" ;
                        skos:prefLabel "ulan2578_trustee_of" .


###  http://vocab.getty.edu/ontology#ulan2579_trustee_was
gvp:ulan2579_trustee_was rdf:type owl:ObjectProperty ;
                         rdfs:subPropertyOf skos:related ;
                         rdfs:domain skos:Concept ;
                         rdfs:range skos:Concept ;
                         dc:identifier "2579" ;
                         dc:title "trustee was - person" ;
                         dct:description """institution - trustee was - person.
Example: National Galleries of Scotland trustee was George Douglas Haig""" ;
                         rdfs:isDefinedBy <http://vocab.getty.edu/ontology> ,
                                          ulan: ;
                         skos:example "National Galleries of Scotland trustee was George Douglas Haig" ;
                         skos:prefLabel "ulan2579_trustee_was" .


###  http://vocab.getty.edu/ontology#ulan2581_administrator_of
gvp:ulan2581_administrator_of rdf:type owl:ObjectProperty ;
                              rdfs:subPropertyOf skos:related ;
                              owl:inverseOf gvp:ulan2582_administered_by ;
                              rdfs:domain skos:Concept ;
                              rdfs:range skos:Concept ;
                              dc:identifier "2581" ;
                              dc:title "administrator of - institution" ;
                              dct:description """person - administrator of - institution.
Example: Georges Mathieu was the administrator of Societe nationale des chemins de fer Francais. Agence des gares""" ;
                              rdfs:isDefinedBy <http://vocab.getty.edu/ontology> ,
                                               ulan: ;
                              skos:example "Georges Mathieu was the administrator of Societe nationale des chemins de fer Francais. Agence des gares" ;
                              skos:prefLabel "ulan2581_administrator_of" .


###  http://vocab.getty.edu/ontology#ulan2582_administered_by
gvp:ulan2582_administered_by rdf:type owl:ObjectProperty ;
                             rdfs:subPropertyOf skos:related ;
                             rdfs:domain skos:Concept ;
                             rdfs:range skos:Concept ;
                             dc:identifier "2582" ;
                             dc:title "administered by - person" ;
                             dct:description """institution - administered by - person.
Example: Societe nationale des chemins de fer Francais. Agence des gares was administered by Georges Mathieu""" ;
                             rdfs:isDefinedBy <http://vocab.getty.edu/ontology> ,
                                              ulan: ;
                             skos:example "Societe nationale des chemins de fer Francais. Agence des gares was administered by Georges Mathieu" ;
                             skos:prefLabel "ulan2582_administered_by" .


###  http://vocab.getty.edu/ontology#ulan2583_chairman_of
gvp:ulan2583_chairman_of rdf:type owl:ObjectProperty ;
                         rdfs:subPropertyOf skos:related ;
                         owl:inverseOf gvp:ulan2584_chaired_by ;
                         rdfs:domain skos:Concept ;
                         rdfs:range skos:Concept ;
                         dc:identifier "2583" ;
                         dc:title "chairman of - institution" ;
                         dct:description "person - chairman of - institution" ;
                         rdfs:isDefinedBy <http://vocab.getty.edu/ontology> ,
                                          ulan: ;
                         skos:prefLabel "ulan2583_chairman_of" .


###  http://vocab.getty.edu/ontology#ulan2584_chaired_by
gvp:ulan2584_chaired_by rdf:type owl:ObjectProperty ;
                        rdfs:subPropertyOf skos:related ;
                        rdfs:domain skos:Concept ;
                        rdfs:range skos:Concept ;
                        dc:identifier "2584" ;
                        dc:title "chaired by - person" ;
                        dct:description "institution - chaired by - person" ;
                        rdfs:isDefinedBy <http://vocab.getty.edu/ontology> ,
                                         ulan: ;
                        skos:prefLabel "ulan2584_chaired_by" .


###  http://vocab.getty.edu/ontology#ulan2650_publisher_was
gvp:ulan2650_publisher_was rdf:type owl:ObjectProperty ;
                           rdfs:subPropertyOf skos:related ;
                           owl:inverseOf gvp:ulan2651_publisher_of ;
                           rdfs:domain skos:Concept ;
                           rdfs:range skos:Concept ;
                           dc:identifier "2650" ;
                           dc:title "publisher was - firm" ;
                           dct:description """person - publisher was - firm.
Example: The publisher for Pierre Joseph Rossier was Negretti and Zambra""" ;
                           rdfs:isDefinedBy <http://vocab.getty.edu/ontology> ,
                                            ulan: ;
                           skos:example "The publisher for Pierre Joseph Rossier was Negretti and Zambra" ;
                           skos:prefLabel "ulan2650_publisher_was" .


###  http://vocab.getty.edu/ontology#ulan2651_publisher_of
gvp:ulan2651_publisher_of rdf:type owl:ObjectProperty ;
                          rdfs:subPropertyOf skos:related ;
                          rdfs:domain skos:Concept ;
                          rdfs:range skos:Concept ;
                          dc:identifier "2651" ;
                          dc:title "publisher of - person" ;
                          dct:description """firm - publisher of - person.
Example: Negretti and Zambra was the publisher of Pierre Joseph Rossier""" ;
                          rdfs:isDefinedBy <http://vocab.getty.edu/ontology> ,
                                           ulan: ;
                          skos:example "Negretti and Zambra was the publisher of Pierre Joseph Rossier" ;
                          skos:prefLabel "ulan2651_publisher_of" .


###  http://vocab.getty.edu/ontology#ulan2674_professor_at
gvp:ulan2674_professor_at rdf:type owl:ObjectProperty ;
                          rdfs:subPropertyOf skos:related ;
                          owl:inverseOf gvp:ulan2675_professor_was ;
                          rdfs:domain skos:Concept ;
                          rdfs:range skos:Concept ;
                          dc:identifier "2674" ;
                          dc:title "professor at - institution" ;
                          dct:description """person - professor at - institution.
Example: Paul Klee was a professor at Bauhaus""" ;
                          rdfs:isDefinedBy <http://vocab.getty.edu/ontology> ,
                                           ulan: ;
                          skos:example "Paul Klee was a professor at Bauhaus" ;
                          skos:prefLabel "ulan2674_professor_at" .


###  http://vocab.getty.edu/ontology#ulan2675_professor_was
gvp:ulan2675_professor_was rdf:type owl:ObjectProperty ;
                           rdfs:subPropertyOf skos:related ;
                           rdfs:domain skos:Concept ;
                           rdfs:range skos:Concept ;
                           dc:identifier "2675" ;
                           dc:title "professor was - person" ;
                           dct:description """institution - professor was - person.
Example: A professor at Bauhaus was Paul Klee""" ;
                           rdfs:isDefinedBy <http://vocab.getty.edu/ontology> ,
                                            ulan: ;
                           skos:example "A professor at Bauhaus was Paul Klee" ;
                           skos:prefLabel "ulan2675_professor_was" .


###  http://vocab.getty.edu/ontology#ulan2676_teacher_at
gvp:ulan2676_teacher_at rdf:type owl:ObjectProperty ;
                        rdfs:subPropertyOf skos:related ;
                        owl:inverseOf gvp:ulan2677_teacher_was ;
                        rdfs:domain skos:Concept ;
                        rdfs:range skos:Concept ;
                        dc:identifier "2676" ;
                        dc:title "teacher at - institution" ;
                        dct:description """person - teacher at - institution.
Example: Willem De Kooning was a teacher at Black Mountain College""" ;
                        rdfs:isDefinedBy <http://vocab.getty.edu/ontology> ,
                                         ulan: ;
                        skos:example "Willem De Kooning was a teacher at Black Mountain College" ;
                        skos:prefLabel "ulan2676_teacher_at" .


###  http://vocab.getty.edu/ontology#ulan2677_teacher_was
gvp:ulan2677_teacher_was rdf:type owl:ObjectProperty ;
                         rdfs:subPropertyOf skos:related ;
                         rdfs:domain skos:Concept ;
                         rdfs:range skos:Concept ;
                         dc:identifier "2677" ;
                         dc:title "teacher was - person" ;
                         dct:description """institution - teacher was - person.
Example: A teacher at Black Mountain College was Willem De Kooning""" ;
                         rdfs:isDefinedBy <http://vocab.getty.edu/ontology> ,
                                          ulan: ;
                         skos:example "A teacher at Black Mountain College was Willem De Kooning" ;
                         skos:prefLabel "ulan2677_teacher_was" .


###  http://vocab.getty.edu/ontology#ulan2692_president_of
gvp:ulan2692_president_of rdf:type owl:ObjectProperty ;
                          rdfs:subPropertyOf skos:related ;
                          owl:inverseOf gvp:ulan2693_president_was ;
                          rdfs:domain skos:Concept ;
                          rdfs:range skos:Concept ;
                          dc:identifier "2692" ;
                          dc:title "president of - institution" ;
                          dct:description """person - president of - institution.
Example: David K. E. Bruce was president of National Gallery of Art""" ;
                          rdfs:isDefinedBy <http://vocab.getty.edu/ontology> ,
                                           ulan: ;
                          skos:example "David K. E. Bruce was president of National Gallery of Art" ;
                          skos:prefLabel "ulan2692_president_of" .


###  http://vocab.getty.edu/ontology#ulan2693_president_was
gvp:ulan2693_president_was rdf:type owl:ObjectProperty ;
                           rdfs:subPropertyOf skos:related ;
                           rdfs:domain skos:Concept ;
                           rdfs:range skos:Concept ;
                           dc:identifier "2693" ;
                           dc:title "president was - person" ;
                           dct:description """institution - president was - person.
Example: A president of National Gallery of Art was David K. E. Bruce""" ;
                           rdfs:isDefinedBy <http://vocab.getty.edu/ontology> ,
                                            ulan: ;
                           skos:example "A president of National Gallery of Art was David K. E. Bruce" ;
                           skos:prefLabel "ulan2693_president_was" .


###  http://vocab.getty.edu/ontology#ulan2696_leader_of
gvp:ulan2696_leader_of rdf:type owl:ObjectProperty ;
                       rdfs:subPropertyOf skos:related ;
                       owl:inverseOf gvp:ulan2697_leader_was ;
                       rdfs:domain skos:Concept ;
                       rdfs:range skos:Concept ;
                       dc:identifier "2696" ;
                       dc:title "leader of - institution" ;
                       dct:description """person - leader of - institution.
Example: Rush Harrison Kress was the leader of Samuel H. Kress Foundation""" ;
                       rdfs:isDefinedBy <http://vocab.getty.edu/ontology> ,
                                        ulan: ;
                       skos:example "Rush Harrison Kress was the leader of Samuel H. Kress Foundation" ;
                       skos:prefLabel "ulan2696_leader_of" .


###  http://vocab.getty.edu/ontology#ulan2697_leader_was
gvp:ulan2697_leader_was rdf:type owl:ObjectProperty ;
                        rdfs:subPropertyOf skos:related ;
                        rdfs:domain skos:Concept ;
                        rdfs:range skos:Concept ;
                        dc:identifier "2697" ;
                        dc:title "leader was - person" ;
                        dct:description """institution - leader was - person.
Example: The leader of Samuel H. Kress Foundation was Rush Harrison Kress""" ;
                        rdfs:isDefinedBy <http://vocab.getty.edu/ontology> ,
                                         ulan: ;
                        skos:example "The leader of Samuel H. Kress Foundation was Rush Harrison Kress" ;
                        skos:prefLabel "ulan2697_leader_was" .


###  http://vocab.getty.edu/ontology#ulan2778_owner_of
gvp:ulan2778_owner_of rdf:type owl:ObjectProperty ;
                      rdfs:subPropertyOf skos:related ;
                      owl:inverseOf gvp:ulan2779_owned_by ;
                      rdfs:domain skos:Concept ;
                      rdfs:range skos:Concept ;
                      dc:identifier "2778" ;
                      dc:title "owner of - person" ;
                      dct:description """firm - owner of - person.
Example: Walter Scott Lenox was the owner of Lenox China Co.""" ;
                      rdfs:isDefinedBy <http://vocab.getty.edu/ontology> ,
                                       ulan: ;
                      skos:example "Walter Scott Lenox was the owner of Lenox China Co." ;
                      skos:prefLabel "ulan2778_owner_of" .


###  http://vocab.getty.edu/ontology#ulan2779_owned_by
gvp:ulan2779_owned_by rdf:type owl:ObjectProperty ;
                      rdfs:subPropertyOf skos:related ;
                      rdfs:domain skos:Concept ;
                      rdfs:range skos:Concept ;
                      dc:identifier "2779" ;
                      dc:title "owned by - firm" ;
                      dct:description """person - owned by - firm.
Example: Walter Scott Lenox was owned by Lenox China Co.""" ;
                      rdfs:isDefinedBy <http://vocab.getty.edu/ontology> ,
                                       ulan: ;
                      skos:example "Walter Scott Lenox was owned by Lenox China Co." ;
                      skos:prefLabel "ulan2779_owned_by" .


###  http://vocab.getty.edu/ontology#ulan2781_dedicatee_of
gvp:ulan2781_dedicatee_of rdf:type owl:ObjectProperty ;
                          rdfs:subPropertyOf skos:related ;
                          owl:inverseOf gvp:ulan2782_dedicated_to ;
                          rdfs:domain skos:Concept ;
                          rdfs:range skos:Concept ;
                          dc:identifier "2781" ;
                          dc:title "dedicatee of - institution" ;
                          dct:description """person - dedicatee of - institution.
Example: Auguste Rodin is the dedicatee of The Rodin Museum in Philadelphia""" ;
                          rdfs:isDefinedBy <http://vocab.getty.edu/ontology> ,
                                           ulan: ;
                          skos:example "Auguste Rodin is the dedicatee of The Rodin Museum in Philadelphia" ;
                          skos:prefLabel "ulan2781_dedicatee_of" .


###  http://vocab.getty.edu/ontology#ulan2782_dedicated_to
gvp:ulan2782_dedicated_to rdf:type owl:ObjectProperty ;
                          rdfs:subPropertyOf skos:related ;
                          rdfs:domain skos:Concept ;
                          rdfs:range skos:Concept ;
                          dc:identifier "2782" ;
                          dc:title "dedicated to - person" ;
                          dct:description """institution - dedicated to - person.
Example: The Rodin Museum in Philadelphia is didicated to Auguste Rodin""" ;
                          rdfs:isDefinedBy <http://vocab.getty.edu/ontology> ,
                                           ulan: ;
                          skos:example "The Rodin Museum in Philadelphia is didicated to Auguste Rodin" ;
                          skos:prefLabel "ulan2782_dedicated_to" .


###  http://vocab.getty.edu/ontology#ulan2794_representative_of
gvp:ulan2794_representative_of rdf:type owl:ObjectProperty ;
                               rdfs:subPropertyOf skos:related ;
                               owl:inverseOf gvp:ulan2795_representative_was ;
                               rdfs:domain skos:Concept ;
                               rdfs:range skos:Concept ;
                               dc:identifier "2794" ;
                               dc:title "representative of - institution" ;
                               dct:description """person - representative of - institution.
Example: The Noguch Museum - representative was Isamu Noguchi""" ;
                               rdfs:isDefinedBy <http://vocab.getty.edu/ontology> ,
                                                ulan: ;
                               skos:example "The Noguch Museum - representative was Isamu Noguchi" ;
                               skos:prefLabel "ulan2794_representative_of" .


###  http://vocab.getty.edu/ontology#ulan2795_representative_was
gvp:ulan2795_representative_was rdf:type owl:ObjectProperty ;
                                rdfs:subPropertyOf skos:related ;
                                rdfs:domain skos:Concept ;
                                rdfs:range skos:Concept ;
                                dc:identifier "2795" ;
                                dc:title "representative was - person" ;
                                dct:description """institution - representative was - person.
Example: The Noguch Museum - representative was Isamu Noguchi""" ;
                                rdfs:isDefinedBy <http://vocab.getty.edu/ontology> ,
                                                 ulan: ;
                                skos:example "The Noguch Museum - representative was Isamu Noguchi" ;
                                skos:prefLabel "ulan2795_representative_was" .


###  http://vocab.getty.edu/ontology#ulan2828_student_at
gvp:ulan2828_student_at rdf:type owl:ObjectProperty ;
                        rdfs:subPropertyOf skos:related ;
                        owl:inverseOf gvp:ulan2829_student_was ;
                        rdfs:domain skos:Concept ;
                        rdfs:range skos:Concept ;
                        dc:identifier "2828" ;
                        dc:title "student at - institution" ;
                        dct:description """person - student at - institution.
Example: Zdanek Rossman was a student at Bauhaus""" ;
                        rdfs:isDefinedBy <http://vocab.getty.edu/ontology> ,
                                         ulan: ;
                        skos:example "Zdanek Rossman was a student at Bauhaus" ;
                        skos:prefLabel "ulan2828_student_at" .


###  http://vocab.getty.edu/ontology#ulan2829_student_was
gvp:ulan2829_student_was rdf:type owl:ObjectProperty ;
                         rdfs:subPropertyOf skos:related ;
                         rdfs:domain skos:Concept ;
                         rdfs:range skos:Concept ;
                         dc:identifier "2829" ;
                         dc:title "student was - person" ;
                         dct:description """institution - student was - person.
Example: Bauhaus student was Zdanek Rossman""" ;
                         rdfs:isDefinedBy <http://vocab.getty.edu/ontology> ,
                                          ulan: ;
                         skos:example "Bauhaus student was Zdanek Rossman" ;
                         skos:prefLabel "ulan2829_student_was" .


###  http://vocab.getty.edu/ontology#ulan2840_performer_with
gvp:ulan2840_performer_with rdf:type owl:ObjectProperty ;
                            rdfs:subPropertyOf skos:related ;
                            owl:inverseOf gvp:ulan2841_performer_was ;
                            rdfs:domain skos:Concept ;
                            rdfs:range skos:Concept ;
                            dc:identifier "2840" ;
                            dc:title "performer with - group" ;
                            dct:description "person - performer with - group" ;
                            rdfs:isDefinedBy <http://vocab.getty.edu/ontology> ,
                                             ulan: ;
                            skos:prefLabel "ulan2840_performer_with" .


###  http://vocab.getty.edu/ontology#ulan2841_performer_was
gvp:ulan2841_performer_was rdf:type owl:ObjectProperty ;
                           rdfs:subPropertyOf skos:related ;
                           rdfs:domain skos:Concept ;
                           rdfs:range skos:Concept ;
                           dc:identifier "2841" ;
                           dc:title "performer was - person" ;
                           dct:description "group - performer was - person" ;
                           rdfs:isDefinedBy <http://vocab.getty.edu/ontology> ,
                                            ulan: ;
                           skos:prefLabel "ulan2841_performer_was" .


###  http://www.w3.org/2004/02/skos/core#altLabel
skos:altLabel rdf:type owl:ObjectProperty ;
              owl:propertyChainAxiom ( skosxl:altLabel
                                       skosxl:literalForm
                                     ) .


###  http://www.w3.org/2004/02/skos/core#hiddenLabel
skos:hiddenLabel rdf:type owl:ObjectProperty ;
                 owl:propertyChainAxiom ( skosxl:hiddenLabel
                                          skosxl:literalForm
                                        ) .


###  http://www.w3.org/2004/02/skos/core#prefLabel
skos:prefLabel rdf:type owl:ObjectProperty ;
               owl:propertyChainAxiom ( skosxl:prefLabel
                                        skosxl:literalForm
                                      ) .


###  http://www.w3.org/2008/05/skos-xl#literalForm
skosxl:literalForm rdf:type owl:ObjectProperty .


#################################################################
#    Data properties
#################################################################

###  http://vocab.getty.edu/ontology#displayOrder
gvp:displayOrder rdf:type owl:DatatypeProperty ;
                 rdfs:range xsd:positiveInteger ;
                 dct:description """Display order of subject or term amongst its siblings.
If all are 1 then use alphabetical. Domain is gvp:Subject or skosxl:Label""" ;
                 rdfs:comment """Display order of subject or term amongst its siblings.
If all are 1 then use alphabetical. Domain is gvp:Subject or skosxl:Label""" ;
                 rdfs:isDefinedBy <http://vocab.getty.edu/ontology> ;
                 rdfs:label "displayOrder" .


###  http://vocab.getty.edu/ontology#estEnd
gvp:estEnd rdf:type owl:DatatypeProperty ;
           dct:description "Estimated end date of term, relation, type assignment, event, biography" ;
           rdfs:comment "Estimated end date of term, relation, type assignment, event, biography" ;
           rdfs:isDefinedBy <http://vocab.getty.edu/ontology> ;
           rdfs:label "estEnd" .


###  http://vocab.getty.edu/ontology#estStart
gvp:estStart rdf:type owl:DatatypeProperty ;
             dct:description "Estimated start date of term, relation, type assignment, event, biography" ;
             rdfs:comment "Estimated start date of term, relation, type assignment, event, biography" ;
             rdfs:isDefinedBy <http://vocab.getty.edu/ontology> ;
             rdfs:label "estStart" .


###  http://vocab.getty.edu/ontology#isNoted
gvp:isNoted rdf:type owl:DatatypeProperty ;
            rdfs:domain gvp:Subject ;
            rdfs:range xsd:boolean ;
            dct:description """One amongst several homographic concepts may be especially noted so it's easier to find.
Example: tgn:7008038 Paris, France is noted but tgn:2106600 Paris, Texas is not (except if you're Fassbinder)""" ;
            rdfs:comment "One amongst several homographic concepts may be especially noted so it's easier to find" ;
            rdfs:isDefinedBy <http://vocab.getty.edu/ontology> ;
            rdfs:label "isNoted" ;
            skos:example "tgn:7008038 Paris, France is noted but tgn:2106600 Paris, Texas is not (except if you're Fassbinder)" .


###  http://vocab.getty.edu/ontology#parentString
gvp:parentString rdf:type owl:DatatypeProperty .


###  http://vocab.getty.edu/ontology#parentStringAbbrev
gvp:parentStringAbbrev rdf:type owl:DatatypeProperty .


###  http://vocab.getty.edu/ontology#qualifier
gvp:qualifier rdf:type owl:DatatypeProperty .


###  http://vocab.getty.edu/ontology#term
gvp:term rdf:type owl:DatatypeProperty .


#################################################################
#    Classes
#################################################################

###  http://purl.org/ontology/bibo/Document
bibo:Document rdf:type owl:Class .


###  http://purl.org/vocab/bio/0.1/Event
bio:Event rdf:type owl:Class .


###  http://purl.org/vocommons/voaf#Vocabulary
voaf:Vocabulary rdf:type owl:Class .


###  http://schema.org/Organization
schema:Organization rdf:type owl:Class .


###  http://schema.org/Place
schema:Place rdf:type owl:Class .


###  http://vocab.getty.edu/ontology#AdminPlaceConcept
gvp:AdminPlaceConcept rdf:type owl:Class ;
                      rdfs:subClassOf gvp:Subject ,
                                      skos:Concept ;
                      dct:description """Place defined by administrative boundaries and conditions, including inhabited places, nations, and empires. Used in TGN only.
Example: Burgundy region in France (TGN)""" ;
                      rdfs:comment "Place defined by administrative boundaries and conditions, including inhabited places, nations, and empires. Used in TGN only" ;
                      rdfs:isDefinedBy <http://vocab.getty.edu/ontology> ;
                      rdfs:label "AdminPlaceConcept" ;
                      skos:example "Burgundy region in France (TGN)" .


###  http://vocab.getty.edu/ontology#Biography
gvp:Biography rdf:type owl:Class ;
              rdfs:comment """Biography of a ULAN agent (schema:Person|Organization). Depending on the agent, has these fields:
- schema:description: one-line-biography
- gvp:estStart
- schema:birthPlace | foundationLocation, pointing to TGN
- gvp:estEnd
- schema:deathPlace | dissolutionLocation, pointing to TGN
- schema:gender, pointing to AAT (male, female, other)
- dct:contributor
The fields of the preferred biogrpahy are also available in the agent.""" ;
              rdfs:isDefinedBy <http://vocab.getty.edu/ontology> .


###  http://vocab.getty.edu/ontology#Concept
gvp:Concept rdf:type owl:Class ;
            rdfs:subClassOf gvp:Subject ,
                            skos:Concept ;
            dct:description """Proper concept. Used in AAT only; TGN & ULAN have their own, e.g. gvp:PhysPlaceConcept & gvp:PersonConcept. Used for indexing and cataloguing.
Example: rhyta (AAT)""" ;
            rdfs:comment "Proper concept. Used in AAT only; TGN & ULAN have their own, e.g. gvp:PhysPlaceConcept & gvp:PersonConcept. Used for indexing and cataloguing" ;
            rdfs:isDefinedBy <http://vocab.getty.edu/ontology> ;
            rdfs:label "Concept" ;
            skos:example "rhyta (AAT)" .


###  http://vocab.getty.edu/ontology#Facet
gvp:Facet rdf:type owl:Class ;
          rdfs:subClassOf iso:ThesaurusArray ,
                          gvp:Subject ;
          dct:description """One of the major divisions of a vocabulary.
Example: Objects Facet (AAT), World (TGN), Artists (ULAN)""" ;
          rdfs:comment "One of the major divisions of a vocabulary" ;
          rdfs:isDefinedBy <http://vocab.getty.edu/ontology> ;
          rdfs:label "Facet" ;
          skos:example "Objects Facet (AAT), World (TGN), Artists (ULAN)" .


###  http://vocab.getty.edu/ontology#GroupConcept
gvp:GroupConcept rdf:type owl:Class ;
                 rdfs:subClassOf gvp:Subject ,
                                 skos:Concept ;
                 dct:description """Two or more people who generally worked together to collectively create art. Not necessarily legally incorporated. A family of artists may be considered a \"corporate body\". Corresponds to crm:E74_Group, not its subclass crm:E40_Legal_Body.
Example: 500356337 Albrecht Duerer Workshop (ULAN)""" ;
                 rdfs:comment "Two or more people who generally worked together to collectively create art. Not necessarily legally incorporated. A family of artists may be considered a \"corporate body\". Corresponds to crm:E74_Group, not its subclass crm:E40_Legal_Body" ;
                 rdfs:isDefinedBy <http://vocab.getty.edu/ontology> ;
                 rdfs:label "GroupConcept" ;
                 skos:example "500356337 Albrecht Duerer Workshop (ULAN)" .


###  http://vocab.getty.edu/ontology#GuideTerm
gvp:GuideTerm rdf:type owl:Class ;
              rdfs:subClassOf iso:ThesaurusArray ,
                              gvp:Subject ;
              dct:description """Guide Term: place holder to create a level in the hierarchy. Used in AAT and ULAN. Not used for indexing or cataloguing..
Example: <vessels for serving and consuming food> (AAT), ulan:500353455 <named animals> under facet Non-Artists (ULAN)""" ;
              rdfs:comment "Guide Term: place holder to create a level in the hierarchy. Used in AAT and ULAN. Not used for indexing or cataloguing." ;
              rdfs:isDefinedBy <http://vocab.getty.edu/ontology> ;
              rdfs:label "GuideTerm" ;
              skos:example "<vessels for serving and consuming food> (AAT), ulan:500353455 <named animals> under facet Non-Artists (ULAN)" .


###  http://vocab.getty.edu/ontology#Hierarchy
gvp:Hierarchy rdf:type owl:Class ;
              rdfs:subClassOf iso:ThesaurusArray ,
                              gvp:Subject ;
              dct:description """Top of a hierarchy. Used in AAT only. Not used for indexing or cataloguing.
Example: Containers (Hierarchy Name) (AAT)""" ;
              rdfs:comment "Top of a hierarchy. Used in AAT only. Not used for indexing or cataloguing" ;
              rdfs:isDefinedBy <http://vocab.getty.edu/ontology> ;
              rdfs:label "Hierarchy" ;
              skos:example "Containers (Hierarchy Name) (AAT)" .


###  http://vocab.getty.edu/ontology#ObsoleteSubject
gvp:ObsoleteSubject rdf:type owl:Class ;
                    rdfs:subClassOf gvp:Subject ;
                    dct:description """Obsolete subject: moved out of the publishable hierarchy, or merged to another (pointed by dct:isReplacedBy).
Example: 300375205 \"shranks\" (AAT) was merged to 300039264 \"schranks\" (AAT), so aat:300375205 dct:isReplacedBy aat:300039264""" ;
                    rdfs:comment "Obsolete subject: moved out of the publishable hierarchy, or merged to another (pointed by dct:isReplacedBy)" ;
                    rdfs:isDefinedBy <http://vocab.getty.edu/ontology> ;
                    rdfs:label "ObsoleteSubject" ;
                    skos:example "300375205 \"shranks\" (AAT) was merged to 300039264 \"schranks\" (AAT), so aat:300375205 dct:isReplacedBy aat:300039264" .


###  http://vocab.getty.edu/ontology#PersonConcept
gvp:PersonConcept rdf:type owl:Class ;
                  rdfs:subClassOf gvp:Subject ,
                                  skos:Concept ;
                  dct:description """A single individual. Usually people engaged in the design or creation of art or architecture (\"Artists\"); but may also include donors, patrons, rulers, sitters, art historians, etc (\"Non-Artists\").
Example: 500115493 Duerer, Albrecht (ULAN)""" ;
                  rdfs:comment "A single individual. Usually people engaged in the design or creation of art or architecture (\"Artists\"); but may also include donors, patrons, rulers, sitters, art historians, etc (\"Non-Artists\")" ;
                  rdfs:isDefinedBy <http://vocab.getty.edu/ontology> ;
                  rdfs:label "PersonConcept" ;
                  skos:example "500115493 Duerer, Albrecht (ULAN)" .


###  http://vocab.getty.edu/ontology#PhysAdminPlaceConcept
gvp:PhysAdminPlaceConcept rdf:type owl:Class ;
                          rdfs:subClassOf gvp:Subject ,
                                          skos:Concept ;
                          dct:description """Place that is both administrative and physical. Rarely used. Used in TGN only.
Example: 6003090 Kiik-Koba (TGN)""" ;
                          rdfs:comment "Place that is both administrative and physical. Rarely used. Used in TGN only" ;
                          rdfs:isDefinedBy <http://vocab.getty.edu/ontology> ;
                          rdfs:label "PhysAdminPlaceConcept" ;
                          skos:example "6003090 Kiik-Koba (TGN)" .


###  http://vocab.getty.edu/ontology#PhysPlaceConcept
gvp:PhysPlaceConcept rdf:type owl:Class ;
                     rdfs:subClassOf gvp:Subject ,
                                     skos:Concept ;
                     dct:description """Physical feature, defined by its physical characteristics on planet Earth, including mountains, rivers, and oceans. Used in TGN only.
Example: Amazon River (TGN)""" ;
                     rdfs:comment "Physical feature, defined by its physical characteristics on planet Earth, including mountains, rivers, and oceans. Used in TGN only" ;
                     rdfs:isDefinedBy <http://vocab.getty.edu/ontology> ;
                     rdfs:label "PhysPlaceConcept" ;
                     skos:example "Amazon River (TGN)" .


###  http://vocab.getty.edu/ontology#ScopeNote
gvp:ScopeNote rdf:type owl:Class ;
              dct:description """Defines a GVP subject or provides usage information. Has fields:
- dc:identifier: numeric ID, also used in the URL.
- rdf:value: the note itself (as per SKOS Primer: 4.2 Advanced Documentation Features) with language tag
- dct:language: matches the language tag
- gvp:displayOrder, order of this note amongst others
- gvp:historicFlag, vp:estStart, gvp:estEnd, rdfs:comment: Historic Information about applicability
- dct:source or subproperties thereof 
- dct:contributor or subproperties thereof""" ;
              rdfs:comment """Defines a GVP subject or provides usage information. Has fields:
- dc:identifier: numeric ID, also used in the URL.
- rdf:value: the note itself (as per SKOS Primer: 4.2 Advanced Documentation Features) with language tag
- dct:language: matches the language tag
- gvp:displayOrder, order of this note amongst others
- gvp:historicFlag, gvp:estStart, gvp:estEnd, rdfs:comment: Historic Information about applicability
- dct:source or subproperties thereof 
- dct:contributor or subproperties thereof""" ;
              rdfs:isDefinedBy <http://vocab.getty.edu/ontology> .


###  http://vocab.getty.edu/ontology#Subject
gvp:Subject rdf:type owl:Class ;
            dct:description """Node in a GVP vocabulary hierarchy. 
May be Facet, GuideTerm, Hierarchy, Concept, AdminPlaceConcept, PhysPlaceConcept, PhysAdminPlaceConcept, or ObsoleteSubject.
Implemented as skos:Concept or iso:ThesaurusArray and skos:Collection""" ;
            rdfs:comment """Node in a GVP vocabulary hierarchy. 
May be Facet, GuideTerm, Hierarchy, Concept, AdminPlaceConcept, PhysPlaceConcept, PhysAdminPlaceConcept, or ObsoleteSubject.
Implemented as skos:Concept or iso:ThesaurusArray and skos:Collection""" ;
            rdfs:isDefinedBy <http://vocab.getty.edu/ontology> ;
            rdfs:label "Subject" .


###  http://vocab.getty.edu/ontology#UnknownPersonConcept
gvp:UnknownPersonConcept rdf:type owl:Class ;
                         rdfs:subClassOf gvp:Subject ,
                                         skos:Concept ;
                         dct:description """Unknown person representing a nationality/culture (the Unknown People by Culture facet).
Example: 500355202 Unknown Bulgarian (modern) (ULAN)""" ;
                         rdfs:comment "Unknown person representing a nationality/culture (the Unknown People by Culture facet)" ;
                         rdfs:isDefinedBy <http://vocab.getty.edu/ontology> ;
                         rdfs:label "UnknownPersonConcept" ;
                         skos:example "500355202 Unknown Bulgarian (modern) (ULAN)" .


###  http://www.ontotext.com/proton/protontop#PropChainRestr
ptop:PropChainRestr rdf:type owl:Class .


###  http://www.ontotext.com/proton/protontop#PropChainType2
ptop:PropChainType2 rdf:type owl:Class .


###  http://www.ontotext.com/proton/protontop#PropRestr
ptop:PropRestr rdf:type owl:Class .


###  http://www.ontotext.com/proton/protontop#TypeRestr
ptop:TypeRestr rdf:type owl:Class .


###  http://www.w3.org/1999/02/22-rdf-syntax-ns#Literal
rdf:Literal rdf:type owl:Class .


###  http://xmlns.com/foaf/0.1/Agent
foaf:Agent rdf:type owl:Class .


###  http://xmlns.com/foaf/0.1/Organization
foaf:Organization rdf:type owl:Class .


#################################################################
#    Individuals
#################################################################

###  http://www.ontotext.com
<http://www.ontotext.com> rdf:type owl:NamedIndividual ,
                                   foaf:Organization ;
                          rdfs:label "Ontotext Corp" ;
                          foaf:name "Ontotext Corp" .


###  http://rdaregistry.info/termList/gender/1001
<http://rdaregistry.info/termList/gender/1001> rdf:type owl:NamedIndividual .


###  http://rdaregistry.info/termList/gender/1002
<http://rdaregistry.info/termList/gender/1002> rdf:type owl:NamedIndividual .


###  http://vocab.getty.edu/ontology
<http://vocab.getty.edu/ontology> rdf:type owl:NamedIndividual ,
                                           voaf:Vocabulary .


###  http://vocab.getty.edu/aat/
aat: rdf:type owl:NamedIndividual ,
              skos:ConceptScheme ;
     dct:created "2014-02-20"^^xsd:date ;
     dct:creator <http://www.ontotext.com> ,
                 <http://www.getty.edu/research/> ;
     vann:preferredNamespacePrefix "aat" ;
     vann:preferredNamespaceUri "http://vocab.getty.edu/aat/" ;
     rdfs:comment "The Art and Architecture Thesaurus concept scheme" ;
     rdfs:label "Art and Architecture Thesaurus" ;
     rdfs:seeAlso <http://vocab.getty.edu/> ,
                  <http://vocab.getty.edu/.well-known/void> ,
                  <http://www.getty.edu/research/tools/vocabularies/lod/> ;
     foaf:homepage <http://www.getty.edu/research/tools/vocabularies/aat/> .


###  http://vocab.getty.edu/aat/300189557
aat: rdf:type owl:NamedIndividual ;
     skos:exactMatch <http://rdaregistry.info/termList/gender/1001> ,
                     <http://www.wikidata.org/entity/Q6581072> .


###  http://vocab.getty.edu/aat/300189559
aat: rdf:type owl:NamedIndividual ;
     skos:exactMatch <http://rdaregistry.info/termList/gender/1002> ,
                     <http://www.wikidata.org/entity/Q6581097> .


###  http://vocab.getty.edu/historic/
<http://vocab.getty.edu/historic/> rdf:type owl:NamedIndividual ,
                                            skos:ConceptScheme ;
                                   dct:description "Historic Flag concept scheme" ;
                                   rdfs:isDefinedBy <http://vocab.getty.edu/ontology> ;
                                   rdfs:label "Historic Flag concept scheme" .


###  http://vocab.getty.edu/historic/current
<http://vocab.getty.edu/historic/current> rdf:type owl:NamedIndividual ,
                                                   skos:Concept ;
                                          skos:inScheme <http://vocab.getty.edu/historic/> ;
                                          skos:notation "C" ;
                                          dct:description "Valid/used currently" ;
                                          skos:prefLabel "Current" ;
                                          skos:scopeNote "Valid/used currently" .


###  http://vocab.getty.edu/historic/currentAndHistoric
<http://vocab.getty.edu/historic/currentAndHistoric> rdf:type owl:NamedIndividual ,
                                                              skos:Concept ;
                                                     skos:inScheme <http://vocab.getty.edu/historic/> ;
                                                     skos:notation "B" ;
                                                     dct:description """Valid/used both in the past and currently.
Example: Saint Petersburg (TGN)""" ;
                                                     skos:example "Saint Petersburg (TGN)" ;
                                                     skos:prefLabel "Both Current and Historic" ;
                                                     skos:scopeNote "Valid/used both in the past and currently" .


###  http://vocab.getty.edu/historic/historic
<http://vocab.getty.edu/historic/historic> rdf:type owl:NamedIndividual ,
                                                    skos:Concept ;
                                           skos:inScheme <http://vocab.getty.edu/historic/> ;
                                           skos:notation "H" ;
                                           dct:description """Valid/used in the past but not currently.
Example: \"Lutetia\" is a historic name for \"Paris\" (TGN). \"weyneschot\" is a 16th-century spelling for \"wainscoting\" (AAT)""" ;
                                           skos:example "\"Lutetia\" is a historic name for \"Paris\" (TGN). \"weyneschot\" is a 16th-century spelling for \"wainscoting\" (AAT)" ;
                                           skos:prefLabel "Historic" ;
                                           skos:scopeNote "Valid/used in the past but not currently" .


###  http://vocab.getty.edu/historic/localUse
<http://vocab.getty.edu/historic/localUse> rdf:type owl:NamedIndividual ,
                                                    skos:Concept ;
                                           skos:inScheme <http://vocab.getty.edu/historic/> ;
                                           skos:notation "LU" ;
                                           dct:description """Used locally for Unidentified Named People mentioned in some document (ULAN only).
Example: 500051176 Abinetti (ULAN) is an unknown artist mentioned in documentation of lot 209 of an auction held 29 Jan 1824 in London""" ;
                                           skos:example "500051176 Abinetti (ULAN) is an unknown artist mentioned in documentation of lot 209 of an auction held 29 Jan 1824 in London" ;
                                           skos:prefLabel "Local Use" ;
                                           skos:scopeNote "Used locally for Unidentified Named People mentioned in some document (ULAN only)" .


###  http://vocab.getty.edu/ontology#Infer_broaderNonConcept_PropChainType2
gvp:Infer_broaderNonConcept_PropChainType2 rdf:type owl:NamedIndividual ,
                                                    ptop:PropChainType2 ;
                                           ptop:conclusion gvp:broaderNonConcept ;
                                           ptop:premise1 gvp:broaderNonConcept ;
                                           ptop:premise2 gvp:broader ;
                                           ptop:type2 gvp:GuideTerm .


###  http://vocab.getty.edu/ontology#Infer_broaderNonConcept_TypeRestr
gvp:Infer_broaderNonConcept_TypeRestr rdf:type owl:NamedIndividual ,
                                               ptop:TypeRestr ;
                                      ptop:conclusion gvp:broaderNonConcept ;
                                      ptop:premise gvp:broader ;
                                      ptop:type1 skos:Concept ;
                                      ptop:type2 gvp:GuideTerm .


###  http://vocab.getty.edu/ontology#Infer_broaderPreferredExtended
gvp:Infer_broaderPreferredExtended rdf:type owl:NamedIndividual ,
                                            ptop:PropChainRestr ;
                                   ptop:conclusion gvp:broaderPreferredExtended ;
                                   ptop:premise1 gvp:broaderPreferredExtended ;
                                   ptop:premise2 gvp:broaderPreferred ;
                                   ptop:restriction gvp:broaderExtended .


###  http://vocab.getty.edu/ontology#Infer_isoBroaderGeneric
gvp:Infer_isoBroaderGeneric rdf:type owl:NamedIndividual ,
                                     ptop:PropRestr ;
                            ptop:conclusion iso:broaderGeneric ;
                            ptop:premise gvp:broaderGenericExtended ;
                            ptop:restriction skos:broader .


###  http://vocab.getty.edu/ontology#Infer_isoBroaderInstantial
gvp:Infer_isoBroaderInstantial rdf:type owl:NamedIndividual ,
                                        ptop:PropRestr ;
                               ptop:conclusion iso:broaderInstantial ;
                               ptop:premise gvp:broaderInstantialExtended ;
                               ptop:restriction skos:broader .


###  http://vocab.getty.edu/ontology#Infer_isoBroaderPartitive
gvp:Infer_isoBroaderPartitive rdf:type owl:NamedIndividual ,
                                       ptop:PropRestr ;
                              ptop:conclusion iso:broaderPartitive ;
                              ptop:premise gvp:broaderPartitiveExtended ;
                              ptop:restriction skos:broader .


###  http://vocab.getty.edu/ontology#Infer_skosBroader_PropChainType2
gvp:Infer_skosBroader_PropChainType2 rdf:type owl:NamedIndividual ,
                                              ptop:PropChainType2 ;
                                     ptop:conclusion skos:broader ;
                                     ptop:premise1 gvp:broaderNonConcept ;
                                     ptop:premise2 gvp:broader ;
                                     ptop:type2 skos:Concept .


###  http://vocab.getty.edu/ontology#Infer_skosBroader_TypeRestr
gvp:Infer_skosBroader_TypeRestr rdf:type owl:NamedIndividual ,
                                         ptop:TypeRestr ;
                                ptop:conclusion skos:broader ;
                                ptop:premise gvp:broader ;
                                ptop:type1 skos:Concept ;
                                ptop:type2 skos:Concept .


###  http://vocab.getty.edu/term/POS/
<http://vocab.getty.edu/term/POS/> rdf:type owl:NamedIndividual ,
                                            skos:ConceptScheme ;
                                   dct:description "Part of Speech concept scheme" ;
                                   rdfs:isDefinedBy <http://vocab.getty.edu/ontology> ;
                                   rdfs:label "Part of Speech concept scheme" .


###  http://vocab.getty.edu/term/POS/Adjectival
<http://vocab.getty.edu/term/POS/Adjectival> rdf:type owl:NamedIndividual ,
                                                      skos:Concept ;
                                             skos:inScheme <http://vocab.getty.edu/term/POS/> ;
                                             skos:notation "A" ;
                                             dct:description """This term may be combined with others in post-coordinated compound terms.
Example: \"Renaissance\" (as in \"Renaissance cathedral\"), \"painter's\" (as in \"painter's smock\")""" ;
                                             skos:example "\"Renaissance\" (as in \"Renaissance cathedral\"), \"painter's\" (as in \"painter's smock\")" ;
                                             skos:prefLabel "Adjectival" ;
                                             skos:scopeNote "This term may be combined with others in post-coordinated compound terms" .


###  http://vocab.getty.edu/term/POS/BothSingularAndPlural
<http://vocab.getty.edu/term/POS/BothSingularAndPlural> rdf:type owl:NamedIndividual ,
                                                                 skos:Concept ;
                                                        skos:inScheme <http://vocab.getty.edu/term/POS/> ;
                                                        skos:notation "B" ;
                                                        dct:description """A term that is used for both the singular and plural in the same language.
Example: \"chassis\" is both singular and plural in French""" ;
                                                        skos:example "\"chassis\" is both singular and plural in French" ;
                                                        skos:prefLabel "Both Singular and Plural" ;
                                                        skos:scopeNote "A term that is used for both the singular and plural in the same language" .


###  http://vocab.getty.edu/term/POS/Noun
<http://vocab.getty.edu/term/POS/Noun> rdf:type owl:NamedIndividual ,
                                                skos:Concept ;
                                       skos:inScheme <http://vocab.getty.edu/term/POS/> ;
                                       skos:notation "N" ;
                                       dct:description """Term is a noun but we are uncertain if it is plural or singular.
Example: Panthera leo""" ;
                                       skos:example "Panthera leo" ;
                                       skos:prefLabel "Noun" ;
                                       skos:scopeNote "Term is a noun but we are uncertain if it is plural or singular" .


###  http://vocab.getty.edu/term/POS/PastParticiple
<http://vocab.getty.edu/term/POS/PastParticiple> rdf:type owl:NamedIndividual ,
                                                          skos:Concept ;
                                                 skos:inScheme <http://vocab.getty.edu/term/POS/> ;
                                                 skos:notation "PP" ;
                                                 dct:description """Rarely used but if at all, is most likely to apply in Attributes and Properties.
Example: hand-painted""" ;
                                                 skos:example "hand-painted" ;
                                                 skos:prefLabel "Past Participle" ;
                                                 skos:scopeNote "Rarely used but if at all, is most likely to apply in Attributes and Properties" .


###  http://vocab.getty.edu/term/POS/PluralNoun
<http://vocab.getty.edu/term/POS/PluralNoun> rdf:type owl:NamedIndividual ,
                                                      skos:Concept ;
                                             skos:inScheme <http://vocab.getty.edu/term/POS/> ;
                                             skos:notation "PN" ;
                                             dct:description """A term that is plural (the same word may be singular in another language).
Example: \"filigrane\" is the Italian plural for \"watermarks\"""" ;
                                             skos:example "\"filigrane\" is the Italian plural for \"watermarks\"" ;
                                             skos:prefLabel "Plural Noun" ;
                                             skos:scopeNote "A term that is plural (the same word may be singular in another language)" .


###  http://vocab.getty.edu/term/POS/SingularNoun
<http://vocab.getty.edu/term/POS/SingularNoun> rdf:type owl:NamedIndividual ,
                                                        skos:Concept ;
                                               skos:inScheme <http://vocab.getty.edu/term/POS/> ;
                                               skos:notation "SN" ;
                                               dct:description """A term that is singular (the same word may be plural in another language).
Example: \"filigrane\" is the French singular for \"watermark\"""" ;
                                               skos:example "\"filigrane\" is the French singular for \"watermark\"" ;
                                               skos:prefLabel "Singular Noun" ;
                                               skos:scopeNote "A term that is singular (the same word may be plural in another language)" .


###  http://vocab.getty.edu/term/POS/VerbalNounGerund
<http://vocab.getty.edu/term/POS/VerbalNounGerund> rdf:type owl:NamedIndividual ,
                                                            skos:Concept ;
                                                   skos:inScheme <http://vocab.getty.edu/term/POS/> ;
                                                   skos:notation "VN" ;
                                                   dct:description """Term is a verbal noun or gerund.
Example: polishing""" ;
                                                   skos:example "polishing" ;
                                                   skos:prefLabel "Verbal Noun/Gerund" ;
                                                   skos:scopeNote "Term is a verbal noun or gerund" .


###  http://vocab.getty.edu/term/display/
<http://vocab.getty.edu/term/display/> rdf:type owl:NamedIndividual ,
                                                skos:ConceptScheme ;
                                       dct:description "Term Display concept scheme" ;
                                       rdfs:isDefinedBy <http://vocab.getty.edu/ontology> ;
                                       rdfs:label "Term Display concept scheme" .


###  http://vocab.getty.edu/term/display/Display
<http://vocab.getty.edu/term/display/Display> rdf:type owl:NamedIndividual ,
                                                       skos:Concept ;
                                              skos:inScheme <http://vocab.getty.edu/term/display/> ;
                                              skos:notation "D" ,
                                                            "Y" ;
                                              dct:description "Use in displays where natural order is appropriate" ;
                                              skos:prefLabel "Use for Display" ;
                                              skos:scopeNote "Use in displays where natural order is appropriate" .


###  http://vocab.getty.edu/term/display/Indexing
<http://vocab.getty.edu/term/display/Indexing> rdf:type owl:NamedIndividual ,
                                                        skos:Concept ;
                                               skos:inScheme <http://vocab.getty.edu/term/display/> ;
                                               skos:notation "I" ;
                                               dct:description "Use in indexes or permuted lists where inverted order is appropriate" ;
                                               skos:prefLabel "Use in Indexes/lists" ;
                                               skos:scopeNote "Use in indexes or permuted lists where inverted order is appropriate" .


###  http://vocab.getty.edu/term/flag/
<http://vocab.getty.edu/term/flag/> rdf:type owl:NamedIndividual ,
                                             skos:ConceptScheme ;
                                    dct:description "Term Flag concept scheme" ;
                                    rdfs:isDefinedBy <http://vocab.getty.edu/ontology> ;
                                    rdfs:label "Term Flag concept scheme" .


###  http://vocab.getty.edu/term/flag/LiteralTranslation
<http://vocab.getty.edu/term/flag/LiteralTranslation> rdf:type owl:NamedIndividual ,
                                                               skos:Concept ;
                                                      skos:inScheme <http://vocab.getty.edu/term/flag/> ;
                                                      skos:notation "T" ;
                                                      dct:description "Literal translation of a name.  Defined for ULAN, but currently there are no examples of this" ;
                                                      skos:prefLabel "Literal Translation" ;
                                                      skos:scopeNote "Literal translation of a name.  Defined for ULAN, but currently there are no examples of this" .


###  http://vocab.getty.edu/term/flag/LoanTerm
<http://vocab.getty.edu/term/flag/LoanTerm> rdf:type owl:NamedIndividual ,
                                                     skos:Concept ;
                                            skos:inScheme <http://vocab.getty.edu/term/flag/> ;
                                            skos:notation "L" ;
                                            dct:description """Term borrowed from another language that has become naturalized in American English.
Example: papier mache""" ;
                                            skos:example "papier mache" ;
                                            skos:prefLabel "Loan Term" ;
                                            skos:scopeNote "Term borrowed from another language that has become naturalized in American English" .


###  http://vocab.getty.edu/term/flag/Vernacular
<http://vocab.getty.edu/term/flag/Vernacular> rdf:type owl:NamedIndividual ,
                                                       skos:Concept ;
                                              skos:inScheme <http://vocab.getty.edu/term/flag/> ;
                                              skos:notation "V" ;
                                              dct:description """Term is the vernacular for a certain place.
Example: \"kachoga\" is the Vernacular for 300266169 \"bird-and-flower paintings\" (AAT). \"Firenze\" is the vernacular in Italian (TGN)""" ;
                                              skos:example "\"kachoga\" is the Vernacular for 300266169 \"bird-and-flower paintings\" (AAT). \"Firenze\" is the vernacular in Italian (TGN)" ;
                                              skos:prefLabel "Vernacular" ;
                                              skos:scopeNote "Term is the vernacular for a certain place" .


###  http://vocab.getty.edu/term/kind/
<http://vocab.getty.edu/term/kind/> rdf:type owl:NamedIndividual ,
                                             skos:ConceptScheme ;
                                    dct:description "Term Kind concept scheme" ;
                                    rdfs:isDefinedBy <http://vocab.getty.edu/ontology> ;
                                    rdfs:label "Term Kind concept scheme" .


###  http://vocab.getty.edu/term/kind/Abbreviation
<http://vocab.getty.edu/term/kind/Abbreviation> rdf:type owl:NamedIndividual ,
                                                         skos:Concept ;
                                                skos:inScheme <http://vocab.getty.edu/term/kind/> ;
                                                skos:notation "A" ;
                                                dct:description """Term is an abbreviation, initialism, or acronym.
Example: \"FLIM\" is abbrevaition for \"fluorescence lifetime imaging microscopy\"""" ;
                                                skos:example "\"FLIM\" is abbrevaition for \"fluorescence lifetime imaging microscopy\"" ;
                                                skos:prefLabel "Abbreviation" ;
                                                skos:scopeNote "Term is an abbreviation, initialism, or acronym" .


###  http://vocab.getty.edu/term/kind/BirthName
<http://vocab.getty.edu/term/kind/BirthName> rdf:type owl:NamedIndividual ,
                                                      skos:Concept ;
                                             skos:inScheme <http://vocab.getty.edu/term/kind/> ;
                                             skos:notation "BN" ;
                                             dct:description """Birth Name of an ULAN agent.
Example: TODO""" ;
                                             skos:example "TODO" ;
                                             skos:prefLabel "Birth Name" ;
                                             skos:scopeNote "Birth Name of an ULAN agent" .


###  http://vocab.getty.edu/term/kind/ChemicalName
<http://vocab.getty.edu/term/kind/ChemicalName> rdf:type owl:NamedIndividual ,
                                                         skos:Concept ;
                                                skos:inScheme <http://vocab.getty.edu/term/kind/> ;
                                                skos:notation "CN" ;
                                                dct:description """Term is the chemical name for the descriptor. Used in AAT only.
Example: \"sodium tetraborate decahydrate\" is chemical name for \"borax\"""" ;
                                                skos:example "\"sodium tetraborate decahydrate\" is chemical name for \"borax\"" ;
                                                skos:prefLabel "Chemical Name" ;
                                                skos:scopeNote "Term is the chemical name for the descriptor. Used in AAT only" .


###  http://vocab.getty.edu/term/kind/Code
<http://vocab.getty.edu/term/kind/Code> rdf:type owl:NamedIndividual ,
                                                 skos:Concept ;
                                        skos:inScheme <http://vocab.getty.edu/term/kind/> ;
                                        skos:notation "79000" ;
                                        dct:description """Code, similar to Abbreviation.
Example: \"sq yds\", \"m2\"""" ;
                                        skos:example "\"sq yds\", \"m2\"" ;
                                        skos:prefLabel "Code" ;
                                        skos:scopeNote "Code, similar to Abbreviation" .


###  http://vocab.getty.edu/term/kind/CommonName
<http://vocab.getty.edu/term/kind/CommonName> rdf:type owl:NamedIndividual ,
                                                       skos:Concept ;
                                              skos:inScheme <http://vocab.getty.edu/term/kind/> ;
                                              skos:notation "CN" ;
                                              dct:description """Common Name of an ULAN agent.
Example: TODO""" ;
                                              skos:example "TODO" ;
                                              skos:prefLabel "Common Name" ;
                                              skos:scopeNote "Common Name of an ULAN agent" .


###  http://vocab.getty.edu/term/kind/CommonTerm
<http://vocab.getty.edu/term/kind/CommonTerm> rdf:type owl:NamedIndividual ,
                                                       skos:Concept ;
                                              skos:inScheme <http://vocab.getty.edu/term/kind/> ;
                                              skos:notation "C" ;
                                              dct:description """Preferred common language term. Used for subjects that also include a Scientific term. Used in AAT only.
Example: \"frankincense\" (species) is common term for \"Boswellia sacra\" (species)""" ;
                                              skos:example "\"frankincense\" (species) is common term for \"Boswellia sacra\" (species)" ;
                                              skos:prefLabel "Common term" ;
                                              skos:scopeNote "Preferred common language term. Used for subjects that also include a Scientific term. Used in AAT only" .


###  http://vocab.getty.edu/term/kind/FIPSCode
<http://vocab.getty.edu/term/kind/FIPSCode> rdf:type owl:NamedIndividual ,
                                                     skos:Concept ;
                                            skos:inScheme <http://vocab.getty.edu/term/kind/> ;
                                            skos:notation "FIPS" ;
                                            dct:description """FIPS region code. Used in TGN.
Example: \"MX21\" for Puebla, Mexico""" ;
                                            skos:example "\"MX21\" for Puebla, Mexico" ;
                                            skos:prefLabel "FIPS Code" ;
                                            skos:scopeNote "FIPS region code. Used in TGN" .


###  http://vocab.getty.edu/term/kind/FullName
<http://vocab.getty.edu/term/kind/FullName> rdf:type owl:NamedIndividual ,
                                                     skos:Concept ;
                                            skos:inScheme <http://vocab.getty.edu/term/kind/> ;
                                            skos:notation "FN" ;
                                            dct:description """Full Name of an ULAN agent.
Example: TODO""" ;
                                            skos:example "TODO" ;
                                            skos:prefLabel "Full Name" ;
                                            skos:scopeNote "Full Name of an ULAN agent" .


###  http://vocab.getty.edu/term/kind/FullTerm
<http://vocab.getty.edu/term/kind/FullTerm> rdf:type owl:NamedIndividual ,
                                                     skos:Concept ;
                                            skos:inScheme <http://vocab.getty.edu/term/kind/> ;
                                            skos:notation "F" ;
                                            dct:description """Full-form term. Used when the descriptor is a shorter form, or the subject also includes an Abbreviation. Used in AAT only.
Example: \"Extensible Markup Language\" is the full term for \"XML\" (which is preferred)""" ;
                                            skos:example "\"Extensible Markup Language\" is the full term for \"XML\" (which is preferred)" ;
                                            skos:prefLabel "Full term" ;
                                            skos:scopeNote "Full-form term. Used when the descriptor is a shorter form, or the subject also includes an Abbreviation. Used in AAT only" .


###  http://vocab.getty.edu/term/kind/ISOalpha2
<http://vocab.getty.edu/term/kind/ISOalpha2> rdf:type owl:NamedIndividual ,
                                                      skos:Concept ;
                                             skos:inScheme <http://vocab.getty.edu/term/kind/> ;
                                             skos:notation "ISO2L" ;
                                             dct:description """ISO 3166-1 alpha-2 country code. Used in TGN.
Example: \"AQ\" for Antarctica""" ;
                                             skos:example "\"AQ\" for Antarctica" ;
                                             skos:prefLabel "ISO alpha-2 code" ;
                                             skos:scopeNote "ISO 3166-1 alpha-2 country code. Used in TGN" .


###  http://vocab.getty.edu/term/kind/ISOalpha3
<http://vocab.getty.edu/term/kind/ISOalpha3> rdf:type owl:NamedIndividual ,
                                                      skos:Concept ;
                                             skos:inScheme <http://vocab.getty.edu/term/kind/> ;
                                             skos:notation "ISO3L" ;
                                             dct:description """ISO 3166-1 alpha-3 country code. Used in TGN.
Example: \"ATA\" for Antarctica""" ;
                                             skos:example "\"ATA\" for Antarctica" ;
                                             skos:prefLabel "ISO alpha-3 code" ;
                                             skos:scopeNote "ISO 3166-1 alpha-3 country code. Used in TGN" .


###  http://vocab.getty.edu/term/kind/ISOnumeric2
<http://vocab.getty.edu/term/kind/ISOnumeric2> rdf:type owl:NamedIndividual ,
                                                        skos:Concept ;
                                               skos:inScheme <http://vocab.getty.edu/term/kind/> ;
                                               skos:notation "ISO2N" ;
                                               dct:description "May be used in TGN, but no code of this kind is present" ;
                                               skos:prefLabel "ISO numeric-2 code" ;
                                               skos:scopeNote "May be used in TGN, but no code of this kind is present" .


###  http://vocab.getty.edu/term/kind/ISOnumeric3
<http://vocab.getty.edu/term/kind/ISOnumeric3> rdf:type owl:NamedIndividual ,
                                                        skos:Concept ;
                                               skos:inScheme <http://vocab.getty.edu/term/kind/> ;
                                               skos:notation "ISO3N" ;
                                               dct:description """ISO 3166-1 numeric country code as \"ISOnnn\" (though ISO specifies only \"nnn\"). Used in TGN only.
Example: \"ISO414\" for Kuwait""" ;
                                               skos:example "\"ISO414\" for Kuwait" ;
                                               skos:prefLabel "ISO numeric-3 code" ;
                                               skos:scopeNote "ISO 3166-1 numeric country code as \"ISOnnn\" (though ISO specifies only \"nnn\"). Used in TGN only" .


###  http://vocab.getty.edu/term/kind/JargonOrSlang
<http://vocab.getty.edu/term/kind/JargonOrSlang> rdf:type owl:NamedIndividual ,
                                                          skos:Concept ;
                                                 skos:inScheme <http://vocab.getty.edu/term/kind/> ;
                                                 skos:notation "J" ;
                                                 dct:description """Slang or jargon term. Used in AAT only.
Example: \"fool's gold\" is slang for \"pyrite\"""" ;
                                                 skos:example "\"fool's gold\" is slang for \"pyrite\"" ;
                                                 skos:prefLabel "Jargon or Slang" ;
                                                 skos:scopeNote "Slang or jargon term. Used in AAT only" .


###  http://vocab.getty.edu/term/kind/Neologism
<http://vocab.getty.edu/term/kind/Neologism> rdf:type owl:NamedIndividual ,
                                                      skos:Concept ;
                                             skos:inScheme <http://vocab.getty.edu/term/kind/> ;
                                             skos:notation "N" ;
                                             dct:description """Term that is new to the language, generally having been coined due to new technology. Used in AAT only..
Example: \"folksonomy\", \"podcasting\"""" ;
                                             skos:example "\"folksonomy\", \"podcasting\"" ;
                                             skos:prefLabel "Neologism" ;
                                             skos:scopeNote "Term that is new to the language, generally having been coined due to new technology. Used in AAT only." .


###  http://vocab.getty.edu/term/kind/OfficialName
<http://vocab.getty.edu/term/kind/OfficialName> rdf:type owl:NamedIndividual ,
                                                         skos:Concept ;
                                                skos:inScheme <http://vocab.getty.edu/term/kind/> ;
                                                skos:notation "O" ;
                                                dct:description """Used in TGN and ULAN.
Example: \"Noyen-sur-Seine\" is official name of 7030197 \"Noyen\" (TGN)""" ;
                                                skos:example "\"Noyen-sur-Seine\" is official name of 7030197 \"Noyen\" (TGN)" ;
                                                skos:prefLabel "Official Name" ;
                                                skos:scopeNote "Used in TGN and ULAN" .


###  http://vocab.getty.edu/term/kind/ProvisionalName
<http://vocab.getty.edu/term/kind/ProvisionalName> rdf:type owl:NamedIndividual ,
                                                            skos:Concept ;
                                                   skos:inScheme <http://vocab.getty.edu/term/kind/> ;
                                                   skos:notation "PN" ;
                                                   dct:description """Used in TGN only.
Example: \"Rockton\" was provisional name considered before adoption of \"Kent\" (Ohio)""" ;
                                                   skos:example "\"Rockton\" was provisional name considered before adoption of \"Kent\" (Ohio)" ;
                                                   skos:prefLabel "Provisional Name" ;
                                                   skos:scopeNote "Used in TGN only" .


###  http://vocab.getty.edu/term/kind/Pseudonym
<http://vocab.getty.edu/term/kind/Pseudonym> rdf:type owl:NamedIndividual ,
                                                      skos:Concept ;
                                             skos:inScheme <http://vocab.getty.edu/term/kind/> ;
                                             skos:notation "P" ;
                                             dct:description """Used in TGN and ULAN.
Example: \"Frisco\" is nickname for San Francisco (TGN)""" ;
                                             skos:example "\"Frisco\" is nickname for San Francisco (TGN)" ;
                                             skos:prefLabel "Pseudonym" ;
                                             skos:scopeNote "Used in TGN and ULAN" .


###  http://vocab.getty.edu/term/kind/ScientificOrTechnical
<http://vocab.getty.edu/term/kind/ScientificOrTechnical> rdf:type owl:NamedIndividual ,
                                                                  skos:Concept ;
                                                         skos:inScheme <http://vocab.getty.edu/term/kind/> ;
                                                         skos:notation "S" ;
                                                         dct:description """Scientific taxon name (genus, species, etc). Used in AAT only. All such are emitted marked with English language, and most have the same string marked with Latin.
Example: \"Boswellia sacra\"@la, also emitted as \"Boswellia sacra\"@en, is scientific name of \"frankincense\"""" ;
                                                         skos:example "\"Boswellia sacra\"@la, also emitted as \"Boswellia sacra\"@en, is scientific name of \"frankincense\"" ;
                                                         skos:prefLabel "Scientific or Technical term" ;
                                                         skos:scopeNote "Scientific taxon name (genus, species, etc). Used in AAT only. All such are emitted marked with English language, and most have the same string marked with Latin" .


###  http://vocab.getty.edu/term/kind/SiteName
<http://vocab.getty.edu/term/kind/SiteName> rdf:type owl:NamedIndividual ,
                                                     skos:Concept ;
                                            skos:inScheme <http://vocab.getty.edu/term/kind/> ;
                                            skos:notation "S" ;
                                            dct:description """Used in TGN only.
Example: \"Flavia Solva\", a deserted settlement and archaeological site (TGN)""" ;
                                            skos:example "\"Flavia Solva\", a deserted settlement and archaeological site (TGN)" ;
                                            skos:prefLabel "Site Name" ;
                                            skos:scopeNote "Used in TGN only" .


###  http://vocab.getty.edu/term/kind/USPSCode
<http://vocab.getty.edu/term/kind/USPSCode> rdf:type owl:NamedIndividual ,
                                                     skos:Concept ;
                                            skos:inScheme <http://vocab.getty.edu/term/kind/> ;
                                            skos:notation "USPS" ;
                                            dct:description """Used in TGN only.
Example: \"CA\" for California""" ;
                                            skos:example "\"CA\" for California" ;
                                            skos:prefLabel "US Postal Service Code" ;
                                            skos:scopeNote "Used in TGN only" .


###  http://vocab.getty.edu/term/type/
<http://vocab.getty.edu/term/type/> rdf:type owl:NamedIndividual ,
                                             skos:ConceptScheme ;
                                    dct:description "Term Type concept scheme" ;
                                    rdfs:isDefinedBy <http://vocab.getty.edu/ontology> ;
                                    rdfs:label "Term Type concept scheme" .


###  http://vocab.getty.edu/term/type/AlternateDescriptor
<http://vocab.getty.edu/term/type/AlternateDescriptor> rdf:type owl:NamedIndividual ,
                                                                skos:Concept ;
                                                       skos:inScheme <http://vocab.getty.edu/term/type/> ;
                                                       skos:notation "AD" ;
                                                       dct:description """A lexical variant, eg singular.
Example: \"manuscript\" (English) instead of \"manuscripts\"""" ;
                                                       skos:example "\"manuscript\" (English) instead of \"manuscripts\"" ;
                                                       skos:prefLabel "Alternate Descriptor" ;
                                                       skos:scopeNote "A lexical variant, eg singular" .


###  http://vocab.getty.edu/term/type/Descriptor
<http://vocab.getty.edu/term/type/Descriptor> rdf:type owl:NamedIndividual ,
                                                       skos:Concept ;
                                              skos:inScheme <http://vocab.getty.edu/term/type/> ;
                                              skos:notation "D" ;
                                              dct:description """Main term. Getty usually uses the plural.
Example: \"manuscripts\" (English)""" ;
                                              skos:example "\"manuscripts\" (English)" ;
                                              skos:prefLabel "Descriptor" ;
                                              skos:scopeNote "Main term. Getty usually uses the plural" .


###  http://vocab.getty.edu/term/type/UsedForTerm
<http://vocab.getty.edu/term/type/UsedForTerm> rdf:type owl:NamedIndividual ,
                                                        skos:Concept ;
                                               skos:inScheme <http://vocab.getty.edu/term/type/> ;
                                               skos:notation "UF" ;
                                               dct:description """A synonym.
Example: \"handschriften\" (Dutch) instead of \"manuscripten\"""" ;
                                               skos:example "\"handschriften\" (Dutch) instead of \"manuscripten\"" ;
                                               skos:prefLabel "Used for Term" ;
                                               skos:scopeNote "A synonym" .


###  http://vocab.getty.edu/tgn/
tgn: rdf:type owl:NamedIndividual ,
              skos:ConceptScheme ;
     dct:created "2014-06-15"^^xsd:date ;
     dct:creator <http://www.ontotext.com> ,
                 <http://www.getty.edu/research/> ;
     vann:preferredNamespacePrefix "tgn" ;
     vann:preferredNamespaceUri "http://vocab.getty.edu/tgn/" ;
     rdfs:comment "The Thesaurus of Geographic Names concept scheme" ;
     rdfs:label "Thesaurus of Geographic Names" ;
     rdfs:seeAlso <http://vocab.getty.edu/> ,
                  <http://vocab.getty.edu/.well-known/void> ,
                  <http://www.getty.edu/research/tools/vocabularies/lod/> ;
     foaf:homepage <http://www.getty.edu/research/tools/vocabularies/tgn/> .


###  http://vocab.getty.edu/ulan/
ulan: rdf:type owl:NamedIndividual ,
               skos:ConceptScheme ;
      dct:created "2015-03-25"^^xsd:date ;
      dct:creator <http://www.ontotext.com> ,
                  <http://www.getty.edu/research/> ;
      vann:preferredNamespacePrefix "ulan" ;
      vann:preferredNamespaceUri "http://vocab.getty.edu/ulan/" ;
      rdfs:comment "The Union List of Artist Names concept scheme" ;
      rdfs:label "Union List of Artist Names" ;
      rdfs:seeAlso <http://vocab.getty.edu/> ,
                   <http://vocab.getty.edu/.well-known/void> ,
                   <http://www.getty.edu/research/tools/vocabularies/lod/> ;
      foaf:homepage <http://www.getty.edu/research/tools/vocabularies/ulan/> .


###  http://www.getty.edu/research/
<http://www.getty.edu/research/> rdf:type owl:NamedIndividual ,
                                          foaf:Organization ;
                                 rdfs:label "Getty Research Institute" ;
                                 foaf:name "Getty Research Institute" .


###  http://www.wikidata.org/entity/Q6581072
<http://www.wikidata.org/entity/Q6581072> rdf:type owl:NamedIndividual .


###  http://www.wikidata.org/entity/Q6581097
<http://www.wikidata.org/entity/Q6581097> rdf:type owl:NamedIndividual .


#################################################################
#    Annotations
#################################################################

gvp:contributorAlternatePreferred rdfs:isDefinedBy <http://vocab.getty.edu/ontology> ;
                                  dct:description "Contributor for which the term is Alternate Preferred. Range is foaf:Agent" ;
                                  rdfs:label "contributorAlternatePreferred" ;
                                  rdfs:comment "Contributor for which the term is Alternate Preferred. Range is foaf:Agent" .


gvp:contributorNonPreferred dct:description """Contributor for which the term is Non-preferred. Range is foaf:Agent.
Example: \"Lycra\" is non-preferred term for WHS""" ;
                            rdfs:label "contributorNonPreferred" ;
                            skos:example "\"Lycra\" is non-preferred term for WHS" ;
                            rdfs:isDefinedBy <http://vocab.getty.edu/ontology> ;
                            rdfs:comment "Contributor for which the term is Non-preferred. Range is foaf:Agent" .


gvp:contributorPreferred dct:description """Contributor for which the term is Preferred. Range is foaf:Agent.
Example: \"organza\" is preferred term for WHS""" ;
                         rdfs:label "contributorPreferred" ;
                         rdfs:comment "Contributor for which the term is Preferred. Range is foaf:Agent" ;
                         rdfs:isDefinedBy <http://vocab.getty.edu/ontology> ;
                         skos:example "\"organza\" is preferred term for WHS" .


gvp:parentString dct:description """Preferred labels of *all* of the subject's preferred ancestors, listed bottom up. Useful to show the subject's full context.
Display version of gvp:broaderPreferredExtended.
For aat:300226882 baking dishes: bakeware, <vessels for cooking food>, <containers for cooking food>, <culinary containers>, <containers by function or context>, containers (receptacles), Containers (Hierarchy Name), Furnishings and Equipment (Hierarchy Name), Objects Facet""" ;
                 rdfs:label "parentString" ;
                 skos:note "Display version of gvp:broaderPreferredExtended" ;
                 skos:example "For aat:300226882 baking dishes: bakeware, <vessels for cooking food>, <containers for cooking food>, <culinary containers>, <containers by function or context>, containers (receptacles), Containers (Hierarchy Name), Furnishings and Equipment (Hierarchy Name), Objects Facet" ;
                 rdfs:comment "Preferred labels of *all* of the subject's preferred ancestors, listed bottom up. Useful to show the subject's full context" ;
                 rdfs:isDefinedBy <http://vocab.getty.edu/ontology> .


gvp:parentStringAbbrev rdfs:comment "Preferred labels of *some* of the subject's preferred ancestors, listed bottom up. Useful to show the subject's context" ;
                       skos:note "Shortened display version of gvp:broaderPreferredExtended" ;
                       skos:example "For aat:300226882 baking dishes: bakeware, <vessels for cooking food>, ... Furnishings and Equipment (Hierarchy Name)" ;
                       rdfs:label "parentStringAbbrev" ;
                       dct:description """Preferred labels of *some* of the subject's preferred ancestors, listed bottom up. Useful to show the subject's context.
Shortened display version of gvp:broaderPreferredExtended.
Example for aat:300226882 baking dishes: bakeware, <vessels for cooking food>, ... Furnishings and Equipment (Hierarchy Name)""" ;
                       rdfs:isDefinedBy <http://vocab.getty.edu/ontology> .


gvp:qualifier dct:description """Clarifies and disambiguates terms with the same spelling but different meaning.
Appended in parentheses to gvp:term, forming skosxsl:literalForm.
Every qualifier is in the same language as the term.
Example: \"Rhea (vessels)\"=rhyta (a kind of drinking vessel) vs \"Rhea (species)\"=Boehmeria nivea (Chinese grass)""" ;
              rdfs:label "qualifier" ;
              skos:example "Rhea (vessels)=rhyta (a kind of drinking vessel) vs rhea (species)=Boehmeria nivea (Chinese grass)" ;
              rdfs:isDefinedBy <http://vocab.getty.edu/ontology> ;
              rdfs:comment """Clarifies and disambiguates terms with the same spelling but different meaning.
Appended in parentheses to gvp:term, forming skosxsl:literalForm.
Every qualifier is in the same language as the term""" .


gvp:term rdfs:comment "Term (label), used as the basic (prefix) part of skosxsl:literalForm" ;
         dct:description "Term (label), used as the basic (prefix) part of skosxsl:literalForm" ;
         rdfs:isDefinedBy <http://vocab.getty.edu/ontology> ;
         rdfs:label "term" .


###  Generated by the OWL API (version 4.2.8.20170104-2310) https://github.com/owlcs/owlapi
