@prefix : <http://purl.oclc.org/NET/ssnx/qu/qu/> .
@prefix cc: <http://creativecommons.org/ns#> .
@prefix dc: <http://purl.org/dc/elements/1.1/> .
@prefix qu: <http://purl.oclc.org/NET/ssnx/qu/qu#> .
@prefix dct: <http://purl.org/dc/terms/> .
@prefix dim: <http://purl.oclc.org/NET/ssnx/qu/dim#> .
@prefix owl: <http://www.w3.org/2002/07/owl#> .
@prefix rdf: <http://www.w3.org/1999/02/22-rdf-syntax-ns#> .
@prefix xml: <http://www.w3.org/XML/1998/namespace> .
@prefix xsd: <http://www.w3.org/2001/XMLSchema#> .
@prefix rdfs: <http://www.w3.org/2000/01/rdf-schema#> .
@prefix skos: <http://www.w3.org/2004/02/skos/core#> .
@prefix unit: <http://purl.oclc.org/NET/ssnx/qu/unit#> .
@prefix prefix: <http://purl.oclc.org/NET/ssnx/qu/prefix#> .
@prefix quantity: <http://purl.oclc.org/NET/ssnx/qu/quantity#> .
@base <http://purl.oclc.org/NET/ssnx/qu/qu> .

<http://purl.oclc.org/NET/ssnx/qu/qu> rdf:type owl:Ontology ;
                                       dc:title "Library for Quantity Kinds and Units: schema, based on QUDV model OMG SysML(TM), Version 1.2" ;
                                       dc:creator "Hans Peter de Koning (ESA, Netherlands and QUDV working group of the SysML 1.2 Revision Task Force (RTF))"^^xsd:string ,
                                                  "Roger Burkhart (John Deere, USA and QUDV working group of the SysML 1.2 Revision Task Force (RTF))"^^xsd:string ,
                                                  "Laurent Lefort (CSIRO, Australia and W3C Semantic Sensor Network Incubator Group)"^^xsd:string ;
                                       rdfs:comment "In order to generalize its potential usage and alignment with other standardization efforts concerning quantities and units, the QU  ontology has been further developed as a complement to the Agriculture Meteorology example showcasing the ontology developed by the W3C Semantic Sensor Networks incubator group (SSN-XG). The Agriculture Meteorology example also includes an application of the QU schema to the UN/CEFACT Recommendation 20 code list. For more information on the group's activities see: http://www.w3.org/2005/Incubator/ssn/ ."^^xsd:string ;
                                       rdfs:seeAlso "http://www.w3.org/2005/Incubator/ssn/" ;
                                       rdfs:comment "The QUDV copyright holders have agreed for the QU ontology to be published by the W3C Semantic Sensor Incubator Group but this does not constitute an endorsement or recommendation by the QUDV working group of the SysML 1.2 Revision Task Force. All other rights reserved."^^xsd:string ;
                                       dct:created "2009-08-26" ;
                                       dc:creator "Nicolas Rouquette (NASA-JPL, USA and QUDV working group of the SysML 1.2 Revision Task Force (RTF))"^^xsd:string ;
                                       dct:modified "2011-06-20" ;
                                       rdfs:comment "This Model Library for Quantities, Units, Dimensions and Values (QUDV)  (Note: in the ontology, the SYSML-QUDV definitions are flagged with a rdfs:seeAlso annotation equal to http://www.omgsysml.org/qudv)."^^xsd:string ,
                                                    ""^^xsd:string ;
                                       dc:rights "qu.owl  Copyright 2010 - 2011 CSIRO" ;
                                       dc:creator "Huascar Espinoza (CEA, France and QUDV working group of the SysML 1.2 Revision Task Force (RTF))"^^xsd:string ;
                                       dc:identifier "http://purl.oclc.org/NET/ssnx/qu/qu" ;
                                       rdfs:comment """This ontology is partially based on the SysML QUDV (Quantities, Units, Dimensions and Values) proposed by a working group of the SysML 1.2 Revision Task Force (RTF), working in close coordination with the OMG MARTE specification group. This model library is specified in a UML/SysML class/block diagram in the OMG SysML, Version 1.2 specification (http://www.omg.org/spec/SysML/1.2/). This model is described in OMG  SysML, Version 1.2 Appendix C.4 Model Library for Quantity Kinds and Units (http://ontolog.cim3.net/file/resource/reference/UoM_Ontology_Standard/available-UoM-references/QUDV-Annex-C4-C5--OMG-SysML-v1-2_Oct-2009.pdf).		
	
The QUDV model has also been represented in the form of an ontology using a formal ontology definition language. The resulting OWL ontology, called the QUDV ontology http://www.omgwiki.org/OMGSysML/doku.php?id=sysml-qudv:qudv_owl has been published by members of the QUDV working group of the SysML 1.2 Revision Task Force (RTF). 

		OMG SysML is a trademark of OMG (see http://www.omg.org/spec/SysML/1.2/PDF/ for the conditions of use of the  OMG  SysML, Version 1.2  specification).
		"""^^xsd:string ,
                                                    "Please report any errors to the Semantic Sensor Network Incubator Activity via the public W3C list public-xg-ssn@w3.org or alternatively, for enquiries about the QUDV model,  to the QUDV mailing list: http://www.omg.org/publicarchives/qudv/"^^xsd:string ;
                                       dc:rights "sysml-qudv:qudv_owl  Copyright 2009 - 2011 The QUDV authors" .

#################################################################
#    Annotation properties
#################################################################

###  http://creativecommons.org/ns#license
cc:license rdf:type owl:AnnotationProperty .


###  http://purl.org/dc/elements/1.1/author
dc:author rdf:type owl:AnnotationProperty .


###  http://purl.org/dc/elements/1.1/creator
dc:creator rdf:type owl:AnnotationProperty .


###  http://purl.org/dc/elements/1.1/description
dc:description rdf:type owl:AnnotationProperty .


###  http://purl.org/dc/elements/1.1/identifier
dc:identifier rdf:type owl:AnnotationProperty .


###  http://purl.org/dc/elements/1.1/rights
dc:rights rdf:type owl:AnnotationProperty .


###  http://purl.org/dc/elements/1.1/source
dc:source rdf:type owl:AnnotationProperty .


###  http://purl.org/dc/elements/1.1/title
dc:title rdf:type owl:AnnotationProperty .


###  http://purl.org/dc/terms/created
dct:created rdf:type owl:AnnotationProperty .


###  http://purl.org/dc/terms/modified
dct:modified rdf:type owl:AnnotationProperty .


###  http://www.w3.org/2000/01/rdf-schema#comment
rdfs:comment rdf:type owl:AnnotationProperty .


###  http://www.w3.org/2000/01/rdf-schema#isDefinedBy
rdfs:isDefinedBy rdf:type owl:AnnotationProperty .


###  http://www.w3.org/2000/01/rdf-schema#label
rdfs:label rdf:type owl:AnnotationProperty .


###  http://www.w3.org/2000/01/rdf-schema#seeAlso
rdfs:seeAlso rdf:type owl:AnnotationProperty .


#################################################################
#    Object Properties
#################################################################

###  http://purl.oclc.org/NET/ssnx/qu/qu#baseDimension
qu:baseDimension rdf:type owl:ObjectProperty ;
                 rdfs:range qu:QuantityKind ;
                 dc:source "skos:exactMatch 'baseDimension' [SysML 1.2-QUDV] http://www.omgwiki.org/OMGSysML/doku.php?id=sysml-qudv:quantities_units_dimensions_values_qudv" ;
                 rdfs:comment "A Reference to the QuantityKind that represents the base quantity dimension in the factor." ;
                 rdfs:isDefinedBy "http://purl.oclc.org/NET/ssnx/qu" ;
                 rdfs:label "baseDimension" ;
                 rdfs:seeAlso "http://www.omgsysml.org/qudv#Dimension" .


###  http://purl.oclc.org/NET/ssnx/qu/qu#baseQuantityKind
qu:baseQuantityKind rdf:type owl:ObjectProperty ;
                    rdfs:subPropertyOf qu:quantityKind ;
                    rdf:type owl:AsymmetricProperty ;
                    rdfs:range qu:QuantityKind ;
                    dc:source "skos:exactMatch 'baseQuantityKind' [SysML 1.2-QUDV] http://www.omgwiki.org/OMGSysML/doku.php?id=sysml-qudv:quantities_units_dimensions_values_qudv" ;
                    rdfs:comment "Ordered set of QuantityKind that specifies the base quantities of the system of quantities. This is a subset of the complete quantityKind list. The base quantities define the basis for the quantity dimension of a kind of quantity." ;
                    rdfs:isDefinedBy "http://purl.oclc.org/NET/ssnx/qu" ;
                    rdfs:label "baseQuantityKind" ;
                    rdfs:seeAlso "http://www.omgsysml.org/qudv#Dimension" .


###  http://purl.oclc.org/NET/ssnx/qu/qu#baseUnit
qu:baseUnit rdf:type owl:ObjectProperty ;
            rdfs:subPropertyOf qu:unit ;
            rdf:type owl:AsymmetricProperty ;
            rdfs:range qu:Unit ;
            dc:source "skos:exactMatch 'baseUnit' [SysML 1.2-QUDV] http://www.omgwiki.org/OMGSysML/doku.php?id=sysml-qudv:quantities_units_dimensions_values_qudv" ;
            rdfs:comment "Ordered set of Unit that specifies the base units of the system of units. A \"base unit\" is defined in [VIM] as a \"measurement unit that is adopted by convention for a base quantity,\" i.e. it is the (preferred) unit in which base quantities of the associated systemOfQuantities are expressed." ;
            rdfs:isDefinedBy "http://purl.oclc.org/NET/ssnx/qu" ;
            rdfs:label "baseUnit" ;
            rdfs:seeAlso "http://www.omgsysml.org/qudv#Dimension" .


###  http://purl.oclc.org/NET/ssnx/qu/qu#dimension
qu:dimension rdf:type owl:ObjectProperty ;
             rdfs:range qu:Dimension ;
             dc:source "skos:exactMatch 'dimension' [SysML 1.2-QUDV] http://www.omgwiki.org/OMGSysML/doku.php?id=sysml-qudv:quantities_units_dimensions_values_qudv" ;
             rdfs:comment "Derived ordered set of Dimension. The actual dimension of a QuantityKind depends on the list of baseQuantityKind that are specified in an actual SystemOfQuantities, see the DerivedDimensions constraint." ;
             rdfs:isDefinedBy "http://purl.oclc.org/NET/ssnx/qu" ;
             rdfs:label "dimension" ;
             rdfs:seeAlso "http://www.omgsysml.org/qudv#Quantity" .


###  http://purl.oclc.org/NET/ssnx/qu/qu#dimensionFactor
qu:dimensionFactor rdf:type owl:ObjectProperty ,
                            owl:AsymmetricProperty ;
                   rdfs:range qu:DimensionFactor ;
                   dc:source "skos:exactMatch 'factor' [SysML 1.2-QUDV] http://www.omgwiki.org/OMGSysML/doku.php?id=sysml-qudv:quantities_units_dimensions_values_qudv" ;
                   rdfs:comment "Rational number that specifies the factor in the dimension conversion relationship." ;
                   rdfs:isDefinedBy "http://purl.oclc.org/NET/ssnx/qu" ;
                   rdfs:label "dimension factor" ;
                   rdfs:seeAlso "http://www.omgsysml.org/qudv#Dimension" .


###  http://purl.oclc.org/NET/ssnx/qu/qu#factorQuantityKind
qu:factorQuantityKind rdf:type owl:ObjectProperty ,
                               owl:AsymmetricProperty ;
                      rdfs:range qu:QuantityKind ;
                      dc:source "skos:exactMatch 'quantityKind' [SysML 1.2-QUDV] http://www.omgwiki.org/OMGSysML/doku.php?id=sysml-qudv:quantities_units_dimensions_values_qudv" ;
                      rdfs:comment "Specification of the associated QuantityKind." ;
                      rdfs:isDefinedBy "http://purl.oclc.org/NET/ssnx/qu" ;
                      rdfs:label "factorQuantityKind" ;
                      rdfs:seeAlso "http://www.omgsysml.org/qudv#Quantity" .


###  http://purl.oclc.org/NET/ssnx/qu/qu#generalQuantityKind
qu:generalQuantityKind rdf:type owl:ObjectProperty ;
                       owl:inverseOf qu:specificQuantityKind ;
                       rdf:type owl:IrreflexiveProperty ;
                       rdfs:range qu:QuantityKind ;
                       dc:source "skos:exactMatch 'general' [SysML 1.2-QUDV] http://www.omgwiki.org/OMGSysML/doku.php?id=sysml-qudv:quantities_units_dimensions_values_qudv" ,
                                 "skos:exactMatch 'generalization' [QUDT] http:qudt.org" ;
                       rdfs:comment "A generalization relationship between two kinds of quantities." ;
                       rdfs:isDefinedBy "http://purl.oclc.org/NET/ssnx/qu" ;
                       rdfs:label "generalQuantityKind" ;
                       rdfs:seeAlso "http://www.omgsysml.org/qudv#Quantity" .


###  http://purl.oclc.org/NET/ssnx/qu/qu#prefix
qu:prefix rdf:type owl:ObjectProperty ,
                   owl:AsymmetricProperty ,
                   owl:IrreflexiveProperty ;
          rdfs:range qu:Prefix ;
          dc:source "skos:exactMatch 'prefix' [SysML 1.2-QUDV] http://www.omgwiki.org/OMGSysML/doku.php?id=sysml-qudv:quantities_units_dimensions_values_qudv" ;
          rdfs:comment "Ordered set of Prefix that specifies the prefixes for multiples and submultiples of units in the system" ;
          rdfs:isDefinedBy "http://purl.oclc.org/NET/ssnx/qu" ;
          rdfs:label "prefix" ;
          rdfs:seeAlso "http://www.omgsysml.org/qudv#Unit" .


###  http://purl.oclc.org/NET/ssnx/qu/qu#propertyType
qu:propertyType rdf:type owl:ObjectProperty ,
                         owl:AsymmetricProperty ;
                rdfs:range qu:PropertyKind ;
                rdfs:comment "Specification of the associated ProeprtyType." ;
                rdfs:isDefinedBy "http://purl.oclc.org/NET/ssnx/qu" ;
                rdfs:label "propertyType" ;
                rdfs:seeAlso "http://www.omgsysml.org/qudv#Quantity" .


###  http://purl.oclc.org/NET/ssnx/qu/qu#quantityComponent
qu:quantityComponent rdf:type owl:ObjectProperty ,
                              owl:AsymmetricProperty ;
                     rdfs:range qu:QuantityKind ;
                     dc:source "skos:exactMatch 'quantityKind' [SysML 1.2-QUDV] http://www.omgwiki.org/OMGSysML/doku.php?id=sysml-qudv:quantities_units_dimensions_values_qudv" ;
                     rdfs:comment "Quantities attached to a system." ;
                     rdfs:isDefinedBy "http://purl.oclc.org/NET/ssnx/qu" ;
                     rdfs:label "quantityComponent" ;
                     rdfs:seeAlso "http://www.omgsysml.org/qudv#Dimension" .


###  http://purl.oclc.org/NET/ssnx/qu/qu#quantityKind
qu:quantityKind rdf:type owl:ObjectProperty ;
                owl:inverseOf qu:unitKind ;
                rdf:type owl:AsymmetricProperty ;
                rdfs:range qu:QuantityKind ;
                dc:source "skos:exactMatch 'quantityKind' [SysML 1.2-QUDV] http://www.omgwiki.org/OMGSysML/doku.php?id=sysml-qudv:quantities_units_dimensions_values_qudv" ;
                rdfs:comment "Specification of the associated QuantityKind." ;
                rdfs:isDefinedBy "http://purl.oclc.org/NET/ssnx/qu" ;
                rdfs:label "quantityKind" ;
                rdfs:seeAlso "http://www.omgsysml.org/qudv#Quantity" .


###  http://purl.oclc.org/NET/ssnx/qu/qu#quantityKindFactor
qu:quantityKindFactor rdf:type owl:ObjectProperty ,
                               owl:AsymmetricProperty ;
                      rdfs:range qu:QuantityKindFactor ;
                      dc:source "skos:exactMatch 'factor' [SysML 1.2-QUDV] http://www.omgwiki.org/OMGSysML/doku.php?id=sysml-qudv:quantities_units_dimensions_values_qudv" ;
                      rdfs:comment "Rational number that specifies the factor in the quantity conversion relationship." ;
                      rdfs:isDefinedBy "http://purl.oclc.org/NET/ssnx/qu" ;
                      rdfs:label "quantity kind factor" ;
                      rdfs:seeAlso "http://www.omgsysml.org/qudv#Quantity" .


###  http://purl.oclc.org/NET/ssnx/qu/qu#referenceUnit
qu:referenceUnit rdf:type owl:ObjectProperty ,
                          owl:AsymmetricProperty ;
                 rdfs:range qu:Unit ;
                 dc:source "skos:exactMatch 'referenceUnit' [SysML 1.2-QUDV] http://www.omgwiki.org/OMGSysML/doku.php?id=sysml-qudv:quantities_units_dimensions_values_qudv" ;
                 rdfs:comment "Specifies the unit with respect to which the ConversionBasedUnit is defined." ;
                 rdfs:isDefinedBy "http://purl.oclc.org/NET/ssnx/qu" ;
                 rdfs:label "referenceUnit" ;
                 rdfs:seeAlso "http://www.omgsysml.org/qudv#Unit" .


###  http://purl.oclc.org/NET/ssnx/qu/qu#scale
qu:scale rdf:type owl:ObjectProperty ,
                  owl:AsymmetricProperty ,
                  owl:IrreflexiveProperty ;
         rdfs:range qu:Scale ;
         dc:source "skos:exactMatch 'scale' [SysML 1.2-QUDV] http://www.omgwiki.org/OMGSysML/doku.php?id=sysml-qudv:quantities_units_dimensions_values_qudv" ;
         rdfs:comment "Specification of a Scale that is associated to the QuantityKind." ;
         rdfs:isDefinedBy "http://purl.oclc.org/NET/ssnx/qu" ;
         rdfs:label "scale" ;
         rdfs:seeAlso "http://www.omgsysml.org/qudv#Scale" .


###  http://purl.oclc.org/NET/ssnx/qu/qu#scaleValueDefinition
qu:scaleValueDefinition rdf:type owl:ObjectProperty ,
                                 owl:AsymmetricProperty ,
                                 owl:IrreflexiveProperty ;
                        rdfs:range qu:ScaleValueDefinition ;
                        dc:source "skos:exactMatch 'valueDefinition' [SysML 1.2-QUDV] http://www.omgwiki.org/OMGSysML/doku.php?id=sysml-qudv:quantities_units_dimensions_values_qudv" ;
                        rdfs:comment "Ordered set of ScaleValueDefinition that specifies the defined numerical value(s) and textual definition(s) for the measurement scale." ;
                        rdfs:isDefinedBy "http://purl.oclc.org/NET/ssnx/qu" ;
                        rdfs:label "scaleValueDefinition" ;
                        rdfs:seeAlso "http://www.omgsysml.org/qudv#Scale" .


###  http://purl.oclc.org/NET/ssnx/qu/qu#specificQuantityKind
qu:specificQuantityKind rdf:type owl:ObjectProperty ,
                                 owl:IrreflexiveProperty ;
                        rdfs:range qu:QuantityKind ,
                                   qu:SpecializedQuantityKind ;
                        dc:source "skos:exactMatch 'specific' [SysML 1.2-QUDV] http://www.omgwiki.org/OMGSysML/doku.php?id=sysml-qudv:quantities_units_dimensions_values_qudv" ;
                        rdfs:comment "A specialization relationship between two kinds of quantities." ;
                        rdfs:isDefinedBy "http://purl.oclc.org/NET/ssnx/qu" ;
                        rdfs:label "specificQuantityKind" ;
                        rdfs:seeAlso "http://www.omgsysml.org/qudv#Quantity" .


###  http://purl.oclc.org/NET/ssnx/qu/qu#systemOfQuantities
qu:systemOfQuantities rdf:type owl:ObjectProperty ;
                      rdfs:range qu:SystemOfQuantities ;
                      dc:source "skos:exactMatch 'systemOfQuantities' [SysML 1.2-QUDV] http://www.omgwiki.org/OMGSysML/doku.php?id=sysml-qudv:quantities_units_dimensions_values_qudv" ;
                      rdfs:comment "Reference to the SystemOfQuantities for which the units are specified." ;
                      rdfs:isDefinedBy "http://purl.oclc.org/NET/ssnx/qu" ;
                      rdfs:label "systemOfQuantities" ;
                      rdfs:seeAlso "http://www.omgsysml.org/qudv#Dimension" .


###  http://purl.oclc.org/NET/ssnx/qu/qu#unit
qu:unit rdf:type owl:ObjectProperty ,
                 owl:AsymmetricProperty ;
        rdfs:range qu:Unit ;
        dc:source "skos:exactMatch 'quantityKind' [SysML 1.2-QUDV] http://www.omgwiki.org/OMGSysML/doku.php?id=sysml-qudv:quantities_units_dimensions_values_qudv" ;
        rdfs:comment "Specification of the associated Unit." ;
        rdfs:isDefinedBy "http://purl.oclc.org/NET/ssnx/qu" ;
        rdfs:label "unit" ;
        rdfs:seeAlso "http://www.omgsysml.org/qudv#Unit" .


###  http://purl.oclc.org/NET/ssnx/qu/qu#unitComponent
qu:unitComponent rdf:type owl:ObjectProperty ,
                          owl:AsymmetricProperty ;
                 rdfs:range qu:Unit ;
                 dc:source "skos:exactMatch 'unit' [SysML 1.2-QUDV] http://www.omgwiki.org/OMGSysML/doku.php?id=sysml-qudv:quantities_units_dimensions_values_qudv" ;
                 rdfs:comment "Ordered set of Unit that specifies the units that are known in the system." ;
                 rdfs:isDefinedBy "http://purl.oclc.org/NET/ssnx/qu" ;
                 rdfs:label "unitComponent" ;
                 rdfs:seeAlso "http://www.omgsysml.org/qudv#Dimension" .


###  http://purl.oclc.org/NET/ssnx/qu/qu#unitFactor
qu:unitFactor rdf:type owl:ObjectProperty ,
                       owl:AsymmetricProperty ;
              rdfs:range qu:UnitFactor ;
              dc:source "skos:exactMatch 'factor' [SysML 1.2-QUDV] http://www.omgwiki.org/OMGSysML/doku.php?id=sysml-qudv:quantities_units_dimensions_values_qudv" ;
              rdfs:comment "Rational number that specifies the factor in the unit conversion relationship." ;
              rdfs:isDefinedBy "http://purl.oclc.org/NET/ssnx/qu" ;
              rdfs:label "unit factor" ;
              rdfs:seeAlso "http://www.omgsysml.org/qudv#Unit" .


###  http://purl.oclc.org/NET/ssnx/qu/qu#unitKind
qu:unitKind rdf:type owl:ObjectProperty ,
                     owl:AsymmetricProperty ;
            rdfs:range qu:Unit ;
            rdfs:comment "Specification of the associated Unit \"Kind\"." ;
            rdfs:isDefinedBy "http://purl.oclc.org/NET/ssnx/qu" ;
            rdfs:label "unitKind" ;
            rdfs:seeAlso "http://www.omgsysml.org/qudv#Unit" .


#################################################################
#    Data properties
#################################################################

###  http://purl.oclc.org/NET/ssnx/qu/qu#code
qu:code rdf:type owl:DatatypeProperty ;
        rdfs:range xsd:string ;
        dc:description "short symbolic name"^^xsd:string ;
        dc:source "skos:closeMatch 'code' [QUDT] http://qudt.org/" ;
        rdfs:comment "A code is a string that uniquely identifies an individual." ;
        rdfs:isDefinedBy "http://purl.oclc.org/NET/ssnx/qu" ;
        rdfs:label "code" ;
        rdfs:seeAlso "http://www.omgsysml.org/qudv#Data" .


###  http://purl.oclc.org/NET/ssnx/qu/qu#conversionFactor
qu:conversionFactor rdf:type owl:DatatypeProperty ;
                    rdfs:range xsd:double ;
                    dc:source "skos:exactMatch 'factor' [SysML 1.2-QUDV] http://www.omgwiki.org/OMGSysML/doku.php?id=sysml-qudv:quantities_units_dimensions_values_qudv" ;
                    rdfs:comment "Rational number that specifies the factor in the unit conversion relationship." ;
                    rdfs:isDefinedBy "http://purl.oclc.org/NET/ssnx/qu" ;
                    rdfs:label "conversionFactor" ;
                    rdfs:seeAlso "http://www.omgsysml.org/qudv#Data" .


###  http://purl.oclc.org/NET/ssnx/qu/qu#conversionOffset
qu:conversionOffset rdf:type owl:DatatypeProperty ;
                    rdfs:range xsd:double ;
                    dc:source "skos:exactMatch 'offset' [SysML 1.2-QUDV] http://www.omgwiki.org/OMGSysML/doku.php?id=sysml-qudv:quantities_units_dimensions_values_qudv" ;
                    rdfs:comment "Rational number that specifies the offset in the unit conversion relationship." ;
                    rdfs:isDefinedBy "http://purl.oclc.org/NET/ssnx/qu" ;
                    rdfs:label "conversionOffset" ;
                    rdfs:seeAlso "http://www.omgsysml.org/qudv#Data" .


###  http://purl.oclc.org/NET/ssnx/qu/qu#definitionURI
qu:definitionURI rdf:type owl:DatatypeProperty ,
                          owl:FunctionalProperty ;
                 rdfs:range xsd:string ;
                 dc:description "URI that contains an authoritative definition of the referent thing"^^xsd:string ;
                 dc:source "skos:exactMatch 'definitionURI' [SysML 1.2-QUDV] http://www.omgwiki.org/OMGSysML/doku.php?id=sysml-qudv:quantities_units_dimensions_values_qudv" ;
                 rdfs:comment "URI that references an external definition." ;
                 rdfs:isDefinedBy "http://purl.oclc.org/NET/ssnx/qu" ;
                 rdfs:label "definitionURI" ;
                 rdfs:seeAlso "http://www.omgsysml.org/qudv#Data" .


###  http://purl.oclc.org/NET/ssnx/qu/qu#description
qu:description rdf:type owl:DatatypeProperty ;
               rdfs:range xsd:string ;
               dc:source "skos:exactMatch 'description' [SysML 1.2-QUDV] http://www.omgwiki.org/OMGSysML/doku.php?id=sysml-qudv:quantities_units_dimensions_values_qudv" ;
               rdfs:comment "Textual description" ;
               rdfs:isDefinedBy "http://purl.oclc.org/NET/ssnx/qu" ;
               rdfs:label "description" ;
               rdfs:seeAlso "http://www.omgsysml.org/qudv#Data" .


###  http://purl.oclc.org/NET/ssnx/qu/qu#exponent
qu:exponent rdf:type owl:DatatypeProperty ;
            rdfs:range xsd:double ;
            dc:source "skos:exactMatch 'exponent' [SysML 1.2-QUDV] http://www.omgwiki.org/OMGSysML/doku.php?id=sysml-qudv:quantities_units_dimensions_values_qudv" ;
            rdfs:comment "Rational number that specifies the exponent of the power to which the unit is raised." ;
            rdfs:isDefinedBy "http://purl.oclc.org/NET/ssnx/qu" ;
            rdfs:label "exponent" ;
            rdfs:seeAlso "http://www.omgsysml.org/qudv#Data" .


###  http://purl.oclc.org/NET/ssnx/qu/qu#expression
qu:expression rdf:type owl:DatatypeProperty ;
              rdfs:range xsd:string ;
              dc:source "skos:exactMatch 'expression' [SysML 1.2-QUDV] http://www.omgwiki.org/OMGSysML/doku.php?id=sysml-qudv:quantities_units_dimensions_values_qudv" ;
              rdfs:comment "Specifies the unit conversion relationship in some expression syntax." ;
              rdfs:isDefinedBy "http://purl.oclc.org/NET/ssnx/qu" ;
              rdfs:label "conversionExpression" ;
              rdfs:seeAlso "http://www.omgsysml.org/qudv#Data" .


###  http://purl.oclc.org/NET/ssnx/qu/qu#name
qu:name rdf:type owl:DatatypeProperty ,
                 owl:FunctionalProperty ;
        rdfs:range xsd:string ;
        dc:description "human-readable word or sequence of words by which a thing is known"^^xsd:string ;
        dc:source "skos:exactMatch 'name' [SysML 1.2-QUDV] http://www.omgwiki.org/OMGSysML/doku.php?id=sysml-qudv:quantities_units_dimensions_values_qudv" ;
        rdfs:isDefinedBy "http://purl.oclc.org/NET/ssnx/qu" ;
        rdfs:label "name" ;
        rdfs:seeAlso "http://www.omgsysml.org/qudv#Data" .


###  http://purl.oclc.org/NET/ssnx/qu/qu#numericalValue
qu:numericalValue rdf:type owl:DatatypeProperty ;
                  rdfs:range xsd:double ;
                  dc:source "skos:exactMatch 'value' [SysML 1.2-QUDV] http://www.omgwiki.org/OMGSysML/doku.php?id=sysml-qudv:quantities_units_dimensions_values_qudv" ;
                  rdfs:comment "Specifies the numerical value." ;
                  rdfs:isDefinedBy "http://purl.oclc.org/NET/ssnx/qu" ;
                  rdfs:label "numericalValue" ;
                  rdfs:seeAlso "http://www.omgsysml.org/qudv#Data" .


###  http://purl.oclc.org/NET/ssnx/qu/qu#symbol
qu:symbol rdf:type owl:DatatypeProperty ;
          rdfs:range xsd:string ;
          dc:description "short symbolic name"^^xsd:string ;
          dc:source "skos:exactMatch 'symbol' [SysML 1.2-QUDV] http://www.omgwiki.org/OMGSysML/doku.php?id=sysml-qudv:quantities_units_dimensions_values_qudv" ;
          rdfs:comment "Short symbolic name." ;
          rdfs:isDefinedBy "http://purl.oclc.org/NET/ssnx/qu" ;
          rdfs:label "symbol" ;
          rdfs:seeAlso "http://www.omgsysml.org/qudv#Data" .


###  http://purl.oclc.org/NET/ssnx/qu/qu#symbolicExpression
qu:symbolicExpression rdf:type owl:DatatypeProperty ;
                      rdfs:range xsd:string ;
                      dc:source "skos:exactMatch 'symbolicExpression' [SysML 1.2-QUDV] http://www.omgwiki.org/OMGSysML/doku.php?id=sysml-qudv:quantities_units_dimensions_values_qudv" ;
                      rdfs:comment "Symbolic expression of the quantity dimension's product of powers, in terms of symbols of the kinds of quantity that represent the base kinds of quantity and their exponents." ;
                      rdfs:isDefinedBy "http://purl.oclc.org/NET/ssnx/qu" ;
                      rdfs:label "symbolicExpression" ;
                      rdfs:seeAlso "http://www.omgsysml.org/qudv#Data" .


###  http://purl.oclc.org/NET/ssnx/qu/qu#unitMultipleFactor
qu:unitMultipleFactor rdf:type owl:DatatypeProperty ,
                               owl:FunctionalProperty ;
                      rdfs:range xsd:double ;
                      dc:source "skos:exactMatch 'factor' [SysML 1.2-QUDV] http://www.omgwiki.org/OMGSysML/doku.php?id=sysml-qudv:quantities_units_dimensions_values_qudv" ;
                      rdfs:comment "Specifies the multiple or submultiple multiplication factor." ;
                      rdfs:isDefinedBy "http://purl.oclc.org/NET/ssnx/qu" ;
                      rdfs:label "unitMultipleFactor" ;
                      rdfs:seeAlso "http://www.omgsysml.org/qudv#Data" .


#################################################################
#    Classes
#################################################################

###  http://purl.oclc.org/NET/ssnx/qu/qu#ConversionBasedUnit
qu:ConversionBasedUnit rdf:type owl:Class ;
                       rdfs:subClassOf qu:Unit ,
                                       [ rdf:type owl:Restriction ;
                                         owl:onProperty qu:referenceUnit ;
                                         owl:qualifiedCardinality "1"^^xsd:nonNegativeInteger ;
                                         owl:onClass qu:Unit
                                       ] ;
                       dc:source "skos:exactMatch 'ConversionBasedUnit' [SysML 1.2-QUDV] http://www.omgwiki.org/OMGSysML/doku.php?id=sysml-qudv:quantities_units_dimensions_values_qudv" ;
                       rdfs:comment """A ConversionBasedUnit is an abstract classifier that is a Unit that represents a measurement unit that is defined with respect to
another reference unit through an explicit conversion relationship.""" ;
                       rdfs:isDefinedBy "http://purl.oclc.org/NET/ssnx/qu" ;
                       rdfs:label "ConversionBasedUnit" ;
                       rdfs:seeAlso "http://www.omgsysml.org/qudv#Unit" .


###  http://purl.oclc.org/NET/ssnx/qu/qu#DerivedQuantityKind
qu:DerivedQuantityKind rdf:type owl:Class ;
                       rdfs:subClassOf qu:QuantityKind ,
                                       [ rdf:type owl:Restriction ;
                                         owl:onProperty qu:quantityKindFactor ;
                                         owl:someValuesFrom qu:QuantityKindFactor
                                       ] ;
                       dc:source "skos:exactMatch 'DerivedQuantityKind ' [SysML 1.2-QUDV] http://www.omgwiki.org/OMGSysML/doku.php?id=sysml-qudv:quantities_units_dimensions_values_qudv" ;
                       rdfs:comment """A DerivedQuantityKind is a QuantityKind that represents a kind of quantity that is defined as a product of powers of one or
more other kinds of quantity. A DerivedQuantityKind may also be used to define a synonym kind of quantity for another kind
of quantity.
For example \"velocity\" can be specified as the product of \"length\" to the power one times \"time\" to the power minus one, and
subsequently \"speed\" can be specified as \"velocity\" to the power one.""" ;
                       rdfs:isDefinedBy "http://purl.oclc.org/NET/ssnx/qu" ;
                       rdfs:label "DerivedQuantityKind" ;
                       rdfs:seeAlso "http://www.omgsysml.org/qudv#Quantity" .


###  http://purl.oclc.org/NET/ssnx/qu/qu#DerivedUnit
qu:DerivedUnit rdf:type owl:Class ;
               rdfs:subClassOf qu:Unit ,
                               [ rdf:type owl:Restriction ;
                                 owl:onProperty qu:unitFactor ;
                                 owl:someValuesFrom qu:UnitFactor
                               ] ;
               dc:source "skos:exactMatch 'DerivedUnit' [SysML 1.2-QUDV] http://www.omgwiki.org/OMGSysML/doku.php?id=sysml-qudv:quantities_units_dimensions_values_qudv" ;
               rdfs:comment """A DerivedUnit is a Unit that represents a measurement unit that is defined as a product of powers of one or more other
measurement units.
For example the measurement unit \"metre per second\" for \"velocity\" is specified as the product of \"metre\" to the power one
times \"second\" to the power minus one""" ;
               rdfs:isDefinedBy "http://purl.oclc.org/NET/ssnx/qu" ;
               rdfs:label "DerivedUnit" ;
               rdfs:seeAlso "http://www.omgsysml.org/qudv#Unit" .


###  http://purl.oclc.org/NET/ssnx/qu/qu#Dimension
qu:Dimension rdf:type owl:Class ;
             rdfs:subClassOf [ owl:intersectionOf ( [ rdf:type owl:Restriction ;
                                                      owl:onProperty qu:dimensionFactor ;
                                                      owl:allValuesFrom qu:DimensionFactor
                                                    ]
                                                    [ rdf:type owl:Restriction ;
                                                      owl:onProperty qu:symbolicExpression ;
                                                      owl:qualifiedCardinality "1"^^xsd:nonNegativeInteger ;
                                                      owl:onDataRange xsd:string
                                                    ]
                                                  ) ;
                               rdf:type owl:Class
                             ] ;
             dc:source "skos:exactMatch 'Dimension' [SysML 1.2-QUDV] http://www.omgwiki.org/OMGSysML/doku.php?id=sysml-qudv:quantities_units_dimensions_values_qudv" ;
             rdfs:comment """A Dimension represents the [VIM] concept of 'quantity dimension' that is defined as 'expression of the dependence of a quantity on the base quantities of a system of quantities as a product of powers of factors corresponding to the base quantities, omitting any numerical factor.'

For example in the ISQ the quantity dimension of 'force' is denoted by dim F = Lï¿½Mï¿½T^2, where 'F' is the symbol for 'force', and 'L', 'M', 'T' are the symbols for the ISQ base quantities 'length', 'mass' and 'time' respectively.

The Dimension of any QuantityKind can be derived through the algorithm that is defined in C.5.3.20 with SystemOfQuantities. The actual Dimension for a given QuantityKind depends on the choice of baseQuantityKind specified in a SystemOfQuantities.""" ;
             rdfs:isDefinedBy "http://purl.oclc.org/NET/ssnx/qu" ;
             rdfs:label "Dimension" ;
             rdfs:seeAlso "http://www.omgsysml.org/qudv#Dimension" .


###  http://purl.oclc.org/NET/ssnx/qu/qu#DimensionFactor
qu:DimensionFactor rdf:type owl:Class ;
                   rdfs:subClassOf [ rdf:type owl:Restriction ;
                                     owl:onProperty qu:baseDimension ;
                                     owl:qualifiedCardinality "1"^^xsd:nonNegativeInteger ;
                                     owl:onClass qu:QuantityKind
                                   ] ;
                   dc:source "skos:exactMatch 'DimensionFactor' [SysML 1.2-QUDV] http://www.omgwiki.org/OMGSysML/doku.php?id=sysml-qudv:quantities_units_dimensions_values_qudv" ;
                   rdfs:comment "A DimensionFactor represents a factor in the product of powers that defines a Dimension." ;
                   rdfs:isDefinedBy "http://purl.oclc.org/NET/ssnx/qu" ;
                   rdfs:label "DimensionFactor" ;
                   rdfs:seeAlso "http://www.omgsysml.org/qudv#Dimension" .


###  http://purl.oclc.org/NET/ssnx/qu/qu#GeneralConversionUnit
qu:GeneralConversionUnit rdf:type owl:Class ;
                         rdfs:subClassOf qu:ConversionBasedUnit ,
                                         [ rdf:type owl:Restriction ;
                                           owl:onProperty qu:expression ;
                                           owl:qualifiedCardinality "1"^^xsd:nonNegativeInteger ;
                                           owl:onDataRange xsd:string
                                         ] ;
                         dc:source "skos:exactMatch 'GeneralConversionUnit' [SysML 1.2-QUDV] http://www.omgwiki.org/OMGSysML/doku.php?id=sysml-qudv:quantities_units_dimensions_values_qudv" ;
                         rdfs:comment """A GeneralConversionUnit is a ConversionBasedUnit that represents a measurement unit that is defined with respect to another
reference measurement unit through a conversion relationship expressed in some syntax through a general mathematical
expression.
The unit conversion relationship is defined by the following equation:
valueRU / valueCU = f(valueRU, valueCU)
where:
valueRU is the quantity value expressed in the referenceUnit, and,
valueCU is the quantity value expressed in the GeneralConversionUnit, and,
f(valueRU, valueCU) is a mathematical expression that includes valueRU and valueCU.""" ;
                         rdfs:isDefinedBy "http://purl.oclc.org/NET/ssnx/qu" ;
                         rdfs:label "GeneralConversionUnit" ;
                         rdfs:seeAlso "http://www.omgsysml.org/qudv#Unit" .


###  http://purl.oclc.org/NET/ssnx/qu/qu#LinearConversionUnit
qu:LinearConversionUnit rdf:type owl:Class ;
                        rdfs:subClassOf qu:ConversionBasedUnit ,
                                        [ rdf:type owl:Restriction ;
                                          owl:onProperty qu:conversionFactor ;
                                          owl:qualifiedCardinality "1"^^xsd:nonNegativeInteger ;
                                          owl:onDataRange xsd:double
                                        ] ;
                        dc:source "skos:exactMatch 'LinearConversionUnit' [SysML 1.2-QUDV] http://www.omgwiki.org/OMGSysML/doku.php?id=sysml-qudv:quantities_units_dimensions_values_qudv" ;
                        rdfs:comment """A LinearConversionUnit is a ConversionBasedUnit that represents a measurement unit that is defined with respect to another
measurement reference unit through a linear conversion relationship with a conversion factor.
The unit conversion relationship is defined by the following equation:
valueRU = factor · valueCU,
where:
valueRU is the quantity value expressed in the referenceUnit, and,
valueCU is the quantity value expressed in the LinearConversionUnit.""" ;
                        rdfs:isDefinedBy "http://purl.oclc.org/NET/ssnx/qu" ;
                        rdfs:label "LinearConversionUnit" ;
                        rdfs:seeAlso "http://www.omgsysml.org/qudv#Unit" .


###  http://purl.oclc.org/NET/ssnx/qu/qu#Prefix
qu:Prefix rdf:type owl:Class ;
          rdfs:subClassOf [ owl:intersectionOf ( [ rdf:type owl:Restriction ;
                                                   owl:onProperty qu:name ;
                                                   owl:qualifiedCardinality "1"^^xsd:nonNegativeInteger ;
                                                   owl:onDataRange xsd:string
                                                 ]
                                                 [ rdf:type owl:Restriction ;
                                                   owl:onProperty qu:symbol ;
                                                   owl:qualifiedCardinality "1"^^xsd:nonNegativeInteger ;
                                                   owl:onDataRange xsd:string
                                                 ]
                                                 [ rdf:type owl:Restriction ;
                                                   owl:onProperty qu:unitMultipleFactor ;
                                                   owl:qualifiedCardinality "1"^^xsd:nonNegativeInteger ;
                                                   owl:onDataRange xsd:double
                                                 ]
                                               ) ;
                            rdf:type owl:Class
                          ] ;
          dc:source "skos:exactMatch 'Prefix' [SysML 1.2-QUDV] http://www.omgwiki.org/OMGSysML/doku.php?id=sysml-qudv:quantities_units_dimensions_values_qudv" ;
          rdfs:comment """A Prefix represents a named multiple or submultiple multiplication factor used in the specification of a PrefixedUnit. A
SystemOfUnits may specify a set of prefixes.""" ;
          rdfs:isDefinedBy "http://purl.oclc.org/NET/ssnx/qu" ;
          rdfs:label "Prefix" ;
          rdfs:seeAlso "http://www.omgsysml.org/qudv#Unit" .


###  http://purl.oclc.org/NET/ssnx/qu/qu#PrefixedUnit
qu:PrefixedUnit rdf:type owl:Class ;
                rdfs:subClassOf qu:ConversionBasedUnit ,
                                [ rdf:type owl:Restriction ;
                                  owl:onProperty qu:prefix ;
                                  owl:qualifiedCardinality "1"^^xsd:nonNegativeInteger ;
                                  owl:onClass qu:Prefix
                                ] ;
                dc:source "skos:exactMatch 'Prefix' [SysML 1.2-QUDV] http://www.omgwiki.org/OMGSysML/doku.php?id=sysml-qudv:quantities_units_dimensions_values_qudv" ;
                rdfs:comment """A Prefix represents a named multiple or submultiple multiplication factor used in the specification of a PrefixedUnit. A
SystemOfUnits may specify a set of prefixes.""" ;
                rdfs:isDefinedBy "http://purl.oclc.org/NET/ssnx/qu" ;
                rdfs:label "PrefixedUnit" ;
                rdfs:seeAlso "http://www.omgsysml.org/qudv#Unit" .


###  http://purl.oclc.org/NET/ssnx/qu/qu#PropertyKind
qu:PropertyKind rdf:type owl:Class ;
                rdfs:comment "A PropertyKind  is a meta-property which helps to characterise categories of properties e.g. scalar, vector" ;
                rdfs:isDefinedBy "http://purl.oclc.org/NET/ssnx/qu" ;
                rdfs:label "PropertyKind " ;
                rdfs:seeAlso "http://www.omgsysml.org/qudv#Quantity" .


###  http://purl.oclc.org/NET/ssnx/qu/qu#QuantityKind
qu:QuantityKind rdf:type owl:Class ;
                rdfs:subClassOf [ owl:intersectionOf ( [ rdf:type owl:Restriction ;
                                                         owl:onProperty qu:scale ;
                                                         owl:maxQualifiedCardinality "1"^^xsd:nonNegativeInteger ;
                                                         owl:onClass qu:Scale
                                                       ]
                                                       [ rdf:type owl:Restriction ;
                                                         owl:onProperty qu:name ;
                                                         owl:qualifiedCardinality "1"^^xsd:nonNegativeInteger ;
                                                         owl:onDataRange xsd:string
                                                       ]
                                                       [ rdf:type owl:Restriction ;
                                                         owl:onProperty qu:symbol ;
                                                         owl:qualifiedCardinality "1"^^xsd:nonNegativeInteger ;
                                                         owl:onDataRange xsd:string
                                                       ]
                                                       [ rdf:type owl:Restriction ;
                                                         owl:onProperty qu:definitionURI ;
                                                         owl:maxQualifiedCardinality "1"^^xsd:nonNegativeInteger ;
                                                         owl:onDataRange xsd:string
                                                       ]
                                                       [ rdf:type owl:Restriction ;
                                                         owl:onProperty qu:description ;
                                                         owl:maxQualifiedCardinality "1"^^xsd:nonNegativeInteger ;
                                                         owl:onDataRange xsd:string
                                                       ]
                                                     ) ;
                                  rdf:type owl:Class
                                ] ;
                dc:source "skos:exactMatch 'QuantityKind' [SysML 1.2-QUDV] http://www.omgwiki.org/OMGSysML/doku.php?id=sysml-qudv:quantities_units_dimensions_values_qudv" ;
                rdfs:comment """A QuantityKind is an abstract classifier that represents the [VIM] concept of \"kind of quantity\" that is defined as \"aspect
common to mutually comparable quantities.\" A QuantityKind represents the essence of a quantity without any numerical
value or unit. Quantities of the same kind within a given system of quantities have the same quantity dimension. However,
quantities of the same dimension are not necessarily of the same kind.""" ;
                rdfs:isDefinedBy "http://purl.oclc.org/NET/ssnx/qu" ;
                rdfs:label "QuantityKind" ;
                rdfs:seeAlso "http://www.omgsysml.org/qudv#Quantity" .


###  http://purl.oclc.org/NET/ssnx/qu/qu#QuantityKindFactor
qu:QuantityKindFactor rdf:type owl:Class ;
                      rdfs:subClassOf [ owl:intersectionOf ( [ rdf:type owl:Restriction ;
                                                               owl:onProperty qu:factorQuantityKind ;
                                                               owl:qualifiedCardinality "1"^^xsd:nonNegativeInteger ;
                                                               owl:onClass qu:QuantityKind
                                                             ]
                                                             [ rdf:type owl:Restriction ;
                                                               owl:onProperty qu:exponent ;
                                                               owl:qualifiedCardinality "1"^^xsd:nonNegativeInteger ;
                                                               owl:onDataRange xsd:double
                                                             ]
                                                           ) ;
                                        rdf:type owl:Class
                                      ] ;
                      dc:source "skos:exactMatch 'QuantityKindFactor' [SysML 1.2-QUDV] http://www.omgwiki.org/OMGSysML/doku.php?id=sysml-qudv:quantities_units_dimensions_values_qudv" ;
                      rdfs:comment "A QuantityKindFactor represents a factor in the product of powers that defines a DerivedQuantityKind." ;
                      rdfs:isDefinedBy "http://purl.oclc.org/NET/ssnx/qu" ;
                      rdfs:label "QuantityKindFactor" ;
                      rdfs:seeAlso "http://www.omgsysml.org/qudv#Quantity" .


###  http://purl.oclc.org/NET/ssnx/qu/qu#Scale
qu:Scale rdf:type owl:Class ;
         rdfs:subClassOf [ owl:intersectionOf ( [ rdf:type owl:Restriction ;
                                                  owl:onProperty qu:scaleValueDefinition ;
                                                  owl:someValuesFrom qu:ScaleValueDefinition
                                                ]
                                                [ rdf:type owl:Restriction ;
                                                  owl:onProperty qu:unit ;
                                                  owl:maxQualifiedCardinality "1"^^xsd:nonNegativeInteger ;
                                                  owl:onClass qu:Unit
                                                ]
                                              ) ;
                           rdf:type owl:Class
                         ] ;
         dc:source "skos:exactMatch 'Scale' [SysML 1.2-QUDV] http://www.omgwiki.org/OMGSysML/doku.php?id=sysml-qudv:quantities_units_dimensions_values_qudv" ;
         rdfs:comment """A Scale represents the [VIM] concept of a \"measurement scale\" that is defined as an \"ordered set of quantity values of
quantities of a given kind of quantity used in ranking, according to magnitude, quantities of that kind.\" A Scale specifies one
or more fixed values that have a specific significance in the definition of the associating QuantityKind.
For example the \"thermodynamic temperature\" kind of quantity is defined by specifying the values of 0 and 273.16 kelvin as
the temperatures of absolute zero and the triple point of water respectively.
A Scale does not always need to specify a unit. For example the \"Rockwell C Hardness Scale\" or the \"Beaufort Wind Force
Scale\" are ordinal scales that do not have a particular associated unit. Similarly, subjective scales for a \"priority\" or \"risk\" kind
of quantity with e.g. value definitions 0 for \"low\", 1 for \"medium\" and 3 for \"high\" do not have a particular associated unit.""" ;
         rdfs:isDefinedBy "http://purl.oclc.org/NET/ssnx/qu" ;
         rdfs:label "Scale" ;
         rdfs:seeAlso "http://www.omgsysml.org/qudv#Scale" .


###  http://purl.oclc.org/NET/ssnx/qu/qu#ScaleValueDefinition
qu:ScaleValueDefinition rdf:type owl:Class ;
                        rdfs:subClassOf [ owl:intersectionOf ( [ rdf:type owl:Restriction ;
                                                                 owl:onProperty qu:description ;
                                                                 owl:qualifiedCardinality "1"^^xsd:nonNegativeInteger ;
                                                                 owl:onDataRange xsd:string
                                                               ]
                                                               [ rdf:type owl:Restriction ;
                                                                 owl:onProperty qu:numericalValue ;
                                                                 owl:qualifiedCardinality "1"^^xsd:nonNegativeInteger ;
                                                                 owl:onDataRange xsd:double
                                                               ]
                                                             ) ;
                                          rdf:type owl:Class
                                        ] ;
                        dc:source "skos:exactMatch 'ScaleValueDefinition' [SysML 1.2-QUDV] http://www.omgwiki.org/OMGSysML/doku.php?id=sysml-qudv:quantities_units_dimensions_values_qudv" ;
                        rdfs:comment "A ScaleValueDefinition represents a specific value for a measurement scale." ;
                        rdfs:isDefinedBy "http://purl.oclc.org/NET/ssnx/qu" ;
                        rdfs:label "ScaleValueDefinition" ;
                        rdfs:seeAlso "http://www.omgsysml.org/qudv#Scale" .


###  http://purl.oclc.org/NET/ssnx/qu/qu#SimpleQuantityKind
qu:SimpleQuantityKind rdf:type owl:Class ;
                      rdfs:subClassOf qu:QuantityKind ;
                      dc:source "skos:exactMatch 'SimpleQuantityKind' [SysML 1.2-QUDV] http://www.omgwiki.org/OMGSysML/doku.php?id=sysml-qudv:quantities_units_dimensions_values_qudv" ;
                      rdfs:comment """A SimpleQuantityKind is a QuantityKind that represents a kind of quantity that does not depend on any other QuantityKind.
Typically a base quantity would be specified as a SimpleQuantityKind.""" ;
                      rdfs:isDefinedBy "http://purl.oclc.org/NET/ssnx/qu" ;
                      rdfs:label "SimpleQuantityKind" ;
                      rdfs:seeAlso "http://www.omgsysml.org/qudv#Quantity" .


###  http://purl.oclc.org/NET/ssnx/qu/qu#SimpleUnit
qu:SimpleUnit rdf:type owl:Class ;
              rdfs:subClassOf qu:Unit ;
              dc:source "skos:exactMatch 'SimpleUnit' [SysML 1.2-QUDV] http://www.omgwiki.org/OMGSysML/doku.php?id=sysml-qudv:quantities_units_dimensions_values_qudv" ;
              rdfs:comment """A SimpleUnit is a Unit that represents a measurement unit that does not depend on any other Unit. Typically a base unit would
be specified as a SimpleUnit.""" ;
              rdfs:isDefinedBy "http://purl.oclc.org/NET/ssnx/qu" ;
              rdfs:label "SimpleUnit" ;
              rdfs:seeAlso "http://www.omgsysml.org/qudv#Unit" .


###  http://purl.oclc.org/NET/ssnx/qu/qu#SpecializedQuantityKind
qu:SpecializedQuantityKind rdf:type owl:Class ;
                           rdfs:subClassOf qu:QuantityKind ,
                                           [ rdf:type owl:Restriction ;
                                             owl:onProperty qu:generalQuantityKind ;
                                             owl:qualifiedCardinality "1"^^xsd:nonNegativeInteger ;
                                             owl:onClass qu:QuantityKind
                                           ] ;
                           dc:source "skos:exactMatch 'SpecializedQuantityKind' [SysML 1.2-QUDV] http://www.omgwiki.org/OMGSysML/doku.php?id=sysml-qudv:quantities_units_dimensions_values_qudv" ;
                           rdfs:comment """A SpecializedQuantityKind is a QuantityKind that represents a kind of quantity that is a specialization of another kind of
quantity.
For example, \"distance\", \"width\", \"depth\", \"radius\" and \"wavelength\" can all be specified as specializations of the \"length\"
SimpleQuantityKind.""" ;
                           rdfs:isDefinedBy "http://purl.oclc.org/NET/ssnx/qu" ;
                           rdfs:label "SpecializedQuantityKind" ;
                           rdfs:seeAlso "http://www.omgsysml.org/qudv#Quantity" .


###  http://purl.oclc.org/NET/ssnx/qu/qu#SystemOfQuantities
qu:SystemOfQuantities rdf:type owl:Class ;
                      rdfs:subClassOf [ owl:intersectionOf ( [ rdf:type owl:Restriction ;
                                                               owl:onProperty qu:dimension ;
                                                               owl:someValuesFrom qu:Dimension
                                                             ]
                                                             [ rdf:type owl:Restriction ;
                                                               owl:onProperty qu:quantityComponent ;
                                                               owl:someValuesFrom qu:QuantityKind
                                                             ]
                                                             [ rdf:type owl:Restriction ;
                                                               owl:onProperty qu:baseQuantityKind ;
                                                               owl:allValuesFrom qu:QuantityKind
                                                             ]
                                                             [ rdf:type owl:Restriction ;
                                                               owl:onProperty qu:name ;
                                                               owl:qualifiedCardinality "1"^^xsd:nonNegativeInteger ;
                                                               owl:onDataRange xsd:string
                                                             ]
                                                             [ rdf:type owl:Restriction ;
                                                               owl:onProperty qu:symbol ;
                                                               owl:qualifiedCardinality "1"^^xsd:nonNegativeInteger ;
                                                               owl:onDataRange xsd:string
                                                             ]
                                                             [ rdf:type owl:Restriction ;
                                                               owl:onProperty qu:definitionURI ;
                                                               owl:maxQualifiedCardinality "1"^^xsd:nonNegativeInteger ;
                                                               owl:onDataRange xsd:string
                                                             ]
                                                             [ rdf:type owl:Restriction ;
                                                               owl:onProperty qu:description ;
                                                               owl:maxQualifiedCardinality "1"^^xsd:nonNegativeInteger ;
                                                               owl:onDataRange xsd:string
                                                             ]
                                                           ) ;
                                        rdf:type owl:Class
                                      ] ;
                      dc:source "skos:exactMatch 'SystemOfQuantities' [SysML 1.2-QUDV] http://www.omgwiki.org/OMGSysML/doku.php?id=sysml-qudv:quantities_units_dimensions_values_qudv" ;
                      rdfs:comment """A SystemOfQuantities represents the [VIM] concept of 'system of quantities' that is defined as a 'set of quantities together with a set of non-contradictory equations relating those quantities'. It collects a list of QuantityKind that specifies the kinds of quantity that are known in the system.

The International System of Quantities (ISQ) is an example of a SystemOfQuantities, defined in ISO 31 and ISO/IEC 80000.""" ;
                      rdfs:isDefinedBy "http://purl.oclc.org/NET/ssnx/qu" ;
                      rdfs:label "SystemOfQuantities" ;
                      rdfs:seeAlso "http://www.omgsysml.org/qudv#Dimension" .


###  http://purl.oclc.org/NET/ssnx/qu/qu#SystemOfUnits
qu:SystemOfUnits rdf:type owl:Class ;
                 rdfs:subClassOf [ owl:intersectionOf ( [ rdf:type owl:Restriction ;
                                                          owl:onProperty qu:unitComponent ;
                                                          owl:someValuesFrom qu:Unit
                                                        ]
                                                        [ rdf:type owl:Restriction ;
                                                          owl:onProperty qu:baseUnit ;
                                                          owl:allValuesFrom qu:Unit
                                                        ]
                                                        [ rdf:type owl:Restriction ;
                                                          owl:onProperty qu:prefix ;
                                                          owl:allValuesFrom qu:Prefix
                                                        ]
                                                        [ rdf:type owl:Restriction ;
                                                          owl:onProperty qu:systemOfQuantities ;
                                                          owl:allValuesFrom qu:SystemOfQuantities
                                                        ]
                                                        [ rdf:type owl:Restriction ;
                                                          owl:onProperty qu:name ;
                                                          owl:qualifiedCardinality "1"^^xsd:nonNegativeInteger ;
                                                          owl:onDataRange xsd:string
                                                        ]
                                                        [ rdf:type owl:Restriction ;
                                                          owl:onProperty qu:symbol ;
                                                          owl:qualifiedCardinality "1"^^xsd:nonNegativeInteger ;
                                                          owl:onDataRange xsd:string
                                                        ]
                                                        [ rdf:type owl:Restriction ;
                                                          owl:onProperty qu:definitionURI ;
                                                          owl:maxQualifiedCardinality "1"^^xsd:nonNegativeInteger ;
                                                          owl:onDataRange xsd:string
                                                        ]
                                                        [ rdf:type owl:Restriction ;
                                                          owl:onProperty qu:description ;
                                                          owl:maxQualifiedCardinality "1"^^xsd:nonNegativeInteger ;
                                                          owl:onDataRange xsd:string
                                                        ]
                                                      ) ;
                                   rdf:type owl:Class
                                 ] ;
                 dc:source "skos:exactMatch 'SystemOfUnits' [SysML 1.2-QUDV] http://www.omgwiki.org/OMGSysML/doku.php?id=sysml-qudv:quantities_units_dimensions_values_qudv" ;
                 rdfs:comment "A SystemOfUnits represents the [VIM] concept of 'system of units' that is defined as 'set of base units and derived units, together with their multiples and submultiples, defined in accordance with given rules, for a given system of quantities'. It collects a list of Unit that are known in the system. A SysML SystemOfUnits only optionally defines multiples and submultiples." ;
                 rdfs:isDefinedBy "http://purl.oclc.org/NET/ssnx/qu" ;
                 rdfs:label "SystemOfUnits" ;
                 rdfs:seeAlso "http://www.omgsysml.org/qudv#Dimension" .


###  http://purl.oclc.org/NET/ssnx/qu/qu#Unit
qu:Unit rdf:type owl:Class ;
        rdfs:subClassOf [ owl:intersectionOf ( [ rdf:type owl:Restriction ;
                                                 owl:onProperty qu:quantityKind ;
                                                 owl:maxQualifiedCardinality "1"^^xsd:nonNegativeInteger ;
                                                 owl:onClass qu:QuantityKind
                                               ]
                                               [ rdf:type owl:Restriction ;
                                                 owl:onProperty qu:name ;
                                                 owl:qualifiedCardinality "1"^^xsd:nonNegativeInteger ;
                                                 owl:onDataRange xsd:string
                                               ]
                                               [ rdf:type owl:Restriction ;
                                                 owl:onProperty qu:symbol ;
                                                 owl:qualifiedCardinality "1"^^xsd:nonNegativeInteger ;
                                                 owl:onDataRange xsd:string
                                               ]
                                               [ rdf:type owl:Restriction ;
                                                 owl:onProperty qu:definitionURI ;
                                                 owl:maxQualifiedCardinality "1"^^xsd:nonNegativeInteger ;
                                                 owl:onDataRange xsd:string
                                               ]
                                               [ rdf:type owl:Restriction ;
                                                 owl:onProperty qu:description ;
                                                 owl:maxQualifiedCardinality "1"^^xsd:nonNegativeInteger ;
                                                 owl:onDataRange xsd:string
                                               ]
                                             ) ;
                          rdf:type owl:Class
                        ] ;
        dc:source "skos:exactMatch 'Unit' [SysML 1.2-QUDV] http://www.omgwiki.org/OMGSysML/doku.php?id=sysml-qudv:quantities_units_dimensions_values_qudv" ;
        rdfs:comment """A Unit is an abstract classifier that represents the [VIM] concept of \"measurement unit\" that is defined as \"real scalar quantity,
defined and adopted by convention, with which any other quantity of the same kind can be compared to express the ratio of the
two quantities as a number.\"""" ;
        rdfs:isDefinedBy "http://purl.oclc.org/NET/ssnx/qu" ;
        rdfs:label "Unit" ;
        rdfs:seeAlso "http://www.omgsysml.org/qudv#Unit" .


###  http://purl.oclc.org/NET/ssnx/qu/qu#UnitFactor
qu:UnitFactor rdf:type owl:Class ;
              rdfs:subClassOf [ owl:intersectionOf ( [ rdf:type owl:Restriction ;
                                                       owl:onProperty qu:unit ;
                                                       owl:qualifiedCardinality "1"^^xsd:nonNegativeInteger ;
                                                       owl:onClass qu:Unit
                                                     ]
                                                     [ rdf:type owl:Restriction ;
                                                       owl:onProperty qu:exponent ;
                                                       owl:qualifiedCardinality "1"^^xsd:nonNegativeInteger ;
                                                       owl:onDataRange xsd:double
                                                     ]
                                                   ) ;
                                rdf:type owl:Class
                              ] ;
              dc:source "skos:exactMatch 'UnitFactor' [SysML 1.2-QUDV] http://www.omgwiki.org/OMGSysML/doku.php?id=sysml-qudv:quantities_units_dimensions_values_qudv" ;
              rdfs:comment "A UnitFactor represents a factor in the product of powers that defines a DerivedUnit." ;
              rdfs:isDefinedBy "http://purl.oclc.org/NET/ssnx/qu" ;
              rdfs:label "UnitFactor" ;
              rdfs:seeAlso "http://www.omgsysml.org/qudv#Unit" .


###  http://www.w3.org/2002/07/owl#Thing
owl:Thing rdf:type owl:Class .


#################################################################
#    General axioms
#################################################################

[ rdf:type owl:AllDisjointClasses ;
  owl:members ( qu:QuantityKind
                qu:QuantityKindFactor
                qu:Scale
                qu:ScaleValueDefinition
                qu:SystemOfQuantities
                qu:SystemOfUnits
                qu:Unit
                qu:UnitFactor
              )
] .


###  Generated by the OWL API (version 4.2.8.20170104-2310) https://github.com/owlcs/owlapi
