@prefix : <http://rdfs.org/sioc/access#> .
@prefix owl: <http://www.w3.org/2002/07/owl#> .
@prefix rdf: <http://www.w3.org/1999/02/22-rdf-syntax-ns#> .
@prefix xml: <http://www.w3.org/XML/1998/namespace> .
@prefix xsd: <http://www.w3.org/2001/XMLSchema#> .
@prefix rdfs: <http://www.w3.org/2000/01/rdf-schema#> .
@prefix sioc: <http://rdfs.org/sioc/ns#> .
@prefix dcterms: <http://purl.org/dc/terms/> .
@base <http://rdfs.org/sioc/access#> .

<http://rdfs.org/sioc/access#> rdf:type owl:Ontology ;
                                owl:imports sioc: ;
                                rdfs:seeAlso <http://rdfs.org/sioc/spec/#sec-modules> .

#################################################################
#    Object Properties
#################################################################

###  http://rdfs.org/sioc/access#has_permission
:has_permission rdf:type owl:ObjectProperty ;
                rdfs:domain sioc:Role ;
                rdfs:range :Permission ;
                rdfs:comment "A Permission assigned to a Role."@en ;
                rdfs:isDefinedBy <http://rdfs.org/sioc/access#> ;
                rdfs:label "has permission"@en .


###  http://rdfs.org/sioc/access#has_status
:has_status rdf:type owl:ObjectProperty ;
            rdfs:domain sioc:Item ;
            rdfs:range :Status ;
            rdfs:comment "The Status of a content Item (e.g. public, draft)."@en ;
            rdfs:isDefinedBy <http://rdfs.org/sioc/access#> ;
            rdfs:label "has status"@en .


#################################################################
#    Classes
#################################################################

###  http://rdfs.org/sioc/access#Permission
:Permission rdf:type owl:Class ;
            rdfs:comment "A Permission describes a type of action that can be performed on an object that is within the scope of a Role, e.g. a Site, Forum, etc."@en ;
            rdfs:isDefinedBy <http://rdfs.org/sioc/access#> ;
            rdfs:label "Permission"@en .


###  http://rdfs.org/sioc/access#Status
:Status rdf:type owl:Class ;
        rdfs:comment "A Status can be assign to content Item to indicate its publication status (e.g. public, draft, etc.). This class is used to define different types of status."@en ;
        rdfs:isDefinedBy <http://rdfs.org/sioc/access#> ;
        rdfs:label "Status"@en .


#################################################################
#    Individuals
#################################################################

###  http://rdfs.org/sioc/access#
<http://rdfs.org/sioc/access#> rdf:type owl:NamedIndividual ,
                                        owl:Thing ;
                               dcterms:description "Extends the SIOC Core Ontology (Semantically-Interlinked Online Communities) by defining basic information on permissions and access rights." ;
                               dcterms:title "SIOC Access Ontology Module" .


###  Generated by the OWL API (version 4.2.8.20170104-2310) https://github.com/owlcs/owlapi
