@prefix : <http://rdfs.org/sioc/services#> .
@prefix owl: <http://www.w3.org/2002/07/owl#> .
@prefix rdf: <http://www.w3.org/1999/02/22-rdf-syntax-ns#> .
@prefix xml: <http://www.w3.org/XML/1998/namespace> .
@prefix xsd: <http://www.w3.org/2001/XMLSchema#> .
@prefix rdfs: <http://www.w3.org/2000/01/rdf-schema#> .
@prefix sioc: <http://rdfs.org/sioc/ns#> .
@prefix dcterms: <http://purl.org/dc/terms/> .
@base <http://rdfs.org/sioc/services#> .

<http://rdfs.org/sioc/services#> rdf:type owl:Ontology ;
                                  owl:imports sioc: ;
                                  rdfs:seeAlso <http://rdfs.org/sioc/spec/#sec-modules> .

#################################################################
#    Object Properties
#################################################################

###  http://rdfs.org/sioc/services#has_service
:has_service rdf:type owl:ObjectProperty ;
             owl:inverseOf :service_of ;
             rdfs:range :Service ;
             rdfs:comment "A Service associated with this SIOC object."@en ;
             rdfs:isDefinedBy <http://rdfs.org/sioc/services#> ;
             rdfs:label "has service"@en .


###  http://rdfs.org/sioc/services#results_format
:results_format rdf:type owl:ObjectProperty ;
                rdfs:domain :Service ;
                rdfs:comment "Format of results returned by a web service."@en ;
                rdfs:isDefinedBy <http://rdfs.org/sioc/services#> ;
                rdfs:label "results format"@en .


###  http://rdfs.org/sioc/services#service_definition
:service_definition rdf:type owl:ObjectProperty ;
                    rdfs:domain :Service ;
                    rdfs:comment "Links to a web service definition of this sioc:Service."@en ;
                    rdfs:isDefinedBy <http://rdfs.org/sioc/services#> ;
                    rdfs:label "service definition"@en .


###  http://rdfs.org/sioc/services#service_endpoint
:service_endpoint rdf:type owl:ObjectProperty ;
                  rdfs:domain :Service ;
                  rdfs:comment "URL of a web service endpoint."@en ;
                  rdfs:isDefinedBy <http://rdfs.org/sioc/services#> ;
                  rdfs:label "service endpoint"@en .


###  http://rdfs.org/sioc/services#service_of
:service_of rdf:type owl:ObjectProperty ;
            rdfs:domain :Service ;
            rdfs:comment "A SIOC object this Service is associated with."@en ;
            rdfs:isDefinedBy <http://rdfs.org/sioc/services#> ;
            rdfs:label "service of"@en .


###  http://rdfs.org/sioc/services#service_protocol
:service_protocol rdf:type owl:ObjectProperty ;
                  rdfs:domain :Service ;
                  rdfs:comment "A protocol used by a web service. Possible protocol values include SOAP, REST, SPARQL-QUERY, GData and OpenSearch. These will be added to this module later."@en ;
                  rdfs:isDefinedBy <http://rdfs.org/sioc/services#> ;
                  rdfs:label "service protocol"@en .


#################################################################
#    Data properties
#################################################################

###  http://rdfs.org/sioc/services#max_results
:max_results rdf:type owl:DatatypeProperty ;
             rdfs:domain :Service ;
             rdfs:range xsd:integer ;
             rdfs:comment "Maximum number of results results returned by a web service."@en ;
             rdfs:isDefinedBy <http://rdfs.org/sioc/services#> ;
             rdfs:label "max results"@en .


#################################################################
#    Classes
#################################################################

###  http://rdfs.org/sioc/services#Service
:Service rdf:type owl:Class ;
         rdfs:comment "A Service is web service associated with a Site or part of it."@en ;
         rdfs:isDefinedBy <http://rdfs.org/sioc/services#> ;
         rdfs:label "Service"@en .


#################################################################
#    Individuals
#################################################################

###  http://rdfs.org/sioc/services#
<http://rdfs.org/sioc/services#> rdf:type owl:NamedIndividual ,
                                          owl:Thing ;
                                 dcterms:description "Extends the SIOC Core Ontology (Semantically-Interlinked Online Communities) by defining basic information on community-related web services." ;
                                 dcterms:title "SIOC Services Ontology Module Namespace" .


###  Generated by the OWL API (version 4.2.8.20170104-2310) https://github.com/owlcs/owlapi
